<?xml version="1.0" encoding="UTF-8"?>
<!DOCTYPE rdf:RDF [
	<!ENTITY dct "http://purl.org/dc/terms/">
	<!ENTITY fibo-be-le-fbo "https://spec.edmcouncil.org/fibo/BE/LegalEntities/FormalBusinessOrganizations/">
	<!ENTITY fibo-be-le-lei "https://spec.edmcouncil.org/fibo/BE/LegalEntities/LEIEntities/">
	<!ENTITY fibo-be-le-lp "https://spec.edmcouncil.org/fibo/BE/LegalEntities/LegalPersons/">
	<!ENTITY fibo-be-oac-opty "https://spec.edmcouncil.org/fibo/BE/OwnershipAndControl/OwnershipParties/">
	<!ENTITY fibo-fbc-fct-breg "https://spec.edmcouncil.org/fibo/FBC/FunctionalEntities/BusinessRegistries/">
	<!ENTITY fibo-fbc-fct-rga "https://spec.edmcouncil.org/fibo/FBC/FunctionalEntities/RegulatoryAgencies/">
	<!ENTITY fibo-fbc-fi-fi "https://spec.edmcouncil.org/fibo/FBC/FinancialInstruments/FinancialInstruments/">
	<!ENTITY fibo-fbc-pas-caa "https://spec.edmcouncil.org/fibo/FBC/ProductsAndServices/ClientsAndAccounts/">
	<!ENTITY fibo-fbc-pas-fpas "https://spec.edmcouncil.org/fibo/FBC/ProductsAndServices/FinancialProductsAndServices/">
	<!ENTITY fibo-fnd-aap-agt "https://spec.edmcouncil.org/fibo/FND/AgentsAndPeople/Agents/">
	<!ENTITY fibo-fnd-aap-ppl "https://spec.edmcouncil.org/fibo/FND/AgentsAndPeople/People/">
	<!ENTITY fibo-fnd-acc-cur "https://spec.edmcouncil.org/fibo/FND/Accounting/CurrencyAmount/">
	<!ENTITY fibo-fnd-agr-agr "https://spec.edmcouncil.org/fibo/FND/Agreements/Agreements/">
	<!ENTITY fibo-fnd-agr-ctr "https://spec.edmcouncil.org/fibo/FND/Agreements/Contracts/">
	<!ENTITY fibo-fnd-arr-arr "https://spec.edmcouncil.org/fibo/FND/Arrangements/Arrangements/">
	<!ENTITY fibo-fnd-arr-cls "https://spec.edmcouncil.org/fibo/FND/Arrangements/ClassificationSchemes/">
	<!ENTITY fibo-fnd-arr-doc "https://spec.edmcouncil.org/fibo/FND/Arrangements/Documents/">
	<!ENTITY fibo-fnd-arr-id "https://spec.edmcouncil.org/fibo/FND/Arrangements/IdentifiersAndIndices/">
	<!ENTITY fibo-fnd-dt-fd "https://spec.edmcouncil.org/fibo/FND/DatesAndTimes/FinancialDates/">
	<!ENTITY fibo-fnd-dt-oc "https://spec.edmcouncil.org/fibo/FND/DatesAndTimes/Occurrences/">
	<!ENTITY fibo-fnd-oac-own "https://spec.edmcouncil.org/fibo/FND/OwnershipAndControl/Ownership/">
	<!ENTITY fibo-fnd-org-fm "https://spec.edmcouncil.org/fibo/FND/Organizations/FormalOrganizations/">
	<!ENTITY fibo-fnd-org-org "https://spec.edmcouncil.org/fibo/FND/Organizations/Organizations/">
	<!ENTITY fibo-fnd-pas-pas "https://spec.edmcouncil.org/fibo/FND/ProductsAndServices/ProductsAndServices/">
	<!ENTITY fibo-fnd-pas-psch "https://spec.edmcouncil.org/fibo/FND/ProductsAndServices/PaymentsAndSchedules/">
	<!ENTITY fibo-fnd-plc-adr "https://spec.edmcouncil.org/fibo/FND/Places/Addresses/">
	<!ENTITY fibo-fnd-plc-cty "https://spec.edmcouncil.org/fibo/FND/Places/Countries/">
	<!ENTITY fibo-fnd-plc-loc "https://spec.edmcouncil.org/fibo/FND/Places/Locations/">
	<!ENTITY fibo-fnd-pty-pty "https://spec.edmcouncil.org/fibo/FND/Parties/Parties/">
	<!ENTITY fibo-fnd-qt-qtu "https://spec.edmcouncil.org/fibo/FND/Quantities/QuantitiesAndUnits/">
	<!ENTITY fibo-fnd-rel-rel "https://spec.edmcouncil.org/fibo/FND/Relations/Relations/">
	<!ENTITY fibo-fnd-utl-av "https://spec.edmcouncil.org/fibo/FND/Utilities/AnnotationVocabulary/">
	<!ENTITY fibo-fnd-utl-bt "https://spec.edmcouncil.org/fibo/FND/Utilities/BusinessFacingTypes/">
	<!ENTITY fibo-ln-ln-up "https://spec.edmcouncil.org/fibo/LOAN/LoanContracts/LoanUpperTemp/">
	<!ENTITY loan "https://spec.edmcouncil.org/fibo/LOAN/LoanContracts/LoanCore/">
	<!ENTITY owl "http://www.w3.org/2002/07/owl#">
	<!ENTITY rdf "http://www.w3.org/1999/02/22-rdf-syntax-ns#">
	<!ENTITY rdfs "http://www.w3.org/2000/01/rdf-schema#">
	<!ENTITY skos "http://www.w3.org/2004/02/skos/core#">
	<!ENTITY sm "http://www.omg.org/techprocess/ab/SpecificationMetadata/">
	<!ENTITY xsd "http://www.w3.org/2001/XMLSchema#">
]>
<rdf:RDF xml:base="https://spec.edmcouncil.org/fibo/LOAN/LoanContracts/LoanUpperTemp/"
	xmlns="https://spec.edmcouncil.org/fibo/LOAN/LoanContracts/LoanUpperTemp/"
	xmlns:dct="http://purl.org/dc/terms/"
	xmlns:fibo-be-le-fbo="https://spec.edmcouncil.org/fibo/BE/LegalEntities/FormalBusinessOrganizations/"
	xmlns:fibo-be-le-lei="https://spec.edmcouncil.org/fibo/BE/LegalEntities/LEIEntities/"
	xmlns:fibo-be-le-lp="https://spec.edmcouncil.org/fibo/BE/LegalEntities/LegalPersons/"
	xmlns:fibo-be-oac-opty="https://spec.edmcouncil.org/fibo/BE/OwnershipAndControl/OwnershipParties/"
	xmlns:fibo-fbc-fct-breg="https://spec.edmcouncil.org/fibo/FBC/FunctionalEntities/BusinessRegistries/"
	xmlns:fibo-fbc-fct-rga="https://spec.edmcouncil.org/fibo/FBC/FunctionalEntities/RegulatoryAgencies/"
	xmlns:fibo-fbc-fi-fi="https://spec.edmcouncil.org/fibo/FBC/FinancialInstruments/FinancialInstruments/"
	xmlns:fibo-fbc-pas-caa="https://spec.edmcouncil.org/fibo/FBC/ProductsAndServices/ClientsAndAccounts/"
	xmlns:fibo-fbc-pas-fpas="https://spec.edmcouncil.org/fibo/FBC/ProductsAndServices/FinancialProductsAndServices/"
	xmlns:fibo-fnd-aap-agt="https://spec.edmcouncil.org/fibo/FND/AgentsAndPeople/Agents/"
	xmlns:fibo-fnd-aap-ppl="https://spec.edmcouncil.org/fibo/FND/AgentsAndPeople/People/"
	xmlns:fibo-fnd-acc-cur="https://spec.edmcouncil.org/fibo/FND/Accounting/CurrencyAmount/"
	xmlns:fibo-fnd-agr-agr="https://spec.edmcouncil.org/fibo/FND/Agreements/Agreements/"
	xmlns:fibo-fnd-agr-ctr="https://spec.edmcouncil.org/fibo/FND/Agreements/Contracts/"
	xmlns:fibo-fnd-arr-arr="https://spec.edmcouncil.org/fibo/FND/Arrangements/Arrangements/"
	xmlns:fibo-fnd-arr-cls="https://spec.edmcouncil.org/fibo/FND/Arrangements/ClassificationSchemes/"
	xmlns:fibo-fnd-arr-doc="https://spec.edmcouncil.org/fibo/FND/Arrangements/Documents/"
	xmlns:fibo-fnd-arr-id="https://spec.edmcouncil.org/fibo/FND/Arrangements/IdentifiersAndIndices/"
	xmlns:fibo-fnd-dt-fd="https://spec.edmcouncil.org/fibo/FND/DatesAndTimes/FinancialDates/"
	xmlns:fibo-fnd-dt-oc="https://spec.edmcouncil.org/fibo/FND/DatesAndTimes/Occurrences/"
	xmlns:fibo-fnd-oac-own="https://spec.edmcouncil.org/fibo/FND/OwnershipAndControl/Ownership/"
	xmlns:fibo-fnd-org-fm="https://spec.edmcouncil.org/fibo/FND/Organizations/FormalOrganizations/"
	xmlns:fibo-fnd-org-org="https://spec.edmcouncil.org/fibo/FND/Organizations/Organizations/"
	xmlns:fibo-fnd-pas-pas="https://spec.edmcouncil.org/fibo/FND/ProductsAndServices/ProductsAndServices/"
	xmlns:fibo-fnd-pas-psch="https://spec.edmcouncil.org/fibo/FND/ProductsAndServices/PaymentsAndSchedules/"
	xmlns:fibo-fnd-plc-adr="https://spec.edmcouncil.org/fibo/FND/Places/Addresses/"
	xmlns:fibo-fnd-plc-cty="https://spec.edmcouncil.org/fibo/FND/Places/Countries/"
	xmlns:fibo-fnd-plc-loc="https://spec.edmcouncil.org/fibo/FND/Places/Locations/"
	xmlns:fibo-fnd-pty-pty="https://spec.edmcouncil.org/fibo/FND/Parties/Parties/"
	xmlns:fibo-fnd-qt-qtu="https://spec.edmcouncil.org/fibo/FND/Quantities/QuantitiesAndUnits/"
	xmlns:fibo-fnd-rel-rel="https://spec.edmcouncil.org/fibo/FND/Relations/Relations/"
	xmlns:fibo-fnd-utl-av="https://spec.edmcouncil.org/fibo/FND/Utilities/AnnotationVocabulary/"
	xmlns:fibo-fnd-utl-bt="https://spec.edmcouncil.org/fibo/FND/Utilities/BusinessFacingTypes/"
	xmlns:fibo-ln-ln-up="https://spec.edmcouncil.org/fibo/LOAN/LoanContracts/LoanUpperTemp/"
	xmlns:loan="https://spec.edmcouncil.org/fibo/LOAN/LoanContracts/LoanCore/"
	xmlns:owl="http://www.w3.org/2002/07/owl#"
	xmlns:rdf="http://www.w3.org/1999/02/22-rdf-syntax-ns#"
	xmlns:rdfs="http://www.w3.org/2000/01/rdf-schema#"
	xmlns:skos="http://www.w3.org/2004/02/skos/core#"
	xmlns:sm="http://www.omg.org/techprocess/ab/SpecificationMetadata/"
	xmlns:xsd="http://www.w3.org/2001/XMLSchema#">
	
	<owl:Ontology rdf:about="https://spec.edmcouncil.org/fibo/LOAN/LoanContracts/LoanUpperTemp/">
		<owl:imports rdf:resource="http://www.omg.org/techprocess/ab/SpecificationMetadata/"/>
		<owl:imports rdf:resource="http://www.w3.org/2004/02/skos/core"/>
		<owl:imports rdf:resource="https://spec.edmcouncil.org/fibo/BE/OwnershipAndControl/OwnershipParties/"/>
		<owl:imports rdf:resource="https://spec.edmcouncil.org/fibo/FBC/20150801/FunctionalEntities/BusinessRegistries/"/>
		<owl:imports rdf:resource="https://spec.edmcouncil.org/fibo/FND/20160201/ProductsAndServices/PaymentsAndSchedules/"/>
		<owl:imports rdf:resource="https://spec.edmcouncil.org/fibo/FND/Accounting/CurrencyAmount/"/>
		<owl:imports rdf:resource="https://spec.edmcouncil.org/fibo/FND/AgentsAndPeople/Agents/"/>
		<owl:imports rdf:resource="https://spec.edmcouncil.org/fibo/FND/AgentsAndPeople/People/"/>
		<owl:imports rdf:resource="https://spec.edmcouncil.org/fibo/FND/Agreements/Agreements/"/>
		<owl:imports rdf:resource="https://spec.edmcouncil.org/fibo/FND/Agreements/Contracts/"/>
		<owl:imports rdf:resource="https://spec.edmcouncil.org/fibo/FND/Arrangements/Arrangements/"/>
		<owl:imports rdf:resource="https://spec.edmcouncil.org/fibo/FND/Arrangements/ClassificationSchemes/"/>
		<owl:imports rdf:resource="https://spec.edmcouncil.org/fibo/FND/DatesAndTimes/FinancialDates/"/>
		<owl:imports rdf:resource="https://spec.edmcouncil.org/fibo/FND/DatesAndTimes/Occurrences/"/>
		<owl:imports rdf:resource="https://spec.edmcouncil.org/fibo/FND/Organizations/FormalOrganizations/"/>
		<owl:imports rdf:resource="https://spec.edmcouncil.org/fibo/FND/Parties/Parties/"/>
		<owl:imports rdf:resource="https://spec.edmcouncil.org/fibo/FND/Places/Addresses/"/>
		<owl:imports rdf:resource="https://spec.edmcouncil.org/fibo/FND/Places/Countries/"/>
		<owl:imports rdf:resource="https://spec.edmcouncil.org/fibo/FND/Places/Locations/"/>
		<owl:imports rdf:resource="https://spec.edmcouncil.org/fibo/FND/ProductsAndServices/ProductsAndServices/"/>
		<owl:imports rdf:resource="https://spec.edmcouncil.org/fibo/FND/Relations/Relations/"/>
		<owl:imports rdf:resource="https://spec.edmcouncil.org/fibo/FND/Utilities/AnnotationVocabulary/"/>
		<owl:versionInfo>Created with e6Tools Graphical OWL Editor from D:\SEMANTIC-ARTS\NAS\ClientsAndPartners\EDM Council\fibo ontologies\LoanOntology\loans.vsdx Page:loanUpper</owl:versionInfo>
		<skos:definition></skos:definition>
		<skos:definition>LoanUpperTemp</skos:definition>
	</owl:Ontology>
	
	<owl:ObjectProperty rdf:about="&fibo-be-oac-opty;guarantees">
		<owl:inverseOf rdf:resource="&fibo-ln-ln-up;opty-isGuaranteedBy"/>
		<skos:editorialNote>Adding inverse of guarantees called isGuaranteedBy</skos:editorialNote>
		<skos:editorialNote>Topic: BE add inverse of guarantees called isGuaranteedBy</skos:editorialNote>
	</owl:ObjectProperty>
	
	<owl:ObjectProperty rdf:about="&fibo-fbc-fct-breg;isSubdivisionOf">
		<owl:inverseOf rdf:resource="&fibo-fbc-fct-breg;hasSubdivision"/>
		<skos:editorialNote>This should be added to the BusinessRegistries ontology</skos:editorialNote>
	</owl:ObjectProperty>
	
	<owl:Class rdf:about="&fibo-fnd-agr-agr;Agreement">
		<rdfs:subClassOf rdf:resource="&fibo-ln-ln-up;Specification"/>
	</owl:Class>
	
	<owl:Class rdf:about="&fibo-fnd-agr-agr;Commitment">
		<rdfs:subClassOf rdf:resource="&fibo-ln-ln-up;Specification"/>
	</owl:Class>
	
	<owl:ObjectProperty rdf:about="&fibo-fnd-agr-ctr;hasEffectiveDate">
		<rdfs:subPropertyOf rdf:resource="&fibo-ln-ln-up;asOfDate"/>
	</owl:ObjectProperty>
	
	<owl:ObjectProperty rdf:about="&fibo-fnd-rel-rel;isComprisedOf">
		<owl:inverseOf rdf:resource="&fibo-fnd-rel-rel;comprises"/>
		<skos:editorialNote>Topic: FND Adding inverse of comprises called isComprisedOf</skos:editorialNote>
	</owl:ObjectProperty>
	
	<owl:Class rdf:about="&fibo-ln-ln-up;Application">
		<rdfs:subClassOf rdf:resource="&fibo-ln-ln-up;fnd-Request"/>
		<rdfs:subClassOf>
			<owl:Restriction>
				<owl:onProperty rdf:resource="&fibo-ln-ln-up;hasDateReceived"/>
				<owl:someValuesFrom rdf:resource="&fibo-fnd-dt-fd;Date"/>
			</owl:Restriction>
		</rdfs:subClassOf>
		<rdfs:label>Application</rdfs:label>
		<skos:definition>A request submitted by an applicant to receive something (e.g. a licence, a loan, a membership).  Is accompanied by documentation of pertinent information to determine whether the request should be granted.</skos:definition>
	</owl:Class>
	
	<owl:Class rdf:about="&fibo-ln-ln-up;BE-ContactPurpose">
		<rdfs:subClassOf rdf:resource="&fibo-fnd-arr-cls;Classifier"/>
		<rdfs:label>contact purpose</rdfs:label>
		<skos:definition>A virtual address for communication via phone.</skos:definition>
	</owl:Class>
	
	<owl:Class rdf:about="&fibo-ln-ln-up;ChargeCategory">
		<rdfs:subClassOf rdf:resource="&fibo-fnd-arr-cls;Classifier"/>
		<rdfs:label>charge cateogry</rdfs:label>
		<skos:definition>A specific indicator of what a charge is for (e.g. closing costs, interest)</skos:definition>
	</owl:Class>
	
	<owl:Class rdf:about="&fibo-ln-ln-up;ContactInfo">
		<rdfs:subClassOf>
			<owl:Restriction>
				<owl:onProperty rdf:resource="&fibo-fnd-rel-rel;comprises"/>
				<owl:onClass rdf:resource="&fibo-fnd-aap-ppl;LegallyCapableAdult"/>
				<owl:minQualifiedCardinality rdf:datatype="&xsd;nonNegativeInteger">0</owl:minQualifiedCardinality>
			</owl:Restriction>
		</rdfs:subClassOf>
		<rdfs:subClassOf>
			<owl:Restriction>
				<owl:onProperty rdf:resource="&fibo-fnd-rel-rel;comprises"/>
				<owl:onClass rdf:resource="&fibo-fnd-org-fm;FormalOrganization"/>
				<owl:minQualifiedCardinality rdf:datatype="&xsd;nonNegativeInteger">0</owl:minQualifiedCardinality>
			</owl:Restriction>
		</rdfs:subClassOf>
		<rdfs:subClassOf>
			<owl:Restriction>
				<owl:onProperty rdf:resource="&fibo-fnd-rel-rel;comprises"/>
				<owl:onClass rdf:resource="&fibo-fnd-plc-adr;PostalAddress"/>
				<owl:minQualifiedCardinality rdf:datatype="&xsd;nonNegativeInteger">0</owl:minQualifiedCardinality>
			</owl:Restriction>
		</rdfs:subClassOf>
		<rdfs:subClassOf>
			<owl:Restriction>
				<owl:onProperty rdf:resource="&fibo-fnd-rel-rel;comprises"/>
				<owl:onClass rdf:resource="&fibo-ln-ln-up;adr-EmailAddress"/>
				<owl:minQualifiedCardinality rdf:datatype="&xsd;nonNegativeInteger">0</owl:minQualifiedCardinality>
			</owl:Restriction>
		</rdfs:subClassOf>
		<rdfs:subClassOf>
			<owl:Restriction>
				<owl:onProperty rdf:resource="&fibo-fnd-rel-rel;comprises"/>
				<owl:onClass rdf:resource="&fibo-ln-ln-up;adr-PhoneNumber"/>
				<owl:minQualifiedCardinality rdf:datatype="&xsd;nonNegativeInteger">0</owl:minQualifiedCardinality>
			</owl:Restriction>
		</rdfs:subClassOf>
		<rdfs:subClassOf>
			<owl:Restriction>
				<owl:onProperty rdf:resource="&fibo-fnd-rel-rel;isClassifiedBy"/>
				<owl:someValuesFrom rdf:resource="&fibo-ln-ln-up;BE-ContactPurpose"/>
			</owl:Restriction>
		</rdfs:subClassOf>
		<rdfs:label>contact information</rdfs:label>
		<skos:definition>A way to make contact with a person or organization for a particular reason regarding something.  The details may be role-specific, so the information cannot always go on the individual or organization.</skos:definition>
		<skos:editorialNote>This approach avoids the need to have multiple properties to connect different things to ContactInfo use for different purposes.</skos:editorialNote>
		<skos:editorialNote>Topic: BE</skos:editorialNote>
		<fibo-fnd-utl-av:usageNote>Make sure to check the existing instances of ContactPurpose and use those before creating new ones.</fibo-fnd-utl-av:usageNote>
	</owl:Class>
	
	<owl:Class rdf:about="&fibo-ln-ln-up;FND-InformationProduct">
		<rdfs:subClassOf rdf:resource="&fibo-fnd-pas-pas;Product"/>
		<rdfs:label>information product</rdfs:label>
		<skos:definition>A Product that is informational in nature, rather than physical.</skos:definition>
	</owl:Class>
	
	<owl:Class rdf:about="&fibo-ln-ln-up;MetroDivision">
		<rdfs:subClassOf rdf:resource="&fibo-fnd-plc-cty;GeopoliticalEntity"/>
		<rdfs:subClassOf>
			<owl:Restriction>
				<owl:onProperty rdf:resource="&fibo-fbc-fct-breg;isSubdivisionOf"/>
				<owl:someValuesFrom rdf:resource="&fibo-ln-ln-up;MetroStatArea"/>
			</owl:Restriction>
		</rdfs:subClassOf>
		<rdfs:label>metropolitan division</rdfs:label>
		<skos:definition>Metropolitan division (MD) is an area specified by the government to describe a subsection of a certain metropolitan statistical area.  In the US, this is governed by the Census Department.</skos:definition>
		<skos:editorialNote>Topic: Regions</skos:editorialNote>
	</owl:Class>
	
	<owl:Class rdf:about="&fibo-ln-ln-up;MetroStatArea">
		<rdfs:subClassOf rdf:resource="&fibo-fnd-plc-cty;GeopoliticalEntity"/>
		<rdfs:label>metropolitan statistical area</rdfs:label>
		<skos:definition>Metropolitan statistical area (MSA) is an area specified by the government to describe a certain metropolitan statistical area.  In the US, this is governed by the Census department.</skos:definition>
		<skos:editorialNote>Topic: Regions</skos:editorialNote>
	</owl:Class>
	
	<owl:Class rdf:about="&fibo-ln-ln-up;PaymentHistory">
		<rdfs:subClassOf rdf:resource="&fibo-fnd-arr-doc;Record"/>
		<rdfs:subClassOf>
			<owl:Restriction>
				<owl:onProperty rdf:resource="&fibo-fnd-rel-rel;hasMember"/>
				<owl:someValuesFrom rdf:resource="&fibo-fnd-pas-psch;Payment"/>
			</owl:Restriction>
		</rdfs:subClassOf>
		<rdfs:subClassOf>
			<owl:Restriction>
				<owl:onProperty rdf:resource="&fibo-ln-ln-up;hasActualUnpaidBalance"/>
				<owl:someValuesFrom rdf:resource="&fibo-fnd-acc-cur;MonetaryAmount"/>
			</owl:Restriction>
		</rdfs:subClassOf>
		<rdfs:label>payment history</rdfs:label>
		<skos:definition>A record of actual payments of principal, interest, and other related amounts made by a borrower to a lender or servicer in order to fulfill their re-payment obligation.</skos:definition>
		<skos:editorialNote>Topic: Payments</skos:editorialNote>
		<fibo-fnd-utl-av:explanatoryNote>Just like a PaymentSchedule except that the dates and amounts are actuals.</fibo-fnd-utl-av:explanatoryNote>
	</owl:Class>
	
	<owl:Class rdf:about="&fibo-ln-ln-up;PaymentSchedule">
		<rdfs:subClassOf rdf:resource="&fibo-fnd-dt-fd;Schedule"/>
		<rdfs:subClassOf>
			<owl:Restriction>
				<owl:onProperty rdf:resource="&fibo-fnd-rel-rel;hasMember"/>
				<owl:someValuesFrom rdf:resource="&fibo-ln-ln-up;ScheduledPayment"/>
			</owl:Restriction>
		</rdfs:subClassOf>
		<rdfs:label>payment schedule</rdfs:label>
		<skos:definition>A Schedule of amounts of principal and interest that are due over the term of the loan in order to fully pay off the obligation.</skos:definition>
		<skos:editorialNote>Topic: Payments
Not using psch:PaymentSchedule because it uses PaymentEvent which is an OccurrenceKind which does not make sense. Also, it should use hasMember not comprises to put items into a Collection. Ripe for coagulation.</skos:editorialNote>
	</owl:Class>
	
	<owl:Class rdf:about="&fibo-ln-ln-up;Report">
		<rdfs:subClassOf>
			<owl:Restriction>
				<owl:onProperty rdf:resource="&fibo-ln-ln-up;rel-isProducedBy_I"/>
				<owl:onClass rdf:resource="&fibo-fnd-aap-agt;AutonomousAgent"/>
				<owl:minQualifiedCardinality rdf:datatype="&xsd;nonNegativeInteger">0</owl:minQualifiedCardinality>
			</owl:Restriction>
		</rdfs:subClassOf>
		<rdfs:subClassOf>
			<owl:Restriction>
				<owl:onProperty rdf:resource="&fibo-ln-ln-up;dt-fd-coversPeriod"/>
				<owl:onClass rdf:resource="&fibo-fnd-dt-fd;DatePeriod"/>
				<owl:minQualifiedCardinality rdf:datatype="&xsd;nonNegativeInteger">0</owl:minQualifiedCardinality>
			</owl:Restriction>
		</rdfs:subClassOf>
		<rdfs:subClassOf>
			<owl:Restriction>
				<owl:onProperty rdf:resource="&fibo-ln-ln-up;hasCreationDate"/>
				<owl:someValuesFrom rdf:resource="&fibo-fnd-dt-fd;Date"/>
			</owl:Restriction>
		</rdfs:subClassOf>
		<rdfs:label>report</rdfs:label>
		<sm:normativeReference>http://www.businessdictionary.com/definition/report.html</sm:normativeReference>
		<skos:definition>A body of information organized in a narrative, graphic, or tabular form, prepared on ad hoc, periodic, recurring, regular, or as required basis. Reports may refer to specific periods, events, occurrences, or subjects, and may be communicated or presented in oral or written form.</skos:definition>
	</owl:Class>
	
	<owl:Class rdf:about="&fibo-ln-ln-up;ScheduledPayment">
		<rdfs:subClassOf rdf:resource="&fibo-fnd-dt-fd;AdHocScheduleEntry"/>
		<rdfs:subClassOf rdf:resource="&fibo-fnd-pas-psch;PaymentObligation"/>
		<rdfs:subClassOf>
			<owl:Restriction>
				<owl:onProperty rdf:resource="&fibo-fnd-pas-psch;hasPaymentAmount"/>
				<owl:someValuesFrom rdf:resource="&fibo-fnd-acc-cur;MonetaryAmount"/>
			</owl:Restriction>
		</rdfs:subClassOf>
		<rdfs:subClassOf>
			<owl:Restriction>
				<owl:onProperty rdf:resource="&fibo-ln-ln-up;hasScheduledUnpaidBalance"/>
				<owl:someValuesFrom rdf:resource="&fibo-fnd-acc-cur;MonetaryAmount"/>
			</owl:Restriction>
		</rdfs:subClassOf>
		<rdfs:label>scheduled payment</rdfs:label>
		<skos:definition>A scheduled payment occurrence that is part of a payment schedule covering the term of the loan.</skos:definition>
		<skos:editorialNote>Topic: Payments</skos:editorialNote>
	</owl:Class>
	
	<owl:Class rdf:about="&fibo-ln-ln-up;Specification">
		<rdfs:label>specification</rdfs:label>
		<skos:definition>A body of information specifying what properties, structure and/or results something should or must have after it has been built, fulfilled or completed. The thing may be physical (a building), organizational (a management structure), computational (a program), job or task related (e.g., a CEO, Chief Judge) or changing oil in a car. It may be a set of characteristics saying what something must be, or a set of instructions saying how to do something.</skos:definition>
	</owl:Class>
	
	<owl:Class rdf:about="&fibo-ln-ln-up;Text">
		<rdfs:subClassOf>
			<owl:Restriction>
				<owl:onProperty rdf:resource="&fibo-ln-ln-up;hasString"/>
				<owl:someValuesFrom rdf:resource="&xsd;string"/>
			</owl:Restriction>
		</rdfs:subClassOf>
		<skos:definition>A set of words and characters expressed in some language. E.g. a description, a message</skos:definition>
		<skos:editorialNote>This probably belongs in a documents messages ontology</skos:editorialNote>
	</owl:Class>
	
	<owl:Class rdf:about="&fibo-ln-ln-up;Valuation">
		<rdfs:subClassOf rdf:resource="&fibo-ln-ln-up;alx-Measurement"/>
		<rdfs:subClassOf>
			<owl:Restriction>
				<owl:onProperty rdf:resource="&fibo-ln-ln-up;thingBeingValued"/>
				<owl:minCardinality rdf:datatype="&xsd;nonNegativeInteger">1</owl:minCardinality>
			</owl:Restriction>
		</rdfs:subClassOf>
		<rdfs:label>valuation</rdfs:label>
		<skos:definition>A Measurement to assess the value of something, e.g. a house, or a bond. The result is in some currency.</skos:definition>
		<fibo-fnd-utl-av:explanatoryNote>TODO: model this out properly, add to analytics (alx) ontology, put it somewhere (in FBC?).</fibo-fnd-utl-av:explanatoryNote>
	</owl:Class>
	
	<owl:Class rdf:about="&fibo-ln-ln-up;adr-EmailAddress">
		<rdfs:subClassOf rdf:resource="&fibo-fnd-plc-adr;VirtualAddress"/>
		<rdfs:subClassOf>
			<owl:Restriction>
				<owl:onProperty rdf:resource="&fibo-ln-ln-up;hasString"/>
				<owl:someValuesFrom rdf:resource="&xsd;string"/>
			</owl:Restriction>
		</rdfs:subClassOf>
		<rdfs:label>email address</rdfs:label>
		<skos:definition>A virtual address for sending email communication to.</skos:definition>
	</owl:Class>
	
	<owl:Class rdf:about="&fibo-ln-ln-up;adr-PhoneNumber">
		<rdfs:subClassOf rdf:resource="&fibo-fnd-plc-adr;VirtualAddress"/>
		<rdfs:subClassOf>
			<owl:Restriction>
				<owl:onProperty rdf:resource="&fibo-ln-ln-up;hasString"/>
				<owl:someValuesFrom rdf:resource="&xsd;string"/>
			</owl:Restriction>
		</rdfs:subClassOf>
		<rdfs:label>phone number</rdfs:label>
		<skos:definition>A virtual address for communication via phone.</skos:definition>
	</owl:Class>
	
	<owl:Class rdf:about="&fibo-ln-ln-up;alx-Measurement">
		<rdfs:subClassOf rdf:resource="&fibo-fnd-dt-oc;Occurrence"/>
		<rdfs:label>measurement</rdfs:label>
		<skos:definition>The act of taking a measurement.  Some measurement procedure is used to measure some aspect of something giving a result typicalliy expressed in some units .  E.g. a valuation measuring the value of an asset expressedin USD</skos:definition>
		<fibo-fnd-utl-av:explanatoryNote>TODO: model this out properly, add to analytics (alx) ontology.</fibo-fnd-utl-av:explanatoryNote>
	</owl:Class>
	
	<owl:ObjectProperty rdf:about="&fibo-ln-ln-up;asOfDate">
		<rdfs:subPropertyOf rdf:resource="&fibo-fnd-dt-fd;hasDate"/>
		<rdfs:label>as of date</rdfs:label>
		<skos:definition>LC to check: relates something to the date on which it is accurate or valid. E.g. a credit report has an asOfDate that means the date when the information was drawn. It is different from the creation date and need not be the last date of the DatePeriod covered.</skos:definition>
	</owl:ObjectProperty>
	
	<owl:ObjectProperty rdf:about="&fibo-ln-ln-up;conformsTo">
		<rdfs:label>conforms to</rdfs:label>
		<rdfs:range rdf:resource="&fibo-ln-ln-up;Specification"/>
		<skos:definition>The Subject  complies with or conforms to what is specified by the Object.  Often the Object  will causally affect the Subject, but not necessarily, hence is not a subproperty of fibo-fnd-rel-rel:causes</skos:definition>
	</owl:ObjectProperty>
	
	<owl:ObjectProperty rdf:about="&fibo-ln-ln-up;cur-hasAmount">
		<rdfs:subPropertyOf rdf:resource="&fibo-fnd-rel-rel;has"/>
		<rdfs:label>has monetary amount</rdfs:label>
		<rdfs:range rdf:resource="&fibo-fnd-acc-cur;MonetaryAmount"/>
		<skos:definition>Relates something to a monetary amount, e.g. credit limit, notional amount.</skos:definition>
		<fibo-fnd-utl-av:explanatoryNote>NOTE: this could be a loan amount, or a credit line. YES, we need to discuss; it could be even more that this.</fibo-fnd-utl-av:explanatoryNote>
	</owl:ObjectProperty>
	
	<owl:ObjectProperty rdf:about="&fibo-ln-ln-up;cur-hasEstimatedValue">
		<skos:definition>A relation between something and its estimated value</skos:definition>
	</owl:ObjectProperty>
	
	<owl:ObjectProperty rdf:about="&fibo-ln-ln-up;dataSourcedFrom">
		<rdfs:label>has estimated value</rdfs:label>
		<skos:definition>A source of data, in a given context. e.g. Experian provides data for a CreditReport</skos:definition>
	</owl:ObjectProperty>
	
	<owl:ObjectProperty rdf:about="&fibo-ln-ln-up;dt-fd-coversPeriod">
		<rdfs:subPropertyOf rdf:resource="&fibo-fnd-dt-fd;hasDatePeriod"/>
		<rdfs:label>covers period</rdfs:label>
		<rdfs:range rdf:resource="&fibo-fnd-dt-fd;DatePeriod"/>
		<skos:definition>The period of time which is covered. e.g. for a reporting period.</skos:definition>
	</owl:ObjectProperty>
	
	<owl:Class rdf:about="&fibo-ln-ln-up;fnd-Request">
		<rdfs:subClassOf rdf:resource="&fibo-fnd-dt-oc;Occurrence"/>
		<rdfs:subClassOf>
			<owl:Restriction>
				<owl:onProperty rdf:resource="&fibo-ln-ln-up;fnd-hasThingRequested"/>
				<owl:minCardinality rdf:datatype="&xsd;nonNegativeInteger">1</owl:minCardinality>
			</owl:Restriction>
		</rdfs:subClassOf>
		<rdfs:subClassOf>
			<owl:Restriction>
				<owl:onProperty rdf:resource="&fibo-ln-ln-up;rel-isFrom"/>
				<owl:someValuesFrom rdf:resource="&fibo-fnd-aap-agt;AutonomousAgent"/>
			</owl:Restriction>
		</rdfs:subClassOf>
		<rdfs:subClassOf>
			<owl:Restriction>
				<owl:onProperty rdf:resource="&fibo-ln-ln-up;rel-isTo"/>
				<owl:someValuesFrom rdf:resource="&fibo-fnd-aap-agt;AutonomousAgent"/>
			</owl:Restriction>
		</rdfs:subClassOf>
		<rdfs:label>request</rdfs:label>
		<skos:definition>An agent asks another agent for something or to do something.</skos:definition>
	</owl:Class>
	
	<owl:Class rdf:about="&fibo-ln-ln-up;fnd-RiskAssessment">
		<rdfs:subClassOf rdf:resource="&fibo-fnd-dt-oc;Occurrence"/>
		<rdfs:label>risk assessment</rdfs:label>
		<skos:definition>The occurrence of assessing the risk of something.</skos:definition>
	</owl:Class>
	
	<owl:ObjectProperty rdf:about="&fibo-ln-ln-up;fnd-hasThingRequested">
		<rdfs:subPropertyOf rdf:resource="&fibo-ln-ln-up;hasParticipant"/>
		<rdfs:label>has thing requested</rdfs:label>
		<skos:definition>Relates a Request to that which is being requested, e.g. a report.</skos:definition>
	</owl:ObjectProperty>
	
	<owl:ObjectProperty rdf:about="&fibo-ln-ln-up;fnd-rel-isResponseTo">
		<rdfs:label>is response to</rdfs:label>
		<rdfs:domain rdf:resource="&fibo-fnd-dt-oc;Occurrence"/>
		<rdfs:range rdf:resource="&fibo-fnd-dt-oc;Occurrence"/>
		<skos:definition>Related an Occurrence to another Occurrence, most often in the context of communication.</skos:definition>
	</owl:ObjectProperty>
	
	<owl:ObjectProperty rdf:about="&fibo-ln-ln-up;hasActualUnpaidBalance">
		<rdfs:subPropertyOf rdf:resource="&fibo-fnd-rel-rel;has"/>
		<rdfs:label>has actual unpaid balance</rdfs:label>
		<rdfs:range rdf:resource="&fibo-fnd-acc-cur;MonetaryAmount"/>
		<skos:definition>What the actual balance is after a payment is made.</skos:definition>
		<skos:editorialNote>Topic: Payments</skos:editorialNote>
	</owl:ObjectProperty>
	
	<owl:ObjectProperty rdf:about="&fibo-ln-ln-up;hasAppraiser">
		<rdfs:subPropertyOf rdf:resource="&fibo-ln-ln-up;hasParticipant"/>
		<rdfs:label>has appraiser</rdfs:label>
		<skos:definition>Relates e.g. an appraisal, to a party that plays the role of conducting a property appraisal.</skos:definition>
	</owl:ObjectProperty>
	
	<owl:ObjectProperty rdf:about="&fibo-ln-ln-up;hasCreationDate">
		<rdfs:subPropertyOf rdf:resource="&fibo-fnd-dt-fd;hasStartDate"/>
		<rdfs:label>has creation date</rdfs:label>
		<skos:definition>Relates something to the date when it came into existence.</skos:definition>
	</owl:ObjectProperty>
	
	<owl:ObjectProperty rdf:about="&fibo-ln-ln-up;hasDateReceived">
		<rdfs:subPropertyOf rdf:resource="&fibo-fnd-dt-fd;hasDate"/>
		<rdfs:label>has date received</rdfs:label>
		<skos:definition>Relates something to the date when it was received, e.g. a loan application request.</skos:definition>
	</owl:ObjectProperty>
	
	<owl:ObjectProperty rdf:about="&fibo-ln-ln-up;hasIndividualContactInfo">
		<rdfs:label>has individual contact information</rdfs:label>
		<rdfs:range rdf:resource="&fibo-ln-ln-up;ContactInfo"/>
		<skos:definition>Relates something to the contact information of an individual (as opposed to an organization).</skos:definition>
		<skos:editorialNote>Topic: BE</skos:editorialNote>
	</owl:ObjectProperty>
	
	<owl:ObjectProperty rdf:about="&fibo-ln-ln-up;hasInput">
		<rdfs:subPropertyOf rdf:resource="&fibo-ln-ln-up;hasParticipant"/>
		<rdfs:label>has input</rdfs:label>
		<owl:inverseOf rdf:resource="&fibo-ln-ln-up;hasInputOn"/>
		<skos:definition>Relates an Occurrence to something that is used as an input to some activity or process.</skos:definition>
	</owl:ObjectProperty>
	
	<owl:ObjectProperty rdf:about="&fibo-ln-ln-up;hasInputOn">
		<rdfs:label>has input on</rdfs:label>
	</owl:ObjectProperty>
	
	<owl:ObjectProperty rdf:about="&fibo-ln-ln-up;hasInterestRate">
		<rdfs:subPropertyOf rdf:resource="&fibo-fnd-rel-rel;has"/>
		<rdfs:label>has interest rate</rdfs:label>
		<skos:definition>Relates, e.g. a loan, to an insterest rate.</skos:definition>
		<skos:editorialNote>Topic: Payments</skos:editorialNote>
	</owl:ObjectProperty>
	
	<owl:ObjectProperty rdf:about="&fibo-ln-ln-up;hasItemOffered">
		<rdfs:subPropertyOf rdf:resource="&fibo-ln-ln-up;hasParticipant"/>
		<rdfs:label>has item offered</rdfs:label>
		<skos:definition>Relates an Offer to the item on offer</skos:definition>
	</owl:ObjectProperty>
	
	<owl:DatatypeProperty rdf:about="&fibo-ln-ln-up;hasNumberOfEntries">
		<rdfs:subPropertyOf rdf:resource="&fibo-ln-ln-up;rel-hasCount"/>
		<rdfs:label>has number of entries</rdfs:label>
		<rdfs:range rdf:resource="&xsd;positiveInteger"/>
		<skos:definition>The number of entries, e.g. in a report.</skos:definition>
	</owl:DatatypeProperty>
	
	<owl:ObjectProperty rdf:about="&fibo-ln-ln-up;hasOrgContactInfo">
		<rdfs:label>has organization contact information</rdfs:label>
		<rdfs:range rdf:resource="&fibo-ln-ln-up;ContactInfo"/>
		<skos:definition>Relates something to the contact information of an organization  (as opposed to an individual).</skos:definition>
		<skos:editorialNote>Topic: BE</skos:editorialNote>
	</owl:ObjectProperty>
	
	<owl:ObjectProperty rdf:about="&fibo-ln-ln-up;hasOutput">
		<rdfs:subPropertyOf rdf:resource="&fibo-ln-ln-up;hasParticipant"/>
		<rdfs:label>has output</rdfs:label>
		<owl:inverseOf rdf:resource="&fibo-ln-ln-up;hasOutputOn"/>
		<skos:definition>Relates an Occurrence to something that is the result of some activity or process.</skos:definition>
	</owl:ObjectProperty>
	
	<owl:ObjectProperty rdf:about="&fibo-ln-ln-up;hasOutputOn">
		<rdfs:label>has output on</rdfs:label>
	</owl:ObjectProperty>
	
	<owl:ObjectProperty rdf:about="&fibo-ln-ln-up;hasParticipant">
		<rdfs:label>has participant</rdfs:label>
		<skos:definition>Relates e.g. an agreement or event to an object or party playing a role.</skos:definition>
		<skos:editorialNote>pty-pty:hasParty should be a subproperty of this property.</skos:editorialNote>
	</owl:ObjectProperty>
	
	<owl:ObjectProperty rdf:about="&fibo-ln-ln-up;hasScheduledUnpaidBalance">
		<rdfs:subPropertyOf rdf:resource="&fibo-fnd-rel-rel;has"/>
		<rdfs:label>has scheduled unpaid balance</rdfs:label>
		<rdfs:range rdf:resource="&fibo-fnd-acc-cur;MonetaryAmount"/>
		<skos:definition>What the unpaid balance should be when a scheduled payment is made according to contract terms</skos:definition>
		<skos:editorialNote>Topic: Payments</skos:editorialNote>
	</owl:ObjectProperty>
	
	<owl:ObjectProperty rdf:about="&fibo-ln-ln-up;hasSeniorAppraiser">
		<rdfs:subPropertyOf rdf:resource="&fibo-ln-ln-up;hasParticipant"/>
		<rdfs:label>has senior appraiser</rdfs:label>
		<skos:definition>Relates e.g. an appraisal to the appraiser with seniority or supervisory responsibilities.</skos:definition>
	</owl:ObjectProperty>
	
	<owl:DatatypeProperty rdf:about="&fibo-ln-ln-up;hasString">
		<rdfs:label></rdfs:label>
		<rdfs:range rdf:resource="&xsd;string"/>
		<skos:definition>A general purpose property pointing from a text object to its string.</skos:definition>
		<skos:editorialNote>TODO:  change name of fibo-fnd-rel-rel:hasUniqueIdentifier to hasUniqueString to avoid confusion with the class, Identifier.</skos:editorialNote>
		<skos:editorialNote>TODO: make a superproperty of fibo-fnd-rel-rel:hasUniqueIdentifier</skos:editorialNote>
	</owl:DatatypeProperty>
	
	<owl:ObjectProperty rdf:about="&fibo-ln-ln-up;instantiates">
		<rdfs:label>instantiates</rdfs:label>
		<skos:definition>Iis an instantiation of e.g. a template, offer or form.</skos:definition>
	</owl:ObjectProperty>
	
	<owl:ObjectProperty rdf:about="&fibo-ln-ln-up;isEvidencedBy_g">
		<rdfs:label>is evidenced by (g)</rdfs:label>
		<skos:definition>A more generic version of the property in the contracts ontology which has domain:WrittenContract and range ContractDocument.</skos:definition>
	</owl:ObjectProperty>
	
	<owl:ObjectProperty rdf:about="&fibo-ln-ln-up;opty-isGuaranteedBy">
		<rdfs:label>is guaranteed by</rdfs:label>
	</owl:ObjectProperty>
	
	<owl:Class rdf:about="&fibo-ln-ln-up;pas-LineItem">
		<rdfs:subClassOf rdf:resource="&fibo-ln-ln-up;Specification"/>
		<rdfs:subClassOf>
			<owl:Restriction>
				<owl:onProperty rdf:resource="&fibo-ln-ln-up;pas-hasUnitCost"/>
				<owl:onClass rdf:resource="&fibo-fnd-acc-cur;MonetaryAmount"/>
				<owl:minQualifiedCardinality rdf:datatype="&xsd;nonNegativeInteger">0</owl:minQualifiedCardinality>
			</owl:Restriction>
		</rdfs:subClassOf>
		<rdfs:subClassOf>
			<owl:Restriction>
				<owl:onProperty rdf:resource="&fibo-fnd-dt-fd;hasCount"/>
				<owl:minQualifiedCardinality rdf:datatype="&xsd;nonNegativeInteger">0</owl:minQualifiedCardinality>
				<owl:onDataRange rdf:resource="&xsd;positiveInteger"/>
			</owl:Restriction>
		</rdfs:subClassOf>
		<rdfs:subClassOf>
			<owl:Restriction>
				<owl:onProperty rdf:resource="&fibo-fnd-rel-rel;has"/>
				<owl:someValuesFrom>
					<owl:Class>
						<owl:unionOf rdf:parseType="Collection">
							<rdf:Description rdf:about="&fibo-fnd-pas-pas;Product">
							</rdf:Description>
							<rdf:Description rdf:about="&fibo-ln-ln-up;ChargeCategory">
							</rdf:Description>
						</owl:unionOf>
					</owl:Class>
				</owl:someValuesFrom>
			</owl:Restriction>
		</rdfs:subClassOf>
		<rdfs:subClassOf>
			<owl:Restriction>
				<owl:onProperty rdf:resource="&fibo-ln-ln-up;pas-hasCost"/>
				<owl:someValuesFrom rdf:resource="&fibo-fnd-acc-cur;MonetaryAmount"/>
			</owl:Restriction>
		</rdfs:subClassOf>
		<rdfs:label>line item</rdfs:label>
		<skos:definition>A description of a product or service including its unit cost, number of units and total cost.</skos:definition>
	</owl:Class>
	
	<owl:Class rdf:about="&fibo-ln-ln-up;pas-MarketCategory">
		<rdfs:subClassOf rdf:resource="&fibo-fnd-arr-cls;Classifier"/>
		<rdfs:label>market category</rdfs:label>
		<skos:definition>Specifies the market domain in which a product is offered.</skos:definition>
	</owl:Class>
	
	<owl:Class rdf:about="&fibo-ln-ln-up;pas-Offer">
		<rdfs:subClassOf rdf:resource="&fibo-fnd-agr-agr;Commitment"/>
		<rdfs:label>offer</rdfs:label>
		<skos:definition>A commitment to provide a product or service for an agreed price, if a buyer comes along.</skos:definition>
		<skos:editorialNote>TODO: model this out properly, add to products and services ontology.</skos:editorialNote>
	</owl:Class>
	
	<owl:ObjectProperty rdf:about="&fibo-ln-ln-up;pas-hasChargeCategory">
		<rdfs:subPropertyOf rdf:resource="&fibo-fnd-rel-rel;has"/>
	</owl:ObjectProperty>
	
	<owl:ObjectProperty rdf:about="&fibo-ln-ln-up;pas-hasCost">
		<rdfs:subPropertyOf rdf:resource="&fibo-ln-ln-up;cur-hasAmount"/>
		<skos:definition>Relates an item to its cost, it can entail adding up other costs (e.g. 4 units * a unit price)</skos:definition>
	</owl:ObjectProperty>
	
	<owl:ObjectProperty rdf:about="&fibo-ln-ln-up;pas-hasProduct">
		<rdfs:subPropertyOf rdf:resource="&fibo-fnd-rel-rel;has"/>
	</owl:ObjectProperty>
	
	<owl:ObjectProperty rdf:about="&fibo-ln-ln-up;pas-hasUnitCost">
	</owl:ObjectProperty>
	
	<owl:ObjectProperty rdf:about="&fibo-ln-ln-up;pas-hasUnitPrice">
		<rdfs:subPropertyOf rdf:resource="&fibo-ln-ln-up;cur-hasAmount"/>
		<skos:definition>Relates an item to its unit cost</skos:definition>
	</owl:ObjectProperty>
	
	<owl:ObjectProperty rdf:about="&fibo-ln-ln-up;performedBy">
		<rdfs:subPropertyOf rdf:resource="&fibo-ln-ln-up;hasParticipant"/>
		<skos:definition>Relates an Occurrence to a party that fully or partially performs the activity or process corresponding to the Occurrence.  Eg. who performed an Inspection.</skos:definition>
	</owl:ObjectProperty>
	
	<owl:Class rdf:about="&fibo-ln-ln-up;pty-CreditReportingAgency_I">
		<rdfs:subClassOf rdf:resource="&fibo-fnd-pty-pty;IndependentParty"/>
		<skos:definition>This is the independent party, not the party in role</skos:definition>
		<skos:editorialNote>Lynn: todo</skos:editorialNote>
	</owl:Class>
	
	<owl:Class rdf:about="&fibo-ln-ln-up;pty-CreditRepository_I">
		<rdfs:subClassOf rdf:resource="&fibo-fnd-pty-pty;IndependentParty"/>
		<skos:definition>This is the independent party, not the party in role</skos:definition>
		<skos:editorialNote>Lynn: todo</skos:editorialNote>
	</owl:Class>
	
	<owl:ObjectProperty rdf:about="&fibo-ln-ln-up;pty-IndependentParty">
		<rdfs:label>pty-independent party</rdfs:label>
	</owl:ObjectProperty>
	
	<owl:DatatypeProperty rdf:about="&fibo-ln-ln-up;rel-hasCount">
		<rdfs:label>has count</rdfs:label>
		<rdfs:range rdf:resource="&xsd;positiveInteger"/>
		<skos:definition>The count of the number of something, e.g. entries in a schedule.</skos:definition>
		<skos:editorialNote>fibo-fnd-dt-fd:hasCount should probably be replaced with this more generic version, or if not made a subproperty of it.</skos:editorialNote>
	</owl:DatatypeProperty>
	
	<owl:DatatypeProperty rdf:about="&fibo-ln-ln-up;rel-hasVersion">
		<rdfs:label>has version</rdfs:label>
		<rdfs:range rdf:resource="&xsd;string"/>
		<skos:definition>Indicates the version for something.</skos:definition>
	</owl:DatatypeProperty>
	
	<owl:ObjectProperty rdf:about="&fibo-ln-ln-up;rel-isFrom">
		<rdfs:label>is from</rdfs:label>
		<skos:definition>Relates something to a source or origin., e.g. the agent originating a request.</skos:definition>
	</owl:ObjectProperty>
	
	<owl:ObjectProperty rdf:about="&fibo-ln-ln-up;rel-isOf">
		<rdfs:label>os of</rdfs:label>
		<owl:inverseOf rdf:resource="&fibo-fnd-rel-rel;has"/>
		<skos:definition>Inverse of fibo-fnd-rel-rel:has</skos:definition>
		<skos:editorialNote></skos:editorialNote>
	</owl:ObjectProperty>
	
	<owl:ObjectProperty rdf:about="&fibo-ln-ln-up;rel-isProducedBy_I">
		<rdfs:label>is produced by (i)</rdfs:label>
		<owl:inverseOf rdf:resource="&fibo-ln-ln-up;rel-produces_I"/>
		<skos:definition>Indicates who or what produced something.</skos:definition>
		<skos:editorialNote>Ideally, this would be a superproperty of pas:isProducedBy in products and services ontology, but that is reserved for use with ThingInRole.  This property is therefore a superproperty of an unnamed property chain from the thing produced  to the independent producing thing that goes through an instance of a class that means PartyInProducerRole.</skos:editorialNote>
	</owl:ObjectProperty>
	
	<owl:ObjectProperty rdf:about="&fibo-ln-ln-up;rel-isSubmittedBy">
		<rdfs:label>is submitted by</rdfs:label>
		<rdfs:range rdf:resource="&fibo-fnd-aap-agt;AutonomousAgent"/>
		<skos:definition>Relates a Report to the Agent that is providing the Report</skos:definition>
		<skos:editorialNote>Ideally, this would be a subproperty of isProvidedBy, but that is reserved for use with ThingInRole.  This property is therefore a subproperty of an unnamed property chain from the thing submitted to the submitting  institution that goes through an instance of a class that means PartyInProviderRole.</skos:editorialNote>
	</owl:ObjectProperty>
	
	<owl:ObjectProperty rdf:about="&fibo-ln-ln-up;rel-isSubmittedTo">
		<rdfs:label>is submitted to</rdfs:label>
		<rdfs:range rdf:resource="&fibo-fnd-aap-agt;AutonomousAgent"/>
		<skos:definition>Relates a Report to the Agent that is receiving the Report</skos:definition>
	</owl:ObjectProperty>
	
	<owl:ObjectProperty rdf:about="&fibo-ln-ln-up;rel-isTo">
		<rdfs:label>is to</rdfs:label>
		<skos:definition>Relates something to a target or destination., e.g. the agent receiving a request.</skos:definition>
	</owl:ObjectProperty>
	
	<owl:ObjectProperty rdf:about="&fibo-ln-ln-up;rel-produces_I">
		<rdfs:label>produces (i)</rdfs:label>
	</owl:ObjectProperty>
	
	<owl:ObjectProperty rdf:about="&fibo-ln-ln-up;rel-uses_g">
		<skos:definition>Indicates who or what produced something.</skos:definition>
		<skos:editorialNote>Check to see if this is still used.</skos:editorialNote>
		<skos:editorialNote>This is a generic version of the fibo-fnd-rel-rel:uses property whose domain is too narrow.  If they fix it, this should be chagned to fibo-fnd-rel-rel:uses.</skos:editorialNote>
	</owl:ObjectProperty>
	
	<owl:ObjectProperty rdf:about="&fibo-ln-ln-up;thingBeingValued">
		<rdfs:label>thing being valued</rdfs:label>
	</owl:ObjectProperty>
	
	<owl:ObjectProperty rdf:about="&fibo-ln-ln-up;worksFor">
		<rdfs:label>works for</rdfs:label>
		<rdfs:domain rdf:resource="&fibo-fnd-aap-ppl;LegallyCapablePerson"/>
		<rdfs:range rdf:resource="&fibo-fnd-pty-pty;IndependentParty"/>
		<skos:definition>Indicates that a person works for some other person or company. Different arrangements are possible, e.g. employee or contractor.</skos:definition>
	</owl:ObjectProperty>

</rdf:RDF>