<?xml version="1.0" encoding="UTF-8"?>
<!DOCTYPE rdf:RDF [
	<!ENTITY dct "http://purl.org/dc/terms/">
	<!ENTITY fibo-be-le-fbo "https://spec.edmcouncil.org/fibo/BE/LegalEntities/FormalBusinessOrganizations/">
	<!ENTITY fibo-be-le-lei "https://spec.edmcouncil.org/fibo/BE/LegalEntities/LEIEntities/">
	<!ENTITY fibo-be-le-lp "https://spec.edmcouncil.org/fibo/BE/LegalEntities/LegalPersons/">
	<!ENTITY fibo-be-oac-opty "https://spec.edmcouncil.org/fibo/BE/OwnershipAndControl/OwnershipParties/">
	<!ENTITY fibo-fbc-dae-dbt "https://spec.edmcouncil.org/fibo/FBC/DebtAndEquities/Debt/">
	<!ENTITY fibo-fbc-fct-breg "https://spec.edmcouncil.org/fibo/FBC/FunctionalEntities/BusinessRegistries/">
	<!ENTITY fibo-fbc-fct-rga "https://spec.edmcouncil.org/fibo/FBC/FunctionalEntities/RegulatoryAgencies/">
	<!ENTITY fibo-fbc-fi-fi "https://spec.edmcouncil.org/fibo/FBC/FinancialInstruments/FinancialInstruments/">
	<!ENTITY fibo-fbc-pas-caa "https://spec.edmcouncil.org/fibo/FBC/ProductsAndServices/ClientsAndAccounts/">
	<!ENTITY fibo-fbc-pas-fpas "https://spec.edmcouncil.org/fibo/FBC/ProductsAndServices/FinancialProductsAndServices/">
	<!ENTITY fibo-fnd-aap-agt "https://spec.edmcouncil.org/fibo/FND/AgentsAndPeople/Agents/">
	<!ENTITY fibo-fnd-aap-ppl "https://spec.edmcouncil.org/fibo/FND/AgentsAndPeople/People/">
	<!ENTITY fibo-fnd-acc-cur "https://spec.edmcouncil.org/fibo/FND/Accounting/CurrencyAmount/">
	<!ENTITY fibo-fnd-agr-agr "https://spec.edmcouncil.org/fibo/FND/Agreements/Agreements/">
	<!ENTITY fibo-fnd-agr-ctr "https://spec.edmcouncil.org/fibo/FND/Agreements/Contracts/">
	<!ENTITY fibo-fnd-arr-arr "https://spec.edmcouncil.org/fibo/FND/Arrangements/Arrangements/">
	<!ENTITY fibo-fnd-arr-cls "https://spec.edmcouncil.org/fibo/FND/Arrangements/ClassificationSchemes/">
	<!ENTITY fibo-fnd-arr-doc "https://spec.edmcouncil.org/fibo/FND/Arrangements/Documents/">
	<!ENTITY fibo-fnd-arr-id "https://spec.edmcouncil.org/fibo/FND/Arrangements/IdentifiersAndIndices/">
	<!ENTITY fibo-fnd-dt-fd "https://spec.edmcouncil.org/fibo/FND/DatesAndTimes/FinancialDates/">
	<!ENTITY fibo-fnd-dt-oc "https://spec.edmcouncil.org/fibo/FND/DatesAndTimes/Occurrences/">
	<!ENTITY fibo-fnd-oac-own "https://spec.edmcouncil.org/fibo/FND/OwnershipAndControl/Ownership/">
	<!ENTITY fibo-fnd-org-fm "https://spec.edmcouncil.org/fibo/FND/Organizations/FormalOrganizations/">
	<!ENTITY fibo-fnd-org-org "https://spec.edmcouncil.org/fibo/FND/Organizations/Organizations/">
	<!ENTITY fibo-fnd-pas-pas "https://spec.edmcouncil.org/fibo/FND/ProductsAndServices/ProductsAndServices/">
	<!ENTITY fibo-fnd-pas-psch "https://spec.edmcouncil.org/fibo/FND/ProductsAndServices/PaymentsAndSchedules/">
	<!ENTITY fibo-fnd-plc-adr "https://spec.edmcouncil.org/fibo/FND/Places/Addresses/">
	<!ENTITY fibo-fnd-plc-cty "https://spec.edmcouncil.org/fibo/FND/Places/Countries/">
	<!ENTITY fibo-fnd-plc-loc "https://spec.edmcouncil.org/fibo/FND/Places/Locations/">
	<!ENTITY fibo-fnd-pty-pty "https://spec.edmcouncil.org/fibo/FND/Parties/Parties/">
	<!ENTITY fibo-fnd-qt-qtu "https://spec.edmcouncil.org/fibo/FND/Quantities/QuantitiesAndUnits/">
	<!ENTITY fibo-fnd-rel-rel "https://spec.edmcouncil.org/fibo/FND/Relations/Relations/">
	<!ENTITY fibo-fnd-utl-av "https://spec.edmcouncil.org/fibo/FND/Utilities/AnnotationVocabulary/">
	<!ENTITY fibo-fnd-utl-bt "https://spec.edmcouncil.org/fibo/FND/Utilities/BusinessFacingTypes/">
	<!ENTITY fibo-ind-ei-ei "https://spec.edmcouncil.org/fibo/IND/EconomicIndicators/EconomicIndicators/">
	<!ENTITY fibo-ind-ir-ir "https://spec.edmcouncil.org/fibo/IND/InterestRates/InterestRates/">
	<!ENTITY fibo-ln-ln-up "https://spec.edmcouncil.org/fibo/LOAN/LoanContracts/LoanUpperTemp/">
	<!ENTITY loan "https://spec.edmcouncil.org/fibo/LOAN/LoanContracts/LoanCore/">
	<!ENTITY owl "http://www.w3.org/2002/07/owl#">
	<!ENTITY rdf "http://www.w3.org/1999/02/22-rdf-syntax-ns#">
	<!ENTITY rdfs "http://www.w3.org/2000/01/rdf-schema#">
	<!ENTITY skos "http://www.w3.org/2004/02/skos/core#">
	<!ENTITY sm "http://www.omg.org/techprocess/ab/SpecificationMetadata/">
	<!ENTITY xsd "http://www.w3.org/2001/XMLSchema#">
]>
<rdf:RDF xml:base="https://spec.edmcouncil.org/fibo/LOAN/LoanContracts/LoanUpperTemp/"
	xmlns="https://spec.edmcouncil.org/fibo/LOAN/LoanContracts/LoanUpperTemp/"
	xmlns:dct="http://purl.org/dc/terms/"
	xmlns:fibo-be-le-fbo="https://spec.edmcouncil.org/fibo/BE/LegalEntities/FormalBusinessOrganizations/"
	xmlns:fibo-be-le-lei="https://spec.edmcouncil.org/fibo/BE/LegalEntities/LEIEntities/"
	xmlns:fibo-be-le-lp="https://spec.edmcouncil.org/fibo/BE/LegalEntities/LegalPersons/"
	xmlns:fibo-be-oac-opty="https://spec.edmcouncil.org/fibo/BE/OwnershipAndControl/OwnershipParties/"
	xmlns:fibo-fbc-dae-dbt="https://spec.edmcouncil.org/fibo/FBC/DebtAndEquities/Debt/"
	xmlns:fibo-fbc-fct-breg="https://spec.edmcouncil.org/fibo/FBC/FunctionalEntities/BusinessRegistries/"
	xmlns:fibo-fbc-fct-rga="https://spec.edmcouncil.org/fibo/FBC/FunctionalEntities/RegulatoryAgencies/"
	xmlns:fibo-fbc-fi-fi="https://spec.edmcouncil.org/fibo/FBC/FinancialInstruments/FinancialInstruments/"
	xmlns:fibo-fbc-pas-caa="https://spec.edmcouncil.org/fibo/FBC/ProductsAndServices/ClientsAndAccounts/"
	xmlns:fibo-fbc-pas-fpas="https://spec.edmcouncil.org/fibo/FBC/ProductsAndServices/FinancialProductsAndServices/"
	xmlns:fibo-fnd-aap-agt="https://spec.edmcouncil.org/fibo/FND/AgentsAndPeople/Agents/"
	xmlns:fibo-fnd-aap-ppl="https://spec.edmcouncil.org/fibo/FND/AgentsAndPeople/People/"
	xmlns:fibo-fnd-acc-cur="https://spec.edmcouncil.org/fibo/FND/Accounting/CurrencyAmount/"
	xmlns:fibo-fnd-agr-agr="https://spec.edmcouncil.org/fibo/FND/Agreements/Agreements/"
	xmlns:fibo-fnd-agr-ctr="https://spec.edmcouncil.org/fibo/FND/Agreements/Contracts/"
	xmlns:fibo-fnd-arr-arr="https://spec.edmcouncil.org/fibo/FND/Arrangements/Arrangements/"
	xmlns:fibo-fnd-arr-cls="https://spec.edmcouncil.org/fibo/FND/Arrangements/ClassificationSchemes/"
	xmlns:fibo-fnd-arr-doc="https://spec.edmcouncil.org/fibo/FND/Arrangements/Documents/"
	xmlns:fibo-fnd-arr-id="https://spec.edmcouncil.org/fibo/FND/Arrangements/IdentifiersAndIndices/"
	xmlns:fibo-fnd-dt-fd="https://spec.edmcouncil.org/fibo/FND/DatesAndTimes/FinancialDates/"
	xmlns:fibo-fnd-dt-oc="https://spec.edmcouncil.org/fibo/FND/DatesAndTimes/Occurrences/"
	xmlns:fibo-fnd-oac-own="https://spec.edmcouncil.org/fibo/FND/OwnershipAndControl/Ownership/"
	xmlns:fibo-fnd-org-fm="https://spec.edmcouncil.org/fibo/FND/Organizations/FormalOrganizations/"
	xmlns:fibo-fnd-org-org="https://spec.edmcouncil.org/fibo/FND/Organizations/Organizations/"
	xmlns:fibo-fnd-pas-pas="https://spec.edmcouncil.org/fibo/FND/ProductsAndServices/ProductsAndServices/"
	xmlns:fibo-fnd-pas-psch="https://spec.edmcouncil.org/fibo/FND/ProductsAndServices/PaymentsAndSchedules/"
	xmlns:fibo-fnd-plc-adr="https://spec.edmcouncil.org/fibo/FND/Places/Addresses/"
	xmlns:fibo-fnd-plc-cty="https://spec.edmcouncil.org/fibo/FND/Places/Countries/"
	xmlns:fibo-fnd-plc-loc="https://spec.edmcouncil.org/fibo/FND/Places/Locations/"
	xmlns:fibo-fnd-pty-pty="https://spec.edmcouncil.org/fibo/FND/Parties/Parties/"
	xmlns:fibo-fnd-qt-qtu="https://spec.edmcouncil.org/fibo/FND/Quantities/QuantitiesAndUnits/"
	xmlns:fibo-fnd-rel-rel="https://spec.edmcouncil.org/fibo/FND/Relations/Relations/"
	xmlns:fibo-fnd-utl-av="https://spec.edmcouncil.org/fibo/FND/Utilities/AnnotationVocabulary/"
	xmlns:fibo-fnd-utl-bt="https://spec.edmcouncil.org/fibo/FND/Utilities/BusinessFacingTypes/"
	xmlns:fibo-ind-ei-ei="https://spec.edmcouncil.org/fibo/IND/EconomicIndicators/EconomicIndicators/"
	xmlns:fibo-ind-ir-ir="https://spec.edmcouncil.org/fibo/IND/InterestRates/InterestRates/"
	xmlns:fibo-ln-ln-up="https://spec.edmcouncil.org/fibo/LOAN/LoanContracts/LoanUpperTemp/"
	xmlns:loan="https://spec.edmcouncil.org/fibo/LOAN/LoanContracts/LoanCore/"
	xmlns:owl="http://www.w3.org/2002/07/owl#"
	xmlns:rdf="http://www.w3.org/1999/02/22-rdf-syntax-ns#"
	xmlns:rdfs="http://www.w3.org/2000/01/rdf-schema#"
	xmlns:skos="http://www.w3.org/2004/02/skos/core#"
	xmlns:sm="http://www.omg.org/techprocess/ab/SpecificationMetadata/"
	xmlns:xsd="http://www.w3.org/2001/XMLSchema#">
	
	<owl:Ontology rdf:about="https://spec.edmcouncil.org/fibo/LOAN/LoanContracts/LoanUpperTemp/">
		<rdfs:label>Loan Upper Temp Ontology</rdfs:label>
		<owl:imports rdf:resource="http://www.omg.org/techprocess/ab/SpecificationMetadata/"/>
		<owl:imports rdf:resource="http://www.w3.org/2004/02/skos/core"/>
		<owl:imports rdf:resource="https://spec.edmcouncil.org/fibo/BE/OwnershipAndControl/OwnershipParties/"/>
		<owl:imports rdf:resource="https://spec.edmcouncil.org/fibo/FBC/20150801/FunctionalEntities/BusinessRegistries/"/>
		<owl:imports rdf:resource="https://spec.edmcouncil.org/fibo/FND/20160201/ProductsAndServices/PaymentsAndSchedules/"/>
		<owl:imports rdf:resource="https://spec.edmcouncil.org/fibo/FND/Accounting/CurrencyAmount/"/>
		<owl:imports rdf:resource="https://spec.edmcouncil.org/fibo/FND/AgentsAndPeople/Agents/"/>
		<owl:imports rdf:resource="https://spec.edmcouncil.org/fibo/FND/AgentsAndPeople/People/"/>
		<owl:imports rdf:resource="https://spec.edmcouncil.org/fibo/FND/Agreements/Agreements/"/>
		<owl:imports rdf:resource="https://spec.edmcouncil.org/fibo/FND/Agreements/Contracts/"/>
		<owl:imports rdf:resource="https://spec.edmcouncil.org/fibo/FND/Arrangements/Arrangements/"/>
		<owl:imports rdf:resource="https://spec.edmcouncil.org/fibo/FND/Arrangements/ClassificationSchemes/"/>
		<owl:imports rdf:resource="https://spec.edmcouncil.org/fibo/FND/DatesAndTimes/FinancialDates/"/>
		<owl:imports rdf:resource="https://spec.edmcouncil.org/fibo/FND/DatesAndTimes/Occurrences/"/>
		<owl:imports rdf:resource="https://spec.edmcouncil.org/fibo/FND/Organizations/FormalOrganizations/"/>
		<owl:imports rdf:resource="https://spec.edmcouncil.org/fibo/FND/Parties/Parties/"/>
		<owl:imports rdf:resource="https://spec.edmcouncil.org/fibo/FND/Places/Addresses/"/>
		<owl:imports rdf:resource="https://spec.edmcouncil.org/fibo/FND/Places/Countries/"/>
		<owl:imports rdf:resource="https://spec.edmcouncil.org/fibo/FND/Places/Locations/"/>
		<owl:imports rdf:resource="https://spec.edmcouncil.org/fibo/FND/ProductsAndServices/ProductsAndServices/"/>
		<owl:imports rdf:resource="https://spec.edmcouncil.org/fibo/FND/Relations/Relations/"/>
		<owl:imports rdf:resource="https://spec.edmcouncil.org/fibo/FND/Utilities/AnnotationVocabulary/"/>
		<owl:imports rdf:resource="https://spec.edmcouncil.org/fibo/FND/Utilities/Values/"/>
		<owl:imports rdf:resource="https://spec.edmcouncil.org/fibo/IND/EconomicIndicators/EconomicIndicators/"/>
		<owl:versionInfo>Created with e6Tools Graphical OWL Editor from D:\SEMANTIC-ARTS\NAS\ClientsAndPartners\EDM Council\fibo ontologies\LoanOntology\loans.vsdx Page:loanUpper</owl:versionInfo>
	</owl:Ontology>
	
	<rdf:Description rdf:about="&fibo-fbc-dae-dbt;hasOutstandingAmount">
		<fibo-fnd-utl-av:synonym>has actual unpaid balance</fibo-fnd-utl-av:synonym>
	</rdf:Description>
	
	<owl:ObjectProperty rdf:about="&fibo-fbc-fct-breg;isSubdivisionOf">
		<owl:inverseOf rdf:resource="&fibo-fbc-fct-breg;hasSubdivision"/>
		<skos:editorialNote>This should be added to the BusinessRegistries ontology</skos:editorialNote>
	</owl:ObjectProperty>
	
	<owl:Class rdf:about="&fibo-fnd-agr-agr;Agreement">
		<rdfs:subClassOf rdf:resource="&fibo-ln-ln-up;Specification"/>
	</owl:Class>
	
	<owl:Class rdf:about="&fibo-fnd-agr-agr;Commitment">
		<rdfs:subClassOf rdf:resource="&fibo-ln-ln-up;Specification"/>
	</owl:Class>
	
	<owl:ObjectProperty rdf:about="&fibo-fnd-agr-ctr;hasEffectiveDate">
		<rdfs:subPropertyOf rdf:resource="&fibo-ln-ln-up;hasAsOfDate"/>
	</owl:ObjectProperty>
	
	<owl:ObjectProperty rdf:about="&fibo-fnd-rel-rel;isComprisedOf">
		<owl:inverseOf rdf:resource="&fibo-fnd-rel-rel;comprises"/>
		<skos:editorialNote>Topic: FND Adding inverse of comprises called isComprisedOf</skos:editorialNote>
	</owl:ObjectProperty>
	
	<owl:AnnotationProperty rdf:about="&fibo-fnd-utl-av;editorialNote">
	</owl:AnnotationProperty>
	
	<fibo-fnd-dt-fd:ExplicitDuration rdf:about="&fibo-ind-ir-ir;OneHundredEightyMonths">
		<rdf:type rdf:resource="&owl;NamedIndividual"/>
		<rdfs:label>one hundred eighty months</rdfs:label>
		<skos:definition>a duration of exactly one hundred eighty (180) months, regardless of the length in days of a given calendar month, but typically 30 days</skos:definition>
		<fibo-fnd-dt-fd:hasDurationValue>P180M</fibo-fnd-dt-fd:hasDurationValue>
	</fibo-fnd-dt-fd:ExplicitDuration>
	
	<fibo-fnd-dt-fd:ExplicitDuration rdf:about="&fibo-ind-ir-ir;ThreeHundredSixtyMonths">
		<rdf:type rdf:resource="&owl;NamedIndividual"/>
		<rdfs:label>three hundred sixty months</rdfs:label>
		<skos:definition>a duration of exactly three hundred sixty (360) months, regardless of the length in days of a given calendar month, but typically 30 days</skos:definition>
		<fibo-fnd-dt-fd:hasDurationValue>P360M</fibo-fnd-dt-fd:hasDurationValue>
	</fibo-fnd-dt-fd:ExplicitDuration>
	
	<owl:Class rdf:about="&fibo-ln-ln-up;Application">
		<rdfs:subClassOf rdf:resource="&fibo-ln-ln-up;fnd-Request"/>
		<rdfs:subClassOf>
			<owl:Restriction>
				<owl:onProperty rdf:resource="&fibo-ln-ln-up;hasDateReceived"/>
				<owl:someValuesFrom rdf:resource="&fibo-fnd-dt-fd;Date"/>
			</owl:Restriction>
		</rdfs:subClassOf>
		<rdfs:label>application</rdfs:label>
		<skos:definition>a request submitted by an applicant to receive something (e.g. a licence, a loan, a membership) accompanied by documentation of pertinent information to determine whether the request should be granted</skos:definition>
	</owl:Class>
	
	<owl:Class rdf:about="&fibo-ln-ln-up;BE-ContactPurpose">
		<rdfs:subClassOf rdf:resource="&fibo-fnd-arr-cls;Classifier"/>
		<rdfs:label>contact purpose</rdfs:label>
		<skos:definition>a virtual address for communication via phone</skos:definition>
	</owl:Class>
	
	<owl:Class rdf:about="&fibo-ln-ln-up;ChargeCategory">
		<rdfs:subClassOf rdf:resource="&fibo-fnd-arr-cls;Classifier"/>
		<rdfs:label>charge cateogry</rdfs:label>
		<skos:definition>a category indicating what a charge is for (e.g. closing costs, interest)</skos:definition>
		<fibo-fnd-utl-av:usageNote>Use with LineItem, (has ChargeCategory instance), (hasNumericalValue for number of units) and (hasCost for the amount of money)</fibo-fnd-utl-av:usageNote>
	</owl:Class>
	
	<owl:Class rdf:about="&fibo-ln-ln-up;ContactInfo">
		<rdfs:subClassOf>
			<owl:Restriction>
				<owl:onProperty rdf:resource="&fibo-fnd-rel-rel;comprises"/>
				<owl:onClass rdf:resource="&fibo-fnd-aap-ppl;LegallyCapableAdult"/>
				<owl:minQualifiedCardinality rdf:datatype="&xsd;nonNegativeInteger">0</owl:minQualifiedCardinality>
			</owl:Restriction>
		</rdfs:subClassOf>
		<rdfs:subClassOf>
			<owl:Restriction>
				<owl:onProperty rdf:resource="&fibo-fnd-rel-rel;comprises"/>
				<owl:onClass rdf:resource="&fibo-fnd-org-fm;FormalOrganization"/>
				<owl:minQualifiedCardinality rdf:datatype="&xsd;nonNegativeInteger">0</owl:minQualifiedCardinality>
			</owl:Restriction>
		</rdfs:subClassOf>
		<rdfs:subClassOf>
			<owl:Restriction>
				<owl:onProperty rdf:resource="&fibo-fnd-rel-rel;comprises"/>
				<owl:onClass rdf:resource="&fibo-fnd-plc-adr;PostalAddress"/>
				<owl:minQualifiedCardinality rdf:datatype="&xsd;nonNegativeInteger">0</owl:minQualifiedCardinality>
			</owl:Restriction>
		</rdfs:subClassOf>
		<rdfs:subClassOf>
			<owl:Restriction>
				<owl:onProperty rdf:resource="&fibo-fnd-rel-rel;comprises"/>
				<owl:onClass rdf:resource="&fibo-ln-ln-up;adr-EmailAddress"/>
				<owl:minQualifiedCardinality rdf:datatype="&xsd;nonNegativeInteger">0</owl:minQualifiedCardinality>
			</owl:Restriction>
		</rdfs:subClassOf>
		<rdfs:subClassOf>
			<owl:Restriction>
				<owl:onProperty rdf:resource="&fibo-fnd-rel-rel;comprises"/>
				<owl:onClass rdf:resource="&fibo-ln-ln-up;adr-PhoneNumber"/>
				<owl:minQualifiedCardinality rdf:datatype="&xsd;nonNegativeInteger">0</owl:minQualifiedCardinality>
			</owl:Restriction>
		</rdfs:subClassOf>
		<rdfs:subClassOf>
			<owl:Restriction>
				<owl:onProperty rdf:resource="&fibo-fnd-rel-rel;isClassifiedBy"/>
				<owl:someValuesFrom rdf:resource="&fibo-ln-ln-up;BE-ContactPurpose"/>
			</owl:Restriction>
		</rdfs:subClassOf>
		<rdfs:label>contact information</rdfs:label>
		<skos:definition>a way to make contact with a person or organization for a particular reason regarding something.  The details may be role-specific, so the information cannot always go on the individual or organization</skos:definition>
		<skos:editorialNote>This approach avoids the need to have multiple properties to connect different things to ContactInfo use for different purposes.</skos:editorialNote>
		<skos:editorialNote>Topic: BE</skos:editorialNote>
		<fibo-fnd-utl-av:usageNote>Make sure to check the existing instances of ContactPurpose and use those before creating new ones.</fibo-fnd-utl-av:usageNote>
	</owl:Class>
	
	<owl:Class rdf:about="&fibo-ln-ln-up;FND-InformationProduct">
		<rdfs:subClassOf rdf:resource="&fibo-fnd-pas-pas;Product"/>
		<rdfs:label>information product</rdfs:label>
		<skos:definition>a product that is informational in nature, rather than physical</skos:definition>
	</owl:Class>
	
	<owl:Class rdf:about="&fibo-ln-ln-up;MetropolitanDivision">
		<rdfs:subClassOf rdf:resource="&fibo-fnd-plc-cty;GeopoliticalEntity"/>
		<rdfs:subClassOf>
			<owl:Restriction>
				<owl:onProperty rdf:resource="&fibo-fbc-fct-breg;isSubdivisionOf"/>
				<owl:someValuesFrom rdf:resource="&fibo-ind-ei-ei;MetropolitanStatisticalArea"/>
			</owl:Restriction>
		</rdfs:subClassOf>
		<rdfs:label>metropolitan division</rdfs:label>
		<skos:definition>an area specified by the government to describe a subsection of a certain metropolitan statistical area</skos:definition>
		<skos:editorialNote>Topic: Regions</skos:editorialNote>
		<fibo-fnd-utl-av:abbreviation>MD</fibo-fnd-utl-av:abbreviation>
		<fibo-fnd-utl-av:adaptedFrom>https://www.forbes.com/2009/10/01/cities-census-metro-lifestyle-metropolitan-statistical-area.html</fibo-fnd-utl-av:adaptedFrom>
		<fibo-fnd-utl-av:explanatoryNote>In the US, this is governed by the Census Department.</fibo-fnd-utl-av:explanatoryNote>
	</owl:Class>
	
	<owl:Class rdf:about="&fibo-ln-ln-up;PaymentHistory">
		<rdfs:subClassOf rdf:resource="&fibo-fnd-arr-doc;Record"/>
		<rdfs:subClassOf>
			<owl:Restriction>
				<owl:onProperty rdf:resource="&fibo-fbc-dae-dbt;hasOutstandingAmount"/>
				<owl:someValuesFrom rdf:resource="&fibo-fnd-acc-cur;MonetaryAmount"/>
			</owl:Restriction>
		</rdfs:subClassOf>
		<rdfs:subClassOf>
			<owl:Restriction>
				<owl:onProperty rdf:resource="&fibo-fnd-rel-rel;hasMember"/>
				<owl:someValuesFrom rdf:resource="&fibo-fnd-pas-psch;Payment"/>
			</owl:Restriction>
		</rdfs:subClassOf>
		<rdfs:label>payment history</rdfs:label>
		<skos:definition>a record of actual payments of principal, interest, and other related amounts made by a borrower to a lender or servicer in order to fulfill their re-payment obligation</skos:definition>
		<skos:editorialNote>Topic: Payments</skos:editorialNote>
		<fibo-fnd-utl-av:explanatoryNote>Just like a PaymentSchedule except that the dates and amounts are actuals.</fibo-fnd-utl-av:explanatoryNote>
	</owl:Class>
	
	<owl:Class rdf:about="&fibo-ln-ln-up;PaymentSchedule">
		<rdfs:subClassOf rdf:resource="&fibo-fnd-dt-fd;Schedule"/>
		<rdfs:subClassOf>
			<owl:Restriction>
				<owl:onProperty rdf:resource="&fibo-fnd-rel-rel;hasMember"/>
				<owl:someValuesFrom rdf:resource="&fibo-ln-ln-up;ScheduledPayment"/>
			</owl:Restriction>
		</rdfs:subClassOf>
		<rdfs:label>payment schedule</rdfs:label>
		<skos:definition>a Schedule of amounts of principal and interest that are due over the term of the loan in order to fully pay off the obligation</skos:definition>
		<skos:editorialNote>Topic: Payments
Not using psch:PaymentSchedule because it uses PaymentEvent which is an OccurrenceKind which does not make sense. Also, it should use hasMember not comprises to put items into a Collection. Ripe for coagulation.</skos:editorialNote>
	</owl:Class>
	
	<owl:Class rdf:about="&fibo-ln-ln-up;Report">
		<rdfs:subClassOf>
			<owl:Restriction>
				<owl:onProperty rdf:resource="&fibo-ln-ln-up;rel-isProducedBy_I"/>
				<owl:onClass rdf:resource="&fibo-fnd-aap-agt;AutonomousAgent"/>
				<owl:minQualifiedCardinality rdf:datatype="&xsd;nonNegativeInteger">0</owl:minQualifiedCardinality>
			</owl:Restriction>
		</rdfs:subClassOf>
		<rdfs:subClassOf>
			<owl:Restriction>
				<owl:onProperty rdf:resource="&fibo-ln-ln-up;dt-fd-coversPeriod"/>
				<owl:onClass rdf:resource="&fibo-fnd-dt-fd;DatePeriod"/>
				<owl:minQualifiedCardinality rdf:datatype="&xsd;nonNegativeInteger">0</owl:minQualifiedCardinality>
			</owl:Restriction>
		</rdfs:subClassOf>
		<rdfs:subClassOf>
			<owl:Restriction>
				<owl:onProperty rdf:resource="&fibo-ln-ln-up;hasCreationDate"/>
				<owl:someValuesFrom rdf:resource="&fibo-fnd-dt-fd;Date"/>
			</owl:Restriction>
		</rdfs:subClassOf>
		<rdfs:label>report</rdfs:label>
		<sm:normativeReference>http://www.businessdictionary.com/definition/report.html</sm:normativeReference>
		<skos:definition>a body of information organized in a narrative, graphic, or tabular form, prepared on ad hoc, periodic, recurring, regular, or as required basis. Reports may refer to specific periods, events, occurrences, or subjects, and may be communicated or presented in oral or written form</skos:definition>
	</owl:Class>
	
	<owl:Class rdf:about="&fibo-ln-ln-up;ScheduledPayment">
		<rdfs:subClassOf rdf:resource="&fibo-fnd-dt-fd;AdHocScheduleEntry"/>
		<rdfs:subClassOf rdf:resource="&fibo-fnd-pas-psch;PaymentObligation"/>
		<rdfs:subClassOf>
			<owl:Restriction>
				<owl:onProperty rdf:resource="&fibo-fnd-pas-psch;hasPaymentAmount"/>
				<owl:someValuesFrom rdf:resource="&fibo-fnd-acc-cur;MonetaryAmount"/>
			</owl:Restriction>
		</rdfs:subClassOf>
		<rdfs:subClassOf>
			<owl:Restriction>
				<owl:onProperty rdf:resource="&fibo-ln-ln-up;hasScheduledUnpaidBalance"/>
				<owl:someValuesFrom rdf:resource="&fibo-fnd-acc-cur;MonetaryAmount"/>
			</owl:Restriction>
		</rdfs:subClassOf>
		<rdfs:label>scheduled payment</rdfs:label>
		<skos:definition>a scheduled payment occurrence that is part of a payment schedule covering the term of the loan</skos:definition>
		<skos:editorialNote>Topic: Payments</skos:editorialNote>
	</owl:Class>
	
	<owl:Class rdf:about="&fibo-ln-ln-up;Specification">
		<rdfs:label>specification</rdfs:label>
		<skos:definition>a body of information specifying what properties, structure and/or results something should or must have after it has been built, fulfilled or completed</skos:definition>
		<fibo-fnd-utl-av:explanatoryNote>The thing specified may be physical (a building), organizational (a management structure), computational (a program), job or task related (e.g., a CEO, Chief Judge) or changing oil in a car. It may be a set of characteristics saying what something must be, or a set of instructions saying how to do something.</fibo-fnd-utl-av:explanatoryNote>
	</owl:Class>
	
	<owl:Class rdf:about="&fibo-ln-ln-up;Valuation">
		<rdfs:subClassOf rdf:resource="&fibo-ln-ln-up;alx-Measurement"/>
		<rdfs:subClassOf>
			<owl:Restriction>
				<owl:onProperty rdf:resource="&fibo-ln-ln-up;isEvaluationOf"/>
				<owl:minCardinality rdf:datatype="&xsd;nonNegativeInteger">1</owl:minCardinality>
			</owl:Restriction>
		</rdfs:subClassOf>
		<rdfs:label>valuation</rdfs:label>
		<skos:definition>a measurement to assess the value of something expressed in some currency</skos:definition>
		<fibo-fnd-utl-av:editorialNote>Future consideration: move this to FND, perhaps to the analytics ontology (fibo-fnd-utl-alx).</fibo-fnd-utl-av:editorialNote>
	</owl:Class>
	
	<owl:Class rdf:about="&fibo-ln-ln-up;adr-EmailAddress">
		<rdfs:subClassOf rdf:resource="&fibo-fnd-plc-adr;VirtualAddress"/>
		<rdfs:subClassOf>
			<owl:Restriction>
				<owl:onProperty rdf:resource="https://spec.edmcouncil.org/fibo/FND/Utilities/Values/hasValue"/>
				<owl:someValuesFrom rdf:resource="&xsd;string"/>
			</owl:Restriction>
		</rdfs:subClassOf>
		<rdfs:label>email address</rdfs:label>
		<skos:definition>a virtual address for communication via email</skos:definition>
	</owl:Class>
	
	<owl:Class rdf:about="&fibo-ln-ln-up;adr-PhoneNumber">
		<rdfs:subClassOf rdf:resource="&fibo-fnd-plc-adr;VirtualAddress"/>
		<rdfs:subClassOf>
			<owl:Restriction>
				<owl:onProperty rdf:resource="https://spec.edmcouncil.org/fibo/FND/Utilities/Values/hasValue"/>
				<owl:someValuesFrom rdf:resource="&xsd;string"/>
			</owl:Restriction>
		</rdfs:subClassOf>
		<rdfs:label>phone number</rdfs:label>
		<skos:definition>a virtual address for communication via phone</skos:definition>
	</owl:Class>
	
	<owl:Class rdf:about="&fibo-ln-ln-up;alx-Measurement">
		<rdfs:subClassOf rdf:resource="&fibo-fnd-dt-oc;Occurrence"/>
		<rdfs:label>measurement</rdfs:label>
		<skos:definition>the act of measuring an aspect of something using some procedure giving a result typically expressed in some units (e.g. a valuation measuring the value of an asset expressedin USD)</skos:definition>
		<fibo-fnd-utl-av:explanatoryNote>Future consideration: move this to FND, perhaps to the analytics ontology (fibo-fnd-utl-alx).</fibo-fnd-utl-av:explanatoryNote>
	</owl:Class>
	
	<owl:ObjectProperty rdf:about="&fibo-ln-ln-up;conformsTo">
		<rdfs:label>conforms to</rdfs:label>
		<rdfs:range rdf:resource="&fibo-ln-ln-up;Specification"/>
		<skos:definition>relates something to a specification that it conforms to or complies with.</skos:definition>
		<fibo-fnd-utl-av:explanatoryNote>The specification need not causally affect that which conforms to it, hence it is not a subproperty of fibo-fnd-rel-rel:causes</fibo-fnd-utl-av:explanatoryNote>
	</owl:ObjectProperty>
	
	<owl:ObjectProperty rdf:about="&fibo-ln-ln-up;cur-hasEstimatedValue">
		<rdfs:subPropertyOf rdf:resource="&fibo-ln-ln-up;cur-hasMonetaryAmount"/>
		<rdfs:label>has estimated value</rdfs:label>
		<skos:definition>relates something to its estimated value</skos:definition>
	</owl:ObjectProperty>
	
	<owl:ObjectProperty rdf:about="&fibo-ln-ln-up;cur-hasMonetaryAmount">
		<rdfs:subPropertyOf rdf:resource="&fibo-fnd-rel-rel;has"/>
		<rdfs:label>has monetary amount</rdfs:label>
		<rdfs:range rdf:resource="&fibo-fnd-acc-cur;MonetaryAmount"/>
		<skos:definition>relates something to a monetary amount (e.g. credit limit, notional amount)</skos:definition>
		<fibo-fnd-utl-av:explanatoryNote>This could be a loan amount, or a limit for a credit line.</fibo-fnd-utl-av:explanatoryNote>
	</owl:ObjectProperty>
	
	<owl:ObjectProperty rdf:about="&fibo-ln-ln-up;dt-fd-coversPeriod">
		<rdfs:subPropertyOf rdf:resource="&fibo-fnd-dt-fd;hasDatePeriod"/>
		<rdfs:label>covers period</rdfs:label>
		<rdfs:range rdf:resource="&fibo-fnd-dt-fd;DatePeriod"/>
		<skos:definition>relates something to the period of time which it covers (e.g. for a report)</skos:definition>
	</owl:ObjectProperty>
	
	<owl:Class rdf:about="&fibo-ln-ln-up;fnd-Request">
		<rdfs:subClassOf rdf:resource="&fibo-fnd-dt-oc;Occurrence"/>
		<rdfs:subClassOf>
			<owl:Restriction>
				<owl:onProperty rdf:resource="&fibo-ln-ln-up;fnd-isRequestFor"/>
				<owl:minCardinality rdf:datatype="&xsd;nonNegativeInteger">1</owl:minCardinality>
			</owl:Restriction>
		</rdfs:subClassOf>
		<rdfs:subClassOf>
			<owl:Restriction>
				<owl:onProperty rdf:resource="&fibo-ln-ln-up;rel-isFrom"/>
				<owl:someValuesFrom rdf:resource="&fibo-fnd-aap-agt;AutonomousAgent"/>
			</owl:Restriction>
		</rdfs:subClassOf>
		<rdfs:subClassOf>
			<owl:Restriction>
				<owl:onProperty rdf:resource="&fibo-ln-ln-up;rel-isTo"/>
				<owl:someValuesFrom rdf:resource="&fibo-fnd-aap-agt;AutonomousAgent"/>
			</owl:Restriction>
		</rdfs:subClassOf>
		<rdfs:label>request</rdfs:label>
		<skos:definition>an occurrence whereby an agent asks another agent for something or to do something</skos:definition>
	</owl:Class>
	
	<owl:Class rdf:about="&fibo-ln-ln-up;fnd-RiskAssessment">
		<rdfs:subClassOf rdf:resource="&fibo-fnd-dt-oc;Occurrence"/>
		<rdfs:label>risk assessment</rdfs:label>
		<skos:definition>the occurrence of assessing the risk of something</skos:definition>
	</owl:Class>
	
	<owl:ObjectProperty rdf:about="&fibo-ln-ln-up;fnd-isRequestFor">
		<rdfs:subPropertyOf rdf:resource="&fibo-ln-ln-up;hasParticipant"/>
		<rdfs:label>is request for</rdfs:label>
		<skos:definition>relates a request to that which is being requested, e.g. a report</skos:definition>
	</owl:ObjectProperty>
	
	<owl:ObjectProperty rdf:about="&fibo-ln-ln-up;fnd-rel-isResponseTo">
		<rdfs:label>is response to</rdfs:label>
		<rdfs:domain rdf:resource="&fibo-fnd-dt-oc;Occurrence"/>
		<rdfs:range rdf:resource="&fibo-fnd-dt-oc;Occurrence"/>
		<skos:definition>relates an occurrence to another occurrence that it is a response to, most often in the context of communication</skos:definition>
	</owl:ObjectProperty>
	
	<owl:ObjectProperty rdf:about="&fibo-ln-ln-up;hasAppraiser">
		<rdfs:subPropertyOf rdf:resource="&fibo-ln-ln-up;hasParticipant"/>
		<rdfs:label>has appraiser</rdfs:label>
		<skos:definition>relates e.g. an appraisal, to a party that plays the role of conducting a property appraisal</skos:definition>
	</owl:ObjectProperty>
	
	<owl:ObjectProperty rdf:about="&fibo-ln-ln-up;hasAsOfDate">
		<rdfs:subPropertyOf rdf:resource="&fibo-fnd-dt-fd;hasDate"/>
		<rdfs:label>as of date</rdfs:label>
		<skos:definition>relates something to the date on which it is accurate or valid (e.g. a credit report has an asOfDate that means the date when the information was drawn)</skos:definition>
		<fibo-fnd-utl-av:explanatoryNote>It is different from the creation date and need not be the last date of the DatePeriod covered.</fibo-fnd-utl-av:explanatoryNote>
	</owl:ObjectProperty>
	
	<owl:ObjectProperty rdf:about="&fibo-ln-ln-up;hasCreationDate">
		<rdfs:subPropertyOf rdf:resource="&fibo-fnd-dt-fd;hasStartDate"/>
		<rdfs:label>has creation date</rdfs:label>
		<skos:definition>relates something to the date when it came into existence</skos:definition>
	</owl:ObjectProperty>
	
	<owl:ObjectProperty rdf:about="&fibo-ln-ln-up;hasDataSource">
		<rdfs:label>has estimated value</rdfs:label>
		<skos:definition>relates an informational entity to a source of data used to produce it (e.g. Experian provides data for a CreditReport)</skos:definition>
	</owl:ObjectProperty>
	
	<owl:ObjectProperty rdf:about="&fibo-ln-ln-up;hasDateReceived">
		<rdfs:subPropertyOf rdf:resource="&fibo-fnd-dt-fd;hasDate"/>
		<rdfs:label>has date received</rdfs:label>
		<skos:definition>relates something to the date when it was received, e.g. a loan application request</skos:definition>
	</owl:ObjectProperty>
	
	<owl:ObjectProperty rdf:about="&fibo-ln-ln-up;hasIndividualContactInfo">
		<rdfs:label>has individual contact information</rdfs:label>
		<rdfs:range rdf:resource="&fibo-ln-ln-up;ContactInfo"/>
		<skos:definition>relates something to the contact information of an individual (as opposed to an organization)</skos:definition>
		<skos:editorialNote>Topic: BE</skos:editorialNote>
	</owl:ObjectProperty>
	
	<owl:ObjectProperty rdf:about="&fibo-ln-ln-up;hasInput">
		<rdfs:subPropertyOf rdf:resource="&fibo-ln-ln-up;hasParticipant"/>
		<rdfs:label>has input</rdfs:label>
		<owl:inverseOf rdf:resource="&fibo-ln-ln-up;isInputOn"/>
		<skos:definition>relates an occurrence to something that is used as an input to some activity or process</skos:definition>
	</owl:ObjectProperty>
	
	<owl:ObjectProperty rdf:about="&fibo-ln-ln-up;hasInterestRate">
		<rdfs:subPropertyOf rdf:resource="&fibo-fnd-rel-rel;has"/>
		<rdfs:label>has interest rate</rdfs:label>
		<skos:definition>relates, e.g. a loan, to an interest rate</skos:definition>
		<skos:editorialNote>Topic: Payments</skos:editorialNote>
	</owl:ObjectProperty>
	
	<owl:DatatypeProperty rdf:about="&fibo-ln-ln-up;hasNumberOfEntries">
		<rdfs:subPropertyOf rdf:resource="&fibo-fnd-dt-fd;hasCount"/>
		<rdfs:label>has number of entries</rdfs:label>
		<rdfs:range rdf:resource="&xsd;positiveInteger"/>
		<skos:definition>the number of entries (e.g. in a report)</skos:definition>
	</owl:DatatypeProperty>
	
	<owl:ObjectProperty rdf:about="&fibo-ln-ln-up;hasOrgContactInfo">
		<rdfs:label>has organization contact information</rdfs:label>
		<rdfs:range rdf:resource="&fibo-ln-ln-up;ContactInfo"/>
		<skos:definition>relates something to the contact information of an organization  (as opposed to an individual)</skos:definition>
		<skos:editorialNote>Topic: BE</skos:editorialNote>
	</owl:ObjectProperty>
	
	<owl:ObjectProperty rdf:about="&fibo-ln-ln-up;hasOutput">
		<rdfs:subPropertyOf rdf:resource="&fibo-ln-ln-up;hasParticipant"/>
		<rdfs:label>has output</rdfs:label>
		<owl:inverseOf rdf:resource="&fibo-ln-ln-up;isOutputOn"/>
		<skos:definition>relates an occurrence to something that is the result of some activity or process</skos:definition>
	</owl:ObjectProperty>
	
	<owl:ObjectProperty rdf:about="&fibo-ln-ln-up;hasParticipant">
		<rdfs:label>has participant</rdfs:label>
		<skos:definition>relates e.g. an agreement or event to an object or party playing a role</skos:definition>
		<skos:editorialNote>fibo-fnd-pty-pty:hasParty should be a subproperty of this property.</skos:editorialNote>
	</owl:ObjectProperty>
	
	<owl:ObjectProperty rdf:about="&fibo-ln-ln-up;hasScheduledUnpaidBalance">
		<rdfs:subPropertyOf rdf:resource="&fibo-fnd-rel-rel;has"/>
		<rdfs:label>has scheduled unpaid balance</rdfs:label>
		<rdfs:range rdf:resource="&fibo-fnd-acc-cur;MonetaryAmount"/>
		<skos:definition>relates to what the balance should be after a scheduled payment is made according to contract terms</skos:definition>
		<skos:editorialNote>Topic: Payments</skos:editorialNote>
	</owl:ObjectProperty>
	
	<owl:ObjectProperty rdf:about="&fibo-ln-ln-up;hasSeniorAppraiser">
		<rdfs:subPropertyOf rdf:resource="&fibo-ln-ln-up;hasParticipant"/>
		<rdfs:label>has senior appraiser</rdfs:label>
		<skos:definition>relates e.g. an appraisal to the appraiser with seniority or supervisory responsibilities</skos:definition>
	</owl:ObjectProperty>
	
	<owl:ObjectProperty rdf:about="&fibo-ln-ln-up;instantiates">
		<rdfs:label>instantiates</rdfs:label>
		<skos:definition>relates something to that which it is an instance of (e.g. a template, offer or form)</skos:definition>
	</owl:ObjectProperty>
	
	<owl:ObjectProperty rdf:about="&fibo-ln-ln-up;isEvaluationOf">
		<rdfs:label>is evaluation of</rdfs:label>
		<skos:definition>relates a valuation to the thing being valued</skos:definition>
	</owl:ObjectProperty>
	
	<owl:ObjectProperty rdf:about="&fibo-ln-ln-up;isInputOn">
		<rdfs:label>is input on</rdfs:label>
		<skos:definition>inverse of has input</skos:definition>
	</owl:ObjectProperty>
	
	<owl:ObjectProperty rdf:about="&fibo-ln-ln-up;isOutputOn">
		<rdfs:label>is output on</rdfs:label>
		<skos:definition>inverse of has output</skos:definition>
	</owl:ObjectProperty>
	
	<owl:ObjectProperty rdf:about="&fibo-ln-ln-up;isPerformedBy">
		<rdfs:subPropertyOf rdf:resource="&fibo-ln-ln-up;hasParticipant"/>
		<rdfs:label>is performed by</rdfs:label>
		<skos:definition>relates an occurrence to a party that fully or partially performs the activity or process corresponding to the occurrence (e.g. who performed an inspection)</skos:definition>
	</owl:ObjectProperty>
	
	<owl:ObjectProperty rdf:about="&fibo-ln-ln-up;offersItem">
		<rdfs:subPropertyOf rdf:resource="&fibo-ln-ln-up;hasParticipant"/>
		<rdfs:label>offers item</rdfs:label>
		<skos:definition>relates an offer to the item on offer</skos:definition>
	</owl:ObjectProperty>
	
	<owl:ObjectProperty rdf:about="&fibo-ln-ln-up;opty-isGuaranteedBy">
		<rdfs:label>is guaranteed by</rdfs:label>
		<owl:inverseOf rdf:resource="&fibo-be-oac-opty;guarantees"/>
		<skos:definition>inverse of guarantees</skos:definition>
		<skos:editorialNote>Topic: BE add inverse of guarantees called isGuaranteedBy</skos:editorialNote>
	</owl:ObjectProperty>
	
	<owl:Class rdf:about="&fibo-ln-ln-up;pas-LineItem">
		<rdfs:subClassOf rdf:resource="&fibo-ln-ln-up;Specification"/>
		<rdfs:subClassOf>
			<owl:Restriction>
				<owl:onProperty rdf:resource="&fibo-ln-ln-up;pas-hasUnitCost"/>
				<owl:onClass rdf:resource="&fibo-fnd-acc-cur;MonetaryAmount"/>
				<owl:minQualifiedCardinality rdf:datatype="&xsd;nonNegativeInteger">0</owl:minQualifiedCardinality>
			</owl:Restriction>
		</rdfs:subClassOf>
		<rdfs:subClassOf>
			<owl:Restriction>
				<owl:onProperty rdf:resource="&fibo-fnd-qt-qtu;hasNumericValue"/>
				<owl:minQualifiedCardinality rdf:datatype="&xsd;nonNegativeInteger">0</owl:minQualifiedCardinality>
				<owl:onDataRange rdf:resource="&xsd;decimal"/>
			</owl:Restriction>
		</rdfs:subClassOf>
		<rdfs:subClassOf>
			<owl:Restriction>
				<owl:onProperty rdf:resource="&fibo-fnd-rel-rel;has"/>
				<owl:someValuesFrom>
					<owl:Class>
						<owl:unionOf rdf:parseType="Collection">
							<rdf:Description rdf:about="&fibo-fnd-pas-pas;Product">
							</rdf:Description>
							<rdf:Description rdf:about="&fibo-ln-ln-up;ChargeCategory">
							</rdf:Description>
						</owl:unionOf>
					</owl:Class>
				</owl:someValuesFrom>
			</owl:Restriction>
		</rdfs:subClassOf>
		<rdfs:subClassOf>
			<owl:Restriction>
				<owl:onProperty rdf:resource="&fibo-ln-ln-up;pas-hasCost"/>
				<owl:someValuesFrom rdf:resource="&fibo-fnd-acc-cur;MonetaryAmount"/>
			</owl:Restriction>
		</rdfs:subClassOf>
		<rdfs:label>line item</rdfs:label>
		<skos:definition>a description of a product or service including its unit cost, number of units and total cost</skos:definition>
	</owl:Class>
	
	<owl:Class rdf:about="&fibo-ln-ln-up;pas-MarketCategory">
		<rdfs:subClassOf rdf:resource="&fibo-fnd-arr-cls;Classifier"/>
		<rdfs:label>market category</rdfs:label>
		<skos:definition>a category indicating the market domain in which a product is offered</skos:definition>
	</owl:Class>
	
	<owl:Class rdf:about="&fibo-ln-ln-up;pas-Offer">
		<rdfs:subClassOf rdf:resource="&fibo-fnd-agr-agr;Commitment"/>
		<rdfs:label>offer</rdfs:label>
		<skos:definition>a commitment to provide a product or service for an agreed price, if a buyer comes along</skos:definition>
		<skos:editorialNote>Future consideration: move to the products and services ontology.</skos:editorialNote>
	</owl:Class>
	
	<owl:ObjectProperty rdf:about="&fibo-ln-ln-up;pas-hasCost">
		<rdfs:subPropertyOf rdf:resource="&fibo-ln-ln-up;cur-hasMonetaryAmount"/>
		<rdfs:label>has cost</rdfs:label>
		<skos:definition>relates an item to its cost</skos:definition>
		<fibo-fnd-utl-av:explanatoryNote>This can entail adding up other costs (e.g. 4 units * a unit price)</fibo-fnd-utl-av:explanatoryNote>
	</owl:ObjectProperty>
	
	<owl:ObjectProperty rdf:about="&fibo-ln-ln-up;pas-hasUnitCost">
		<rdfs:subPropertyOf rdf:resource="&fibo-ln-ln-up;cur-hasMonetaryAmount"/>
		<rdfs:label>has unit cost</rdfs:label>
		<skos:definition>relates an item to its unit cost</skos:definition>
	</owl:ObjectProperty>
	
	<owl:DatatypeProperty rdf:about="&fibo-ln-ln-up;rel-hasVersion">
		<rdfs:label>has version</rdfs:label>
		<rdfs:range rdf:resource="&xsd;string"/>
		<skos:definition>relates something to its version</skos:definition>
	</owl:DatatypeProperty>
	
	<owl:ObjectProperty rdf:about="&fibo-ln-ln-up;rel-isFrom">
		<rdfs:label>is from</rdfs:label>
		<skos:definition>relates something to its source or origin (e.g. the agent originating a request)</skos:definition>
	</owl:ObjectProperty>
	
	<owl:ObjectProperty rdf:about="&fibo-ln-ln-up;rel-isProducedBy_I">
		<rdfs:label>is produced by (i)</rdfs:label>
		<owl:inverseOf rdf:resource="&fibo-ln-ln-up;rel-produces_I"/>
		<skos:definition>relates something to who or what produced it</skos:definition>
		<skos:editorialNote>Ideally, this would be a superproperty of pas:isProducedBy in products and services ontology, but that is reserved for use with ThingInRole.  This property is therefore a superproperty of an unnamed property chain from the thing produced  to the independent producing thing that goes through an instance of a class that means PartyInProducerRole.</skos:editorialNote>
	</owl:ObjectProperty>
	
	<owl:ObjectProperty rdf:about="&fibo-ln-ln-up;rel-isSubmittedBy">
		<rdfs:label>is submitted by</rdfs:label>
		<rdfs:range rdf:resource="&fibo-fnd-aap-agt;AutonomousAgent"/>
		<skos:definition>relates something to that agent that provided or submitted it (e.g. the person or organization that submitted a report)</skos:definition>
		<skos:editorialNote>Ideally, this would be a subproperty of isProvidedBy, but that is reserved for use with ThingInRole.  This property is therefore a subproperty of an unnamed property chain from the thing submitted to the submitting institution that goes through an instance of a class that means PartyInProviderRole.</skos:editorialNote>
	</owl:ObjectProperty>
	
	<owl:ObjectProperty rdf:about="&fibo-ln-ln-up;rel-isSubmittedTo">
		<rdfs:label>is submitted to</rdfs:label>
		<rdfs:range rdf:resource="&fibo-fnd-aap-agt;AutonomousAgent"/>
		<skos:definition>relates something to which it is submitted (e.g. the organization receiving a report)</skos:definition>
	</owl:ObjectProperty>
	
	<owl:ObjectProperty rdf:about="&fibo-ln-ln-up;rel-isTo">
		<rdfs:label>is to</rdfs:label>
		<skos:definition>relates something to a target or destination (e.g. the agent receiving a request)</skos:definition>
	</owl:ObjectProperty>
	
	<owl:ObjectProperty rdf:about="&fibo-ln-ln-up;rel-produces_I">
		<rdfs:label>produces (i)</rdfs:label>
		<skos:definition>inverse of is produced by</skos:definition>
	</owl:ObjectProperty>
	
	<owl:ObjectProperty rdf:about="&fibo-ln-ln-up;worksFor">
		<rdfs:label>works for</rdfs:label>
		<rdfs:domain rdf:resource="&fibo-fnd-aap-ppl;LegallyCapablePerson"/>
		<rdfs:range rdf:resource="&fibo-fnd-pty-pty;IndependentParty"/>
		<skos:definition>relates a person to the organization or company that they work for either as an employee or contractor</skos:definition>
		<fibo-fnd-utl-av:usageNote>Use this property to connect appraisers to the appraisal management company.</fibo-fnd-utl-av:usageNote>
	</owl:ObjectProperty>

</rdf:RDF>