<?xml version="1.0" encoding="UTF-8"?>
<!DOCTYPE rdf:RDF [
	<!ENTITY dct "http://purl.org/dc/terms/">
	<!ENTITY fibo-be-le-lp "https://spec.edmcouncil.org/fibo/ontology/BE/LegalEntities/LegalPersons/">
	<!ENTITY fibo-cae-ce-cae "https://spec.edmcouncil.org/fibo/ontology/CAE/CorporateEvents/CorporateActionsEvents/">
	<!ENTITY fibo-der-drc-raw "https://spec.edmcouncil.org/fibo/ontology/DER/DerivativesContracts/RightsAndWarrants/">
	<!ENTITY fibo-fbc-dae-cre "https://spec.edmcouncil.org/fibo/ontology/FBC/DebtAndEquities/CreditEvents/">
	<!ENTITY fibo-fbc-fi-fi "https://spec.edmcouncil.org/fibo/ontology/FBC/FinancialInstruments/FinancialInstruments/">
	<!ENTITY fibo-fnd-acc-cur "https://spec.edmcouncil.org/fibo/ontology/FND/Accounting/CurrencyAmount/">
	<!ENTITY fibo-fnd-agr-ctr "https://spec.edmcouncil.org/fibo/ontology/FND/Agreements/Contracts/">
	<!ENTITY fibo-fnd-arr-cls "https://spec.edmcouncil.org/fibo/ontology/FND/Arrangements/ClassificationSchemes/">
	<!ENTITY fibo-fnd-arr-doc "https://spec.edmcouncil.org/fibo/ontology/FND/Arrangements/Documents/">
	<!ENTITY fibo-fnd-arr-lif "https://spec.edmcouncil.org/fibo/ontology/FND/Arrangements/Lifecycles/">
	<!ENTITY fibo-fnd-dt-fd "https://spec.edmcouncil.org/fibo/ontology/FND/DatesAndTimes/FinancialDates/">
	<!ENTITY fibo-fnd-dt-oc "https://spec.edmcouncil.org/fibo/ontology/FND/DatesAndTimes/Occurrences/">
	<!ENTITY fibo-fnd-gao-obj "https://spec.edmcouncil.org/fibo/ontology/FND/GoalsAndObjectives/Objectives/">
	<!ENTITY fibo-fnd-law-lcap "https://spec.edmcouncil.org/fibo/ontology/FND/Law/LegalCapacity/">
	<!ENTITY fibo-fnd-rel-rel "https://spec.edmcouncil.org/fibo/ontology/FND/Relations/Relations/">
	<!ENTITY fibo-fnd-utl-av "https://spec.edmcouncil.org/fibo/ontology/FND/Utilities/AnnotationVocabulary/">
	<!ENTITY fibo-md-temx-trs "https://spec.edmcouncil.org/fibo/ontology/MD/TemporalCore/SecurityTradingStatuses/">
	<!ENTITY fibo-sec-dbt-bnd "https://spec.edmcouncil.org/fibo/ontology/SEC/Debt/Bonds/">
	<!ENTITY fibo-sec-dbt-dbti "https://spec.edmcouncil.org/fibo/ontology/SEC/Debt/DebtInstruments/">
	<!ENTITY fibo-sec-eq-eq "https://spec.edmcouncil.org/fibo/ontology/SEC/Equities/EquityInstruments/">
	<!ENTITY lcc-cr "https://www.omg.org/spec/LCC/Countries/CountryRepresentation/">
	<!ENTITY lcc-lr "https://www.omg.org/spec/LCC/Languages/LanguageRepresentation/">
	<!ENTITY owl "http://www.w3.org/2002/07/owl#">
	<!ENTITY rdf "http://www.w3.org/1999/02/22-rdf-syntax-ns#">
	<!ENTITY rdfs "http://www.w3.org/2000/01/rdf-schema#">
	<!ENTITY skos "http://www.w3.org/2004/02/skos/core#">
	<!ENTITY sm "http://www.omg.org/techprocess/ab/SpecificationMetadata/">
	<!ENTITY xsd "http://www.w3.org/2001/XMLSchema#">
]>
<rdf:RDF xml:base="https://spec.edmcouncil.org/fibo/ontology/CAE/CorporateEvents/CorporateActionsEvents/"
	xmlns:dct="http://purl.org/dc/terms/"
	xmlns:fibo-be-le-lp="https://spec.edmcouncil.org/fibo/ontology/BE/LegalEntities/LegalPersons/"
	xmlns:fibo-cae-ce-cae="https://spec.edmcouncil.org/fibo/ontology/CAE/CorporateEvents/CorporateActionsEvents/"
	xmlns:fibo-der-drc-raw="https://spec.edmcouncil.org/fibo/ontology/DER/DerivativesContracts/RightsAndWarrants/"
	xmlns:fibo-fbc-dae-cre="https://spec.edmcouncil.org/fibo/ontology/FBC/DebtAndEquities/CreditEvents/"
	xmlns:fibo-fbc-fi-fi="https://spec.edmcouncil.org/fibo/ontology/FBC/FinancialInstruments/FinancialInstruments/"
	xmlns:fibo-fnd-acc-cur="https://spec.edmcouncil.org/fibo/ontology/FND/Accounting/CurrencyAmount/"
	xmlns:fibo-fnd-agr-ctr="https://spec.edmcouncil.org/fibo/ontology/FND/Agreements/Contracts/"
	xmlns:fibo-fnd-arr-cls="https://spec.edmcouncil.org/fibo/ontology/FND/Arrangements/ClassificationSchemes/"
	xmlns:fibo-fnd-arr-doc="https://spec.edmcouncil.org/fibo/ontology/FND/Arrangements/Documents/"
	xmlns:fibo-fnd-arr-lif="https://spec.edmcouncil.org/fibo/ontology/FND/Arrangements/Lifecycles/"
	xmlns:fibo-fnd-dt-fd="https://spec.edmcouncil.org/fibo/ontology/FND/DatesAndTimes/FinancialDates/"
	xmlns:fibo-fnd-dt-oc="https://spec.edmcouncil.org/fibo/ontology/FND/DatesAndTimes/Occurrences/"
	xmlns:fibo-fnd-gao-obj="https://spec.edmcouncil.org/fibo/ontology/FND/GoalsAndObjectives/Objectives/"
	xmlns:fibo-fnd-law-lcap="https://spec.edmcouncil.org/fibo/ontology/FND/Law/LegalCapacity/"
	xmlns:fibo-fnd-rel-rel="https://spec.edmcouncil.org/fibo/ontology/FND/Relations/Relations/"
	xmlns:fibo-fnd-utl-av="https://spec.edmcouncil.org/fibo/ontology/FND/Utilities/AnnotationVocabulary/"
	xmlns:fibo-md-temx-trs="https://spec.edmcouncil.org/fibo/ontology/MD/TemporalCore/SecurityTradingStatuses/"
	xmlns:fibo-sec-dbt-bnd="https://spec.edmcouncil.org/fibo/ontology/SEC/Debt/Bonds/"
	xmlns:fibo-sec-dbt-dbti="https://spec.edmcouncil.org/fibo/ontology/SEC/Debt/DebtInstruments/"
	xmlns:fibo-sec-eq-eq="https://spec.edmcouncil.org/fibo/ontology/SEC/Equities/EquityInstruments/"
	xmlns:lcc-cr="https://www.omg.org/spec/LCC/Countries/CountryRepresentation/"
	xmlns:lcc-lr="https://www.omg.org/spec/LCC/Languages/LanguageRepresentation/"
	xmlns:owl="http://www.w3.org/2002/07/owl#"
	xmlns:rdf="http://www.w3.org/1999/02/22-rdf-syntax-ns#"
	xmlns:rdfs="http://www.w3.org/2000/01/rdf-schema#"
	xmlns:skos="http://www.w3.org/2004/02/skos/core#"
	xmlns:sm="http://www.omg.org/techprocess/ab/SpecificationMetadata/"
	xmlns:xsd="http://www.w3.org/2001/XMLSchema#">
	
	<owl:Ontology rdf:about="https://spec.edmcouncil.org/fibo/ontology/CAE/CorporateEvents/CorporateActionsEvents/">
		<rdfs:label xml:lang="en">CorporateActionsEvents</rdfs:label>
		<dct:abstract>This ontology covers income and corporate action events as specified in SWIFT ISO 15022, including extensions as of 3 September 2020. Scope has been limited to events and actions only, and excludes notification and meetings related events and message definitions associated with ISO 15022 as well as related messages covered by ISO 20022.</dct:abstract>
		<dct:license rdf:datatype="&xsd;anyURI">http://opensource.org/licenses/MIT</dct:license>
		<sm:contentLanguage rdf:resource="https://www.w3.org/TR/owl2-quick-reference/"/>
		<sm:copyright>Copyright (c) 2016-2020 EDM Council, Inc.</sm:copyright>
		<sm:dependsOn rdf:datatype="&xsd;anyURI">https://spec.edmcouncil.org/fibo/ontology/BE/</sm:dependsOn>
		<sm:dependsOn rdf:datatype="&xsd;anyURI">https://spec.edmcouncil.org/fibo/ontology/FBC/</sm:dependsOn>
		<sm:dependsOn rdf:datatype="&xsd;anyURI">https://spec.edmcouncil.org/fibo/ontology/FND/</sm:dependsOn>
		<sm:dependsOn rdf:datatype="&xsd;anyURI">https://spec.edmcouncil.org/fibo/ontology/SEC/</sm:dependsOn>
		<sm:dependsOn rdf:datatype="&xsd;anyURI">https://www.omg.org/spec/LCC/</sm:dependsOn>
		<sm:fileAbbreviation>fibo-cae-ce-cae</sm:fileAbbreviation>
		<sm:filename>CorporateActionsEvents.rdf</sm:filename>
		<owl:imports rdf:resource="http://www.omg.org/techprocess/ab/SpecificationMetadata/"/>
		<owl:imports rdf:resource="https://spec.edmcouncil.org/fibo/ontology/BE/LegalEntities/LegalPersons/"/>
		<owl:imports rdf:resource="https://spec.edmcouncil.org/fibo/ontology/DER/DerivativesContracts/RightsAndWarrants/"/>
		<owl:imports rdf:resource="https://spec.edmcouncil.org/fibo/ontology/FBC/DebtAndEquities/CreditEvents/"/>
		<owl:imports rdf:resource="https://spec.edmcouncil.org/fibo/ontology/FBC/FinancialInstruments/FinancialInstruments/"/>
		<owl:imports rdf:resource="https://spec.edmcouncil.org/fibo/ontology/FND/Accounting/CurrencyAmount/"/>
		<owl:imports rdf:resource="https://spec.edmcouncil.org/fibo/ontology/FND/AgentsAndPeople/Agents/"/>
		<owl:imports rdf:resource="https://spec.edmcouncil.org/fibo/ontology/FND/Agreements/Contracts/"/>
		<owl:imports rdf:resource="https://spec.edmcouncil.org/fibo/ontology/FND/Arrangements/ClassificationSchemes/"/>
		<owl:imports rdf:resource="https://spec.edmcouncil.org/fibo/ontology/FND/Arrangements/Documents/"/>
		<owl:imports rdf:resource="https://spec.edmcouncil.org/fibo/ontology/FND/Arrangements/Lifecycles/"/>
		<owl:imports rdf:resource="https://spec.edmcouncil.org/fibo/ontology/FND/DatesAndTimes/FinancialDates/"/>
		<owl:imports rdf:resource="https://spec.edmcouncil.org/fibo/ontology/FND/DatesAndTimes/Occurrences/"/>
		<owl:imports rdf:resource="https://spec.edmcouncil.org/fibo/ontology/FND/GoalsAndObjectives/Objectives/"/>
		<owl:imports rdf:resource="https://spec.edmcouncil.org/fibo/ontology/FND/Law/LegalCapacity/"/>
		<owl:imports rdf:resource="https://spec.edmcouncil.org/fibo/ontology/FND/Relations/Relations/"/>
		<owl:imports rdf:resource="https://spec.edmcouncil.org/fibo/ontology/FND/Utilities/AnnotationVocabulary/"/>
		<owl:imports rdf:resource="https://spec.edmcouncil.org/fibo/ontology/MD/TemporalCore/SecurityTradingStatuses/"/>
		<owl:imports rdf:resource="https://spec.edmcouncil.org/fibo/ontology/SEC/Debt/Bonds/"/>
		<owl:imports rdf:resource="https://spec.edmcouncil.org/fibo/ontology/SEC/Debt/DebtInstruments/"/>
		<owl:imports rdf:resource="https://spec.edmcouncil.org/fibo/ontology/SEC/Equities/EquityInstruments/"/>
		<owl:imports rdf:resource="https://www.omg.org/spec/LCC/Countries/CountryRepresentation/"/>
		<owl:imports rdf:resource="https://www.omg.org/spec/LCC/Languages/LanguageRepresentation/"/>
		<owl:versionIRI rdf:resource="https://spec.edmcouncil.org/fibo/ontology/CAE/CorporateEvents/CorporateActionsEvents/"/>
		<fibo-fnd-utl-av:hasMaturityLevel rdf:resource="&fibo-fnd-utl-av;Provisional"/>
	</owl:Ontology>
	
	<owl:Class rdf:about="&fibo-cae-ce-cae;AttachmentAction">
		<rdfs:subClassOf rdf:resource="&fibo-cae-ce-cae;CorporateAction"/>
		<rdfs:label xml:lang="en">attachment action</rdfs:label>
		<owl:disjointWith rdf:resource="&fibo-cae-ce-cae;DetachmentAction"/>
		<skos:definition xml:lang="en">The combination of different security types to create a unit. Units are usually comprised of warrants and bond or warrants and equity. Securities may be combined at the request of the security holder or based on market convention. Further NOtes: is there some common term for these (see Detachment event)?; Are there separate scenarios for attachment of different kinds of security. Definition says &quot;usually&quot; Warrant. Probably applies to any fungible securities, whether or not warrants. For example two fungible tranches of a debt issues, that are funged later on in their life. Are these ever notified differently or have different details for warrants, fungible debt etc.? No. the message can relate to any, and the event defined here can be defined in terms of &quot;any&quot; securities.</skos:definition>
	</owl:Class>
	
	<owl:NamedIndividual rdf:about="&fibo-cae-ce-cae;BIDS">
		<rdf:type rdf:resource="&fibo-cae-ce-cae;BusinessStrategyOrientedAction"/>
		<rdfs:label xml:lang="en">BIDS</rdfs:label>
		<skos:definition xml:lang="en">SWIFT ISO 15022 classifier for corporate actions in which an offer is made to existing shareholders by the issuing company to repurchase equity or other securities convertible into equity</skos:definition>
		<fibo-fnd-rel-rel:isDefinedIn rdf:resource="&fibo-cae-ce-cae;ISO15022CorporateActionClassificationScheme"/>
		<lcc-cr:classifies rdf:resource="&fibo-cae-ce-cae;RepurchaseOffer"/>
		<lcc-lr:denotes rdf:resource="&fibo-cae-ce-cae;RepurchaseOffer"/>
		<lcc-lr:hasTag>BIDS</lcc-lr:hasTag>
		<lcc-lr:isMemberOf rdf:resource="&fibo-cae-ce-cae;ISO15022CorporateActionClassificationScheme"/>
	</owl:NamedIndividual>
	
	<owl:NamedIndividual rdf:about="&fibo-cae-ce-cae;BONU">
		<rdf:type rdf:resource="&fibo-cae-ce-cae;BusinessStrategyOrientedAction"/>
		<rdfs:label xml:lang="en">BONU</rdfs:label>
		<skos:definition xml:lang="en">SWIFT ISO 15022 classifier for corporate actions in which security holders are awarded additional assets free of payment from the issuer in proportion to their holding</skos:definition>
		<fibo-fnd-rel-rel:isDefinedIn rdf:resource="&fibo-cae-ce-cae;ISO15022CorporateActionClassificationScheme"/>
		<lcc-cr:classifies rdf:resource="&fibo-cae-ce-cae;BonusIssue"/>
		<lcc-lr:denotes rdf:resource="&fibo-cae-ce-cae;BonusIssue"/>
		<lcc-lr:hasTag>BONU</lcc-lr:hasTag>
		<lcc-lr:isMemberOf rdf:resource="&fibo-cae-ce-cae;ISO15022CorporateActionClassificationScheme"/>
	</owl:NamedIndividual>
	
	<owl:NamedIndividual rdf:about="&fibo-cae-ce-cae;BPUT">
		<rdf:type rdf:resource="&fibo-cae-ce-cae;BusinessStrategyOrientedAction"/>
		<rdfs:label xml:lang="en">BPUT</rdfs:label>
		<skos:definition xml:lang="en">SWIFT ISO 15022 classifier for corporate actions that involve early redemption of a security at the election of the holder subject to the terms and condition of the issue with no reduction in nominal value</skos:definition>
		<fibo-fnd-rel-rel:isDefinedIn rdf:resource="&fibo-cae-ce-cae;ISO15022CorporateActionClassificationScheme"/>
		<lcc-cr:classifies rdf:resource="&fibo-cae-ce-cae;PutRedemptionAction"/>
		<lcc-lr:denotes rdf:resource="&fibo-cae-ce-cae;PutRedemptionAction"/>
		<lcc-lr:hasTag>BPUT</lcc-lr:hasTag>
		<lcc-lr:isMemberOf rdf:resource="&fibo-cae-ce-cae;ISO15022CorporateActionClassificationScheme"/>
	</owl:NamedIndividual>
	
	<owl:Class rdf:about="&fibo-cae-ce-cae;BondDefaultAction">
		<rdfs:subClassOf rdf:resource="&fibo-cae-ce-cae;MandatoryCorporateAction"/>
		<rdfs:subClassOf rdf:resource="&fibo-fbc-dae-cre;ObligationDefault"/>
		<rdfs:subClassOf>
			<owl:Restriction>
				<owl:onProperty rdf:resource="&fibo-fnd-rel-rel;appliesTo"/>
				<owl:someValuesFrom rdf:resource="&fibo-sec-dbt-bnd;Bond"/>
			</owl:Restriction>
		</rdfs:subClassOf>
		<rdfs:label xml:lang="en">bond default event</rdfs:label>
		<skos:definition xml:lang="en">corporate action which indicates a failure by the issuer to perform obligations defined as default events under the bond agreement and that have not been remedied</skos:definition>
	</owl:Class>
	
	<owl:Class rdf:about="&fibo-cae-ce-cae;BonusIssue">
		<rdfs:subClassOf rdf:resource="&fibo-cae-ce-cae;MandatoryCorporateAction"/>
		<rdfs:label xml:lang="en">bonus issue</rdfs:label>
		<skos:definition xml:lang="en">corporate action in which security holders are awarded additional assets free of payment from the issuer in proportion to their holding</skos:definition>
		<fibo-fnd-utl-av:explanatoryNote xml:lang="en">There are different taxation rules for the bonus issue compared to the dividend. There could also be a difference in the ranking of the shares that are given to what the holder already holds. Dividends are paid from current profits and bonus may be from accumulated reserves of the company. A scrip issue is the issue of new shares at no charge pro rata to the holder of existing shares.</fibo-fnd-utl-av:explanatoryNote>
		<fibo-fnd-utl-av:synonym xml:lang="en">capitalisation issue</fibo-fnd-utl-av:synonym>
		<fibo-fnd-utl-av:synonym xml:lang="en">scrip issue</fibo-fnd-utl-av:synonym>
	</owl:Class>
	
	<owl:Class rdf:about="&fibo-cae-ce-cae;BonusRightsIssue">
		<rdfs:subClassOf rdf:resource="&fibo-cae-ce-cae;RightsIssue"/>
		<rdfs:label xml:lang="en">bonus rights issue</rdfs:label>
		<skos:definition xml:lang="en">A Rights Issue in which the rights are given to the holders of the referenced shares for free.</skos:definition>
		<fibo-fnd-utl-av:explanatoryNote xml:lang="en">Rights = right to buy shares at a specified price. May be given the right for nothing (Bonus Rights Issue) or you may be offered to purchase that right at a subscription price (which you take up or don&apos;t). Bonus Rights Issue: given the option for free. May exercise at the Exercise Price.</fibo-fnd-utl-av:explanatoryNote>
	</owl:Class>
	
	<owl:Class rdf:about="&fibo-cae-ce-cae;BonusSharePlanDistribution">
		<rdfs:subClassOf rdf:resource="&fibo-cae-ce-cae;CapitalDistribution"/>
		<rdfs:label xml:lang="en">bonus share plan distribution</rdfs:label>
		<skos:definition xml:lang="en">Event in which shares are issued from the Share Premium Reserve of the company and are considered as a capital distribution rather than a disbursement of income, with different tax implications. SWIFT Definition (adapted above) &quot;Typically found in Australia, shares are issued from the Share Premium Reserve of the company and are considered as a capital distribution rather than a disbursement of income, with different tax implications.&quot; To be researches further. There are certainly Share Plans in Australia, where you can take a dividend as shares. Thewse would be in the nature of Bonus Shares. They are a tradeoff from cash dividends. Other terms to model: A &quot;Scheme of Arrangment&quot; - does this change the capital reserves or is it just another word for restructure. An arrangement with the company&apos;s debtors, and coule potentially change the capital base by converting the debt to shares (see other diagram note with these in).</skos:definition>
	</owl:Class>
	
	<owl:Class rdf:about="&fibo-cae-ce-cae;BusinessStrategyOrientedAction">
		<rdfs:subClassOf rdf:resource="&fibo-cae-ce-cae;CorporateActionClassifier"/>
		<rdfs:label xml:lang="en">business strategy oriented action</rdfs:label>
		<skos:definition xml:lang="en">classifier of corporate actions that involves improving liquidity or changing the overall structure of the organization through diversification, combining and closing parts of the business, etc, to increase long-term profitability</skos:definition>
	</owl:Class>
	
	<owl:NamedIndividual rdf:about="&fibo-cae-ce-cae;CAPD">
		<rdf:type rdf:resource="&fibo-cae-ce-cae;IncomeOrientedAction"/>
		<rdfs:label xml:lang="en">CAPD</rdfs:label>
		<skos:definition xml:lang="en">SWIFT ISO 15022 classifier for corporate actions that pay shareholders an amount in cash issued from the issuer&apos;s capital account</skos:definition>
		<fibo-fnd-rel-rel:isDefinedIn rdf:resource="&fibo-cae-ce-cae;ISO15022CorporateActionClassificationScheme"/>
		<lcc-cr:classifies rdf:resource="&fibo-cae-ce-cae;CapitalDistribution"/>
		<lcc-lr:denotes rdf:resource="&fibo-cae-ce-cae;CapitalDistribution"/>
		<lcc-lr:hasTag>CAPD</lcc-lr:hasTag>
		<lcc-lr:isMemberOf rdf:resource="&fibo-cae-ce-cae;ISO15022CorporateActionClassificationScheme"/>
	</owl:NamedIndividual>
	
	<owl:NamedIndividual rdf:about="&fibo-cae-ce-cae;CAPG">
		<rdf:type rdf:resource="&fibo-cae-ce-cae;IncomeOrientedAction"/>
		<rdfs:label xml:lang="en">CAPG</rdfs:label>
		<skos:definition xml:lang="en">SWIFT ISO 15022 classifier for corporate actions that distribute profits resulting from the sale of company assets to shareholders</skos:definition>
		<fibo-fnd-rel-rel:isDefinedIn rdf:resource="&fibo-cae-ce-cae;ISO15022CorporateActionClassificationScheme"/>
		<lcc-cr:classifies rdf:resource="&fibo-cae-ce-cae;CapitalGainsDistribution"/>
		<lcc-lr:denotes rdf:resource="&fibo-cae-ce-cae;CapitalGainsDistribution"/>
		<lcc-lr:hasTag>CAPG</lcc-lr:hasTag>
		<lcc-lr:isMemberOf rdf:resource="&fibo-cae-ce-cae;ISO15022CorporateActionClassificationScheme"/>
	</owl:NamedIndividual>
	
	<owl:NamedIndividual rdf:about="&fibo-cae-ce-cae;CHAN">
		<rdf:type rdf:resource="&fibo-cae-ce-cae;BusinessStrategyOrientedAction"/>
		<rdfs:label xml:lang="en">CHAN</rdfs:label>
		<skos:definition xml:lang="en">SWIFT ISO 15022 classifier for corporate actions that disseminate information regarding a change further described in the corporate action details</skos:definition>
		<fibo-fnd-rel-rel:isDefinedIn rdf:resource="&fibo-cae-ce-cae;ISO15022CorporateActionClassificationScheme"/>
		<lcc-cr:classifies rdf:resource="&fibo-cae-ce-cae;ChangeAction"/>
		<lcc-lr:denotes rdf:resource="&fibo-cae-ce-cae;ChangeAction"/>
		<lcc-lr:hasTag>CHAN</lcc-lr:hasTag>
		<lcc-lr:isMemberOf rdf:resource="&fibo-cae-ce-cae;ISO15022CorporateActionClassificationScheme"/>
	</owl:NamedIndividual>
	
	<owl:NamedIndividual rdf:about="&fibo-cae-ce-cae;CLSA">
		<rdf:type rdf:resource="&fibo-cae-ce-cae;BusinessStrategyOrientedAction"/>
		<rdfs:label xml:lang="en">CLSA</rdfs:label>
		<skos:definition xml:lang="en">SWIFT ISO 15022 classifier for corporate actions involving a situation where interested parties seek restitution for financial loss</skos:definition>
		<fibo-fnd-rel-rel:isDefinedIn rdf:resource="&fibo-cae-ce-cae;ISO15022CorporateActionClassificationScheme"/>
		<lcc-cr:classifies rdf:resource="&fibo-cae-ce-cae;ClassAction"/>
		<lcc-lr:denotes rdf:resource="&fibo-cae-ce-cae;ClassAction"/>
		<lcc-lr:hasTag>CLSA</lcc-lr:hasTag>
		<lcc-lr:isMemberOf rdf:resource="&fibo-cae-ce-cae;ISO15022CorporateActionClassificationScheme"/>
	</owl:NamedIndividual>
	
	<owl:NamedIndividual rdf:about="&fibo-cae-ce-cae;CONS">
		<rdf:type rdf:resource="&fibo-cae-ce-cae;BusinessStrategyOrientedAction"/>
		<rdfs:label xml:lang="en">CONS</rdfs:label>
		<skos:definition xml:lang="en">SWIFT ISO 15022 classifier for corporate actions that involve procedures aiming to obtain consent of holder to a proposal by the issuer or a third party without convening a meeting</skos:definition>
		<fibo-fnd-rel-rel:isDefinedIn rdf:resource="&fibo-cae-ce-cae;ISO15022CorporateActionClassificationScheme"/>
		<lcc-cr:classifies rdf:resource="&fibo-cae-ce-cae;ConsentSolicitation"/>
		<lcc-lr:denotes rdf:resource="&fibo-cae-ce-cae;ConsentSolicitation"/>
		<lcc-lr:hasTag>CONS</lcc-lr:hasTag>
		<lcc-lr:isMemberOf rdf:resource="&fibo-cae-ce-cae;ISO15022CorporateActionClassificationScheme"/>
	</owl:NamedIndividual>
	
	<owl:NamedIndividual rdf:about="&fibo-cae-ce-cae;CONV">
		<rdf:type rdf:resource="&fibo-cae-ce-cae;BusinessStrategyOrientedAction"/>
		<rdfs:label xml:lang="en">CONV</rdfs:label>
		<skos:definition xml:lang="en">SWIFT ISO 15022 classifier for corporate actions that involve conversion of securities (generally convertible bonds or preferred shares) into another form of securities (usually common shares) at a pre-stated price/ratio</skos:definition>
		<fibo-fnd-rel-rel:isDefinedIn rdf:resource="&fibo-cae-ce-cae;ISO15022CorporateActionClassificationScheme"/>
		<lcc-cr:classifies rdf:resource="&fibo-cae-ce-cae;ConversionAction"/>
		<lcc-lr:denotes rdf:resource="&fibo-cae-ce-cae;ConversionAction"/>
		<lcc-lr:hasTag>CONV</lcc-lr:hasTag>
		<lcc-lr:isMemberOf rdf:resource="&fibo-cae-ce-cae;ISO15022CorporateActionClassificationScheme"/>
	</owl:NamedIndividual>
	
	<owl:Class rdf:about="&fibo-cae-ce-cae;CancellationOfShares">
		<rdfs:subClassOf rdf:resource="&fibo-cae-ce-cae;CorporateAction"/>
		<rdfs:label xml:lang="en">cancellation of shares</rdfs:label>
		<skos:definition xml:lang="en">The cancellation of shares. Further Notes Only possible with shares not publicly issued i.e. treasury shares</skos:definition>
	</owl:Class>
	
	<owl:Class rdf:about="&fibo-cae-ce-cae;CapitalDistribution">
		<rdfs:subClassOf rdf:resource="&fibo-cae-ce-cae;VoluntaryCorporateAction"/>
		<rdfs:label xml:lang="en">capital distribution</rdfs:label>
		<skos:definition xml:lang="en">corporate action that pays shareholders an amount in cash issued from the issuer&apos;s capital account</skos:definition>
		<fibo-fnd-utl-av:explanatoryNote xml:lang="en">This action does not result in a reduction of the face value of a share or in a change to the number of shares in circulation.</fibo-fnd-utl-av:explanatoryNote>
	</owl:Class>
	
	<owl:Class rdf:about="&fibo-cae-ce-cae;CapitalGainsDistribution">
		<rdfs:subClassOf rdf:resource="&fibo-cae-ce-cae;VoluntaryCorporateAction"/>
		<rdfs:label xml:lang="en">capital gains distribution</rdfs:label>
		<skos:definition xml:lang="en">corporate action that distributes profits resulting from the sale of company assets to shareholders</skos:definition>
		<skos:example xml:lang="en">Shareholders of Mutual Funds, Unit Trusts, or SICAVs are recipients of capital gains distributions which are often reinvested in additional shares of the fund</skos:example>
	</owl:Class>
	
	<owl:Class rdf:about="&fibo-cae-ce-cae;CashDividendAction">
		<rdfs:subClassOf rdf:resource="&fibo-cae-ce-cae;MandatoryCorporateAction"/>
		<rdfs:label xml:lang="en">cash dividend action</rdfs:label>
		<skos:definition xml:lang="en">corporate action that distributes cash to shareholders in proportion to their equity holding</skos:definition>
		<fibo-fnd-utl-av:explanatoryNote xml:lang="en">Ordinary dividends are typically recurring and regular.  The shareholder must take cash, and may be offered a choice of currency.</fibo-fnd-utl-av:explanatoryNote>
	</owl:Class>
	
	<owl:Class rdf:about="&fibo-cae-ce-cae;ChangeAction">
		<rdfs:subClassOf rdf:resource="&fibo-cae-ce-cae;MandatoryCorporateAction"/>
		<rdfs:label xml:lang="en">change action</rdfs:label>
		<skos:definition xml:lang="en">corporate action to disseminate information regarding a change further described in the corporate action details</skos:definition>
		<fibo-fnd-utl-av:explanatoryNote xml:lang="en">Generic changes may include a change in the terms of an issue, change in the identification of a security, change of board lot, change from global to definitive, etc.</fibo-fnd-utl-av:explanatoryNote>
	</owl:Class>
	
	<owl:Class rdf:about="&fibo-cae-ce-cae;ChangeOfSecurityTradingStatusEvent">
		<rdfs:subClassOf rdf:resource="&fibo-cae-ce-cae;CorporateChangeOfStatusEvent"/>
		<rdfs:subClassOf>
			<owl:Restriction>
				<owl:onProperty rdf:resource="&fibo-fnd-rel-rel;appliesTo"/>
				<owl:someValuesFrom rdf:resource="&fibo-md-temx-trs;SecurityTradingStatus"/>
			</owl:Restriction>
		</rdfs:subClassOf>
		<rdfs:label xml:lang="en">change of security trading status event</rdfs:label>
		<skos:definition xml:lang="en">An event in which the trading status of a tradable security changes.</skos:definition>
	</owl:Class>
	
	<owl:Class rdf:about="&fibo-cae-ce-cae;ChangeToSmallestNegotiableUnit">
		<rdfs:subClassOf rdf:resource="&fibo-cae-ce-cae;CorporateAction"/>
		<rdfs:label xml:lang="en">change to smallest negotiable unit</rdfs:label>
		<skos:definition xml:lang="en">Modification of the smallest negotiable unit of shares in order to obtain a new negotiable unit. SWIFT:SMAL</skos:definition>
	</owl:Class>
	
	<owl:Class rdf:about="&fibo-cae-ce-cae;ClassAction">
		<rdfs:subClassOf rdf:resource="&fibo-cae-ce-cae;VoluntaryCorporateAction"/>
		<rdfs:label xml:lang="en">class action</rdfs:label>
		<skos:definition xml:lang="en">corporate action involving a situation where interested parties seek restitution for financial loss</skos:definition>
		<fibo-fnd-utl-av:explanatoryNote xml:lang="en">The security holder may be offered the opportunity to join a class action proceeding and would need to respond with an instruction.</fibo-fnd-utl-av:explanatoryNote>
		<fibo-fnd-utl-av:synonym xml:lang="en">proposed settlement</fibo-fnd-utl-av:synonym>
	</owl:Class>
	
	<owl:Class rdf:about="&fibo-cae-ce-cae;ConsentSolicitation">
		<rdfs:subClassOf rdf:resource="&fibo-cae-ce-cae;VoluntaryCorporateAction"/>
		<rdfs:label xml:lang="en">consent solicitation</rdfs:label>
		<skos:definition xml:lang="en">corporate action that is a procedure that aims to obtain consent of holder to a proposal by the issuer or a third party without convening a meeting</skos:definition>
		<skos:example xml:lang="en">For example, consent to change the terms of a bond.</skos:example>
	</owl:Class>
	
	<owl:Class rdf:about="&fibo-cae-ce-cae;ConversionAction">
		<rdfs:subClassOf rdf:resource="&fibo-cae-ce-cae;VoluntaryCorporateAction"/>
		<rdfs:subClassOf>
			<owl:Restriction>
				<owl:onProperty rdf:resource="&fibo-cae-ce-cae;isConversionFrom"/>
				<owl:someValuesFrom rdf:resource="&fibo-fbc-fi-fi;Security"/>
			</owl:Restriction>
		</rdfs:subClassOf>
		<rdfs:subClassOf>
			<owl:Restriction>
				<owl:onProperty rdf:resource="&fibo-cae-ce-cae;isConversionTo"/>
				<owl:someValuesFrom rdf:resource="&fibo-fbc-fi-fi;Security"/>
			</owl:Restriction>
		</rdfs:subClassOf>
		<rdfs:label xml:lang="en">conversion action</rdfs:label>
		<skos:definition xml:lang="en">corporate action involving conversion of securities (generally convertible bonds or preferred shares) into another form of securities (usually common shares) at a pre-stated price/ratio</skos:definition>
	</owl:Class>
	
	<owl:Class rdf:about="&fibo-cae-ce-cae;ConversionSuspensionAction">
		<rdfs:subClassOf rdf:resource="&fibo-cae-ce-cae;CorporateAction"/>
		<rdfs:label xml:lang="en">conversion suspension action</rdfs:label>
		<skos:definition xml:lang="en">Suspensiion of conversion of securities generally a couple of weeks before a meeting takes place. SWIFT = SCOP</skos:definition>
	</owl:Class>
	
	<owl:Class rdf:about="&fibo-cae-ce-cae;CorporateAction">
		<rdfs:subClassOf rdf:resource="&fibo-fnd-dt-oc;OccurrenceKind"/>
		<rdfs:subClassOf>
			<owl:Restriction>
				<owl:onProperty rdf:resource="&fibo-fnd-rel-rel;appliesTo"/>
				<owl:someValuesFrom>
					<owl:Class>
						<owl:unionOf rdf:parseType="Collection">
							<rdf:Description rdf:about="&fibo-be-le-lp;LegalEntity">
							</rdf:Description>
							<rdf:Description rdf:about="&fibo-fbc-fi-fi;Security">
							</rdf:Description>
						</owl:unionOf>
					</owl:Class>
				</owl:someValuesFrom>
			</owl:Restriction>
		</rdfs:subClassOf>
		<rdfs:subClassOf>
			<owl:Restriction>
				<owl:onProperty rdf:resource="&lcc-cr;isClassifiedBy"/>
				<owl:someValuesFrom rdf:resource="&fibo-cae-ce-cae;CorporateActionClassifier"/>
			</owl:Restriction>
		</rdfs:subClassOf>
		<rdfs:label xml:lang="en">corporate action</rdfs:label>
		<skos:definition xml:lang="en">event carried out by a legal entity that affects the securities it issues and may have a material impact on its stakeholders, such as shareholders and creditors</skos:definition>
		<skos:example xml:lang="en">Examples of corporate actions include stock splits, dividends, mergers and acquisitions, rights issues, and spin-offs.</skos:example>
		<fibo-fnd-utl-av:explanatoryNote xml:lang="en">Corporate actions are typically approved by a company&apos;s board of directors and authorized by the shareholders.</fibo-fnd-utl-av:explanatoryNote>
	</owl:Class>
	
	<owl:Class rdf:about="&fibo-cae-ce-cae;CorporateActionClassificationScheme">
		<rdfs:subClassOf rdf:resource="&fibo-fnd-arr-cls;ClassificationScheme"/>
		<rdfs:subClassOf rdf:resource="&lcc-lr;CodeSet"/>
		<rdfs:subClassOf>
			<owl:Restriction>
				<owl:onProperty rdf:resource="&lcc-lr;hasMember"/>
				<owl:allValuesFrom rdf:resource="&fibo-cae-ce-cae;CorporateActionClassifier"/>
			</owl:Restriction>
		</rdfs:subClassOf>
		<rdfs:subClassOf>
			<owl:Restriction>
				<owl:onProperty rdf:resource="&fibo-fnd-rel-rel;defines"/>
				<owl:someValuesFrom rdf:resource="&fibo-cae-ce-cae;CorporateActionClassifier"/>
			</owl:Restriction>
		</rdfs:subClassOf>
		<rdfs:label>corporate action classification scheme</rdfs:label>
		<skos:definition>scheme for classifying corporate actions</skos:definition>
		<fibo-fnd-utl-av:usageNote>The set of corporate actions and income events included herein are a subset of those specified in ISO 15022 Securities - Scheme for Messages (Data Field Dictionary). Other schemes that are specific to a custodian, depository, or regulatory agency may also be important, and should take a similar approach with respect to classification.</fibo-fnd-utl-av:usageNote>
	</owl:Class>
	
	<owl:Class rdf:about="&fibo-cae-ce-cae;CorporateActionClassifier">
		<rdfs:subClassOf rdf:resource="&fibo-fnd-arr-cls;Classifier"/>
		<rdfs:subClassOf rdf:resource="&lcc-lr;CodeElement"/>
		<rdfs:subClassOf>
			<owl:Restriction>
				<owl:onProperty rdf:resource="&fibo-fnd-rel-rel;isDefinedIn"/>
				<owl:onClass rdf:resource="&fibo-cae-ce-cae;CorporateActionClassificationScheme"/>
				<owl:qualifiedCardinality rdf:datatype="&xsd;nonNegativeInteger">1</owl:qualifiedCardinality>
			</owl:Restriction>
		</rdfs:subClassOf>
		<rdfs:subClassOf>
			<owl:Restriction>
				<owl:onProperty rdf:resource="&lcc-lr;isMemberOf"/>
				<owl:onClass rdf:resource="&fibo-cae-ce-cae;CorporateActionClassificationScheme"/>
				<owl:qualifiedCardinality rdf:datatype="&xsd;nonNegativeInteger">1</owl:qualifiedCardinality>
			</owl:Restriction>
		</rdfs:subClassOf>
		<rdfs:subClassOf>
			<owl:Restriction>
				<owl:onProperty rdf:resource="&lcc-cr;classifies"/>
				<owl:someValuesFrom rdf:resource="&fibo-cae-ce-cae;CorporateAction"/>
			</owl:Restriction>
		</rdfs:subClassOf>
		<rdfs:subClassOf>
			<owl:Restriction>
				<owl:onProperty rdf:resource="&lcc-lr;denotes"/>
				<owl:someValuesFrom rdf:resource="&fibo-cae-ce-cae;CorporateAction"/>
			</owl:Restriction>
		</rdfs:subClassOf>
		<rdfs:subClassOf>
			<owl:Restriction>
				<owl:onProperty rdf:resource="&lcc-lr;hasTag"/>
				<owl:someValuesFrom rdf:resource="&xsd;string"/>
			</owl:Restriction>
		</rdfs:subClassOf>
		<rdfs:label xml:lang="en">corporate action classifier</rdfs:label>
		<skos:definition xml:lang="en">classifier that distinguishes income-oriented events from other corporate actions</skos:definition>
		<fibo-fnd-utl-av:explanatoryNote xml:lang="en">ISO 15022 classifies events as impacting income vs. others.  Other classification schemes distinguish between actions that return profits to shareholders, actions that are designed to influence the share price, and actions involving a change in structure to the issuer organization.</fibo-fnd-utl-av:explanatoryNote>
	</owl:Class>
	
	<owl:Class rdf:about="&fibo-cae-ce-cae;CorporateActionObligation">
		<rdfs:subClassOf rdf:resource="&fibo-cae-ce-cae;CorporateAction"/>
		<rdfs:subClassOf rdf:resource="&fibo-fnd-law-lcap;Duty"/>
		<rdfs:label xml:lang="en">corporate action obligation</rdfs:label>
		<skos:definition xml:lang="en">An obligation related to the holding of a Security.</skos:definition>
		<fibo-fnd-utl-av:explanatoryNote xml:lang="en">Delivery of a security. Not defining direction at this level of the model - one party may have an obligation to deliver security or to pay; other party may have an obligation to deliver or to pay. Or there may be just one.</fibo-fnd-utl-av:explanatoryNote>
	</owl:Class>
	
	<owl:Class rdf:about="&fibo-cae-ce-cae;CorporateActionPaymentObligation">
		<rdfs:subClassOf rdf:resource="&fibo-cae-ce-cae;CorporateActionObligation"/>
		<rdfs:label xml:lang="en">corporate action payment obligation</rdfs:label>
	</owl:Class>
	
	<owl:Class rdf:about="&fibo-cae-ce-cae;CorporateActionSecuritiesDeliveryObligation">
		<rdfs:subClassOf rdf:resource="&fibo-cae-ce-cae;CorporateActionObligation"/>
		<rdfs:label xml:lang="en">corporate action securities delivery obligation</rdfs:label>
		<skos:definition xml:lang="en">Some obligation to deliver some security in the thr context of corporate actions. All cash proceeds and security proceeds can be represented a s acontractual obligation. Where does that obligation arise? Usually in the Contract itself - but there may be other answers to this. Defines what has to be delivered. or paid. Entitlement meanwhile is a calculation based on the Contract.</skos:definition>
	</owl:Class>
	
	<owl:Class rdf:about="&fibo-cae-ce-cae;CorporateChangeOfStatusEvent">
		<rdfs:subClassOf rdf:resource="&fibo-cae-ce-cae;CorporateAction"/>
		<rdfs:label xml:lang="en">corporate change of status event</rdfs:label>
		<skos:definition xml:lang="en">Some change to the status of some security.</skos:definition>
		<fibo-fnd-utl-av:explanatoryNote xml:lang="en">This is generally described by a corporate event message. For example, change in trading status, listing status.</fibo-fnd-utl-av:explanatoryNote>
	</owl:Class>
	
	<owl:Class rdf:about="&fibo-cae-ce-cae;CorporateModificationEvent">
		<rdfs:subClassOf rdf:resource="&fibo-cae-ce-cae;CorporateAction"/>
		<rdfs:label xml:lang="en">corporate modification event</rdfs:label>
		<skos:definition xml:lang="en">Some change in details of some company, which needs to be described for publicly issued securities issued by that company.</skos:definition>
		<fibo-fnd-utl-av:explanatoryNote xml:lang="en">Usually described in a corporate event message. Note that the change relates to the company, but notification about this, for publicly issued securities (shares, bonds) is notificed to the holders of each such security, as corporate event messages.</fibo-fnd-utl-av:explanatoryNote>
	</owl:Class>
	
	<owl:Class rdf:about="&fibo-cae-ce-cae;CouponStrip">
		<rdfs:subClassOf rdf:resource="&fibo-cae-ce-cae;CorporateAction"/>
		<rdfs:subClassOf>
			<owl:Restriction>
				<owl:onProperty rdf:resource="&fibo-fnd-rel-rel;appliesTo"/>
				<owl:someValuesFrom rdf:resource="&fibo-sec-dbt-bnd;Bond"/>
			</owl:Restriction>
		</rdfs:subClassOf>
		<rdfs:label xml:lang="en">coupon strip</rdfs:label>
		<skos:definition xml:lang="en">Coupon stripping is the process whereby interest coupons for future payment dates are separated from the security corpus that entitles the holder to the principal repayment.</skos:definition>
	</owl:Class>
	
	<owl:NamedIndividual rdf:about="&fibo-cae-ce-cae;DECR">
		<rdf:type rdf:resource="&fibo-cae-ce-cae;IncomeOrientedAction"/>
		<rdfs:label xml:lang="en">DECR</rdfs:label>
		<skos:definition xml:lang="en">SWIFT ISO 15022 classifier for corporate actions that reduce the face value of a share or the value of fund assets</skos:definition>
		<fibo-fnd-rel-rel:isDefinedIn rdf:resource="&fibo-cae-ce-cae;ISO15022CorporateActionClassificationScheme"/>
		<lcc-cr:classifies rdf:resource="&fibo-cae-ce-cae;DecreaseInValueAction"/>
		<lcc-lr:denotes rdf:resource="&fibo-cae-ce-cae;DecreaseInValueAction"/>
		<lcc-lr:hasTag>DECR</lcc-lr:hasTag>
		<lcc-lr:isMemberOf rdf:resource="&fibo-cae-ce-cae;ISO15022CorporateActionClassificationScheme"/>
	</owl:NamedIndividual>
	
	<owl:NamedIndividual rdf:about="&fibo-cae-ce-cae;DFLT">
		<rdf:type rdf:resource="&fibo-cae-ce-cae;BusinessStrategyOrientedAction"/>
		<rdfs:label xml:lang="en">DFLT</rdfs:label>
		<skos:definition xml:lang="en">SWIFT ISO 15022 classifier for corporate actions that indicate a failure by the issuer to perform obligations defined as default events under the bond agreement and that have not been remedied</skos:definition>
		<fibo-fnd-rel-rel:isDefinedIn rdf:resource="&fibo-cae-ce-cae;ISO15022CorporateActionClassificationScheme"/>
		<lcc-cr:classifies rdf:resource="&fibo-cae-ce-cae;BondDefaultAction"/>
		<lcc-lr:denotes rdf:resource="&fibo-cae-ce-cae;BondDefaultAction"/>
		<lcc-lr:hasTag>DFLT</lcc-lr:hasTag>
		<lcc-lr:isMemberOf rdf:resource="&fibo-cae-ce-cae;ISO15022CorporateActionClassificationScheme"/>
	</owl:NamedIndividual>
	
	<owl:NamedIndividual rdf:about="&fibo-cae-ce-cae;DRIP">
		<rdf:type rdf:resource="&fibo-cae-ce-cae;BusinessStrategyOrientedAction"/>
		<rdfs:label xml:lang="en">DRIP</rdfs:label>
		<skos:definition xml:lang="en">SWIFT ISO 15022 classifier for corporate actions that involve a dividend payment whereby holders can keep cash or have the cash reinvested into additional shares in the issuing company</skos:definition>
		<fibo-fnd-rel-rel:isDefinedIn rdf:resource="&fibo-cae-ce-cae;ISO15022CorporateActionClassificationScheme"/>
		<lcc-cr:classifies rdf:resource="&fibo-cae-ce-cae;DividendReinvestmentAction"/>
		<lcc-lr:denotes rdf:resource="&fibo-cae-ce-cae;DividendReinvestmentAction"/>
		<lcc-lr:hasTag>DRIP</lcc-lr:hasTag>
		<lcc-lr:isMemberOf rdf:resource="&fibo-cae-ce-cae;ISO15022CorporateActionClassificationScheme"/>
	</owl:NamedIndividual>
	
	<owl:NamedIndividual rdf:about="&fibo-cae-ce-cae;DSCL">
		<rdf:type rdf:resource="&fibo-cae-ce-cae;BusinessStrategyOrientedAction"/>
		<rdfs:label xml:lang="en">DSCL</rdfs:label>
		<skos:definition xml:lang="en">SWIFT ISO 15022 classifier for corporate actions that involve a requirement for holders or beneficial owners to disclose their name, location and holdings of any issue to the issuer</skos:definition>
		<fibo-fnd-rel-rel:isDefinedIn rdf:resource="&fibo-cae-ce-cae;ISO15022CorporateActionClassificationScheme"/>
		<lcc-cr:classifies rdf:resource="&fibo-cae-ce-cae;DisclosureAction"/>
		<lcc-lr:denotes rdf:resource="&fibo-cae-ce-cae;DisclosureAction"/>
		<lcc-lr:hasTag>DSCL</lcc-lr:hasTag>
		<lcc-lr:isMemberOf rdf:resource="&fibo-cae-ce-cae;ISO15022CorporateActionClassificationScheme"/>
	</owl:NamedIndividual>
	
	<owl:NamedIndividual rdf:about="&fibo-cae-ce-cae;DVCA">
		<rdf:type rdf:resource="&fibo-cae-ce-cae;IncomeOrientedAction"/>
		<rdfs:label xml:lang="en">DVCA</rdfs:label>
		<skos:definition xml:lang="en">SWIFT ISO 15022 classifier for corporate actions that distribute cash to shareholders in proportion to their equity holding</skos:definition>
		<fibo-fnd-rel-rel:isDefinedIn rdf:resource="&fibo-cae-ce-cae;ISO15022CorporateActionClassificationScheme"/>
		<lcc-cr:classifies rdf:resource="&fibo-cae-ce-cae;CashDividendAction"/>
		<lcc-lr:denotes rdf:resource="&fibo-cae-ce-cae;CashDividendAction"/>
		<lcc-lr:hasTag>DVCA</lcc-lr:hasTag>
		<lcc-lr:isMemberOf rdf:resource="&fibo-cae-ce-cae;ISO15022CorporateActionClassificationScheme"/>
	</owl:NamedIndividual>
	
	<owl:NamedIndividual rdf:about="&fibo-cae-ce-cae;DVOP">
		<rdf:type rdf:resource="&fibo-cae-ce-cae;BusinessStrategyOrientedAction"/>
		<rdfs:label xml:lang="en">DVOP</rdfs:label>
		<skos:definition xml:lang="en">SWIFT ISO 15022 classifier for corporate actions that involve distribution of a dividend to shareholders with a choice of benefit to receive</skos:definition>
		<fibo-fnd-rel-rel:isDefinedIn rdf:resource="&fibo-cae-ce-cae;ISO15022CorporateActionClassificationScheme"/>
		<lcc-cr:classifies rdf:resource="&fibo-cae-ce-cae;DividendOptionAction"/>
		<lcc-lr:denotes rdf:resource="&fibo-cae-ce-cae;DividendOptionAction"/>
		<lcc-lr:hasTag>DVOP</lcc-lr:hasTag>
		<lcc-lr:isMemberOf rdf:resource="&fibo-cae-ce-cae;ISO15022CorporateActionClassificationScheme"/>
	</owl:NamedIndividual>
	
	<owl:NamedIndividual rdf:about="&fibo-cae-ce-cae;DVSE">
		<rdf:type rdf:resource="&fibo-cae-ce-cae;BusinessStrategyOrientedAction"/>
		<rdfs:label xml:lang="en">DVSE</rdfs:label>
		<skos:definition xml:lang="en">SWIFT ISO 15022 classifier for corporate actions that involve distribution of a dividend to shareholders in the form of equities of the issuing corporation</skos:definition>
		<fibo-fnd-rel-rel:isDefinedIn rdf:resource="&fibo-cae-ce-cae;ISO15022CorporateActionClassificationScheme"/>
		<lcc-cr:classifies rdf:resource="&fibo-cae-ce-cae;StockDividendAction"/>
		<lcc-lr:denotes rdf:resource="&fibo-cae-ce-cae;StockDividendAction"/>
		<lcc-lr:hasTag>DVSE</lcc-lr:hasTag>
		<lcc-lr:isMemberOf rdf:resource="&fibo-cae-ce-cae;ISO15022CorporateActionClassificationScheme"/>
	</owl:NamedIndividual>
	
	<owl:Class rdf:about="&fibo-cae-ce-cae;DebtDrawingNotification">
		<rdfs:subClassOf rdf:resource="&fibo-fnd-arr-doc;Notice"/>
		<rdfs:label xml:lang="en">debt drawing notification</rdfs:label>
		<skos:definition xml:lang="en">Redemption in part before the scheduled final maturity date of a security. SWIFT = DRAW</skos:definition>
	</owl:Class>
	
	<owl:Class rdf:about="&fibo-cae-ce-cae;DebtInstrumentBuybackNotification">
		<rdfs:subClassOf rdf:resource="&fibo-fnd-arr-doc;Notice"/>
		<rdfs:label xml:lang="en">debt instrument buyback notification</rdfs:label>
		<skos:definition xml:lang="en">Notification of an event where det securities are bought back by the issuer.</skos:definition>
		<fibo-fnd-utl-av:explanatoryNote xml:lang="en">See also puts and calls (these are usually pre-arranged). Here the company goes out to the market and buys back their own debt. This does not really need to be a corporate event, they just do it. REVIEW: This term may not be needed. Not a corporate action.</fibo-fnd-utl-av:explanatoryNote>
	</owl:Class>
	
	<owl:Class rdf:about="&fibo-cae-ce-cae;DecreaseInValueAction">
		<rdfs:subClassOf rdf:resource="&fibo-cae-ce-cae;MandatoryCorporateAction"/>
		<rdfs:label xml:lang="en">decrease in value action</rdfs:label>
		<skos:definition xml:lang="en">corporate action resulting in a reduction of face value of a share or the value of fund assets</skos:definition>
		<fibo-fnd-utl-av:explanatoryNote xml:lang="en">The number of circulating shares/units remains unchanged. This event may include a cash pay out to holders.</fibo-fnd-utl-av:explanatoryNote>
	</owl:Class>
	
	<owl:Class rdf:about="&fibo-cae-ce-cae;DetachmentAction">
		<rdfs:subClassOf rdf:resource="&fibo-cae-ce-cae;CorporateAction"/>
		<rdfs:label xml:lang="en">detachment action</rdfs:label>
	</owl:Class>
	
	<owl:Class rdf:about="&fibo-cae-ce-cae;DisclosureAction">
		<rdfs:subClassOf rdf:resource="&fibo-cae-ce-cae;VoluntaryCorporateAction"/>
		<rdfs:label xml:lang="en">disclosure action</rdfs:label>
		<skos:definition xml:lang="en">corporate action involving a requirement for holders or beneficial owners to disclose their name, location and holdings of any issue to the issuer</skos:definition>
		<fibo-fnd-utl-av:explanatoryNote xml:lang="en">This event only occurs with the characteristic VOLU, otherwise it is part of the SRD II.</fibo-fnd-utl-av:explanatoryNote>
	</owl:Class>
	
	<owl:Class rdf:about="&fibo-cae-ce-cae;DividendOptionAction">
		<rdfs:subClassOf rdf:resource="&fibo-cae-ce-cae;MandatoryWithChoiceCorporateAction"/>
		<rdfs:label xml:lang="en">dividend option action</rdfs:label>
		<skos:definition xml:lang="en">corporate action that involves distribution of a dividend to shareholders with a choice of benefit to receive</skos:definition>
		<fibo-fnd-utl-av:explanatoryNote xml:lang="en">Shareholders may choose to receive shares or cash. A dividend option action is distinguished from reinvestment (DRIP) as, like a cash dividend, the company creates new share capital in exchange for the dividend rather than investing the dividend in the market.</fibo-fnd-utl-av:explanatoryNote>
	</owl:Class>
	
	<owl:Class rdf:about="&fibo-cae-ce-cae;DividendReinvestmentAction">
		<rdfs:subClassOf rdf:resource="&fibo-cae-ce-cae;MandatoryWithChoiceCorporateAction"/>
		<rdfs:label xml:lang="en">dividend reinvestment action</rdfs:label>
		<skos:definition xml:lang="en">corporate action that involves a dividend payment whereby holders can keep cash or have the cash reinvested into additional shares in the issuing company</skos:definition>
		<fibo-fnd-utl-av:explanatoryNote xml:lang="en">Dividend reinvestment is distinguished from a cash dividend in that the issuer invests the dividend in the market rather than creating new share capital in exchange for the dividend.</fibo-fnd-utl-av:explanatoryNote>
	</owl:Class>
	
	<owl:Class rdf:about="&fibo-cae-ce-cae;Drawing">
		<rdfs:subClassOf rdf:resource="&fibo-cae-ce-cae;MandatoryCorporateAction"/>
		<rdfs:label xml:lang="en">drawing</rdfs:label>
		<skos:definition xml:lang="en">Redemption in part before the scheduled final maturity date of a security.</skos:definition>
		<fibo-fnd-utl-av:explanatoryNote xml:lang="en">Notification in advance of this happening.</fibo-fnd-utl-av:explanatoryNote>
	</owl:Class>
	
	<owl:Class rdf:about="&fibo-cae-ce-cae;DutchAuction">
		<rdfs:subClassOf rdf:resource="&fibo-cae-ce-cae;VoluntaryCorporateAction"/>
		<rdfs:label xml:lang="en">dutch auction</rdfs:label>
		<skos:definition xml:lang="en">Similar to a tender offer, a Dutch auction is an action by a party wishing to acquire a particular security. Current holders of the targeted security are invited to make an offer in which they would be willling to sell their holdings. UPDATE THIS DEFINITION: Similar to a tender offer, a Dutch auction is the result of an action by a third party wishing to acquire a particular security. Current holders of the targeted security are invited (and given a message by the issuer) to make an offer in which they would be willling to sell their holdings. OR It might also represent a separate scenario where third parties do this, as per the original SWIFT defition. You can only go to the Registrar which would the other scenario impossible. Agents and Registrars: The issue issuer os the company which issued the shares (as modeled); Most companies don&apos;t interact directly with the market to find out who they need to disseminate the info to. They can, but more likely the employ &quot;Issuers Agent&quot;. That provides one point of contact from the organization. That agent handles all coms with the Registrars, and to the news wires etc., to disseminate the corporate action. Context: CAE only, or in the context of the Issue? When you issue the security you nominate an Agent, in the prospectus, there is specified an Issuing Agent. This is the one that does these things. Usually a merchant bank etc. in the old days. This is who will have directly facilitated that direct market engagement. Next question: This is part of going public, so these agents are appointed as part of going public.</skos:definition>
		<fibo-fnd-utl-av:explanatoryNote xml:lang="en">The party to which the offer is made need not be the holder. Details: Question on &quot;Who is the actor?&quot; Dutch auction would have multiple parties? What is the scenario? Usually happens when a company is about to go into administration. Looking at the scneario descried in the SWIFT definition - not clear if this is the only such scenario. Possibly the issuer has to notif ythe shareholders that the offer is being made. The offer is made by the third party but the notice is sent by the issuer (via their agent) and via the registrar who holds the details of who holds all the shares. Example: Lloyds banking group - most shares would be owned by the market, and a small percentage might be held by private investors. So in this scenario everyone has to be given the opportunity to sell at the given price. so the CAE message is still issued by the Issuer. SWIFT detailed names (synonym?) &quot;Dutch Auction, Bid Tender&quot;</fibo-fnd-utl-av:explanatoryNote>
	</owl:Class>
	
	<owl:NamedIndividual rdf:about="&fibo-cae-ce-cae;EXTM">
		<rdf:type rdf:resource="&fibo-cae-ce-cae;BusinessStrategyOrientedAction"/>
		<rdfs:label xml:lang="en">EXTM</rdfs:label>
		<skos:definition xml:lang="en">SWIFT ISO 15022 classifier for corporate actions that involve prolonging the maturity date of a bond</skos:definition>
		<fibo-fnd-rel-rel:isDefinedIn rdf:resource="&fibo-cae-ce-cae;ISO15022CorporateActionClassificationScheme"/>
		<lcc-cr:classifies rdf:resource="&fibo-cae-ce-cae;MaturityExtension"/>
		<lcc-lr:denotes rdf:resource="&fibo-cae-ce-cae;MaturityExtension"/>
		<lcc-lr:hasTag>EXTM</lcc-lr:hasTag>
		<lcc-lr:isMemberOf rdf:resource="&fibo-cae-ce-cae;ISO15022CorporateActionClassificationScheme"/>
	</owl:NamedIndividual>
	
	<owl:NamedIndividual rdf:about="&fibo-cae-ce-cae;EXWA">
		<rdf:type rdf:resource="&fibo-cae-ce-cae;IncomeOrientedAction"/>
		<rdfs:label xml:lang="en">EXWA</rdfs:label>
		<skos:definition xml:lang="en">SWIFT ISO 15022 classifier for corporate actions that offer holders the option to buy (call warrant) or to sell (put warrant) a specific amount of stock, cash, or commodity, at a predetermined price, during a predetermined period of time</skos:definition>
		<fibo-fnd-rel-rel:isDefinedIn rdf:resource="&fibo-cae-ce-cae;ISO15022CorporateActionClassificationScheme"/>
		<lcc-cr:classifies rdf:resource="&fibo-cae-ce-cae;WarrantExerciseAction"/>
		<lcc-lr:denotes rdf:resource="&fibo-cae-ce-cae;WarrantExerciseAction"/>
		<lcc-lr:hasTag>EXWA</lcc-lr:hasTag>
		<lcc-lr:isMemberOf rdf:resource="&fibo-cae-ce-cae;ISO15022CorporateActionClassificationScheme"/>
	</owl:NamedIndividual>
	
	<owl:Class rdf:about="&fibo-cae-ce-cae;ExchangeOffer">
		<rdfs:subClassOf rdf:resource="&fibo-cae-ce-cae;CorporateAction"/>
		<rdfs:subClassOf>
			<owl:Restriction>
				<owl:onProperty rdf:resource="&fibo-fnd-rel-rel;appliesTo"/>
				<owl:someValuesFrom rdf:resource="&fibo-fbc-fi-fi;Security"/>
			</owl:Restriction>
		</rdfs:subClassOf>
		<rdfs:label xml:lang="en">exchange offer</rdfs:label>
		<skos:definition xml:lang="en">Exchange offer; Capital reorganisation. Offer to shareholders to exchange their holdings for other securities and/or cash. Exchange offers are usually voluntary. Example: Where the &quot;usually voluntary&quot; comes in is that Announcement Payout Option 1: Cash 2. Stocks 3. Cash and Stock Holder picks option 1, 2 or 3 (= 1 &amp; 2). the voluntary aspect is where it&apos;s an Exchange Offer. It&apos;s mandatory to pick one of 1 - 3. Otherwise defaults to cash on payment date. Option Payout Componnet is the terms for the choice. Exchange Offer may be voluntary, not always Mandator With Choice. for example, there are legal qualifications on what is possible. Preceded by Tender Offer. Consequences dependent on scenarios. Once the firm making the offer gets to a given (legally defined) threshold e.g. 90% then they have the right to acquire all of the outstanding shares. An Exchange Offer is therefore a specialization of a Tender Offer. It&apos;s the specialization where the above mentioned requirements have been met. Further detail: Happens in a wider range of circumsntaces. Is soecifically associated with the issuer. this could be voluntary or not. EXOF could be any of the three (mand, vol, man w choice). tendre is always voluntary.</skos:definition>
	</owl:Class>
	
	<owl:Class rdf:about="&fibo-cae-ce-cae;FormalOffer">
		<rdfs:subClassOf rdf:resource="&fibo-cae-ce-cae;VoluntaryCorporateAction"/>
		<rdfs:label xml:lang="en">formal offer</rdfs:label>
		<owl:equivalentClass>
			<owl:Class>
				<owl:unionOf rdf:parseType="Collection">
					<rdf:Description rdf:about="&fibo-cae-ce-cae;DutchAuction">
					</rdf:Description>
					<rdf:Description rdf:about="&fibo-cae-ce-cae;ExchangeOffer">
					</rdf:Description>
					<rdf:Description rdf:about="&fibo-cae-ce-cae;RepurchaseOffer">
					</rdf:Description>
					<rdf:Description rdf:about="&fibo-cae-ce-cae;TenderOffer">
					</rdf:Description>
				</owl:unionOf>
			</owl:Class>
		</owl:equivalentClass>
		<skos:definition xml:lang="en">Event which is an offer to the holder or potential holder or other intersted party, to enter into a trade which is or would be legally binding on the part of the party making the offer (the offeror).</skos:definition>
	</owl:Class>
	
	<owl:Class rdf:about="&fibo-cae-ce-cae;FullCallEarlyRedemptionAction">
		<rdfs:subClassOf rdf:resource="&fibo-cae-ce-cae;MandatoryCorporateAction"/>
		<rdfs:label xml:lang="en">full call early redemption action</rdfs:label>
		<skos:definition xml:lang="en">corporate action that involves redemption of an entire issue outstanding of securities prior to maturity</skos:definition>
		<skos:example xml:lang="en">Examples securities that may be subject to a full call/early redemption include bonds, preferred equity, funds, that may be redeemed by the issuer or its agent before final maturity.</skos:example>
	</owl:Class>
	
	<owl:NamedIndividual rdf:about="&fibo-cae-ce-cae;INTR">
		<rdf:type rdf:resource="&fibo-cae-ce-cae;IncomeOrientedAction"/>
		<rdfs:label xml:lang="en">INTR</rdfs:label>
		<skos:definition xml:lang="en">SWIFT ISO 15022 classifier for corporate actions that involve distribution of a regular interest payment to holders of an interest-bearing asset</skos:definition>
		<fibo-fnd-rel-rel:isDefinedIn rdf:resource="&fibo-cae-ce-cae;ISO15022CorporateActionClassificationScheme"/>
		<lcc-cr:classifies rdf:resource="&fibo-cae-ce-cae;InterestPaymentAction"/>
		<lcc-lr:denotes rdf:resource="&fibo-cae-ce-cae;InterestPaymentAction"/>
		<lcc-lr:hasTag>INTR</lcc-lr:hasTag>
		<lcc-lr:isMemberOf rdf:resource="&fibo-cae-ce-cae;ISO15022CorporateActionClassificationScheme"/>
	</owl:NamedIndividual>
	
	<owl:NamedIndividual rdf:about="&fibo-cae-ce-cae;ISO15022CorporateActionClassificationScheme">
		<rdf:type rdf:resource="&fibo-cae-ce-cae;CorporateActionClassificationScheme"/>
		<rdfs:label>ISO 15022 corporate action classification scheme</rdfs:label>
		<skos:definition>scheme for classifying corporate actions according to ISO 15022 Securities - Scheme for Messages (Data Field Dictionary)</skos:definition>
	</owl:NamedIndividual>
	
	<owl:Class rdf:about="&fibo-cae-ce-cae;IncomeOrientedAction">
		<rdfs:subClassOf rdf:resource="&fibo-cae-ce-cae;CorporateActionClassifier"/>
		<rdfs:label xml:lang="en">income-oriented action</rdfs:label>
		<skos:definition xml:lang="en">classifier of corporate actions that impacts income to shareholders</skos:definition>
		<fibo-fnd-utl-av:explanatoryNote xml:lang="en">Cash dividends are a classic example where a public company declares a dividend to be paid on each outstanding share. Bonus is another case where the shareholder is rewarded. In a stricter sense, the bonus issue should not impact the share price but in reality, in rare cases, it does and results in an overall increase in value.</fibo-fnd-utl-av:explanatoryNote>
	</owl:Class>
	
	<owl:Class rdf:about="&fibo-cae-ce-cae;InterestPaymentAction">
		<rdfs:subClassOf rdf:resource="&fibo-cae-ce-cae;MandatoryCorporateAction"/>
		<rdfs:label xml:lang="en">interest payment action</rdfs:label>
		<skos:definition xml:lang="en">corporate action that involves distribution of a regular interest payment to holders of an interest-bearing asset</skos:definition>
		<skos:editorialNote xml:lang="en">Further notes: Are there options on the Holder? Yes, you can opt to be paid in a certain currency. It is not always defined in the security terms. So if the Terms in the Security terms sheet gives you an option, there is a choice for the Holder at this point. Such choices would include: - Currency - Pay in Kind (&quot;Spinoff&quot; or PiK - see PiK corporate Action) Could be mandatory. If there were an option then the letter announcing it would require a response. This is usually stated in the message. Is there a message even if there is no option? Yes. Usually have to generate the events artificially as the Servicing organization. you can&apos;t rely on a feed or message coming in but because it is part of the security contract the above has to generate at the expected time, and arrange the payments. Q: That is the point at there was a choice you would expect to see a message, or end up still having to generate it but with the choices. A: The ones with Choices come as announcements and don&apos;t ave to be generated by the Service. Older definitin (re-scoped now: An Event in which a payment occurs. Anything can have a payment event. If a thing hits a pay date, whether it&apos;s voluntary or mandatory, that&apos;s a payment event. Divide into: Securities Cash Combination Payment or Distribution? Are these exclusive? Take an event that&apos;s always a combination of options, and an option is a combination of payouts. Generates transactions - determine what txns happen when a customer chooses that option. Distribution / delivery: generic concept Payment - implis cash distribution. So payment is specialization of distribution.</skos:editorialNote>
	</owl:Class>
	
	<owl:Class rdf:about="&fibo-cae-ce-cae;InterestPaymentInKind">
		<rdfs:subClassOf rdf:resource="&fibo-cae-ce-cae;InterestPaymentAction"/>
		<rdfs:label xml:lang="en">interest payment in kind</rdfs:label>
		<skos:definition xml:lang="en">Interest payment, in any kind except cash, distributed to holders of an interest bearing asset. SWIFT = PINK</skos:definition>
	</owl:Class>
	
	<owl:Class rdf:about="&fibo-cae-ce-cae;InterestPaymentWithPrincipal">
		<rdfs:subClassOf rdf:resource="&fibo-cae-ce-cae;InterestPaymentAction"/>
		<rdfs:label xml:lang="en">interest payment with principal</rdfs:label>
		<skos:definition xml:lang="en">A payment of a portion of the principal of an interest bearing asset, in addition to the interest payment. SWIFT = PRII</skos:definition>
	</owl:Class>
	
	<owl:Class rdf:about="&fibo-cae-ce-cae;InterestRateAdjustment">
		<rdfs:subClassOf rdf:resource="&fibo-cae-ce-cae;MandatoryCorporateAction"/>
		<rdfs:subClassOf>
			<owl:Restriction>
				<owl:onProperty rdf:resource="&fibo-fnd-rel-rel;appliesTo"/>
				<owl:someValuesFrom rdf:resource="&fibo-sec-dbt-bnd;VariableCouponBond"/>
			</owl:Restriction>
		</rdfs:subClassOf>
		<rdfs:label xml:lang="en">interest rate adjustment</rdfs:label>
		<skos:definition xml:lang="en">Scheduled change to the coupon rate for a floating or adjustable rate security.</skos:definition>
		<fibo-fnd-utl-av:explanatoryNote xml:lang="en">The SWIFT definition as given defines the notification of the interest rate change, not the adjustment. Adjusted to describe the event. REVIEW: Is this really an action? Usually consider that it&apos;s expected. Given definition was for the announcement. SWIFT full definition &quot;Announcement of the current coupon rate for a floating or adjustable rate security.&quot;</fibo-fnd-utl-av:explanatoryNote>
	</owl:Class>
	
	<owl:Class rdf:about="&fibo-cae-ce-cae;LiquidationAction">
		<rdfs:subClassOf rdf:resource="&fibo-cae-ce-cae;MandatoryCorporateAction"/>
		<rdfs:label xml:lang="en">liquidation action</rdfs:label>
		<skos:definition xml:lang="en">Liquidating dividend/Liquidation consist of a distribution of cash, assets, or both. Debt may be paid in order of priority based on preferred claims to assets specified by the security. SWIFT = LIQU</skos:definition>
	</owl:Class>
	
	<owl:Class rdf:about="&fibo-cae-ce-cae;ListingStatusDelistingMessage">
		<rdfs:subClassOf rdf:resource="&fibo-fnd-arr-doc;Notice"/>
		<rdfs:label xml:lang="en">listing status delisting message</rdfs:label>
		<skos:definition xml:lang="en">Security is no longer able to comply with the listing requirements of a stock exchange and is removed from official board quotation.</skos:definition>
	</owl:Class>
	
	<owl:NamedIndividual rdf:about="&fibo-cae-ce-cae;MCAL">
		<rdf:type rdf:resource="&fibo-cae-ce-cae;IncomeOrientedAction"/>
		<rdfs:label xml:lang="en">MCAL</rdfs:label>
		<skos:definition xml:lang="en">SWIFT ISO 15022 classifier for corporate actions that involve redemption of an entire issue outstanding of securities prior to maturity</skos:definition>
		<fibo-fnd-rel-rel:isDefinedIn rdf:resource="&fibo-cae-ce-cae;ISO15022CorporateActionClassificationScheme"/>
		<lcc-cr:classifies rdf:resource="&fibo-cae-ce-cae;FullCallEarlyRedemptionAction"/>
		<lcc-lr:denotes rdf:resource="&fibo-cae-ce-cae;FullCallEarlyRedemptionAction"/>
		<lcc-lr:hasTag>MCAL</lcc-lr:hasTag>
		<lcc-lr:isMemberOf rdf:resource="&fibo-cae-ce-cae;ISO15022CorporateActionClassificationScheme"/>
	</owl:NamedIndividual>
	
	<owl:Class rdf:about="&fibo-cae-ce-cae;MandatoryCorporateAction">
		<rdfs:subClassOf rdf:resource="&fibo-cae-ce-cae;CorporateAction"/>
		<rdfs:label xml:lang="en">mandatory corporate action</rdfs:label>
		<skos:definition xml:lang="en">event initiated by the board of directors of the corporation that affects all shareholders</skos:definition>
		<skos:example xml:lang="en">Examples of mandatory corporate actions include cash dividends, stock splits, mergers, pre-refunding, return of capital, bonus issue, asset ID change, and spin-offs.</skos:example>
		<fibo-fnd-utl-av:explanatoryNote xml:lang="en">Mandatory means mandatory participation by all shareholders, however the shareholder is not required to do anything.  Shareholders are passive beneficiaries of mandatory actions.</fibo-fnd-utl-av:explanatoryNote>
	</owl:Class>
	
	<owl:Class rdf:about="&fibo-cae-ce-cae;MandatoryWithChoiceCorporateAction">
		<rdfs:subClassOf rdf:resource="&fibo-cae-ce-cae;MandatoryCorporateAction"/>
		<rdfs:label xml:lang="en">mandatory with choice corporate action</rdfs:label>
		<skos:definition xml:lang="en">mandatory corporate action where shareholders are given an opportunity to choose among several options</skos:definition>
		<fibo-fnd-utl-av:explanatoryNote xml:lang="en">In case a shareholder does not submit the election, the default option will be applied.</fibo-fnd-utl-av:explanatoryNote>
	</owl:Class>
	
	<owl:Class rdf:about="&fibo-cae-ce-cae;MaturityExtension">
		<rdfs:subClassOf rdf:resource="&fibo-cae-ce-cae;CorporateAction"/>
		<rdfs:subClassOf>
			<owl:Restriction>
				<owl:onProperty rdf:resource="&fibo-fnd-rel-rel;appliesTo"/>
				<owl:someValuesFrom rdf:resource="&fibo-sec-eq-eq;Share"/>
			</owl:Restriction>
		</rdfs:subClassOf>
		<rdfs:label xml:lang="en">maturity extension</rdfs:label>
		<skos:definition xml:lang="en">corporate action that, as stipulated in a bond&apos;s terms and conditions, the issuer or the bondholder may prolong the maturity date of a bond</skos:definition>
		<fibo-fnd-utl-av:explanatoryNote xml:lang="en">After extension, the security may differ from original issue (new rate or maturity date). May be subject to bondholder&apos;s approval. May be mandatory or voluntary, depending on who initiates it and the surrounding circumstances.</fibo-fnd-utl-av:explanatoryNote>
	</owl:Class>
	
	<owl:Class rdf:about="&fibo-cae-ce-cae;NotificationEvent">
		<rdfs:subClassOf rdf:resource="&fibo-cae-ce-cae;MandatoryCorporateAction"/>
		<rdfs:label xml:lang="en">notification event</rdfs:label>
		<skos:definition xml:lang="en">A notification to the shareholders that therre is a corporate action out there. This is distinct from the CA itself. not the same as Event Announcement. There are steps between when the announcement happens and the rest Announcement: at the level of sub custodians. then you gether the people who are affected by the event that&apos;s to come. Then you send the announcement - a notification to the holder, informing them of the options that are available to them. If it&apos;s mandatory these distinctions still happen, but there is no choice. So still announcement is made, then when it effects people you send out notificaiton and collect responses. &quot;EVENT&quot;: two aspects: The event itself Events within the Corporat eAction, e.g. notification, deadline when a responses is due by, payment dates, Define as: lifecycle of the Corporate Action. Sometimes have to re-notify, there may be changes in the life oc the &quot;Corporate Event&quot;. So the Corporate Event is a sequence of events.</skos:definition>
	</owl:Class>
	
	<owl:Class rdf:about="&fibo-cae-ce-cae;OddLotOffer">
		<rdfs:subClassOf rdf:resource="&fibo-cae-ce-cae;VoluntaryCorporateAction"/>
		<rdfs:label xml:lang="en">odd lot offer</rdfs:label>
		<skos:definition xml:lang="en">Offer by issuer to allow holders of an odd lot of a security to order a commission-free transaction at market price, to sell the odd lot, or to buy an amount of shares which will bring the position to a round lot (board lot). SWIFT = ODLT</skos:definition>
	</owl:Class>
	
	<owl:Class rdf:about="&fibo-cae-ce-cae;OrganizationNameChange">
		<rdfs:subClassOf rdf:resource="&fibo-cae-ce-cae;CorporateModificationEvent"/>
		<rdfs:label xml:lang="en">organization name change</rdfs:label>
		<skos:definition xml:lang="en">The issuing company changes it&apos;s name. Event shows the change from old name to new name and may involve surrendering physical shares with the old name to the registrar. SWIFT = NAME</skos:definition>
	</owl:Class>
	
	<owl:NamedIndividual rdf:about="&fibo-cae-ce-cae;PARI">
		<rdf:type rdf:resource="&fibo-cae-ce-cae;BusinessStrategyOrientedAction"/>
		<rdfs:label xml:lang="en">PARI</rdfs:label>
		<skos:definition xml:lang="en">SWIFT ISO 15022 classifier for corporate actions that occur when securities with different characteristics become identical in all respects</skos:definition>
		<fibo-fnd-rel-rel:isDefinedIn rdf:resource="&fibo-cae-ce-cae;ISO15022CorporateActionClassificationScheme"/>
		<lcc-cr:classifies rdf:resource="&fibo-cae-ce-cae;PariPassuAction"/>
		<lcc-lr:denotes rdf:resource="&fibo-cae-ce-cae;PariPassuAction"/>
		<lcc-lr:hasTag>PARI</lcc-lr:hasTag>
		<lcc-lr:isMemberOf rdf:resource="&fibo-cae-ce-cae;ISO15022CorporateActionClassificationScheme"/>
	</owl:NamedIndividual>
	
	<owl:NamedIndividual rdf:about="&fibo-cae-ce-cae;PCAL">
		<rdf:type rdf:resource="&fibo-cae-ce-cae;IncomeOrientedAction"/>
		<rdfs:label xml:lang="en">PCAL</rdfs:label>
		<skos:definition xml:lang="en">SWIFT ISO 15022 classifier for corporate actions that involve redemption of securities in part before their scheduled final maturity date with reduction of the nominal value of the securities</skos:definition>
		<fibo-fnd-rel-rel:isDefinedIn rdf:resource="&fibo-cae-ce-cae;ISO15022CorporateActionClassificationScheme"/>
		<lcc-cr:classifies rdf:resource="&fibo-cae-ce-cae;PartialRedemptionWithReductionOfNominalValueAction"/>
		<lcc-lr:denotes rdf:resource="&fibo-cae-ce-cae;PartialRedemptionWithReductionOfNominalValueAction"/>
		<lcc-lr:hasTag>PCAL</lcc-lr:hasTag>
		<lcc-lr:isMemberOf rdf:resource="&fibo-cae-ce-cae;ISO15022CorporateActionClassificationScheme"/>
	</owl:NamedIndividual>
	
	<owl:NamedIndividual rdf:about="&fibo-cae-ce-cae;PRED">
		<rdf:type rdf:resource="&fibo-cae-ce-cae;IncomeOrientedAction"/>
		<rdfs:label xml:lang="en">PRED</rdfs:label>
		<skos:definition xml:lang="en">SWIFT ISO 15022 classifier for corporate actions that involve redemption of securities in part before their scheduled final maturity date with no reduction in nominal value</skos:definition>
		<fibo-fnd-rel-rel:isDefinedIn rdf:resource="&fibo-cae-ce-cae;ISO15022CorporateActionClassificationScheme"/>
		<lcc-cr:classifies rdf:resource="&fibo-cae-ce-cae;PartialRedemptionWithoutReductionOfNominalValueAction"/>
		<lcc-lr:denotes rdf:resource="&fibo-cae-ce-cae;PartialRedemptionWithoutReductionOfNominalValueAction"/>
		<lcc-lr:hasTag>PRED</lcc-lr:hasTag>
		<lcc-lr:isMemberOf rdf:resource="&fibo-cae-ce-cae;ISO15022CorporateActionClassificationScheme"/>
	</owl:NamedIndividual>
	
	<owl:NamedIndividual rdf:about="&fibo-cae-ce-cae;PRIO">
		<rdf:type rdf:resource="&fibo-cae-ce-cae;BusinessStrategyOrientedAction"/>
		<rdfs:label xml:lang="en">PRIO</rdfs:label>
		<skos:definition xml:lang="en">SWIFT ISO 15022 classifier for corporate actions that involve a public offer where priority is given to existing shareholders</skos:definition>
		<fibo-fnd-rel-rel:isDefinedIn rdf:resource="&fibo-cae-ce-cae;ISO15022CorporateActionClassificationScheme"/>
		<lcc-cr:classifies rdf:resource="&fibo-cae-ce-cae;PriorityIssue"/>
		<lcc-lr:denotes rdf:resource="&fibo-cae-ce-cae;PriorityIssue"/>
		<lcc-lr:hasTag>PRIO</lcc-lr:hasTag>
		<lcc-lr:isMemberOf rdf:resource="&fibo-cae-ce-cae;ISO15022CorporateActionClassificationScheme"/>
	</owl:NamedIndividual>
	
	<owl:Class rdf:about="&fibo-cae-ce-cae;PariPassuAction">
		<rdfs:subClassOf rdf:resource="&fibo-cae-ce-cae;MandatoryCorporateAction"/>
		<rdfs:label xml:lang="en">pari-passu action</rdfs:label>
		<skos:definition xml:lang="en">corporate action that occurs when securities with different characteristics become identical in all respects</skos:definition>
		<fibo-fnd-utl-av:explanatoryNote xml:lang="en">A pari-passu event includes cases, for example, when shares with different entitlements to dividend or voting rights become equivalent through assimilation or pari-passu. Such an event may be scheduled in advance, for example, when shares resulting from a bonus may become fungible after a pre-set period of time, or may result from outside events, for example, merger, reorganisation, issue of supplementary tranches, etc.</fibo-fnd-utl-av:explanatoryNote>
		<fibo-fnd-utl-av:explanatoryNote xml:lang="en">The term, pari-passu, means &apos;at the same rate or on an equal footing&apos;, and in finance is used to describe situations where two or more assets, securities, creditors, or obligations are equally managed without preference. An example of pari-passu occurs during bankruptcy proceedings: When the court reaches a verdict, the court regards all creditors equally, and the trustee will repay them the same fractional amount as other creditors and at the same time.</fibo-fnd-utl-av:explanatoryNote>
		<fibo-fnd-utl-av:synonym xml:lang="en">assimilation</fibo-fnd-utl-av:synonym>
	</owl:Class>
	
	<owl:Class rdf:about="&fibo-cae-ce-cae;PartialDefeasanceAction">
		<rdfs:subClassOf rdf:resource="&fibo-cae-ce-cae;CorporateAction"/>
		<rdfs:label xml:lang="en">partial defeasance action</rdfs:label>
		<skos:definition xml:lang="en">The setting aside by a borrower of cash or bonds sufficient to service the borrower&apos;s debt.</skos:definition>
		<fibo-fnd-utl-av:explanatoryNote xml:lang="en">From Free dictionary: Both the borrower&apos;s debt and the offsetting cash or bonds are removed from the balance sheet. In securities trading, where a clearing house becomes counterparty to each side of a trade, after the trade has been agreed. This is necessary to facilitate netting, and reduce counterparty risk exposure. The term has become popular recently, because of the growth of central counterparty clearing services in European cash equities markets. Origin: http://financial-dictionary.thefreedictionary.com/defeasance SWIFT: Term:PDEF; &quot;Partial Defeasance/Prefunding&quot; Definition:&quot;Issuer has money set aside to redeem a portion of an issue and the indenture states that the securities could be called earlier than the stated maturity.&quot;</fibo-fnd-utl-av:explanatoryNote>
	</owl:Class>
	
	<owl:Class rdf:about="&fibo-cae-ce-cae;PartialRedemptionWithReductionOfNominalValueAction">
		<rdfs:subClassOf rdf:resource="&fibo-cae-ce-cae;VoluntaryCorporateAction"/>
		<rdfs:label xml:lang="en">partial redemption with reduction of nominal value action</rdfs:label>
		<skos:definition xml:lang="en">corporate action that involves redemption of securities in part before their scheduled final maturity date with reduction of the nominal value of the securities</skos:definition>
		<fibo-fnd-utl-av:explanatoryNote xml:lang="en">The outstanding amount of securities will be reduced proportionally.</fibo-fnd-utl-av:explanatoryNote>
	</owl:Class>
	
	<owl:Class rdf:about="&fibo-cae-ce-cae;PartialRedemptionWithoutReductionOfNominalValueAction">
		<rdfs:subClassOf rdf:resource="&fibo-cae-ce-cae;VoluntaryCorporateAction"/>
		<rdfs:label xml:lang="en">partial redemption without reduction of nominal value action</rdfs:label>
		<skos:definition xml:lang="en">corporate action that involves redemption of securities in part before their scheduled final maturity date with no reduction in nominal value</skos:definition>
		<fibo-fnd-utl-av:explanatoryNote xml:lang="en">This is commonly done by pool factor reduction.</fibo-fnd-utl-av:explanatoryNote>
	</owl:Class>
	
	<owl:Class rdf:about="&fibo-cae-ce-cae;PlaceOfIncorporationChange">
		<rdfs:subClassOf rdf:resource="&fibo-cae-ce-cae;CorporateModificationEvent"/>
		<rdfs:label xml:lang="en">place of incorporation change</rdfs:label>
		<skos:definition xml:lang="en">Changes in the state of incorporation for US companies and changes in the place of incorporation for foreign companies. Where shares need to be registered following the incorporation change, the holder(s) may have to elect the registrar. SWIFT = PLAC</skos:definition>
	</owl:Class>
	
	<owl:Class rdf:about="&fibo-cae-ce-cae;PostMergerSecuritiesExchange">
		<rdfs:subClassOf rdf:resource="&fibo-cae-ce-cae;CorporateAction"/>
		<rdfs:subClassOf>
			<owl:Restriction>
				<owl:onProperty rdf:resource="&fibo-cae-ce-cae;definesAdditional"/>
				<owl:allValuesFrom rdf:resource="&fibo-fnd-acc-cur;AmountOfMoney"/>
			</owl:Restriction>
		</rdfs:subClassOf>
		<rdfs:subClassOf>
			<owl:Restriction>
				<owl:onProperty rdf:resource="&fibo-cae-ce-cae;exchangesFrom"/>
				<owl:someValuesFrom rdf:resource="&fibo-fbc-fi-fi;Security"/>
			</owl:Restriction>
		</rdfs:subClassOf>
		<rdfs:subClassOf>
			<owl:Restriction>
				<owl:onProperty rdf:resource="&fibo-cae-ce-cae;exchangesInto"/>
				<owl:someValuesFrom rdf:resource="&fibo-fbc-fi-fi;Security"/>
			</owl:Restriction>
		</rdfs:subClassOf>
		<rdfs:label xml:lang="en">post merger securities exchange</rdfs:label>
		<skos:definition xml:lang="en">Mandatory or voluntary exchange of an outstanding securities as the result of two or more companies combining assets. Cash payments may accompany share exchange.</skos:definition>
		<fibo-fnd-utl-av:explanatoryNote xml:lang="en">This is an action as a result of the Merger, not the merger itself.</fibo-fnd-utl-av:explanatoryNote>
	</owl:Class>
	
	<owl:Class rdf:about="&fibo-cae-ce-cae;PriorityIssue">
		<rdfs:subClassOf rdf:resource="&fibo-cae-ce-cae;VoluntaryCorporateAction"/>
		<rdfs:label xml:lang="en">priority issue</rdfs:label>
		<skos:definition xml:lang="en">corporate action that is a public offer where, due to a limited amount of securities available, priority is given to existing shareholders</skos:definition>
	</owl:Class>
	
	<owl:Class rdf:about="&fibo-cae-ce-cae;PutRedemptionAction">
		<rdfs:subClassOf rdf:resource="&fibo-cae-ce-cae;VoluntaryCorporateAction"/>
		<rdfs:label xml:lang="en">put redemption action</rdfs:label>
		<skos:definition xml:lang="en">corporate action involving early redemption of a security at the election of the holder subject to the terms and condition of the issue with no reduction in nominal value</skos:definition>
	</owl:Class>
	
	<owl:NamedIndividual rdf:about="&fibo-cae-ce-cae;REDM">
		<rdf:type rdf:resource="&fibo-cae-ce-cae;IncomeOrientedAction"/>
		<rdfs:label xml:lang="en">REDM</rdfs:label>
		<skos:definition xml:lang="en">SWIFT ISO 15022 classifier for corporate actions that involve redemption of an entire issue outstanding of securities at final maturity</skos:definition>
		<fibo-fnd-rel-rel:isDefinedIn rdf:resource="&fibo-cae-ce-cae;ISO15022CorporateActionClassificationScheme"/>
		<lcc-cr:classifies rdf:resource="&fibo-cae-ce-cae;RedemptionAtMaturityAction"/>
		<lcc-lr:denotes rdf:resource="&fibo-cae-ce-cae;RedemptionAtMaturityAction"/>
		<lcc-lr:hasTag>REDM</lcc-lr:hasTag>
		<lcc-lr:isMemberOf rdf:resource="&fibo-cae-ce-cae;ISO15022CorporateActionClassificationScheme"/>
	</owl:NamedIndividual>
	
	<owl:NamedIndividual rdf:about="&fibo-cae-ce-cae;REDO">
		<rdf:type rdf:resource="&fibo-cae-ce-cae;BusinessStrategyOrientedAction"/>
		<rdfs:label xml:lang="en">REDO</rdfs:label>
		<skos:definition xml:lang="en">SWIFT ISO 15022 classifier for corporate actions by which the unit (currency and/or nominal) of a security is restated</skos:definition>
		<fibo-fnd-rel-rel:isDefinedIn rdf:resource="&fibo-cae-ce-cae;ISO15022CorporateActionClassificationScheme"/>
		<lcc-cr:classifies rdf:resource="&fibo-cae-ce-cae;RedenominationAction"/>
		<lcc-lr:denotes rdf:resource="&fibo-cae-ce-cae;RedenominationAction"/>
		<lcc-lr:hasTag>REDO</lcc-lr:hasTag>
		<lcc-lr:isMemberOf rdf:resource="&fibo-cae-ce-cae;ISO15022CorporateActionClassificationScheme"/>
	</owl:NamedIndividual>
	
	<owl:Class rdf:about="&fibo-cae-ce-cae;RedemptionAtMaturityAction">
		<rdfs:subClassOf rdf:resource="&fibo-cae-ce-cae;MandatoryCorporateAction"/>
		<rdfs:label xml:lang="en">redemption at maturity action</rdfs:label>
		<skos:definition xml:lang="en">corporate action that involves redemption of an entire issue outstanding of securities at final maturity</skos:definition>
	</owl:Class>
	
	<owl:Class rdf:about="&fibo-cae-ce-cae;RedenominationAction">
		<rdfs:subClassOf rdf:resource="&fibo-cae-ce-cae;MandatoryCorporateAction"/>
		<rdfs:label xml:lang="en">redenomination action</rdfs:label>
		<skos:definition xml:lang="en">corporate action by which the unit (currency and/or nominal) of a security is restated</skos:definition>
		<fibo-fnd-utl-av:explanatoryNote xml:lang="en">For example, the nominal/par value of security in a national currency is restated in another currency.</fibo-fnd-utl-av:explanatoryNote>
	</owl:Class>
	
	<owl:Class rdf:about="&fibo-cae-ce-cae;RepurchaseOffer">
		<rdfs:subClassOf rdf:resource="&fibo-cae-ce-cae;VoluntaryCorporateAction"/>
		<rdfs:label xml:lang="en">repurchase offer</rdfs:label>
		<skos:definition xml:lang="en">corporate action in which an offer is made to existing shareholders by the issuing company to repurchase equity or other securities convertible into equity</skos:definition>
		<fibo-fnd-utl-av:explanatoryNote xml:lang="en">The objective of the offer is to reduce the number of outstanding equities.</fibo-fnd-utl-av:explanatoryNote>
		<fibo-fnd-utl-av:synonym xml:lang="en">issuer bid</fibo-fnd-utl-av:synonym>
		<fibo-fnd-utl-av:synonym xml:lang="en">reverse rights</fibo-fnd-utl-av:synonym>
	</owl:Class>
	
	<owl:Class rdf:about="&fibo-cae-ce-cae;ReverseStockSplit">
		<rdfs:subClassOf rdf:resource="&fibo-cae-ce-cae;MandatoryCorporateAction"/>
		<rdfs:subClassOf>
			<owl:Restriction>
				<owl:onProperty rdf:resource="&fibo-fnd-rel-rel;appliesTo"/>
				<owl:someValuesFrom rdf:resource="&fibo-sec-eq-eq;Share"/>
			</owl:Restriction>
		</rdfs:subClassOf>
		<rdfs:label xml:lang="en">reverse stock split</rdfs:label>
		<owl:disjointWith rdf:resource="&fibo-cae-ce-cae;StockSplit"/>
		<skos:definition xml:lang="en">corporate action involving a decrease in a company&apos;s number of outstanding equities without any change in the shareholder&apos;s equity or the aggregate market value at the time of the split</skos:definition>
		<fibo-fnd-utl-av:explanatoryNote xml:lang="en">Equity price and nominal value are increased accordingly.</fibo-fnd-utl-av:explanatoryNote>
		<fibo-fnd-utl-av:synonym xml:lang="en">change in nominal value</fibo-fnd-utl-av:synonym>
	</owl:Class>
	
	<owl:Class rdf:about="&fibo-cae-ce-cae;RightsDistribution">
		<rdfs:subClassOf rdf:resource="&fibo-cae-ce-cae;RightsIssue"/>
		<rdfs:subClassOf>
			<owl:Restriction>
				<owl:onProperty rdf:resource="&fibo-cae-ce-cae;oversubscriptionAmount"/>
				<owl:onClass rdf:resource="&fibo-fnd-acc-cur;MonetaryAmount"/>
				<owl:maxQualifiedCardinality rdf:datatype="&xsd;nonNegativeInteger">1</owl:maxQualifiedCardinality>
			</owl:Restriction>
		</rdfs:subClassOf>
		<rdfs:subClassOf>
			<owl:Restriction>
				<owl:onProperty rdf:resource="&fibo-fnd-rel-rel;appliesTo"/>
				<owl:someValuesFrom rdf:resource="&fibo-sec-eq-eq;Share"/>
			</owl:Restriction>
		</rdfs:subClassOf>
		<rdfs:label xml:lang="en">rights distribution</rdfs:label>
		<skos:definition xml:lang="en">The distribution of rights to shareholders, in proportion to their equity holding.</skos:definition>
		<fibo-fnd-utl-av:explanatoryNote xml:lang="en">Does the Rights Distribution have to be proportion to the Shareholding? Sometimes this is offered at market prices, so all you are doing is offering shareholders the right to purchase. Conclusion: Not &quot;in proportion&quot; at all. REVISE: May also have Bonus Rights Issue, where you don&apos; have a subscriptiojn price. This works like a rights issue but without a price attached to it. The rate of how many you can buy is definitely in proportion to your holding. The rate of distribution of the right is proportional to the holdings. Another difference: A Rights thing you have to pay for the additional shares if you choose to purchase them (exercise the right) whereas a Bonus Issue you do not pay, you get them outright for free. TWO PARTS: 1. Distribution of the rights in proportion to their holding 2. Exercise of the Rights. Hence RHDI v EXRI where EXRI is the exercising of the right to purchase the shares. The Rights that are distributed is a formal &quot;Rights&quot; instrument. This may have the sort of features we see in other rights instruments, such as restriction in when you can exercise it.</fibo-fnd-utl-av:explanatoryNote>
	</owl:Class>
	
	<owl:Class rdf:about="&fibo-cae-ce-cae;RightsExerciseEvent">
		<rdfs:subClassOf rdf:resource="&fibo-cae-ce-cae;CorporateAction"/>
		<rdfs:label xml:lang="en">rights exercise event</rdfs:label>
		<skos:definition xml:lang="en">Exercising the right to purchase the shares. Furhter Notes: This is an action on the part of the holder. SWIFT: Call/exercise on nil-paid securities/rights resulting from a rights distribution (RHDI) (To be used for the second event in case rights issue is dealt with in 2 events, first event being the RHDI).</skos:definition>
		<fibo-fnd-utl-av:explanatoryNote xml:lang="en">There is a rights trading period overlaps with rights subscriptiuon period (you can trade the rights) Rights exercise period - expiry date. Some time after the expiry the new shares are distributed. This is the distribution.</fibo-fnd-utl-av:explanatoryNote>
	</owl:Class>
	
	<owl:Class rdf:about="&fibo-cae-ce-cae;RightsIssue">
		<rdfs:subClassOf rdf:resource="&fibo-cae-ce-cae;MandatoryCorporateAction"/>
		<rdfs:subClassOf>
			<owl:Restriction>
				<owl:onProperty rdf:resource="&fibo-cae-ce-cae;isDistributionOf"/>
				<owl:someValuesFrom rdf:resource="&fibo-der-drc-raw;SubscriptionRight"/>
			</owl:Restriction>
		</rdfs:subClassOf>
		<rdfs:label xml:lang="en">rights issue</rdfs:label>
		<skos:definition xml:lang="en">Some issue of rights to holders.</skos:definition>
	</owl:Class>
	
	<owl:NamedIndividual rdf:about="&fibo-cae-ce-cae;SHPR">
		<rdf:type rdf:resource="&fibo-cae-ce-cae;IncomeOrientedAction"/>
		<rdfs:label xml:lang="en">SHPR</rdfs:label>
		<skos:definition xml:lang="en">SWIFT ISO 15022 classifier for corporate actions that pay shareholders an amount in cash issued from the shares premium reserve</skos:definition>
		<fibo-fnd-rel-rel:isDefinedIn rdf:resource="&fibo-cae-ce-cae;ISO15022CorporateActionClassificationScheme"/>
		<lcc-cr:classifies rdf:resource="&fibo-cae-ce-cae;SharesPremiumDividendAction"/>
		<lcc-lr:denotes rdf:resource="&fibo-cae-ce-cae;SharesPremiumDividendAction"/>
		<lcc-lr:hasTag>SHPR</lcc-lr:hasTag>
		<lcc-lr:isMemberOf rdf:resource="&fibo-cae-ce-cae;ISO15022CorporateActionClassificationScheme"/>
	</owl:NamedIndividual>
	
	<owl:NamedIndividual rdf:about="&fibo-cae-ce-cae;SOFF">
		<rdf:type rdf:resource="&fibo-cae-ce-cae;BusinessStrategyOrientedAction"/>
		<rdfs:label xml:lang="en">SOFF</rdfs:label>
		<skos:definition xml:lang="en">SWIFT ISO 15022 classifier for corporate actions that involve the distribution of subsidiary stock to the shareholders of the parent company without a surrender of shares</skos:definition>
		<fibo-fnd-rel-rel:isDefinedIn rdf:resource="&fibo-cae-ce-cae;ISO15022CorporateActionClassificationScheme"/>
		<lcc-cr:classifies rdf:resource="&fibo-cae-ce-cae;SpinOff"/>
		<lcc-lr:denotes rdf:resource="&fibo-cae-ce-cae;SpinOff"/>
		<lcc-lr:hasTag>SOFF</lcc-lr:hasTag>
		<lcc-lr:isMemberOf rdf:resource="&fibo-cae-ce-cae;ISO15022CorporateActionClassificationScheme"/>
	</owl:NamedIndividual>
	
	<owl:NamedIndividual rdf:about="&fibo-cae-ce-cae;SPLF">
		<rdf:type rdf:resource="&fibo-cae-ce-cae;BusinessStrategyOrientedAction"/>
		<rdfs:label xml:lang="en">SPLF</rdfs:label>
		<skos:definition xml:lang="en">SWIFT ISO 15022 classifier for corporate actions that involve an increase in a corporation&apos;s number of outstanding equities without any change in the shareholder&apos;s equity or the aggregate market value at the time of the split</skos:definition>
		<fibo-fnd-rel-rel:isDefinedIn rdf:resource="&fibo-cae-ce-cae;ISO15022CorporateActionClassificationScheme"/>
		<lcc-cr:classifies rdf:resource="&fibo-cae-ce-cae;StockSplit"/>
		<lcc-lr:denotes rdf:resource="&fibo-cae-ce-cae;StockSplit"/>
		<lcc-lr:hasTag>SPLF</lcc-lr:hasTag>
		<lcc-lr:isMemberOf rdf:resource="&fibo-cae-ce-cae;ISO15022CorporateActionClassificationScheme"/>
	</owl:NamedIndividual>
	
	<owl:NamedIndividual rdf:about="&fibo-cae-ce-cae;SPLR">
		<rdf:type rdf:resource="&fibo-cae-ce-cae;BusinessStrategyOrientedAction"/>
		<rdfs:label xml:lang="en">SPLR</rdfs:label>
		<skos:definition xml:lang="en">SWIFT ISO 15022 classifier for corporate actions that involve a decrease in a company&apos;s number of outstanding equities without any change in the shareholder&apos;s equity or the aggregate market value at the time of the split</skos:definition>
		<fibo-fnd-rel-rel:isDefinedIn rdf:resource="&fibo-cae-ce-cae;ISO15022CorporateActionClassificationScheme"/>
		<lcc-cr:classifies rdf:resource="&fibo-cae-ce-cae;ReverseStockSplit"/>
		<lcc-lr:denotes rdf:resource="&fibo-cae-ce-cae;ReverseStockSplit"/>
		<lcc-lr:hasTag>SPLR</lcc-lr:hasTag>
		<lcc-lr:isMemberOf rdf:resource="&fibo-cae-ce-cae;ISO15022CorporateActionClassificationScheme"/>
	</owl:NamedIndividual>
	
	<owl:Class rdf:about="&fibo-cae-ce-cae;SharesPremiumDividendAction">
		<rdfs:subClassOf rdf:resource="&fibo-cae-ce-cae;MandatoryWithChoiceCorporateAction"/>
		<rdfs:label xml:lang="en">shares premium dividend action</rdfs:label>
		<skos:definition xml:lang="en">corporate action that pays shareholders an amount in cash issued from the shares premium reserve</skos:definition>
		<fibo-fnd-utl-av:explanatoryNote xml:lang="en">It is similar to a dividend but with different tax implications.</fibo-fnd-utl-av:explanatoryNote>
	</owl:Class>
	
	<owl:Class rdf:about="&fibo-cae-ce-cae;SpinOff">
		<rdfs:subClassOf rdf:resource="&fibo-cae-ce-cae;MandatoryCorporateAction"/>
		<rdfs:label xml:lang="en">spin off</rdfs:label>
		<skos:definition xml:lang="en">corporate action involving the distribution of subsidiary stock to the shareholders of the parent company without a surrender of shares</skos:definition>
		<fibo-fnd-utl-av:explanatoryNote xml:lang="en">Spin-off represents a form of divestiture usually resulting in an independent company or in an existing company. For example, demerger, distribution, unbundling.</fibo-fnd-utl-av:explanatoryNote>
	</owl:Class>
	
	<owl:Class rdf:about="&fibo-cae-ce-cae;StockDividendAction">
		<rdfs:subClassOf rdf:resource="&fibo-cae-ce-cae;MandatoryCorporateAction"/>
		<rdfs:label xml:lang="en">stock dividend action</rdfs:label>
		<skos:definition xml:lang="en">corporate action that involves distribution of a dividend to shareholders in the form of equities of the issuing corporation</skos:definition>
	</owl:Class>
	
	<owl:Class rdf:about="&fibo-cae-ce-cae;StockSplit">
		<rdfs:subClassOf rdf:resource="&fibo-cae-ce-cae;MandatoryCorporateAction"/>
		<rdfs:subClassOf>
			<owl:Restriction>
				<owl:onProperty rdf:resource="&fibo-fnd-rel-rel;appliesTo"/>
				<owl:someValuesFrom rdf:resource="&fibo-sec-eq-eq;Share"/>
			</owl:Restriction>
		</rdfs:subClassOf>
		<rdfs:label xml:lang="en">stock split</rdfs:label>
		<skos:definition xml:lang="en">corporate action involving an increase in a corporation&apos;s number of outstanding equities without any change in the shareholder&apos;s equity or the aggregate market value at the time of the split</skos:definition>
		<fibo-fnd-utl-av:explanatoryNote xml:lang="en">Equity price and nominal value are reduced accordingly.</fibo-fnd-utl-av:explanatoryNote>
		<fibo-fnd-utl-av:synonym xml:lang="en">change in nominal value</fibo-fnd-utl-av:synonym>
		<fibo-fnd-utl-av:synonym xml:lang="en">subdivision</fibo-fnd-utl-av:synonym>
	</owl:Class>
	
	<owl:Class rdf:about="&fibo-cae-ce-cae;TenderOffer">
		<rdfs:subClassOf rdf:resource="&fibo-cae-ce-cae;VoluntaryCorporateAction"/>
		<rdfs:subClassOf>
			<owl:Restriction>
				<owl:onProperty rdf:resource="&fibo-fnd-rel-rel;appliesTo"/>
				<owl:someValuesFrom rdf:resource="&fibo-sec-eq-eq;Share"/>
			</owl:Restriction>
		</rdfs:subClassOf>
		<rdfs:label xml:lang="en">tender offer</rdfs:label>
		<skos:definition xml:lang="en">Offer made to shareholders, normally by a third party, requesting them to sell (tender) their shares for a specified price usually at a premium over prevailing market prices. Generally, the objective of a tender is to take control of the target company.</skos:definition>
		<fibo-fnd-utl-av:explanatoryNote xml:lang="en">The announcer is not the issuer of the shares. The party to which the offer is made need not be the holder. Assumption: someone else trying to take over ythe company.</fibo-fnd-utl-av:explanatoryNote>
	</owl:Class>
	
	<owl:Class rdf:about="&fibo-cae-ce-cae;TradingStatusActiveMessage">
		<rdfs:subClassOf rdf:resource="&fibo-cae-ce-cae;TradingStatusMessage"/>
		<rdfs:label xml:lang="en">trading status active message</rdfs:label>
		<skos:definition xml:lang="en">Trading in security has commenced or security has been re-activated after a supsension in trading.</skos:definition>
	</owl:Class>
	
	<owl:Class rdf:about="&fibo-cae-ce-cae;TradingStatusMessage">
		<rdfs:subClassOf rdf:resource="&fibo-fnd-arr-doc;Notice"/>
		<rdfs:subClassOf>
			<owl:Restriction>
				<owl:onProperty rdf:resource="&fibo-fnd-arr-doc;isAbout"/>
				<owl:someValuesFrom rdf:resource="&fibo-md-temx-trs;SecurityTradingStatus"/>
			</owl:Restriction>
		</rdfs:subClassOf>
		<rdfs:subClassOf>
			<owl:Restriction>
				<owl:onProperty rdf:resource="&fibo-fnd-rel-rel;refersTo"/>
				<owl:someValuesFrom rdf:resource="&fibo-fbc-fi-fi;Security"/>
			</owl:Restriction>
		</rdfs:subClassOf>
		<rdfs:label xml:lang="en">trading status message</rdfs:label>
		<skos:definition xml:lang="en">A message about trading status.</skos:definition>
		<fibo-fnd-utl-av:explanatoryNote xml:lang="en">There are a number of such messages. Events v Status: See e.g. Active: this relates to one state OR two transitions (transition from pre-issuance to Trading, or from Suspended to Trading).</fibo-fnd-utl-av:explanatoryNote>
	</owl:Class>
	
	<owl:Class rdf:about="&fibo-cae-ce-cae;TradingStatusSuspendedMessage">
		<rdfs:subClassOf rdf:resource="&fibo-cae-ce-cae;TradingStatusMessage"/>
		<rdfs:label xml:lang="en">trading status suspended message</rdfs:label>
		<skos:definition xml:lang="en">Trading in the security has been suspended.</skos:definition>
	</owl:Class>
	
	<owl:Class rdf:about="&fibo-cae-ce-cae;VoluntaryCorporateAction">
		<rdfs:subClassOf rdf:resource="&fibo-cae-ce-cae;CorporateAction"/>
		<rdfs:label xml:lang="en">voluntary corporate action</rdfs:label>
		<owl:disjointWith rdf:resource="&fibo-cae-ce-cae;MandatoryCorporateAction"/>
		<skos:definition xml:lang="en">event in which the shareholders elect to participate and must respond in order for the issuer to process the action</skos:definition>
		<skos:example xml:lang="en">An example of a voluntary corporate action is a tender offer, in which the issuer may request shareholders to tender their shares at a predetermined price.</skos:example>
		<fibo-fnd-utl-av:explanatoryNote xml:lang="en">Shareholders send responses to the issuer&apos;s agents, and the issuer will send the proceeds of the action to those shareholders who elect to participate.</fibo-fnd-utl-av:explanatoryNote>
	</owl:Class>
	
	<owl:NamedIndividual rdf:about="&fibo-cae-ce-cae;WRTH">
		<rdf:type rdf:resource="&fibo-cae-ce-cae;BusinessStrategyOrientedAction"/>
		<rdf:type rdf:resource="&fibo-cae-ce-cae;IncomeOrientedAction"/>
		<rdfs:label xml:lang="en">WRTH</rdfs:label>
		<skos:definition xml:lang="en">SWIFT ISO 15022 classifier for corporate actions that involve booking out of valueless securities</skos:definition>
		<fibo-fnd-rel-rel:isDefinedIn rdf:resource="&fibo-cae-ce-cae;ISO15022CorporateActionClassificationScheme"/>
		<lcc-cr:classifies rdf:resource="&fibo-cae-ce-cae;WorthlessSecurityAction"/>
		<lcc-lr:denotes rdf:resource="&fibo-cae-ce-cae;WorthlessSecurityAction"/>
		<lcc-lr:hasTag>WRTH</lcc-lr:hasTag>
		<lcc-lr:isMemberOf rdf:resource="&fibo-cae-ce-cae;ISO15022CorporateActionClassificationScheme"/>
	</owl:NamedIndividual>
	
	<owl:Class rdf:about="&fibo-cae-ce-cae;WarrantExerciseAction">
		<rdfs:subClassOf rdf:resource="&fibo-cae-ce-cae;CorporateAction"/>
		<rdfs:label xml:lang="en">warrant exercise action</rdfs:label>
		<skos:definition xml:lang="en">corporate action that offers holders the option to buy (call warrant) or to sell (put warrant) a specific amount of stock, cash, or commodity, at a predetermined price, during a predetermined period of time (which usually corresponds to the life of the issue)</skos:definition>
		<fibo-fnd-utl-av:explanatoryNote xml:lang="en">Note that participation by the warrant holder may be mandatory or voluntary and may involve a choice in the mandatory case.</fibo-fnd-utl-av:explanatoryNote>
	</owl:Class>
	
	<owl:Class rdf:about="&fibo-cae-ce-cae;WorthlessSecurityAction">
		<rdfs:subClassOf rdf:resource="&fibo-cae-ce-cae;MandatoryCorporateAction"/>
		<rdfs:label xml:lang="en">worthless security action</rdfs:label>
		<skos:definition xml:lang="en">corporate action that involves booking out of valueless securities</skos:definition>
	</owl:Class>
	
	<owl:ObjectProperty rdf:about="&fibo-cae-ce-cae;definesAdditional">
		<rdfs:label xml:lang="en">defines additional</rdfs:label>
		<rdfs:domain rdf:resource="&fibo-cae-ce-cae;PostMergerSecuritiesExchange"/>
		<rdfs:range rdf:resource="&fibo-fnd-acc-cur;AmountOfMoney"/>
	</owl:ObjectProperty>
	
	<owl:ObjectProperty rdf:about="&fibo-cae-ce-cae;exchangesFrom">
		<rdfs:label xml:lang="en">exchanges from</rdfs:label>
		<rdfs:domain rdf:resource="&fibo-cae-ce-cae;PostMergerSecuritiesExchange"/>
		<rdfs:range rdf:resource="&fibo-fbc-fi-fi;Security"/>
	</owl:ObjectProperty>
	
	<owl:ObjectProperty rdf:about="&fibo-cae-ce-cae;exchangesInto">
		<rdfs:label xml:lang="en">exchanges into</rdfs:label>
		<rdfs:domain rdf:resource="&fibo-cae-ce-cae;PostMergerSecuritiesExchange"/>
		<rdfs:range rdf:resource="&fibo-fbc-fi-fi;Security"/>
	</owl:ObjectProperty>
	
	<owl:ObjectProperty rdf:about="&fibo-cae-ce-cae;isConversionFrom">
		<rdfs:label xml:lang="en">is conversion from</rdfs:label>
		<rdfs:domain rdf:resource="&fibo-cae-ce-cae;ConversionAction"/>
		<rdfs:range rdf:resource="&fibo-fbc-fi-fi;Security"/>
	</owl:ObjectProperty>
	
	<owl:ObjectProperty rdf:about="&fibo-cae-ce-cae;isConversionTo">
		<rdfs:label xml:lang="en">is conversion to</rdfs:label>
		<rdfs:domain rdf:resource="&fibo-cae-ce-cae;ConversionAction"/>
		<rdfs:range rdf:resource="&fibo-fbc-fi-fi;Security"/>
	</owl:ObjectProperty>
	
	<owl:ObjectProperty rdf:about="&fibo-cae-ce-cae;isDistributionOf">
		<rdfs:label xml:lang="en">is distribution of</rdfs:label>
		<rdfs:domain rdf:resource="&fibo-cae-ce-cae;RightsIssue"/>
		<rdfs:range rdf:resource="&fibo-der-drc-raw;SubscriptionRight"/>
	</owl:ObjectProperty>
	
	<owl:ObjectProperty rdf:about="&fibo-cae-ce-cae;isIssueOf">
		<rdfs:label xml:lang="en">is issue of</rdfs:label>
		<rdfs:domain rdf:resource="&fibo-cae-ce-cae;BonusIssue"/>
		<rdfs:range rdf:resource="&fibo-sec-eq-eq;Share"/>
	</owl:ObjectProperty>
	
	<owl:ObjectProperty rdf:about="&fibo-cae-ce-cae;oversubscriptionAmount">
		<rdfs:label xml:lang="en">oversubscription amount</rdfs:label>
		<rdfs:domain rdf:resource="&fibo-cae-ce-cae;RightsDistribution"/>
		<rdfs:range rdf:resource="&fibo-fnd-acc-cur;MonetaryAmount"/>
		<skos:definition xml:lang="en">The amount of additional rights that may be purchased by the holder over and above the initial allocation. Further notes: In addition to a Subscription Price (see the Price term in the Subscription rights term), there is an additional privilege extended to the holders, to subscribe to additional shares. This also is in a certain proportion. This is to catch if not enough rights were subscribed, you may be left with some left over. These can then be given to the over-subscribers. Additional terms: if this exists there is a ratio for this as well. Notes Some people may pass up the right, and another person may pick this up through over-subscription. Therefore there is no oversubscription on a Bonus issue because people are getting it for free.</skos:definition>
	</owl:ObjectProperty>

</rdf:RDF>