<?xml version="1.0" encoding="UTF-8"?>
<!DOCTYPE rdf:RDF [
	<!ENTITY dct "http://purl.org/dc/terms/">
	<!ENTITY fibo-be-fct-pub "https://spec.edmcouncil.org/fibo/ontology/BE/FunctionalEntities/Publishers/">
	<!ENTITY fibo-der-com-ctr "https://spec.edmcouncil.org/fibo/ontology/DER/CommoditiesDerivatives/CommoditiesContracts/">
	<!ENTITY fibo-der-der-fwd "https://spec.edmcouncil.org/fibo/ontology/DER/DerivativesContracts/Forwards/">
	<!ENTITY fibo-der-der-opt "https://spec.edmcouncil.org/fibo/ontology/DER/DerivativesContracts/Options/">
	<!ENTITY fibo-der-drc-bsc "https://spec.edmcouncil.org/fibo/ontology/DER/DerivativesContracts/DerivativesBasics/">
	<!ENTITY fibo-der-sbd-sbd "https://spec.edmcouncil.org/fibo/ontology/DER/SecurityBasedDerivatives/SecurityBasedDerivatives/">
	<!ENTITY fibo-fbc-fct-ra "https://spec.edmcouncil.org/fibo/ontology/FBC/FunctionalEntities/RegistrationAuthorities/">
	<!ENTITY fibo-fbc-fi-fi "https://spec.edmcouncil.org/fibo/ontology/FBC/FinancialInstruments/FinancialInstruments/">
	<!ENTITY fibo-fbc-pas-fpas "https://spec.edmcouncil.org/fibo/ontology/FBC/ProductsAndServices/FinancialProductsAndServices/">
	<!ENTITY fibo-fnd-acc-cur "https://spec.edmcouncil.org/fibo/ontology/FND/Accounting/CurrencyAmount/">
	<!ENTITY fibo-fnd-agr-ctr "https://spec.edmcouncil.org/fibo/ontology/FND/Agreements/Contracts/">
	<!ENTITY fibo-fnd-arr-asmt "https://spec.edmcouncil.org/fibo/ontology/FND/Arrangements/Assessments/">
	<!ENTITY fibo-fnd-dt-fd "https://spec.edmcouncil.org/fibo/ontology/FND/DatesAndTimes/FinancialDates/">
	<!ENTITY fibo-fnd-qt-qtu "https://spec.edmcouncil.org/fibo/ontology/FND/Quantities/QuantitiesAndUnits/">
	<!ENTITY fibo-fnd-rel-rel "https://spec.edmcouncil.org/fibo/ontology/FND/Relations/Relations/">
	<!ENTITY fibo-fnd-utl-av "https://spec.edmcouncil.org/fibo/ontology/FND/Utilities/AnnotationVocabulary/">
	<!ENTITY fibo-ind-ei-ei "https://spec.edmcouncil.org/fibo/ontology/IND/EconomicIndicators/EconomicIndicators/">
	<!ENTITY fibo-ind-mkt-bas "https://spec.edmcouncil.org/fibo/ontology/IND/MarketIndices/BasketIndices/">
	<!ENTITY fibo-sec-dbt-bnd "https://spec.edmcouncil.org/fibo/ontology/SEC/Debt/Bonds/">
	<!ENTITY fibo-sec-dbt-dbti "https://spec.edmcouncil.org/fibo/ontology/SEC/Debt/DebtInstruments/">
	<!ENTITY fibo-sec-dbt-tstd "https://spec.edmcouncil.org/fibo/ontology/SEC/Debt/TradedShortTermDebt/">
	<!ENTITY fibo-sec-eq-eq "https://spec.edmcouncil.org/fibo/ontology/SEC/Equities/EquityInstruments/">
	<!ENTITY fibo-sec-sec-lst "https://spec.edmcouncil.org/fibo/ontology/SEC/Securities/SecuritiesListings/">
	<!ENTITY owl "http://www.w3.org/2002/07/owl#">
	<!ENTITY rdf "http://www.w3.org/1999/02/22-rdf-syntax-ns#">
	<!ENTITY rdfs "http://www.w3.org/2000/01/rdf-schema#">
	<!ENTITY skos "http://www.w3.org/2004/02/skos/core#">
	<!ENTITY sm "http://www.omg.org/techprocess/ab/SpecificationMetadata/">
	<!ENTITY xsd "http://www.w3.org/2001/XMLSchema#">
]>
<rdf:RDF xml:base="https://spec.edmcouncil.org/fibo/ontology/DER/DerivativesContracts/Forwards/"
	xmlns:dct="http://purl.org/dc/terms/"
	xmlns:fibo-be-fct-pub="https://spec.edmcouncil.org/fibo/ontology/BE/FunctionalEntities/Publishers/"
	xmlns:fibo-der-com-ctr="https://spec.edmcouncil.org/fibo/ontology/DER/CommoditiesDerivatives/CommoditiesContracts/"
	xmlns:fibo-der-der-fwd="https://spec.edmcouncil.org/fibo/ontology/DER/DerivativesContracts/Forwards/"
	xmlns:fibo-der-der-opt="https://spec.edmcouncil.org/fibo/ontology/DER/DerivativesContracts/Options/"
	xmlns:fibo-der-drc-bsc="https://spec.edmcouncil.org/fibo/ontology/DER/DerivativesContracts/DerivativesBasics/"
	xmlns:fibo-der-sbd-sbd="https://spec.edmcouncil.org/fibo/ontology/DER/SecurityBasedDerivatives/SecurityBasedDerivatives/"
	xmlns:fibo-fbc-fct-ra="https://spec.edmcouncil.org/fibo/ontology/FBC/FunctionalEntities/RegistrationAuthorities/"
	xmlns:fibo-fbc-fi-fi="https://spec.edmcouncil.org/fibo/ontology/FBC/FinancialInstruments/FinancialInstruments/"
	xmlns:fibo-fbc-pas-fpas="https://spec.edmcouncil.org/fibo/ontology/FBC/ProductsAndServices/FinancialProductsAndServices/"
	xmlns:fibo-fnd-acc-cur="https://spec.edmcouncil.org/fibo/ontology/FND/Accounting/CurrencyAmount/"
	xmlns:fibo-fnd-agr-ctr="https://spec.edmcouncil.org/fibo/ontology/FND/Agreements/Contracts/"
	xmlns:fibo-fnd-arr-asmt="https://spec.edmcouncil.org/fibo/ontology/FND/Arrangements/Assessments/"
	xmlns:fibo-fnd-dt-fd="https://spec.edmcouncil.org/fibo/ontology/FND/DatesAndTimes/FinancialDates/"
	xmlns:fibo-fnd-qt-qtu="https://spec.edmcouncil.org/fibo/ontology/FND/Quantities/QuantitiesAndUnits/"
	xmlns:fibo-fnd-rel-rel="https://spec.edmcouncil.org/fibo/ontology/FND/Relations/Relations/"
	xmlns:fibo-fnd-utl-av="https://spec.edmcouncil.org/fibo/ontology/FND/Utilities/AnnotationVocabulary/"
	xmlns:fibo-ind-ei-ei="https://spec.edmcouncil.org/fibo/ontology/IND/EconomicIndicators/EconomicIndicators/"
	xmlns:fibo-ind-mkt-bas="https://spec.edmcouncil.org/fibo/ontology/IND/MarketIndices/BasketIndices/"
	xmlns:fibo-sec-dbt-bnd="https://spec.edmcouncil.org/fibo/ontology/SEC/Debt/Bonds/"
	xmlns:fibo-sec-dbt-dbti="https://spec.edmcouncil.org/fibo/ontology/SEC/Debt/DebtInstruments/"
	xmlns:fibo-sec-dbt-tstd="https://spec.edmcouncil.org/fibo/ontology/SEC/Debt/TradedShortTermDebt/"
	xmlns:fibo-sec-eq-eq="https://spec.edmcouncil.org/fibo/ontology/SEC/Equities/EquityInstruments/"
	xmlns:fibo-sec-sec-lst="https://spec.edmcouncil.org/fibo/ontology/SEC/Securities/SecuritiesListings/"
	xmlns:owl="http://www.w3.org/2002/07/owl#"
	xmlns:rdf="http://www.w3.org/1999/02/22-rdf-syntax-ns#"
	xmlns:rdfs="http://www.w3.org/2000/01/rdf-schema#"
	xmlns:skos="http://www.w3.org/2004/02/skos/core#"
	xmlns:sm="http://www.omg.org/techprocess/ab/SpecificationMetadata/"
	xmlns:xsd="http://www.w3.org/2001/XMLSchema#">
	
	<owl:Ontology rdf:about="https://spec.edmcouncil.org/fibo/ontology/DER/DerivativesContracts/Forwards/">
		<rdfs:label xml:lang="en">Forwards Ontology</rdfs:label>
		<dct:abstract>Concepts defining a derivative contract in which one side represents a commitment to sell or purchase the underlier at a defined price at a given time in the future.</dct:abstract>
		<dct:license rdf:datatype="&xsd;anyURI">http://opensource.org/licenses/MIT</dct:license>
		<sm:contentLanguage rdf:resource="http://www.w3.org/2002/07/owl#"/>
		<sm:copyright>Copyright (c) 2015-2020 EDM Council, Inc.</sm:copyright>
		<sm:dependsOn rdf:resource="https://spec.edmcouncil.org/fibo/ontology/BE/"/>
		<sm:dependsOn rdf:resource="https://spec.edmcouncil.org/fibo/ontology/FBC/"/>
		<sm:dependsOn rdf:resource="https://spec.edmcouncil.org/fibo/ontology/FND/"/>
		<sm:dependsOn rdf:resource="https://spec.edmcouncil.org/fibo/ontology/IND/"/>
		<sm:dependsOn rdf:resource="https://spec.edmcouncil.org/fibo/ontology/SEC/"/>
		<sm:fileAbbreviation>fibo-der-der-fwd</sm:fileAbbreviation>
		<sm:filename>Forwards.rdf</sm:filename>
		<owl:imports rdf:resource="https://spec.edmcouncil.org/fibo/ontology/BE/FunctionalEntities/Publishers/"/>
		<owl:imports rdf:resource="https://spec.edmcouncil.org/fibo/ontology/DER/CommoditiesDerivatives/CommoditiesContracts/"/>
		<owl:imports rdf:resource="https://spec.edmcouncil.org/fibo/ontology/DER/DerivativesContracts/DerivativesBasics/"/>
		<owl:imports rdf:resource="https://spec.edmcouncil.org/fibo/ontology/DER/DerivativesContracts/Options/"/>
		<owl:imports rdf:resource="https://spec.edmcouncil.org/fibo/ontology/DER/RateDerivatives/RateDerivatives/"/>
		<owl:imports rdf:resource="https://spec.edmcouncil.org/fibo/ontology/DER/SecurityBasedDerivatives/SecurityBasedDerivatives/"/>
		<owl:imports rdf:resource="https://spec.edmcouncil.org/fibo/ontology/FBC/FinancialInstruments/FinancialInstruments/"/>
		<owl:imports rdf:resource="https://spec.edmcouncil.org/fibo/ontology/FBC/FunctionalEntities/RegistrationAuthorities/"/>
		<owl:imports rdf:resource="https://spec.edmcouncil.org/fibo/ontology/FBC/ProductsAndServices/FinancialProductsAndServices/"/>
		<owl:imports rdf:resource="https://spec.edmcouncil.org/fibo/ontology/FND/Accounting/CurrencyAmount/"/>
		<owl:imports rdf:resource="https://spec.edmcouncil.org/fibo/ontology/FND/Agreements/Contracts/"/>
		<owl:imports rdf:resource="https://spec.edmcouncil.org/fibo/ontology/FND/Arrangements/Assessments/"/>
		<owl:imports rdf:resource="https://spec.edmcouncil.org/fibo/ontology/FND/DatesAndTimes/FinancialDates/"/>
		<owl:imports rdf:resource="https://spec.edmcouncil.org/fibo/ontology/FND/Parties/Parties/"/>
		<owl:imports rdf:resource="https://spec.edmcouncil.org/fibo/ontology/FND/Quantities/QuantitiesAndUnits/"/>
		<owl:imports rdf:resource="https://spec.edmcouncil.org/fibo/ontology/FND/Relations/Relations/"/>
		<owl:imports rdf:resource="https://spec.edmcouncil.org/fibo/ontology/FND/Utilities/AnnotationVocabulary/"/>
		<owl:imports rdf:resource="https://spec.edmcouncil.org/fibo/ontology/IND/EconomicIndicators/EconomicIndicators/"/>
		<owl:imports rdf:resource="https://spec.edmcouncil.org/fibo/ontology/IND/MarketIndices/BasketIndices/"/>
		<owl:imports rdf:resource="https://spec.edmcouncil.org/fibo/ontology/SEC/Debt/Bonds/"/>
		<owl:imports rdf:resource="https://spec.edmcouncil.org/fibo/ontology/SEC/Debt/DebtInstruments/"/>
		<owl:imports rdf:resource="https://spec.edmcouncil.org/fibo/ontology/SEC/Debt/TradedShortTermDebt/"/>
		<owl:imports rdf:resource="https://spec.edmcouncil.org/fibo/ontology/SEC/Equities/EquityInstruments/"/>
		<owl:imports rdf:resource="https://spec.edmcouncil.org/fibo/ontology/SEC/Securities/SecuritiesListings/"/>
		<owl:versionIRI rdf:resource="https://spec.edmcouncil.org/fibo/ontology/DER/DerivativesContracts/Forwards/"/>
		<fibo-fnd-utl-av:hasMaturityLevel rdf:resource="&fibo-fnd-utl-av;Provisional"/>
	</owl:Ontology>
	
	<owl:Class rdf:about="&fibo-der-der-fwd;BondFuture">
		<rdfs:subClassOf rdf:resource="&fibo-der-der-fwd;InterestRateFuture"/>
		<rdfs:subClassOf>
			<owl:Restriction>
				<owl:onProperty rdf:resource="&fibo-der-drc-bsc;hasUnderlier"/>
				<owl:someValuesFrom rdf:resource="&fibo-sec-dbt-bnd;Bond"/>
			</owl:Restriction>
		</rdfs:subClassOf>
		<rdfs:label xml:lang="en">bond future</rdfs:label>
		<skos:definition xml:lang="en">A future instrument where the underlying is a bond.</skos:definition>
	</owl:Class>
	
	<owl:Class rdf:about="&fibo-der-der-fwd;CashCloseout">
		<rdfs:subClassOf rdf:resource="&fibo-der-der-fwd;ForwardDeliveryCommitment"/>
		<rdfs:subClassOf>
			<owl:Restriction>
				<owl:onProperty rdf:resource="&fibo-der-der-fwd;closedOutBy"/>
				<owl:someValuesFrom rdf:resource="&fibo-der-der-fwd;Forward"/>
			</owl:Restriction>
		</rdfs:subClassOf>
		<rdfs:label xml:lang="en">cash closeout</rdfs:label>
		<skos:definition xml:lang="en">Closeout of the contract in the form of the cash equivalent of the asset or commodity rather than the underlying asset or commodity itself.</skos:definition>
		<skos:editorialNote xml:lang="en">Various SME REview notes from OTC sessions: This is where you go into the market and buy the offsetting contract. Exchange Traded: Standard process for exchange traded: if you have an open contract you close out the contract by taking the reverse contract, then present those contracts to the clearing house to be closed out. What clearing house? What is the relationship between the two partie sand the clearing house. That&apos;s for futures. What about OTC? Does this exist? Closeout does exist for OTC. For OTC. Terms of contract are that they are cash settled. Except maybe gold.</skos:editorialNote>
	</owl:Class>
	
	<owl:Class rdf:about="&fibo-der-der-fwd;CloseTime">
		<rdfs:subClassOf rdf:resource="&fibo-der-der-fwd;ValuationTimeType"/>
		<rdfs:label xml:lang="en">close time</rdfs:label>
	</owl:Class>
	
	<owl:Class rdf:about="&fibo-der-der-fwd;CommodityFuture">
		<rdfs:subClassOf rdf:resource="&fibo-der-com-ctr;CommodityDerivative"/>
		<rdfs:subClassOf rdf:resource="&fibo-fbc-fi-fi;Future"/>
		<rdfs:label xml:lang="en">commodity future</rdfs:label>
		<skos:definition xml:lang="en">A futures contract tied to the movement of a particular commodity. This enables contract buyers to buy a specific amount of a commodity at a specific price on a particular date in the future.</skos:definition>
		<fibo-fnd-utl-av:explanatoryNote xml:lang="en">The price of the contract is determined using the &quot;Open Outcry&quot; system on the floor of a commodity exchange such as the Chicago Board of Trade or the Commodity Exchange in New York. There are commodity futures contracts based on meats such as cattle and pork bellies; grains such as corn, oats, soybeans and wheat; metals such as gold, silver and platinum; and energy products such as heating oil, natural gas and crude oil.</fibo-fnd-utl-av:explanatoryNote>
	</owl:Class>
	
	<owl:Class rdf:about="&fibo-der-der-fwd;DeliverPhysical">
		<rdfs:subClassOf rdf:resource="&fibo-der-drc-bsc;DeliveryTerms"/>
		<rdfs:label xml:lang="en">deliver physical</rdfs:label>
		<skos:definition xml:lang="en">Delivery means physically delivering the underlying asset on the agreed date. Term in an options or futures contract which requires the actual underlying asset to be delivered upon the specified delivery date, rather than being traded out with offsetting contracts.</skos:definition>
		<fibo-fnd-utl-av:explanatoryNote xml:lang="en">If you sell a gold futures contract of say 1 kilogram then you will have to give real gold to the buyer on the mutually agreed date. Most derivatives are not actually exercised, but are traded out before their delivery date. However, physical delivery still occurs with some trades: it is most common with commodities, but can also occur with other financial instruments.</fibo-fnd-utl-av:explanatoryNote>
	</owl:Class>
	
	<owl:Class rdf:about="&fibo-der-der-fwd;DeliverySquaringOff">
		<rdfs:subClassOf rdf:resource="&fibo-der-drc-bsc;DeliveryTerms"/>
		<rdfs:label xml:lang="en">delivery squaring off</rdfs:label>
		<skos:definition xml:lang="en">Squaring off means taking a position opposite your initial one. For example, you square off the purchase of a gold futures contract by selling the identical contract.</skos:definition>
	</owl:Class>
	
	<owl:Class rdf:about="&fibo-der-der-fwd;DerivativesCloseTime">
		<rdfs:subClassOf rdf:resource="&fibo-der-der-fwd;ValuationTimeType"/>
		<rdfs:label xml:lang="en">derivatives close time</rdfs:label>
	</owl:Class>
	
	<owl:Class rdf:about="&fibo-der-der-fwd;EquityFuture">
		<rdfs:subClassOf rdf:resource="&fibo-der-sbd-sbd;EquityDerivative"/>
		<rdfs:subClassOf rdf:resource="&fibo-fbc-fi-fi;Future"/>
		<rdfs:subClassOf>
			<owl:Restriction>
				<owl:onProperty rdf:resource="&fibo-der-drc-bsc;hasUnderlier"/>
				<owl:someValuesFrom rdf:resource="&fibo-sec-eq-eq;ListedShare"/>
			</owl:Restriction>
		</rdfs:subClassOf>
		<rdfs:label xml:lang="en">equity future</rdfs:label>
		<skos:definition xml:lang="en">A Futures instrument which is based on an equity security or securities, specifically a publicly issued and traded share.</skos:definition>
	</owl:Class>
	
	<owl:Class rdf:about="&fibo-der-der-fwd;Forward">
		<rdfs:subClassOf rdf:resource="&fibo-der-drc-bsc;OTCInstrument"/>
		<rdfs:subClassOf rdf:resource="&fibo-fbc-fi-fi;DerivativeInstrument"/>
		<rdfs:subClassOf>
			<owl:Restriction>
				<owl:onProperty rdf:resource="&fibo-der-der-fwd;hasBuyer"/>
				<owl:someValuesFrom rdf:resource="&fibo-der-drc-bsc;PayingParty"/>
			</owl:Restriction>
		</rdfs:subClassOf>
		<rdfs:subClassOf>
			<owl:Restriction>
				<owl:onProperty rdf:resource="&fibo-der-der-fwd;hasSeller"/>
				<owl:someValuesFrom rdf:resource="&fibo-der-drc-bsc;ReceivingParty"/>
			</owl:Restriction>
		</rdfs:subClassOf>
		<rdfs:subClassOf>
			<owl:Restriction>
				<owl:onProperty rdf:resource="&fibo-der-der-fwd;hasValuationTerms"/>
				<owl:someValuesFrom rdf:resource="&fibo-der-der-fwd;ForwardValuationTerms"/>
			</owl:Restriction>
		</rdfs:subClassOf>
		<rdfs:subClassOf>
			<owl:Restriction>
				<owl:onProperty rdf:resource="&fibo-fnd-agr-ctr;hasContractualElement"/>
				<owl:someValuesFrom rdf:resource="&fibo-der-der-fwd;ForwardCashSettlementCommitment"/>
			</owl:Restriction>
		</rdfs:subClassOf>
		<rdfs:subClassOf>
			<owl:Restriction>
				<owl:onProperty rdf:resource="&fibo-fnd-agr-ctr;hasContractualElement"/>
				<owl:someValuesFrom rdf:resource="&fibo-der-der-fwd;ForwardDeliveryCommitment"/>
			</owl:Restriction>
		</rdfs:subClassOf>
		<rdfs:label xml:lang="en">forward</rdfs:label>
		<skos:definition xml:lang="en">A cash market transaction in which a seller agrees to deliver a specific cash commodity to a buyer at some point in the future.</skos:definition>
		<fibo-fnd-utl-av:explanatoryNote xml:lang="en">Unlike futures contracts (which occur through a clearing firm), forward contracts are privately negotiated and are not standardized. Further, the two parties must bear each other&apos;s credit risk, which is not the case with a futures contract. Also, since the contracts are not exchange traded, there is no marking to market requirement, which allows a buyer to avoid almost all capital outflow initially (though some counterparties might set collateral requirements). Given the lack of standardization in these contracts, there is very little scope for a secondary market in forwards. The price specified in a forward contract for a specific commodity. The forward price makes the forward contract have no value when the contract is written. However, if the value of the underlying commodity changes, the value of the forward contract becomes positive or negative, depending on the position held. Forwards are priced in a manner similar to futures. Like in the case of a futures contract, the first step in pricing a forward is to add the spot price to the cost of carry (interest forgone, convenience yield, storage costs and interest/dividend received on the underlying). Unlike a futures contract though, the price may also include a premium for counterparty credit risk, and the fact that there is not daily marking to market process to minimize default risk. If there is no allowance for these credit risks, then the forward price will equal the futures price.</fibo-fnd-utl-av:explanatoryNote>
	</owl:Class>
	
	<owl:Class rdf:about="&fibo-der-der-fwd;ForwardCashSettlementCommitment">
		<rdfs:subClassOf rdf:resource="&fibo-der-drc-bsc;DerivativeTransactionTerms"/>
		<rdfs:subClassOf rdf:resource="&fibo-fbc-pas-fpas;SettlementTerms"/>
		<rdfs:subClassOf>
			<owl:Restriction>
				<owl:onProperty rdf:resource="&fibo-der-der-fwd;hasAdditionalCosts"/>
				<owl:onClass rdf:resource="&fibo-fnd-acc-cur;MonetaryAmount"/>
				<owl:minQualifiedCardinality rdf:datatype="&xsd;nonNegativeInteger">0</owl:minQualifiedCardinality>
			</owl:Restriction>
		</rdfs:subClassOf>
		<rdfs:label xml:lang="en">forward cash settlement commitment</rdfs:label>
		<skos:definition xml:lang="en">commitment to settle a cash amount at an agreed date in the future</skos:definition>
		<fibo-fnd-utl-av:explanatoryNote xml:lang="en">Note the earliest possible date as in a Spot. FpML exchangedCurrency2 referred to as a &quot;Currency Stream&quot; &apos;This is the second of the two currency flows that define a single leg of a standard foreign exchange transaction.&apos;</fibo-fnd-utl-av:explanatoryNote>
	</owl:Class>
	
	<owl:Class rdf:about="&fibo-der-der-fwd;ForwardDeliveryCommitment">
		<rdfs:subClassOf rdf:resource="&fibo-der-drc-bsc;DeliveryTerms"/>
		<rdfs:subClassOf>
			<owl:Restriction>
				<owl:onProperty rdf:resource="&fibo-der-der-fwd;hasAdditionalCosts"/>
				<owl:onClass rdf:resource="&fibo-fnd-acc-cur;MonetaryAmount"/>
				<owl:minQualifiedCardinality rdf:datatype="&xsd;nonNegativeInteger">0</owl:minQualifiedCardinality>
			</owl:Restriction>
		</rdfs:subClassOf>
		<rdfs:subClassOf>
			<owl:Restriction>
				<owl:onProperty rdf:resource="&fibo-der-der-fwd;hasForwardUnderlierPrice"/>
				<owl:onClass rdf:resource="&fibo-fnd-acc-cur;MonetaryAmount"/>
				<owl:minQualifiedCardinality rdf:datatype="&xsd;nonNegativeInteger">0</owl:minQualifiedCardinality>
			</owl:Restriction>
		</rdfs:subClassOf>
		<rdfs:subClassOf>
			<owl:Restriction>
				<owl:onProperty rdf:resource="&fibo-fnd-rel-rel;appliesTo"/>
				<owl:someValuesFrom rdf:resource="&fibo-der-der-opt;OptionUnderlyingSeller"/>
			</owl:Restriction>
		</rdfs:subClassOf>
		<rdfs:label xml:lang="en">forward delivery commitment</rdfs:label>
		<skos:definition xml:lang="en">commitment to deliver something in the future, at an agreed date or dates and under agreed terms</skos:definition>
		<fibo-fnd-utl-av:explanatoryNote xml:lang="en">Typically this is a commitment to deliver cash, but it could also involve some other underlying asset. In an Option, there is still a commitment on one side to deliver in the event that the other side chooses to exercise the option.</fibo-fnd-utl-av:explanatoryNote>
	</owl:Class>
	
	<owl:Class rdf:about="&fibo-der-der-fwd;ForwardTransaction">
		<rdfs:subClassOf rdf:resource="&fibo-fbc-fi-fi;SecuritiesTransaction"/>
		<rdfs:subClassOf>
			<owl:Restriction>
				<owl:onProperty rdf:resource="&fibo-fnd-rel-rel;embodies"/>
				<owl:someValuesFrom rdf:resource="&fibo-der-der-fwd;Forward"/>
			</owl:Restriction>
		</rdfs:subClassOf>
		<rdfs:label xml:lang="en">forward transaction</rdfs:label>
		<skos:definition xml:lang="en">A transaction in which one party commits at the present to delivery of something in the future.</skos:definition>
	</owl:Class>
	
	<owl:Class rdf:about="&fibo-der-der-fwd;ForwardValuationTerms">
		<rdfs:subClassOf rdf:resource="&fibo-fnd-agr-ctr;ContractualCommitment"/>
		<rdfs:subClassOf>
			<owl:Restriction>
				<owl:onProperty rdf:resource="&fibo-der-der-fwd;hasValuationTiming"/>
				<owl:someValuesFrom rdf:resource="&fibo-der-der-fwd;ValuationTiming"/>
			</owl:Restriction>
		</rdfs:subClassOf>
		<rdfs:subClassOf>
			<owl:Restriction>
				<owl:onProperty rdf:resource="&fibo-fbc-fct-ra;specifies"/>
				<owl:someValuesFrom rdf:resource="&fibo-der-drc-bsc;UnderlyingAssetValuation"/>
			</owl:Restriction>
		</rdfs:subClassOf>
		<rdfs:subClassOf>
			<owl:Restriction>
				<owl:onProperty rdf:resource="&fibo-fnd-arr-asmt;hasDateOfAssessment"/>
				<owl:someValuesFrom rdf:resource="&fibo-fnd-dt-fd;ExplicitDate"/>
			</owl:Restriction>
		</rdfs:subClassOf>
		<rdfs:label xml:lang="en">forward valuation terms</rdfs:label>
		<skos:definition xml:lang="en">contract terms specific to valuation of underlier(s) for a forward contract</skos:definition>
		<fibo-fnd-utl-av:explanatoryNote xml:lang="en">Note this includes contractual details regarding the time(s) of day at which valuation can occur, as &quot;As Specified in Master Confirmation&quot;.</fibo-fnd-utl-av:explanatoryNote>
	</owl:Class>
	
	<owl:Class rdf:about="&fibo-der-der-fwd;FuturesListing">
		<rdfs:subClassOf rdf:resource="&fibo-sec-sec-lst;Listing"/>
		<rdfs:subClassOf>
			<owl:Restriction>
				<owl:onProperty rdf:resource="&fibo-sec-sec-lst;lists"/>
				<owl:onClass rdf:resource="&fibo-fbc-fi-fi;Future"/>
				<owl:qualifiedCardinality rdf:datatype="&xsd;nonNegativeInteger">1</owl:qualifiedCardinality>
			</owl:Restriction>
		</rdfs:subClassOf>
		<rdfs:subClassOf>
			<owl:Restriction>
				<owl:onProperty rdf:resource="&fibo-der-der-fwd;marginCall"/>
				<owl:someValuesFrom rdf:resource="&xsd;boolean"/>
			</owl:Restriction>
		</rdfs:subClassOf>
		<rdfs:subClassOf>
			<owl:Restriction>
				<owl:onProperty rdf:resource="&fibo-der-der-fwd;marginProvision"/>
				<owl:someValuesFrom rdf:resource="&fibo-fnd-acc-cur;MonetaryAmount"/>
			</owl:Restriction>
		</rdfs:subClassOf>
		<rdfs:label xml:lang="en">futures listing</rdfs:label>
		<skos:definition xml:lang="en">A listing of a futures instrument on a derivatives exchange.</skos:definition>
	</owl:Class>
	
	<owl:Class rdf:about="&fibo-der-der-fwd;FuturesTradingAccountProvider">
		<rdfs:subClassOf rdf:resource="&fibo-fnd-agr-ctr;ContractPrincipal"/>
		<rdfs:subClassOf>
			<owl:Restriction>
				<owl:onProperty rdf:resource="&fibo-fnd-rel-rel;hasIdentity"/>
				<owl:someValuesFrom rdf:resource="&fibo-der-drc-bsc;DesignatedContractMarket"/>
			</owl:Restriction>
		</rdfs:subClassOf>
		<rdfs:label xml:lang="en">futures trading account provider</rdfs:label>
		<skos:definition xml:lang="en">The party which is the principal of the Futures contract. This is the party that sets the terms of the contract.</skos:definition>
		<fibo-fnd-utl-av:explanatoryNote xml:lang="en">This party is by definition a futures trading exchange or derivatives exchange.</fibo-fnd-utl-av:explanatoryNote>
	</owl:Class>
	
	<owl:Class rdf:about="&fibo-der-der-fwd;FuturesTransaction">
		<rdfs:subClassOf rdf:resource="&fibo-der-der-fwd;ForwardTransaction"/>
		<rdfs:label xml:lang="en">futures transaction</rdfs:label>
		<skos:definition xml:lang="en">A forward settlement transaction which is defined by the Futures market in which they are traded.</skos:definition>
		<skos:editorialNote xml:lang="en">This is a specialization of the Forward Transaction, which is distinguished by specific rules around for example novation. These are Market rules. So OTC v Futures are distinguished as markets where transactions occur. Action: Define &quot;OTC Market&quot; and &quot;Futures Market&quot; as types of the existing term &quot;Market&quot;. In some futures markets the line between notional physical is graded as some markets which were Open Outcry (physical place) become Notional Place.</skos:editorialNote>
	</owl:Class>
	
	<owl:Class rdf:about="&fibo-der-der-fwd;IndexFuture">
		<rdfs:subClassOf rdf:resource="&fibo-fbc-fi-fi;Future"/>
		<rdfs:subClassOf>
			<owl:Restriction>
				<owl:onProperty rdf:resource="&fibo-der-drc-bsc;hasUnderlier"/>
				<owl:someValuesFrom>
					<owl:Class>
						<owl:unionOf rdf:parseType="Collection">
							<rdf:Description rdf:about="&fibo-ind-ei-ei;EconomicIndicator">
							</rdf:Description>
							<rdf:Description rdf:about="&fibo-ind-mkt-bas;ReferenceIndex">
							</rdf:Description>
						</owl:unionOf>
					</owl:Class>
				</owl:someValuesFrom>
			</owl:Restriction>
		</rdfs:subClassOf>
		<rdfs:label xml:lang="en">index future</rdfs:label>
		<skos:definition xml:lang="en">A futures contract on a stock or financial index. For each index there may be a different multiple for determining the price of the futures contract.</skos:definition>
	</owl:Class>
	
	<owl:Class rdf:about="&fibo-der-der-fwd;InterestRateFuture">
		<rdfs:subClassOf rdf:resource="&fibo-fbc-fi-fi;Future"/>
		<rdfs:subClassOf>
			<owl:Restriction>
				<owl:onProperty rdf:resource="&fibo-der-drc-bsc;hasUnderlier"/>
				<owl:someValuesFrom rdf:resource="&fibo-sec-dbt-dbti;TradableDebtInstrument"/>
			</owl:Restriction>
		</rdfs:subClassOf>
		<rdfs:label xml:lang="en">interest rate future</rdfs:label>
		<skos:definition xml:lang="en">An Interest Rate Future is a futures contract with an interest-bearing instrument as the underlying asset.</skos:definition>
	</owl:Class>
	
	<owl:Class rdf:about="&fibo-der-der-fwd;MoneyMarketFuture">
		<rdfs:subClassOf rdf:resource="&fibo-der-der-fwd;InterestRateFuture"/>
		<rdfs:subClassOf>
			<owl:Restriction>
				<owl:onProperty rdf:resource="&fibo-der-drc-bsc;hasUnderlier"/>
				<owl:someValuesFrom rdf:resource="&fibo-sec-dbt-tstd;MoneyMarketInstrument"/>
			</owl:Restriction>
		</rdfs:subClassOf>
		<rdfs:label xml:lang="en">money market future</rdfs:label>
		<skos:definition xml:lang="en">A future instrument where the underlying is a money market instrument.</skos:definition>
	</owl:Class>
	
	<owl:Class rdf:about="&fibo-der-der-fwd;OSP">
		<rdfs:subClassOf rdf:resource="&fibo-der-der-fwd;ValuationTimeType"/>
		<rdfs:label xml:lang="en">o s p</rdfs:label>
	</owl:Class>
	
	<owl:Class rdf:about="&fibo-der-der-fwd;OpenTime">
		<rdfs:subClassOf rdf:resource="&fibo-der-der-fwd;ValuationTimeType"/>
		<rdfs:label xml:lang="en">open time</rdfs:label>
	</owl:Class>
	
	<owl:Class rdf:about="&fibo-der-der-fwd;StandardizedFuturesListingTerms">
		<rdfs:subClassOf rdf:resource="&fibo-fbc-fi-fi;StandardizedTerms"/>
		<rdfs:subClassOf>
			<owl:Restriction>
				<owl:onProperty rdf:resource="&fibo-be-fct-pub;hasPublisher"/>
				<owl:someValuesFrom rdf:resource="&fibo-der-drc-bsc;DesignatedContractMarket"/>
			</owl:Restriction>
		</rdfs:subClassOf>
		<rdfs:subClassOf>
			<owl:Restriction>
				<owl:onProperty rdf:resource="&fibo-fnd-rel-rel;appliesTo"/>
				<owl:someValuesFrom rdf:resource="&fibo-der-der-fwd;FuturesListing"/>
			</owl:Restriction>
		</rdfs:subClassOf>
		<rdfs:label xml:lang="en">standardized futures listing terms</rdfs:label>
		<skos:definition xml:lang="en">Standard terms out by the exchange which will apply to any listing of a futures contract on this exchange.</skos:definition>
		<fibo-fnd-utl-av:explanatoryNote xml:lang="en">Individual listings will take on these standard terms but they are not contractual terms of the futures contract, they are facts about that listing on that exchange.</fibo-fnd-utl-av:explanatoryNote>
	</owl:Class>
	
	<owl:Class rdf:about="&fibo-der-der-fwd;StandardizedFuturesTerms">
		<rdfs:subClassOf rdf:resource="&fibo-fbc-fi-fi;StandardizedTerms"/>
		<rdfs:subClassOf>
			<owl:Restriction>
				<owl:onProperty rdf:resource="&fibo-fbc-fct-ra;specifies"/>
				<owl:someValuesFrom rdf:resource="&fibo-der-drc-bsc;DeliveryTerms"/>
			</owl:Restriction>
		</rdfs:subClassOf>
		<rdfs:subClassOf>
			<owl:Restriction>
				<owl:onProperty rdf:resource="&fibo-fnd-rel-rel;appliesTo"/>
				<owl:someValuesFrom rdf:resource="&fibo-fbc-fi-fi;Future"/>
			</owl:Restriction>
		</rdfs:subClassOf>
		<rdfs:label xml:lang="en">standardized futures terms</rdfs:label>
		<skos:definition xml:lang="en">A set of standard terms for futures contracts, as set out by the derivatives exchange. Futures contracts issued by and traded on that exchange will take on these terms or override them.</skos:definition>
		<fibo-fnd-utl-av:explanatoryNote xml:lang="en">Standard symbology for the commodities are standardized by the exchanges as part of their standard contracts, for example trading in standard bushels, commonly defined kinds of oil and so on. These give the units in which lot sizes are described and defined.</fibo-fnd-utl-av:explanatoryNote>
	</owl:Class>
	
	<owl:Class rdf:about="&fibo-der-der-fwd;ValuationTimeType">
		<rdfs:subClassOf rdf:resource="&fibo-fnd-dt-fd;DateTime"/>
		<rdfs:label xml:lang="en">valuation time type</rdfs:label>
		<skos:definition xml:lang="en">The time of day at which the calculation agent values the underlying, for example the official closing time of the exchange.</skos:definition>
	</owl:Class>
	
	<owl:Class rdf:about="&fibo-der-der-fwd;ValuationTiming">
		<rdfs:subClassOf rdf:resource="&fibo-fnd-agr-ctr;ContractualElement"/>
		<rdfs:subClassOf>
			<owl:Restriction>
				<owl:onProperty rdf:resource="&fibo-der-der-fwd;hasValuationTimeOfDay"/>
				<owl:someValuesFrom rdf:resource="&fibo-fnd-dt-fd;DateTime"/>
			</owl:Restriction>
		</rdfs:subClassOf>
		<rdfs:subClassOf>
			<owl:Restriction>
				<owl:onProperty rdf:resource="&fibo-fnd-rel-rel;isCharacterizedBy"/>
				<owl:someValuesFrom rdf:resource="&fibo-der-der-fwd;ValuationTimeType"/>
			</owl:Restriction>
		</rdfs:subClassOf>
		<rdfs:label xml:lang="en">valuation timing</rdfs:label>
		<skos:definition xml:lang="en">terms specifying the timing specific to valuation of an underlying asset</skos:definition>
		<fibo-fnd-utl-av:explanatoryNote xml:lang="en">Note this is referred to in the selection list for times of day at which valuation can occur, as &quot;As Specified in Master Confirmation&quot;. Since that is not a time of day, Master confirmation is added here. Presumably the Master Confirmation (contract / covering agreement) has other terms. REVIEW</fibo-fnd-utl-av:explanatoryNote>
	</owl:Class>
	
	<owl:Class rdf:about="&fibo-der-der-fwd;XETRA">
		<rdfs:subClassOf rdf:resource="&fibo-der-der-fwd;ValuationTimeType"/>
		<rdfs:label xml:lang="en">x e t r a</rdfs:label>
	</owl:Class>
	
	<owl:ObjectProperty rdf:about="&fibo-der-der-fwd;closedOutBy">
		<rdfs:label xml:lang="en">closed out by</rdfs:label>
		<rdfs:domain rdf:resource="&fibo-der-der-fwd;CashCloseout"/>
		<rdfs:range rdf:resource="&fibo-der-der-fwd;Forward"/>
	</owl:ObjectProperty>
	
	<owl:ObjectProperty rdf:about="&fibo-der-der-fwd;firstDeliveryDate">
		<rdfs:label xml:lang="en">first delivery date</rdfs:label>
		<rdfs:domain rdf:resource="&fibo-fbc-fi-fi;Future"/>
		<rdfs:range rdf:resource="&fibo-fnd-dt-fd;Date"/>
		<skos:definition xml:lang="en">The start date of the range of dates by which the underlying for a futures contract must be delivered in order for the terms of the contract to be fulfilled.</skos:definition>
	</owl:ObjectProperty>
	
	<owl:ObjectProperty rdf:about="&fibo-der-der-fwd;firstNoticeDate">
		<rdfs:label xml:lang="en">first notice date</rdfs:label>
		<rdfs:domain rdf:resource="&fibo-fbc-fi-fi;Future"/>
		<rdfs:range rdf:resource="&fibo-fnd-dt-fd;Date"/>
		<skos:definition xml:lang="en">The first date at which a delivery notice can be issued.</skos:definition>
	</owl:ObjectProperty>
	
	<owl:ObjectProperty rdf:about="&fibo-der-der-fwd;hasAdditionalCosts">
		<rdfs:subPropertyOf rdf:resource="&fibo-fnd-acc-cur;hasMonetaryAmount"/>
		<rdfs:label xml:lang="en">has additional costs</rdfs:label>
		<rdfs:range rdf:resource="&fibo-fnd-acc-cur;MonetaryAmount"/>
		<skos:definition xml:lang="en">indicates costs, such as up front costs, brokerage fees and the like, that must be paid on delivery</skos:definition>
	</owl:ObjectProperty>
	
	<owl:ObjectProperty rdf:about="&fibo-der-der-fwd;hasBuyer">
		<rdfs:subPropertyOf rdf:resource="&fibo-fnd-agr-ctr;hasCounterparty"/>
		<rdfs:label xml:lang="en">has buyer</rdfs:label>
		<rdfs:domain rdf:resource="&fibo-der-der-fwd;Forward"/>
		<rdfs:range rdf:resource="&fibo-der-drc-bsc;PayingParty"/>
	</owl:ObjectProperty>
	
	<owl:DatatypeProperty rdf:about="&fibo-der-der-fwd;hasContractSize">
		<rdfs:label xml:lang="en">has contract size</rdfs:label>
		<rdfs:domain rdf:resource="&fibo-der-der-fwd;Forward"/>
		<rdfs:range rdf:resource="&xsd;integer"/>
		<skos:definition xml:lang="en">indicates the deliverable quantity of goods, commodities, or shares underlying the futures contract. This is denominated as a multiple of the lot size in the case of a commodity future. For financial futures this is the number of units of the underlying security.</skos:definition>
	</owl:DatatypeProperty>
	
	<owl:DatatypeProperty rdf:about="&fibo-der-der-fwd;hasConversionFactor">
		<rdfs:label xml:lang="en">has conversion factor</rdfs:label>
		<rdfs:domain rdf:resource="&fibo-der-der-fwd;BondFuture"/>
		<rdfs:range rdf:resource="&xsd;decimal"/>
		<skos:definition xml:lang="en">indicates the price of the delivered bond/note ($1 par value) to yield a fixed rate. The conversion factor is used to calculate a final delivery price.</skos:definition>
	</owl:DatatypeProperty>
	
	<owl:ObjectProperty rdf:about="&fibo-der-der-fwd;hasForwardUnderlierPrice">
		<rdfs:subPropertyOf rdf:resource="&fibo-fnd-acc-cur;hasPrice"/>
		<rdfs:label xml:lang="en">has forward underlier price</rdfs:label>
		<rdfs:range rdf:resource="&fibo-fnd-acc-cur;MonetaryAmount"/>
		<skos:definition xml:lang="en">indicates the price of the underlier of the forward as specified in delivery terms</skos:definition>
	</owl:ObjectProperty>
	
	<owl:ObjectProperty rdf:about="&fibo-der-der-fwd;hasLotSize">
		<rdfs:label xml:lang="en">lot size</rdfs:label>
		<rdfs:domain rdf:resource="&fibo-der-der-fwd;CommodityFuture"/>
		<rdfs:range rdf:resource="&fibo-fnd-qt-qtu;QuantityValue"/>
		<skos:definition xml:lang="en">How many of the underlying commodity can be sold. The groupings of certain units of measure in the underlying commodity.</skos:definition>
	</owl:ObjectProperty>
	
	<owl:DatatypeProperty rdf:about="&fibo-der-der-fwd;hasMultiple">
		<rdfs:label xml:lang="en">has multiple</rdfs:label>
		<rdfs:domain rdf:resource="&fibo-der-der-fwd;IndexFuture"/>
		<rdfs:range rdf:resource="&xsd;decimal"/>
		<skos:definition xml:lang="en">indicates the multiple for determining the price of the futures contract in relation to the underlying index rate</skos:definition>
	</owl:DatatypeProperty>
	
	<owl:ObjectProperty rdf:about="&fibo-der-der-fwd;hasSeller">
		<rdfs:subPropertyOf rdf:resource="&fibo-fnd-agr-ctr;hasPrincipalParty"/>
		<rdfs:label xml:lang="en">has seller</rdfs:label>
		<rdfs:domain rdf:resource="&fibo-der-der-fwd;Forward"/>
		<rdfs:range rdf:resource="&fibo-der-drc-bsc;ReceivingParty"/>
	</owl:ObjectProperty>
	
	<owl:ObjectProperty rdf:about="&fibo-der-der-fwd;hasSettlementArrangement">
		<rdfs:label xml:lang="en">has settlement arrangement</rdfs:label>
		<rdfs:domain rdf:resource="&fibo-fbc-fi-fi;Future"/>
		<rdfs:range rdf:resource="&fibo-der-drc-bsc;DeliveryTerms"/>
		<skos:definition xml:lang="en">The action by which an underlying commodity, security, cash value, or delivery instrument covering a contract is tendered and received by the contract holder.</skos:definition>
		<fibo-fnd-utl-av:explanatoryNote xml:lang="en">This determines what is delivered to the holder when the future is exercised.</fibo-fnd-utl-av:explanatoryNote>
	</owl:ObjectProperty>
	
	<owl:ObjectProperty rdf:about="&fibo-der-der-fwd;hasValuationTerms">
		<rdfs:subPropertyOf rdf:resource="&fibo-fnd-agr-ctr;hasContractualElement"/>
		<rdfs:label xml:lang="en">has valuation terms</rdfs:label>
		<rdfs:domain rdf:resource="&fibo-der-der-fwd;Forward"/>
		<rdfs:range rdf:resource="&fibo-der-der-fwd;ForwardValuationTerms"/>
	</owl:ObjectProperty>
	
	<owl:ObjectProperty rdf:about="&fibo-der-der-fwd;hasValuationTimeOfDay">
		<rdfs:subPropertyOf rdf:resource="&fibo-fnd-dt-fd;hasDateTime"/>
		<rdfs:label xml:lang="en">has valuation time of day</rdfs:label>
		<rdfs:domain rdf:resource="&fibo-der-der-fwd;ValuationTiming"/>
		<rdfs:range rdf:resource="&fibo-fnd-dt-fd;DateTime"/>
	</owl:ObjectProperty>
	
	<owl:ObjectProperty rdf:about="&fibo-der-der-fwd;hasValuationTiming">
		<rdfs:label xml:lang="en">has valuation timing</rdfs:label>
		<rdfs:domain rdf:resource="&fibo-der-der-fwd;ForwardValuationTerms"/>
		<rdfs:range rdf:resource="&fibo-der-der-fwd;ValuationTiming"/>
	</owl:ObjectProperty>
	
	<owl:ObjectProperty rdf:about="&fibo-der-der-fwd;lastDeliveryDate">
		<rdfs:label xml:lang="en">last delivery date</rdfs:label>
		<rdfs:domain rdf:resource="&fibo-fbc-fi-fi;Future"/>
		<rdfs:range rdf:resource="&fibo-fnd-dt-fd;Date"/>
		<skos:definition xml:lang="en">The last date in the range of dates by which the underlying for a futures contract must be delivered in order for the terms of the contract to be fulfilled.</skos:definition>
	</owl:ObjectProperty>
	
	<owl:ObjectProperty rdf:about="&fibo-der-der-fwd;lastNoticeDate">
		<rdfs:label xml:lang="en">last notice date</rdfs:label>
		<rdfs:domain rdf:resource="&fibo-fbc-fi-fi;Future"/>
		<rdfs:range rdf:resource="&fibo-fnd-dt-fd;Date"/>
		<skos:definition xml:lang="en">The last date at which a delivery notice can be issued.</skos:definition>
	</owl:ObjectProperty>
	
	<owl:DatatypeProperty rdf:about="&fibo-der-der-fwd;marginCall">
		<rdfs:label xml:lang="en">has margin call</rdfs:label>
		<rdfs:domain rdf:resource="&fibo-der-der-fwd;FuturesListing"/>
		<rdfs:range rdf:resource="&xsd;boolean"/>
		<skos:definition xml:lang="en">A broker&apos;s demand on an investor using margin to deposit additional money or securities so that the margin account is brought up to the minimum maintenance margin. This is sometimes called a &apos;fed call&apos; or &apos;maintenance call&apos;.</skos:definition>
	</owl:DatatypeProperty>
	
	<owl:DatatypeProperty rdf:about="&fibo-der-der-fwd;marginCallApplicable">
		<rdfs:label xml:lang="en">margin call applicable</rdfs:label>
		<rdfs:domain rdf:resource="&fibo-der-der-fwd;StandardizedFuturesListingTerms"/>
		<rdfs:range rdf:resource="&xsd;boolean"/>
		<skos:definition xml:lang="en">Whether or not a Margin Call may be applicable to the listing.</skos:definition>
	</owl:DatatypeProperty>
	
	<owl:ObjectProperty rdf:about="&fibo-der-der-fwd;marginProvision">
		<rdfs:label xml:lang="en">has margin provision</rdfs:label>
		<rdfs:domain rdf:resource="&fibo-der-der-fwd;FuturesListing"/>
		<rdfs:range rdf:resource="&fibo-fnd-acc-cur;MonetaryAmount"/>
		<skos:definition xml:lang="en">An amount necessary to cover the purchase of the underlying security since delivery is mandatory, be it physical or cash. Failing to provide a sufficient provision will result in a margin call.</skos:definition>
	</owl:ObjectProperty>
	
	<owl:ObjectProperty rdf:about="&fibo-der-der-fwd;settlementAmount">
		<rdfs:label xml:lang="en">settlement amount</rdfs:label>
		<rdfs:domain rdf:resource="&fibo-der-der-fwd;ForwardCashSettlementCommitment"/>
		<rdfs:range rdf:resource="&fibo-fnd-acc-cur;MonetaryAmount"/>
	</owl:ObjectProperty>
	
	<owl:DatatypeProperty rdf:about="&fibo-der-der-fwd;settlementDate">
		<rdfs:label xml:lang="en">settlement date</rdfs:label>
		<rdfs:domain rdf:resource="&fibo-der-der-fwd;ForwardCashSettlementCommitment"/>
		<skos:definition xml:lang="en">FpML = valueDate Definition for &apos;valueDate&apos; in FpML &apos;The date on which both currencies traded will settle.&apos; Definition for &apos;currency2ValueDate&apos; in FpML &apos;The date on which the currency2 amount will be settled. To be used in a split value date scenario.&apos; Notes 20 Jan: This is the scenario where &quot;t&quot; for one leg is different to &quot;t&quot; for the other leg.</skos:definition>
	</owl:DatatypeProperty>
	
	<owl:ObjectProperty rdf:about="&fibo-der-der-fwd;tickValue">
		<rdfs:label xml:lang="en">tick value</rdfs:label>
		<rdfs:domain>
			<owl:Class>
				<owl:unionOf rdf:parseType="Collection">
					<rdf:Description rdf:about="&fibo-fbc-fi-fi;Future">
					</rdf:Description>
					<rdf:Description rdf:about="&fibo-der-der-fwd;StandardizedFuturesTerms">
					</rdf:Description>
				</owl:unionOf>
			</owl:Class>
		</rdfs:domain>
		<rdfs:range rdf:resource="&fibo-fnd-acc-cur;MonetaryAmount"/>
		<skos:definition xml:lang="en">The minimum value of the upward or downward movement of the contract. This is the contract size multiplied by the tick size.</skos:definition>
	</owl:ObjectProperty>
	
	<owl:DatatypeProperty rdf:about="&fibo-der-der-fwd;unitOfTrading">
		<rdfs:label xml:lang="en">unit of trading</rdfs:label>
		<rdfs:domain>
			<owl:Class>
				<owl:unionOf rdf:parseType="Collection">
					<rdf:Description rdf:about="&fibo-fbc-fi-fi;Future">
					</rdf:Description>
					<rdf:Description rdf:about="&fibo-der-der-fwd;StandardizedFuturesTerms">
					</rdf:Description>
				</owl:unionOf>
			</owl:Class>
		</rdfs:domain>
		<rdfs:range rdf:resource="&xsd;integer"/>
		<skos:definition xml:lang="en">How many of the underlying securities can be sold.</skos:definition>
	</owl:DatatypeProperty>
	
	<owl:Class rdf:about="&fibo-fbc-fi-fi;Future">
		<rdfs:subClassOf rdf:resource="&fibo-der-der-fwd;Forward"/>
		<fibo-fnd-utl-av:explanatoryNote xml:lang="en">A futures contract obligates the buyer to purchase the underlying commodity, currency or financial instrument and the seller to sell it unless the contract is sold to another before settlement date which may happen if a trader waits to take a profit or cut a loss. Further notes: This contrasts with options trading in which the option buyer may choose whether or not to exercise the option by the exercise date. Unlike options, futures convey an obligation to buy. The risk to the holder is unlimited, and because the payoff pattern is symmetrical, the risk to the seller is unlimited as well. Dollars lost and gained by each party on a futures contract are equal and opposite. In other words, futures trading is a zero-sum game. Futures contracts are forward contracts, meaning they represent a pledge to make a certain transaction at a future date. The exchange of assets occurs on the date specified in the contract. Futures are distinguished from generic forward contracts in that they contain standardized terms, trade on a formal exchange, are regulated by overseeing agencies, and are guaranteed by clearinghouses. Also, in order to insure that payment will occur, futures have a margin requirement that must be settled daily. Finally, by making an offsetting trade, taking delivery of goods, or arranging for an exchange of goods, futures contracts can be closed. Hedgers often trade futures for the purpose of keeping price risk in check. Definition origin: Barrons, adapted by EDMC SMER.</fibo-fnd-utl-av:explanatoryNote>
	</owl:Class>

</rdf:RDF>