<?xml version="1.0" encoding="UTF-8"?>
<!DOCTYPE rdf:RDF [
	<!ENTITY dct "http://purl.org/dc/terms/">
	<!ENTITY fibo-be-fct-pub "https://spec.edmcouncil.org/fibo/ontology/BE/FunctionalEntities/Publishers/">
	<!ENTITY fibo-be-le-lp "https://spec.edmcouncil.org/fibo/ontology/BE/LegalEntities/LegalPersons/">
	<!ENTITY fibo-der-com-ctr "https://spec.edmcouncil.org/fibo/ontology/DER/CommoditiesDerivatives/CommoditiesContracts/">
	<!ENTITY fibo-der-der-opt "https://spec.edmcouncil.org/fibo/ontology/DER/DerivativesContracts/Options/">
	<!ENTITY fibo-der-drc-bsc "https://spec.edmcouncil.org/fibo/ontology/DER/DerivativesContracts/DerivativesBasics/">
	<!ENTITY fibo-der-drc-swp "https://spec.edmcouncil.org/fibo/ontology/DER/DerivativesContracts/Swaps/">
	<!ENTITY fibo-der-fx-ctr "https://spec.edmcouncil.org/fibo/ontology/DER/FxDerivatives/FxContracts/">
	<!ENTITY fibo-der-sbd-sbd "https://spec.edmcouncil.org/fibo/ontology/DER/SecurityBasedDerivatives/SecurityBasedDerivatives/">
	<!ENTITY fibo-fbc-dae-gty "https://spec.edmcouncil.org/fibo/ontology/FBC/DebtAndEquities/Guaranty/">
	<!ENTITY fibo-fbc-fct-mkt "https://spec.edmcouncil.org/fibo/ontology/FBC/FunctionalEntities/Markets/">
	<!ENTITY fibo-fbc-fct-ra "https://spec.edmcouncil.org/fibo/ontology/FBC/FunctionalEntities/RegistrationAuthorities/">
	<!ENTITY fibo-fbc-fi-fi "https://spec.edmcouncil.org/fibo/ontology/FBC/FinancialInstruments/FinancialInstruments/">
	<!ENTITY fibo-fbc-fi-ip "https://spec.edmcouncil.org/fibo/ontology/FBC/FinancialInstruments/InstrumentPricing/">
	<!ENTITY fibo-fbc-pas-caa "https://spec.edmcouncil.org/fibo/ontology/FBC/ProductsAndServices/ClientsAndAccounts/">
	<!ENTITY fibo-fbc-pas-fpas "https://spec.edmcouncil.org/fibo/ontology/FBC/ProductsAndServices/FinancialProductsAndServices/">
	<!ENTITY fibo-fnd-acc-cur "https://spec.edmcouncil.org/fibo/ontology/FND/Accounting/CurrencyAmount/">
	<!ENTITY fibo-fnd-agr-ctr "https://spec.edmcouncil.org/fibo/ontology/FND/Agreements/Contracts/">
	<!ENTITY fibo-fnd-arr-arr "https://spec.edmcouncil.org/fibo/ontology/FND/Arrangements/Arrangements/">
	<!ENTITY fibo-fnd-dt-fd "https://spec.edmcouncil.org/fibo/ontology/FND/DatesAndTimes/FinancialDates/">
	<!ENTITY fibo-fnd-dt-oc "https://spec.edmcouncil.org/fibo/ontology/FND/DatesAndTimes/Occurrences/">
	<!ENTITY fibo-fnd-gao-obj "https://spec.edmcouncil.org/fibo/ontology/FND/GoalsAndObjectives/Objectives/">
	<!ENTITY fibo-fnd-law-lcap "https://spec.edmcouncil.org/fibo/ontology/FND/Law/LegalCapacity/">
	<!ENTITY fibo-fnd-oac-own "https://spec.edmcouncil.org/fibo/ontology/FND/OwnershipAndControl/Ownership/">
	<!ENTITY fibo-fnd-pas-pas "https://spec.edmcouncil.org/fibo/ontology/FND/ProductsAndServices/ProductsAndServices/">
	<!ENTITY fibo-fnd-pty-pty "https://spec.edmcouncil.org/fibo/ontology/FND/Parties/Parties/">
	<!ENTITY fibo-fnd-pty-rl "https://spec.edmcouncil.org/fibo/ontology/FND/Parties/Roles/">
	<!ENTITY fibo-fnd-qt-qtu "https://spec.edmcouncil.org/fibo/ontology/FND/Quantities/QuantitiesAndUnits/">
	<!ENTITY fibo-fnd-rel-rel "https://spec.edmcouncil.org/fibo/ontology/FND/Relations/Relations/">
	<!ENTITY fibo-fnd-utl-alx "https://spec.edmcouncil.org/fibo/ontology/FND/Utilities/Analytics/">
	<!ENTITY fibo-fnd-utl-av "https://spec.edmcouncil.org/fibo/ontology/FND/Utilities/AnnotationVocabulary/">
	<!ENTITY fibo-ind-fx-fx "https://spec.edmcouncil.org/fibo/ontology/IND/ForeignExchange/ForeignExchange/">
	<!ENTITY fibo-ind-ind-ind "https://spec.edmcouncil.org/fibo/ontology/IND/Indicators/Indicators/">
	<!ENTITY fibo-ind-mkt-bas "https://spec.edmcouncil.org/fibo/ontology/IND/MarketIndices/BasketIndices/">
	<!ENTITY fibo-sec-dbt-bnd "https://spec.edmcouncil.org/fibo/ontology/SEC/Debt/Bonds/">
	<!ENTITY fibo-sec-dbt-ex "https://spec.edmcouncil.org/fibo/ontology/SEC/Debt/ExerciseConventions/">
	<!ENTITY fibo-sec-eq-eq "https://spec.edmcouncil.org/fibo/ontology/SEC/Equities/EquityInstruments/">
	<!ENTITY fibo-sec-sec-bsk "https://spec.edmcouncil.org/fibo/ontology/SEC/Securities/Baskets/">
	<!ENTITY fibo-sec-sec-lst "https://spec.edmcouncil.org/fibo/ontology/SEC/Securities/SecuritiesListings/">
	<!ENTITY owl "http://www.w3.org/2002/07/owl#">
	<!ENTITY rdf "http://www.w3.org/1999/02/22-rdf-syntax-ns#">
	<!ENTITY rdfs "http://www.w3.org/2000/01/rdf-schema#">
	<!ENTITY skos "http://www.w3.org/2004/02/skos/core#">
	<!ENTITY sm "http://www.omg.org/techprocess/ab/SpecificationMetadata/">
	<!ENTITY xsd "http://www.w3.org/2001/XMLSchema#">
]>
<rdf:RDF xml:base="https://spec.edmcouncil.org/fibo/ontology/DER/DerivativesContracts/Options/"
	xmlns:dct="http://purl.org/dc/terms/"
	xmlns:fibo-be-fct-pub="https://spec.edmcouncil.org/fibo/ontology/BE/FunctionalEntities/Publishers/"
	xmlns:fibo-be-le-lp="https://spec.edmcouncil.org/fibo/ontology/BE/LegalEntities/LegalPersons/"
	xmlns:fibo-der-com-ctr="https://spec.edmcouncil.org/fibo/ontology/DER/CommoditiesDerivatives/CommoditiesContracts/"
	xmlns:fibo-der-der-opt="https://spec.edmcouncil.org/fibo/ontology/DER/DerivativesContracts/Options/"
	xmlns:fibo-der-drc-bsc="https://spec.edmcouncil.org/fibo/ontology/DER/DerivativesContracts/DerivativesBasics/"
	xmlns:fibo-der-drc-swp="https://spec.edmcouncil.org/fibo/ontology/DER/DerivativesContracts/Swaps/"
	xmlns:fibo-der-fx-ctr="https://spec.edmcouncil.org/fibo/ontology/DER/FxDerivatives/FxContracts/"
	xmlns:fibo-der-sbd-sbd="https://spec.edmcouncil.org/fibo/ontology/DER/SecurityBasedDerivatives/SecurityBasedDerivatives/"
	xmlns:fibo-fbc-dae-gty="https://spec.edmcouncil.org/fibo/ontology/FBC/DebtAndEquities/Guaranty/"
	xmlns:fibo-fbc-fct-mkt="https://spec.edmcouncil.org/fibo/ontology/FBC/FunctionalEntities/Markets/"
	xmlns:fibo-fbc-fct-ra="https://spec.edmcouncil.org/fibo/ontology/FBC/FunctionalEntities/RegistrationAuthorities/"
	xmlns:fibo-fbc-fi-fi="https://spec.edmcouncil.org/fibo/ontology/FBC/FinancialInstruments/FinancialInstruments/"
	xmlns:fibo-fbc-fi-ip="https://spec.edmcouncil.org/fibo/ontology/FBC/FinancialInstruments/InstrumentPricing/"
	xmlns:fibo-fbc-pas-caa="https://spec.edmcouncil.org/fibo/ontology/FBC/ProductsAndServices/ClientsAndAccounts/"
	xmlns:fibo-fbc-pas-fpas="https://spec.edmcouncil.org/fibo/ontology/FBC/ProductsAndServices/FinancialProductsAndServices/"
	xmlns:fibo-fnd-acc-cur="https://spec.edmcouncil.org/fibo/ontology/FND/Accounting/CurrencyAmount/"
	xmlns:fibo-fnd-agr-ctr="https://spec.edmcouncil.org/fibo/ontology/FND/Agreements/Contracts/"
	xmlns:fibo-fnd-arr-arr="https://spec.edmcouncil.org/fibo/ontology/FND/Arrangements/Arrangements/"
	xmlns:fibo-fnd-dt-fd="https://spec.edmcouncil.org/fibo/ontology/FND/DatesAndTimes/FinancialDates/"
	xmlns:fibo-fnd-dt-oc="https://spec.edmcouncil.org/fibo/ontology/FND/DatesAndTimes/Occurrences/"
	xmlns:fibo-fnd-gao-obj="https://spec.edmcouncil.org/fibo/ontology/FND/GoalsAndObjectives/Objectives/"
	xmlns:fibo-fnd-law-lcap="https://spec.edmcouncil.org/fibo/ontology/FND/Law/LegalCapacity/"
	xmlns:fibo-fnd-oac-own="https://spec.edmcouncil.org/fibo/ontology/FND/OwnershipAndControl/Ownership/"
	xmlns:fibo-fnd-pas-pas="https://spec.edmcouncil.org/fibo/ontology/FND/ProductsAndServices/ProductsAndServices/"
	xmlns:fibo-fnd-pty-pty="https://spec.edmcouncil.org/fibo/ontology/FND/Parties/Parties/"
	xmlns:fibo-fnd-pty-rl="https://spec.edmcouncil.org/fibo/ontology/FND/Parties/Roles/"
	xmlns:fibo-fnd-qt-qtu="https://spec.edmcouncil.org/fibo/ontology/FND/Quantities/QuantitiesAndUnits/"
	xmlns:fibo-fnd-rel-rel="https://spec.edmcouncil.org/fibo/ontology/FND/Relations/Relations/"
	xmlns:fibo-fnd-utl-alx="https://spec.edmcouncil.org/fibo/ontology/FND/Utilities/Analytics/"
	xmlns:fibo-fnd-utl-av="https://spec.edmcouncil.org/fibo/ontology/FND/Utilities/AnnotationVocabulary/"
	xmlns:fibo-ind-fx-fx="https://spec.edmcouncil.org/fibo/ontology/IND/ForeignExchange/ForeignExchange/"
	xmlns:fibo-ind-ind-ind="https://spec.edmcouncil.org/fibo/ontology/IND/Indicators/Indicators/"
	xmlns:fibo-ind-mkt-bas="https://spec.edmcouncil.org/fibo/ontology/IND/MarketIndices/BasketIndices/"
	xmlns:fibo-sec-dbt-bnd="https://spec.edmcouncil.org/fibo/ontology/SEC/Debt/Bonds/"
	xmlns:fibo-sec-dbt-ex="https://spec.edmcouncil.org/fibo/ontology/SEC/Debt/ExerciseConventions/"
	xmlns:fibo-sec-eq-eq="https://spec.edmcouncil.org/fibo/ontology/SEC/Equities/EquityInstruments/"
	xmlns:fibo-sec-sec-bsk="https://spec.edmcouncil.org/fibo/ontology/SEC/Securities/Baskets/"
	xmlns:fibo-sec-sec-lst="https://spec.edmcouncil.org/fibo/ontology/SEC/Securities/SecuritiesListings/"
	xmlns:owl="http://www.w3.org/2002/07/owl#"
	xmlns:rdf="http://www.w3.org/1999/02/22-rdf-syntax-ns#"
	xmlns:rdfs="http://www.w3.org/2000/01/rdf-schema#"
	xmlns:skos="http://www.w3.org/2004/02/skos/core#"
	xmlns:sm="http://www.omg.org/techprocess/ab/SpecificationMetadata/"
	xmlns:xsd="http://www.w3.org/2001/XMLSchema#">
	
	<owl:Ontology rdf:about="https://spec.edmcouncil.org/fibo/ontology/DER/DerivativesContracts/Options/">
		<rdfs:label xml:lang="en">Options Ontology</rdfs:label>
		<dct:abstract>Concepts common to all option contracts and their corresponding transactions. An option gives one party (the holder) the right to purchase or sell the underlying commodity at a given time or times in the future (as determined by the exercise convention), if they choose to do so. Includes option features, these being definitions of how the option comes into or ceases being in force when a given event occurs along with a range of other variations.</dct:abstract>
		<dct:license rdf:datatype="&xsd;anyURI">http://opensource.org/licenses/MIT</dct:license>
		<sm:contentLanguage rdf:datatype="&xsd;anyURI">https://www.w3.org/TR/owl2-quick-reference/</sm:contentLanguage>
		<sm:copyright>Copyright (c) 2015-2021 EDM Council, Inc.</sm:copyright>
		<sm:dependsOn rdf:resource="https://spec.edmcouncil.org/fibo/ontology/BE/"/>
		<sm:dependsOn rdf:resource="https://spec.edmcouncil.org/fibo/ontology/FBC/"/>
		<sm:dependsOn rdf:resource="https://spec.edmcouncil.org/fibo/ontology/FND/"/>
		<sm:dependsOn rdf:resource="https://spec.edmcouncil.org/fibo/ontology/IND/"/>
		<sm:dependsOn rdf:resource="https://spec.edmcouncil.org/fibo/ontology/SEC/"/>
		<sm:fileAbbreviation>fibo-der-der-opt</sm:fileAbbreviation>
		<sm:filename>Options.rdf</sm:filename>
		<owl:imports rdf:resource="https://spec.edmcouncil.org/fibo/ontology/BE/FunctionalEntities/Publishers/"/>
		<owl:imports rdf:resource="https://spec.edmcouncil.org/fibo/ontology/BE/LegalEntities/LegalPersons/"/>
		<owl:imports rdf:resource="https://spec.edmcouncil.org/fibo/ontology/DER/CommoditiesDerivatives/CommoditiesContracts/"/>
		<owl:imports rdf:resource="https://spec.edmcouncil.org/fibo/ontology/DER/DerivativesContracts/DerivativesBasics/"/>
		<owl:imports rdf:resource="https://spec.edmcouncil.org/fibo/ontology/DER/DerivativesContracts/Swaps/"/>
		<owl:imports rdf:resource="https://spec.edmcouncil.org/fibo/ontology/DER/FxDerivatives/FxContracts/"/>
		<owl:imports rdf:resource="https://spec.edmcouncil.org/fibo/ontology/DER/SecurityBasedDerivatives/SecurityBasedDerivatives/"/>
		<owl:imports rdf:resource="https://spec.edmcouncil.org/fibo/ontology/FBC/DebtAndEquities/Guaranty/"/>
		<owl:imports rdf:resource="https://spec.edmcouncil.org/fibo/ontology/FBC/FinancialInstruments/FinancialInstruments/"/>
		<owl:imports rdf:resource="https://spec.edmcouncil.org/fibo/ontology/FBC/FinancialInstruments/InstrumentPricing/"/>
		<owl:imports rdf:resource="https://spec.edmcouncil.org/fibo/ontology/FBC/FunctionalEntities/Markets/"/>
		<owl:imports rdf:resource="https://spec.edmcouncil.org/fibo/ontology/FBC/FunctionalEntities/RegistrationAuthorities/"/>
		<owl:imports rdf:resource="https://spec.edmcouncil.org/fibo/ontology/FBC/ProductsAndServices/ClientsAndAccounts/"/>
		<owl:imports rdf:resource="https://spec.edmcouncil.org/fibo/ontology/FBC/ProductsAndServices/FinancialProductsAndServices/"/>
		<owl:imports rdf:resource="https://spec.edmcouncil.org/fibo/ontology/FND/Accounting/CurrencyAmount/"/>
		<owl:imports rdf:resource="https://spec.edmcouncil.org/fibo/ontology/FND/Agreements/Contracts/"/>
		<owl:imports rdf:resource="https://spec.edmcouncil.org/fibo/ontology/FND/Arrangements/Arrangements/"/>
		<owl:imports rdf:resource="https://spec.edmcouncil.org/fibo/ontology/FND/DatesAndTimes/FinancialDates/"/>
		<owl:imports rdf:resource="https://spec.edmcouncil.org/fibo/ontology/FND/DatesAndTimes/Occurrences/"/>
		<owl:imports rdf:resource="https://spec.edmcouncil.org/fibo/ontology/FND/GoalsAndObjectives/Objectives/"/>
		<owl:imports rdf:resource="https://spec.edmcouncil.org/fibo/ontology/FND/Law/LegalCapacity/"/>
		<owl:imports rdf:resource="https://spec.edmcouncil.org/fibo/ontology/FND/OwnershipAndControl/Ownership/"/>
		<owl:imports rdf:resource="https://spec.edmcouncil.org/fibo/ontology/FND/Parties/Parties/"/>
		<owl:imports rdf:resource="https://spec.edmcouncil.org/fibo/ontology/FND/Parties/Roles/"/>
		<owl:imports rdf:resource="https://spec.edmcouncil.org/fibo/ontology/FND/ProductsAndServices/ProductsAndServices/"/>
		<owl:imports rdf:resource="https://spec.edmcouncil.org/fibo/ontology/FND/Quantities/QuantitiesAndUnits/"/>
		<owl:imports rdf:resource="https://spec.edmcouncil.org/fibo/ontology/FND/Relations/Relations/"/>
		<owl:imports rdf:resource="https://spec.edmcouncil.org/fibo/ontology/FND/Utilities/Analytics/"/>
		<owl:imports rdf:resource="https://spec.edmcouncil.org/fibo/ontology/FND/Utilities/AnnotationVocabulary/"/>
		<owl:imports rdf:resource="https://spec.edmcouncil.org/fibo/ontology/IND/ForeignExchange/ForeignExchange/"/>
		<owl:imports rdf:resource="https://spec.edmcouncil.org/fibo/ontology/IND/Indicators/Indicators/"/>
		<owl:imports rdf:resource="https://spec.edmcouncil.org/fibo/ontology/IND/MarketIndices/BasketIndices/"/>
		<owl:imports rdf:resource="https://spec.edmcouncil.org/fibo/ontology/SEC/Debt/Bonds/"/>
		<owl:imports rdf:resource="https://spec.edmcouncil.org/fibo/ontology/SEC/Debt/ExerciseConventions/"/>
		<owl:imports rdf:resource="https://spec.edmcouncil.org/fibo/ontology/SEC/Equities/EquityInstruments/"/>
		<owl:imports rdf:resource="https://spec.edmcouncil.org/fibo/ontology/SEC/Securities/Baskets/"/>
		<owl:imports rdf:resource="https://spec.edmcouncil.org/fibo/ontology/SEC/Securities/SecuritiesListings/"/>
		<owl:versionIRI rdf:resource="https://spec.edmcouncil.org/fibo/ontology/DER/DerivativesContracts/Options/"/>
		<fibo-fnd-utl-av:hasMaturityLevel rdf:resource="&fibo-fnd-utl-av;Provisional"/>
	</owl:Ontology>
	
	<owl:Class rdf:about="&fibo-der-drc-bsc;DerivativesClearingOrganization">
		<fibo-fnd-utl-av:explanatoryNote xml:lang="en">For options, the derivatives clearing organization is responsible for clearing transactions for put and call options on common stocks and other equity issues, stock indexes, foreign currencies, interest rate composites and single-stock futures. e.g. Options Clearing Corporation (US). In Canada the equivalent is In the US, the Options Clearing Corporation defines defaults e.g. lot sizes. This applies to equity options, index options, flex options, yield based options and short dated options. It does not apply to other types of option. Its roles are: 1. Clearing 2. Advocate for sound business practice. Similar to regulator though not officially one. Has a role in risk management Full list from OCC website: OCC clears transactions for put and call options on common stocks and other equity issues, stock indexes, foreign currencies, interest rate composites and single-stock futures</fibo-fnd-utl-av:explanatoryNote>
	</owl:Class>
	
	<owl:Class rdf:about="&fibo-der-der-opt;BasketOption">
		<rdfs:subClassOf rdf:resource="&fibo-fbc-fi-fi;Option"/>
		<rdfs:subClassOf>
			<owl:Restriction>
				<owl:onProperty rdf:resource="&fibo-der-drc-bsc;hasUnderlier"/>
				<owl:someValuesFrom rdf:resource="&fibo-sec-sec-bsk;MixedBasket"/>
			</owl:Restriction>
		</rdfs:subClassOf>
		<rdfs:label xml:lang="en">basket option</rdfs:label>
		<skos:definition xml:lang="en">option whose underlying asset is a basket of securities and/or indices</skos:definition>
	</owl:Class>
	
	<owl:Class rdf:about="&fibo-der-der-opt;BondOption">
		<rdfs:subClassOf rdf:resource="&fibo-der-der-opt;DebtInstrumentOption"/>
		<rdfs:subClassOf>
			<owl:Restriction>
				<owl:onProperty rdf:resource="&fibo-der-drc-bsc;hasUnderlier"/>
				<owl:someValuesFrom rdf:resource="&fibo-sec-dbt-bnd;Bond"/>
			</owl:Restriction>
		</rdfs:subClassOf>
		<rdfs:label xml:lang="en">bond option</rdfs:label>
		<skos:definition xml:lang="en">option giving the buyer (holder) the right, but not the obligation, to buy or sell (depending on whether it is a call or a put) a bond at a certain price on or before a specified date</skos:definition>
	</owl:Class>
	
	<owl:Class rdf:about="&fibo-der-der-opt;CallOption">
		<rdfs:subClassOf rdf:resource="&fibo-fbc-fi-fi;Option"/>
		<rdfs:subClassOf>
			<owl:Restriction>
				<owl:onProperty rdf:resource="&fibo-fnd-pas-pas;hasBuyer"/>
				<owl:someValuesFrom>
					<owl:Class>
						<owl:unionOf rdf:parseType="Collection">
							<rdf:Description rdf:about="&fibo-der-der-opt;OptionHolder">
							</rdf:Description>
							<rdf:Description rdf:about="&fibo-der-drc-bsc;PayingParty">
							</rdf:Description>
						</owl:unionOf>
					</owl:Class>
				</owl:someValuesFrom>
			</owl:Restriction>
		</rdfs:subClassOf>
		<rdfs:subClassOf>
			<owl:Restriction>
				<owl:onProperty rdf:resource="&fibo-fnd-pas-pas;hasSeller"/>
				<owl:someValuesFrom>
					<owl:Class>
						<owl:unionOf rdf:parseType="Collection">
							<rdf:Description rdf:about="&fibo-der-der-opt;OptionIssuer">
							</rdf:Description>
							<rdf:Description rdf:about="&fibo-der-drc-bsc;ReceivingParty">
							</rdf:Description>
						</owl:unionOf>
					</owl:Class>
				</owl:someValuesFrom>
			</owl:Restriction>
		</rdfs:subClassOf>
		<rdfs:label xml:lang="en">call option</rdfs:label>
		<skos:definition xml:lang="en">option giving the buyer (holder) the right, but not the obligation, to buy the assets specified at a fixed price or formula, on or before a specified date</skos:definition>
		<fibo-fnd-utl-av:adaptedFrom xml:lang="en">ISO 10962, Securities and related financial instruments - Classification of financial instruments (CFI) code, Fourth Edition, 2019.</fibo-fnd-utl-av:adaptedFrom>
		<fibo-fnd-utl-av:explanatoryNote xml:lang="en">The seller (issuer) of the call option assumes the obligation of delivering the assets specified should the buyer exercise the option. The buyer has the option, but not the obligation, to purchase the underlying asset.</fibo-fnd-utl-av:explanatoryNote>
	</owl:Class>
	
	<owl:Class rdf:about="&fibo-der-der-opt;CommodityOption">
		<rdfs:subClassOf rdf:resource="&fibo-der-com-ctr;CommodityDerivative"/>
		<rdfs:subClassOf rdf:resource="&fibo-fbc-fi-fi;Option"/>
		<rdfs:label xml:lang="en">commodity option</rdfs:label>
		<skos:definition xml:lang="en">option whose underlying asset is at least one commodity, commodity index, and/or commodity-specific contract</skos:definition>
	</owl:Class>
	
	<owl:Class rdf:about="&fibo-der-der-opt;CurrencyOption">
		<rdfs:subClassOf rdf:resource="&fibo-der-der-opt;ExchangeTradedOption"/>
		<rdfs:subClassOf rdf:resource="&fibo-der-fx-ctr;CurrencyDerivative"/>
		<rdfs:subClassOf>
			<owl:Restriction>
				<owl:onProperty rdf:resource="&fibo-der-drc-bsc;hasUnderlier"/>
				<owl:onClass rdf:resource="&fibo-ind-fx-fx;CurrencySpotBuyRate"/>
				<owl:minQualifiedCardinality rdf:datatype="&xsd;nonNegativeInteger">0</owl:minQualifiedCardinality>
			</owl:Restriction>
		</rdfs:subClassOf>
		<rdfs:subClassOf>
			<owl:Restriction>
				<owl:onProperty rdf:resource="&fibo-der-der-opt;hasStrikeRate"/>
				<owl:someValuesFrom rdf:resource="&fibo-fnd-acc-cur;ExchangeRate"/>
			</owl:Restriction>
		</rdfs:subClassOf>
		<rdfs:label xml:lang="en">currency option</rdfs:label>
		<skos:definition xml:lang="en">option giving the buyer (holder) the right, but not the obligation, to buy or sell currency at a specified exchange rate during a specified period of time.</skos:definition>
		<fibo-fnd-utl-av:abbreviation xml:lang="en">FX option</fibo-fnd-utl-av:abbreviation>
		<fibo-fnd-utl-av:explanatoryNote xml:lang="en">For this right, a premium is paid to the broker, which will vary depending on the number of contracts purchased. Currency options are one of the best ways for corporations or individuals to hedge against adverse movements in exchange rates. Investors can hedge against foreign currency risk by purchasing a currency option put or call. For example, assume that an investor believes that the USD/EUR rate is going to increase from 0.80 to 0.90 (meaning that it will become more expensive for a European investor to buy U.S dollars). In this case, the investor would want to buy a call option on USD/EUR so that he or she could stand to gain from an increase in the exchange rate (or the USD rise).</fibo-fnd-utl-av:explanatoryNote>
		<fibo-fnd-utl-av:synonym xml:lang="en">foreign exchange option</fibo-fnd-utl-av:synonym>
		<fibo-fnd-utl-av:synonym xml:lang="en">forex option</fibo-fnd-utl-av:synonym>
	</owl:Class>
	
	<owl:Class rdf:about="&fibo-der-der-opt;CurrencyVolatilityOption">
		<rdfs:subClassOf rdf:resource="&fibo-der-der-opt;CurrencyOption"/>
		<rdfs:subClassOf>
			<owl:Restriction>
				<owl:onProperty rdf:resource="&fibo-der-drc-bsc;hasUnderlier"/>
				<owl:someValuesFrom rdf:resource="&fibo-ind-fx-fx;CurrencySpotVolatility"/>
			</owl:Restriction>
		</rdfs:subClassOf>
		<rdfs:label xml:lang="en">currency volatility option</rdfs:label>
		<skos:definition xml:lang="en">currency option whose underlying asset is based on the volatility of a foreign exchange rate</skos:definition>
	</owl:Class>
	
	<owl:Class rdf:about="&fibo-der-der-opt;DebtInstrumentOption">
		<rdfs:subClassOf rdf:resource="&fibo-der-sbd-sbd;DebtInstrumentDerivative"/>
		<rdfs:subClassOf rdf:resource="&fibo-fbc-fi-fi;Option"/>
		<rdfs:label xml:lang="en">debt instrument option</rdfs:label>
		<skos:definition xml:lang="en">option whose underlying asset is a debt observable</skos:definition>
	</owl:Class>
	
	<owl:Class rdf:about="&fibo-der-der-opt;EquityOption">
		<rdfs:subClassOf rdf:resource="&fibo-der-sbd-sbd;EquityDerivative"/>
		<rdfs:subClassOf rdf:resource="&fibo-fbc-fi-fi;Option"/>
		<rdfs:subClassOf>
			<owl:Restriction>
				<owl:onProperty rdf:resource="&fibo-der-der-opt;hasOptionMultiplier"/>
				<owl:minQualifiedCardinality rdf:datatype="&xsd;nonNegativeInteger">0</owl:minQualifiedCardinality>
				<owl:onDataRange rdf:resource="&xsd;decimal"/>
			</owl:Restriction>
		</rdfs:subClassOf>
		<rdfs:subClassOf>
			<owl:Restriction>
				<owl:onProperty rdf:resource="&fibo-der-drc-bsc;hasUnderlier"/>
				<owl:someValuesFrom rdf:resource="&fibo-der-sbd-sbd;EquityObservable"/>
			</owl:Restriction>
		</rdfs:subClassOf>
		<rdfs:label xml:lang="en">equity option</rdfs:label>
		<skos:definition xml:lang="en">Equity options are the most common type of equity derivative. They provide the right, but not the obligation to trade a quantity of stock at a set price at a future time.</skos:definition>
	</owl:Class>
	
	<owl:Class rdf:about="&fibo-der-der-opt;ExchangeTradedOption">
		<rdfs:subClassOf rdf:resource="&fibo-fbc-fi-fi;Option"/>
		<rdfs:subClassOf>
			<owl:Restriction>
				<owl:onProperty rdf:resource="&fibo-fbc-dae-gty;hasGuarantor"/>
				<owl:someValuesFrom rdf:resource="&fibo-der-der-opt;OptionGuarantor"/>
			</owl:Restriction>
		</rdfs:subClassOf>
		<rdfs:subClassOf>
			<owl:Restriction>
				<owl:onProperty rdf:resource="&fibo-fbc-fi-ip;hasPriceDeterminationMethod"/>
				<owl:someValuesFrom rdf:resource="&fibo-fbc-fi-ip;PriceDeterminationMethod"/>
			</owl:Restriction>
		</rdfs:subClassOf>
		<rdfs:subClassOf>
			<owl:Restriction>
				<owl:onProperty rdf:resource="&fibo-fnd-agr-ctr;hasContractDuration"/>
				<owl:someValuesFrom rdf:resource="&fibo-fnd-dt-fd;ExplicitDuration"/>
			</owl:Restriction>
		</rdfs:subClassOf>
		<rdfs:subClassOf>
			<owl:Restriction>
				<owl:onProperty rdf:resource="&fibo-fnd-agr-ctr;hasCounterparty"/>
				<owl:someValuesFrom rdf:resource="&fibo-der-der-opt;TradedOptionsCounterparty"/>
			</owl:Restriction>
		</rdfs:subClassOf>
		<rdfs:subClassOf>
			<owl:Restriction>
				<owl:onProperty rdf:resource="&fibo-fnd-pas-pas;hasSeller"/>
				<owl:someValuesFrom>
					<owl:Class>
						<owl:intersectionOf rdf:parseType="Collection">
							<rdf:Description rdf:about="&fibo-der-der-opt;OptionIssuer">
							</rdf:Description>
							<rdf:Description rdf:about="&fibo-der-der-opt;OptionsExchangeParticipant">
							</rdf:Description>
						</owl:intersectionOf>
					</owl:Class>
				</owl:someValuesFrom>
			</owl:Restriction>
		</rdfs:subClassOf>
		<rdfs:label xml:lang="en">exchange-traded option</rdfs:label>
		<skos:definition xml:lang="en">standardized option giving the buyer (holder) the right, but not the obligation, to buy (via a call option) or sell (via a put option) the underlying assets specified at a pre-determined price (i.e., the strike price, fixed or calculated), on or before a specified date (the expiration date)</skos:definition>
	</owl:Class>
	
	<owl:Class rdf:about="&fibo-der-der-opt;InterestRateOption">
		<rdfs:subClassOf rdf:resource="&fibo-der-der-opt;OptionOnFuture"/>
		<rdfs:subClassOf>
			<owl:Restriction>
				<owl:onProperty rdf:resource="&fibo-der-drc-bsc;hasUnderlier"/>
				<owl:someValuesFrom rdf:resource="&fibo-fnd-acc-cur;InterestRate"/>
			</owl:Restriction>
		</rdfs:subClassOf>
		<rdfs:label xml:lang="en">interest rate option</rdfs:label>
		<skos:definition xml:lang="en">option on some underlying interest rate</skos:definition>
		<fibo-fnd-utl-av:explanatoryNote xml:lang="en">If the option is exercised, delivery is in the form of the corresponding interest rate future.</fibo-fnd-utl-av:explanatoryNote>
	</owl:Class>
	
	<owl:Class rdf:about="&fibo-der-der-opt;LongTermEquityOption">
		<rdfs:subClassOf rdf:resource="&fibo-der-der-opt;EquityOption"/>
		<rdfs:subClassOf>
			<owl:Restriction>
				<owl:onProperty rdf:resource="&fibo-fnd-agr-ctr;hasContractDuration"/>
				<owl:someValuesFrom rdf:resource="&fibo-fnd-dt-fd;Duration"/>
			</owl:Restriction>
		</rdfs:subClassOf>
		<rdfs:label xml:lang="en">long term equity option</rdfs:label>
		<skos:definition xml:lang="en">An option whose contract expires at a date longer than one year. Also known as long-term equity anticipation securities (LEAPS). From Investopedia: These options are called long-term equity anticipation securities (LEAPS). By providing opportunities to control and manage risk or even to speculate, LEAPS are virtually identical to regular options. LEAPS, however, provide these opportunities for much longer periods of time. Although they are not available on all stocks, LEAPS are available on most widely held issues.</skos:definition>
	</owl:Class>
	
	<owl:Class rdf:about="&fibo-der-der-opt;NovatedOptionContract">
		<rdfs:subClassOf rdf:resource="&fibo-der-der-opt;ExchangeTradedOption"/>
		<rdfs:subClassOf>
			<owl:Restriction>
				<owl:onProperty rdf:resource="&fibo-fnd-pas-pas;hasSeller"/>
				<owl:someValuesFrom rdf:resource="&fibo-der-der-opt;NovatedOptionContractPrincipal"/>
			</owl:Restriction>
		</rdfs:subClassOf>
		<rdfs:label xml:lang="en">novated option contract</rdfs:label>
		<skos:definition xml:lang="en">An Option Contract after the stage where a Derivatives Exchange has novated this contract and become the principal to it, for purposes of clearing and settlement. The Clearing House novates both contract. So when you are on the floor (as a Broker), you trade with another Broker. Then you take it to th eRing, and present it to the Ring. So you write a contract and give it to the ringleader, who then books it. So the party you dealt with deals with the exahcnge, and you deal with the exchange. THen there are two contracts for one deal. So the answer here is that there are two novated contracts for one Options deal. Difference: If not open outcry? In OO the deal is done and given to the ringleader, who represents the Cleaing house. When it&apos;s not open outcry, the clearing house gets the deal, books the deal, and margins it. So you don&apos;t know as much about the deal and process. This eliminiates stickiness of a market that has credit. Similar to what occurs in share markets, where clearing takes place, e.g. when someone defaults on delivery. Clearing House simply closes out the contract.</skos:definition>
	</owl:Class>
	
	<owl:Class rdf:about="&fibo-der-der-opt;NovatedOptionContractPrincipal">
		<rdfs:subClassOf rdf:resource="&fibo-der-der-opt;TradedOptionPrincipal"/>
		<rdfs:subClassOf>
			<owl:Restriction>
				<owl:onProperty rdf:resource="&fibo-fnd-rel-rel;hasIdentity"/>
				<owl:someValuesFrom>
					<owl:Class>
						<owl:unionOf rdf:parseType="Collection">
							<rdf:Description rdf:about="&fibo-der-drc-bsc;DesignatedContractMarket">
							</rdf:Description>
							<rdf:Description rdf:about="&fibo-der-drc-bsc;DerivativesClearingOrganization">
							</rdf:Description>
						</owl:unionOf>
					</owl:Class>
				</owl:someValuesFrom>
			</owl:Restriction>
		</rdfs:subClassOf>
		<rdfs:label xml:lang="en">novated option contract principal</rdfs:label>
	</owl:Class>
	
	<owl:Class rdf:about="&fibo-der-der-opt;OptionGuarantor">
		<rdfs:subClassOf rdf:resource="&fibo-fbc-dae-gty;Guarantor"/>
		<rdfs:subClassOf>
			<owl:Restriction>
				<owl:onProperty rdf:resource="&fibo-fnd-rel-rel;hasIdentity"/>
				<owl:someValuesFrom>
					<owl:Class>
						<owl:unionOf rdf:parseType="Collection">
							<rdf:Description rdf:about="&fibo-der-drc-bsc;DesignatedContractMarket">
							</rdf:Description>
							<rdf:Description rdf:about="&fibo-der-drc-bsc;DerivativesClearingOrganization">
							</rdf:Description>
						</owl:unionOf>
					</owl:Class>
				</owl:someValuesFrom>
			</owl:Restriction>
		</rdfs:subClassOf>
		<rdfs:label xml:lang="en">option guarantor</rdfs:label>
		<skos:definition xml:lang="en">guarantor that is an options exchange or clearinghouse that guarantees fulfillment of the terms of the option</skos:definition>
		<fibo-fnd-utl-av:explanatoryNote xml:lang="en">In other words, the exchange or clearinghouse guarantees the trade with respect to any losses incurred by the holder in the event of a default by the issuer, not the value of the underlying asset.</fibo-fnd-utl-av:explanatoryNote>
	</owl:Class>
	
	<owl:Class rdf:about="&fibo-der-der-opt;OptionHolder">
		<rdfs:subClassOf rdf:resource="&fibo-fnd-oac-own;Owner"/>
		<rdfs:subClassOf>
			<owl:Restriction>
				<owl:onProperty rdf:resource="&fibo-fnd-rel-rel;holds"/>
				<owl:someValuesFrom rdf:resource="&fibo-fbc-fi-fi;Option"/>
			</owl:Restriction>
		</rdfs:subClassOf>
		<rdfs:label xml:lang="en">option holder</rdfs:label>
		<skos:definition xml:lang="en">party that owns an option</skos:definition>
		<fibo-fnd-utl-av:explanatoryNote xml:lang="en">In a call, the option holder has the right, but not the obligation, to buy the underlying asset, while, in a put, the option holder has the right to sell the underlying asset. An option holder may sell the option contract itself, at which point the buyer becomes the option holder. The holder has an obligation to inform the seller by a certain time if they wish to exercise. Once the instrument is exercised there are typically additional, relevant obligations with regard to settlement.</fibo-fnd-utl-av:explanatoryNote>
	</owl:Class>
	
	<owl:Class rdf:about="&fibo-der-der-opt;OptionIssuer">
		<rdfs:subClassOf rdf:resource="&fibo-fbc-fi-fi;Issuer"/>
		<rdfs:subClassOf>
			<owl:Restriction>
				<owl:onProperty rdf:resource="&fibo-fnd-pty-rl;isPlayedBy"/>
				<owl:someValuesFrom>
					<owl:Restriction>
						<owl:onProperty rdf:resource="&fibo-fnd-pty-pty;isAPartyTo"/>
						<owl:someValuesFrom rdf:resource="&fibo-fbc-fi-fi;Option"/>
					</owl:Restriction>
				</owl:someValuesFrom>
			</owl:Restriction>
		</rdfs:subClassOf>
		<rdfs:label xml:lang="en">option issuer</rdfs:label>
		<skos:definition xml:lang="en">issuer granting the rights defined in the option in exchange for some consideration</skos:definition>
	</owl:Class>
	
	<owl:Class rdf:about="&fibo-der-der-opt;OptionOnFuture">
		<rdfs:subClassOf rdf:resource="&fibo-fbc-fi-fi;Option"/>
		<rdfs:subClassOf>
			<owl:Restriction>
				<owl:onProperty rdf:resource="&fibo-der-drc-bsc;hasUnderlier"/>
				<owl:someValuesFrom rdf:resource="&fibo-fbc-fi-fi;Future"/>
			</owl:Restriction>
		</rdfs:subClassOf>
		<rdfs:subClassOf>
			<owl:Restriction>
				<owl:onProperty rdf:resource="&fibo-sec-dbt-ex;hasExerciseTerms"/>
				<owl:someValuesFrom rdf:resource="&fibo-sec-dbt-ex;AmericanExerciseTerms"/>
			</owl:Restriction>
		</rdfs:subClassOf>
		<rdfs:label xml:lang="en">option on future</rdfs:label>
		<skos:definition xml:lang="en">option that gives the holder the right, but not the obligation, to buy or sell a specific futures contract at a specified price on or before the option&apos;s expiration date</skos:definition>
	</owl:Class>
	
	<owl:Class rdf:about="&fibo-der-der-opt;OptionPremium">
		<rdfs:subClassOf rdf:resource="&fibo-fbc-fi-ip;MarketPrice"/>
		<rdfs:subClassOf rdf:resource="&fibo-fnd-acc-cur;CalculatedPrice"/>
		<rdfs:subClassOf>
			<owl:Restriction>
				<owl:onProperty rdf:resource="&fibo-fnd-acc-cur;hasMonetaryAmount"/>
				<owl:onClass rdf:resource="&fibo-fnd-acc-cur;MonetaryAmount"/>
				<owl:minQualifiedCardinality rdf:datatype="&xsd;nonNegativeInteger">0</owl:minQualifiedCardinality>
			</owl:Restriction>
		</rdfs:subClassOf>
		<rdfs:subClassOf>
			<owl:Restriction>
				<owl:onProperty rdf:resource="&fibo-fnd-qt-qtu;hasQuantityValue"/>
				<owl:onClass rdf:resource="&fibo-fnd-acc-cur;PercentageMonetaryAmount"/>
				<owl:minQualifiedCardinality rdf:datatype="&xsd;nonNegativeInteger">0</owl:minQualifiedCardinality>
			</owl:Restriction>
		</rdfs:subClassOf>
		<rdfs:subClassOf>
			<owl:Restriction>
				<owl:onProperty rdf:resource="&fibo-der-der-opt;hasRelativePaymentDate"/>
				<owl:someValuesFrom rdf:resource="&fibo-fnd-dt-fd;RelativeDate"/>
			</owl:Restriction>
		</rdfs:subClassOf>
		<rdfs:label xml:lang="en">option premium</rdfs:label>
		<skos:definition xml:lang="en">current market price of an option contract</skos:definition>
		<fibo-fnd-utl-av:explanatoryNote xml:lang="en">The option premium is the income received by the seller (writer) of an option contract to another party. In-the-money option premiums are composed of two factors: intrinsic and extrinsic value. Out-of-the-money options&apos; premiums consist solely of extrinsic value. For stock options, the premium is quoted as a dollar amount per share, and most contracts represent the commitment of 100 shares.</fibo-fnd-utl-av:explanatoryNote>
	</owl:Class>
	
	<owl:Class rdf:about="&fibo-der-der-opt;OptionTerms">
		<rdfs:subClassOf rdf:resource="&fibo-der-drc-bsc;DerivativeTerms"/>
		<rdfs:subClassOf>
			<owl:Restriction>
				<owl:onProperty rdf:resource="&fibo-fbc-fct-ra;specifies"/>
				<owl:someValuesFrom rdf:resource="&fibo-sec-dbt-ex;ExerciseTerms"/>
			</owl:Restriction>
		</rdfs:subClassOf>
		<rdfs:label xml:lang="en">option terms</rdfs:label>
	</owl:Class>
	
	<owl:Class rdf:about="&fibo-der-der-opt;OptionsExchangeParticipant">
		<rdfs:subClassOf rdf:resource="&fibo-fnd-pty-pty;PartyInRole"/>
		<rdfs:label xml:lang="en">options exchange participant</rdfs:label>
	</owl:Class>
	
	<owl:Class rdf:about="&fibo-der-der-opt;OptionsListing">
		<rdfs:subClassOf rdf:resource="&fibo-sec-sec-lst;Listing"/>
		<rdfs:subClassOf>
			<owl:Restriction>
				<owl:onProperty rdf:resource="&fibo-fnd-rel-rel;isProvidedBy"/>
				<owl:allValuesFrom>
					<owl:Class>
						<owl:unionOf rdf:parseType="Collection">
							<rdf:Description rdf:about="&fibo-der-drc-bsc;DesignatedContractMarket">
							</rdf:Description>
							<rdf:Description rdf:about="&fibo-der-drc-bsc;DerivativesClearingOrganization">
							</rdf:Description>
						</owl:unionOf>
					</owl:Class>
				</owl:allValuesFrom>
			</owl:Restriction>
		</rdfs:subClassOf>
		<rdfs:label xml:lang="en">options listing</rdfs:label>
		<skos:definition xml:lang="en">A listing of an options instrument on a derivatives exchange. The listing is a product of the individual exchange.</skos:definition>
		<skos:editorialNote xml:lang="en">This term sdoes not exist. If there was a listing of something that was an option, it would be a warrant. Review: We agreed to come back to this definition and verify whether it means the same as listing in the equities sense .</skos:editorialNote>
	</owl:Class>
	
	<owl:Class rdf:about="&fibo-der-der-opt;PutOption">
		<rdfs:subClassOf rdf:resource="&fibo-fbc-fi-fi;Option"/>
		<rdfs:subClassOf>
			<owl:Restriction>
				<owl:onProperty rdf:resource="&fibo-fnd-pas-pas;hasBuyer"/>
				<owl:someValuesFrom>
					<owl:Class>
						<owl:unionOf rdf:parseType="Collection">
							<rdf:Description rdf:about="&fibo-der-der-opt;OptionHolder">
							</rdf:Description>
							<rdf:Description rdf:about="&fibo-der-drc-bsc;ReceivingParty">
							</rdf:Description>
						</owl:unionOf>
					</owl:Class>
				</owl:someValuesFrom>
			</owl:Restriction>
		</rdfs:subClassOf>
		<rdfs:subClassOf>
			<owl:Restriction>
				<owl:onProperty rdf:resource="&fibo-fnd-pas-pas;hasSeller"/>
				<owl:someValuesFrom>
					<owl:Class>
						<owl:unionOf rdf:parseType="Collection">
							<rdf:Description rdf:about="&fibo-der-der-opt;OptionIssuer">
							</rdf:Description>
							<rdf:Description rdf:about="&fibo-der-drc-bsc;PayingParty">
							</rdf:Description>
						</owl:unionOf>
					</owl:Class>
				</owl:someValuesFrom>
			</owl:Restriction>
		</rdfs:subClassOf>
		<rdfs:label xml:lang="en">put option</rdfs:label>
		<skos:definition xml:lang="en">option giving the buyer (holder) the right, but not the obligation, to to sell the assets specified at a fixed price or formula, on or before a specified date</skos:definition>
		<fibo-fnd-utl-av:adaptedFrom xml:lang="en">ISO 10962, Securities and related financial instruments - Classification of financial instruments (CFI) code, Fourth Edition, 2019.</fibo-fnd-utl-av:adaptedFrom>
		<fibo-fnd-utl-av:explanatoryNote xml:lang="en">The seller of the put option assumes the obligation of buying the assets specified should the buyer exercise the option.</fibo-fnd-utl-av:explanatoryNote>
	</owl:Class>
	
	<owl:Class rdf:about="&fibo-der-der-opt;SingleStockOption">
		<rdfs:subClassOf rdf:resource="&fibo-der-der-opt;EquityOption"/>
		<rdfs:subClassOf>
			<owl:Restriction>
				<owl:onProperty rdf:resource="&fibo-der-drc-bsc;hasUnderlier"/>
				<owl:someValuesFrom>
					<owl:Restriction>
						<owl:onProperty rdf:resource="&fibo-fnd-rel-rel;hasIdentity"/>
						<owl:someValuesFrom rdf:resource="&fibo-sec-eq-eq;ListedShare"/>
					</owl:Restriction>
				</owl:someValuesFrom>
			</owl:Restriction>
		</rdfs:subClassOf>
		<rdfs:label xml:lang="en">single stock option</rdfs:label>
		<skos:definition xml:lang="en">equity option whose underlier is a specific equity instrument</skos:definition>
	</owl:Class>
	
	<owl:Class rdf:about="&fibo-der-der-opt;StandardizedExerciseTerms">
		<rdfs:subClassOf rdf:resource="&fibo-der-der-opt;StandardizedOptionsTerms"/>
		<rdfs:subClassOf rdf:resource="&fibo-sec-dbt-ex;ExerciseTerms"/>
		<rdfs:subClassOf>
			<owl:Restriction>
				<owl:onProperty rdf:resource="&fibo-fbc-fct-ra;specifies"/>
				<owl:someValuesFrom rdf:resource="&fibo-fbc-fi-fi;FinancialInstrument"/>
			</owl:Restriction>
		</rdfs:subClassOf>
		<rdfs:label xml:lang="en">standardized exercise terms</rdfs:label>
		<skos:definition xml:lang="en">Standard exercise terms for an option contract, determined in advance by the exchange. These will become exercise terms of an individual option contract. These may be varied or overridden for individual contracts.</skos:definition>
	</owl:Class>
	
	<owl:Class rdf:about="&fibo-der-der-opt;StandardizedOptionsTerms">
		<rdfs:subClassOf rdf:resource="&fibo-fbc-fi-fi;StandardizedTerms"/>
		<rdfs:subClassOf>
			<owl:Restriction>
				<owl:onProperty rdf:resource="&fibo-be-fct-pub;hasPublisher"/>
				<owl:someValuesFrom>
					<owl:Class>
						<owl:unionOf rdf:parseType="Collection">
							<rdf:Description rdf:about="&fibo-fbc-fct-mkt;Exchange">
							</rdf:Description>
							<rdf:Description rdf:about="&fibo-der-drc-bsc;DerivativesClearingOrganization">
							</rdf:Description>
						</owl:unionOf>
					</owl:Class>
				</owl:someValuesFrom>
			</owl:Restriction>
		</rdfs:subClassOf>
		<rdfs:subClassOf>
			<owl:Restriction>
				<owl:onProperty rdf:resource="&fibo-fbc-fi-ip;hasPriceDeterminationMethod"/>
				<owl:someValuesFrom rdf:resource="&fibo-fbc-fi-ip;PriceDeterminationMethod"/>
			</owl:Restriction>
		</rdfs:subClassOf>
		<rdfs:subClassOf>
			<owl:Restriction>
				<owl:onProperty rdf:resource="&fibo-fnd-rel-rel;appliesTo"/>
				<owl:someValuesFrom rdf:resource="&fibo-der-der-opt;ExchangeTradedOption"/>
			</owl:Restriction>
		</rdfs:subClassOf>
		<rdfs:label xml:lang="en">standardized options terms</rdfs:label>
		<skos:definition xml:lang="en">standardized contract terms established by a securities or options exchange or by an options clearing entity</skos:definition>
		<fibo-fnd-utl-av:adaptedFrom xml:lang="en">ISO 10962, Securities and related financial instruments - Classification of financial instruments (CFI) code, Fourth Edition, 2019.</fibo-fnd-utl-av:adaptedFrom>
		<fibo-fnd-utl-av:explanatoryNote xml:lang="en">Such terms may relate to the underlying instruments, exercise price, expiration date, and contract size, for example.</fibo-fnd-utl-av:explanatoryNote>
	</owl:Class>
	
	<owl:Class rdf:about="&fibo-der-der-opt;StrikePrice">
		<rdfs:subClassOf rdf:resource="&fibo-fnd-acc-cur;MonetaryPrice"/>
		<rdfs:label xml:lang="en">strike price</rdfs:label>
		<skos:definition xml:lang="en">The strike price for the option is the agreed price for the transaction if this takes place. Applies to all options types. Action: Make sure that&apos;s there for all Options types.</skos:definition>
	</owl:Class>
	
	<owl:Class rdf:about="&fibo-der-der-opt;Swaption">
		<rdfs:subClassOf rdf:resource="&fibo-fbc-fi-fi;Option"/>
		<rdfs:subClassOf>
			<owl:Restriction>
				<owl:onProperty rdf:resource="&fibo-der-drc-bsc;hasUnderlier"/>
				<owl:someValuesFrom rdf:resource="&fibo-der-drc-swp;Swap"/>
			</owl:Restriction>
		</rdfs:subClassOf>
		<rdfs:label xml:lang="en">swaption</rdfs:label>
		<skos:definition xml:lang="en">over-the-counter option that confers the right but not the obligation, to enter into a swap transaction at some time in the future</skos:definition>
		<fibo-fnd-utl-av:explanatoryNote xml:lang="en">A swaption, also known as a swap option, refers to an option to enter into an interest rate swap or some other type of swap. In exchange for an options premium, the buyer gains the right but not the obligation to enter into a specified swap agreement with the issuer on a specified future date.</fibo-fnd-utl-av:explanatoryNote>
		<fibo-fnd-utl-av:synonym xml:lang="en">swap option</fibo-fnd-utl-av:synonym>
	</owl:Class>
	
	<owl:Class rdf:about="&fibo-der-der-opt;TradedOptionPrincipal">
		<rdfs:subClassOf rdf:resource="&fibo-der-der-opt;OptionIssuer"/>
		<rdfs:subClassOf rdf:resource="&fibo-der-der-opt;OptionsExchangeParticipant"/>
		<rdfs:label xml:lang="en">traded option principal</rdfs:label>
		<owl:disjointWith rdf:resource="&fibo-der-der-opt;TradedOptionsCounterparty"/>
		<skos:definition xml:lang="en">The principal to the Traded Option contract. THis is the party which gives the other party the right to take up the obligation, and which is obliged to honor that transaction if that option is taken up.</skos:definition>
	</owl:Class>
	
	<owl:Class rdf:about="&fibo-der-der-opt;TradedOptionsCounterparty">
		<rdfs:subClassOf rdf:resource="&fibo-der-der-opt;OptionHolder"/>
		<rdfs:subClassOf rdf:resource="&fibo-der-der-opt;OptionsExchangeParticipant"/>
		<rdfs:label xml:lang="en">traded options counterparty</rdfs:label>
	</owl:Class>
	
	<owl:Class rdf:about="&fibo-der-der-opt;UnderlyingAssetBuyer">
		<rdfs:subClassOf rdf:resource="&fibo-fnd-pas-pas;Buyer"/>
		<rdfs:label xml:lang="en">underlying asset buyer</rdfs:label>
		<skos:definition xml:lang="en">buyer of the underlying asset in an option-related transaction</skos:definition>
		<fibo-fnd-utl-av:explanatoryNote xml:lang="en">This is the party which buys the underlying in the event that the transaction goes ahead.</fibo-fnd-utl-av:explanatoryNote>
	</owl:Class>
	
	<owl:Class rdf:about="&fibo-der-der-opt;UnderlyingAssetSeller">
		<rdfs:subClassOf rdf:resource="&fibo-fnd-pas-pas;Seller"/>
		<rdfs:label xml:lang="en">underlying asset seller</rdfs:label>
		<skos:definition xml:lang="en">seller of the underlying asset in an option transaction</skos:definition>
	</owl:Class>
	
	<owl:ObjectProperty rdf:about="&fibo-der-der-opt;hasExercisePrice">
		<rdfs:subPropertyOf rdf:resource="&fibo-fnd-acc-cur;hasPrice"/>
		<rdfs:label xml:lang="en">has exercise price</rdfs:label>
		<rdfs:range rdf:resource="&fibo-fnd-acc-cur;MonetaryPrice"/>
		<skos:definition xml:lang="en">predetermined price at which the holder commits to buy or sell an underlying asset</skos:definition>
		<fibo-fnd-utl-av:synonym xml:lang="en">has strike price</fibo-fnd-utl-av:synonym>
	</owl:ObjectProperty>
	
	<owl:ObjectProperty rdf:about="&fibo-der-der-opt;hasExerciseSchedule">
		<rdfs:subPropertyOf rdf:resource="&fibo-fnd-dt-fd;hasSchedule"/>
		<rdfs:label xml:lang="en">has exercise schedule</rdfs:label>
		<rdfs:domain rdf:resource="&fibo-fbc-fi-fi;Option"/>
		<rdfs:range rdf:resource="&fibo-fnd-dt-fd;Schedule"/>
	</owl:ObjectProperty>
	
	<owl:DatatypeProperty rdf:about="&fibo-der-der-opt;hasOptionMultiplier">
		<rdfs:subPropertyOf rdf:resource="&fibo-fnd-qt-qtu;hasNumericValue"/>
		<rdfs:label xml:lang="en">has option multiplier</rdfs:label>
		<rdfs:range rdf:resource="&xsd;decimal"/>
		<skos:definition xml:lang="en">numeric multiplying factor associated with an option underlier</skos:definition>
		<skos:example xml:lang="en">In exchange-traded equity options (index and single-stock) the standard multiplier is 100. A single option represents 100 shares of stock.</skos:example>
	</owl:DatatypeProperty>
	
	<owl:ObjectProperty rdf:about="&fibo-der-der-opt;hasPremium">
		<rdfs:label xml:lang="en">has premium</rdfs:label>
		<rdfs:domain rdf:resource="&fibo-fbc-fi-fi;Option"/>
		<rdfs:range rdf:resource="&fibo-der-der-opt;OptionPremium"/>
	</owl:ObjectProperty>
	
	<owl:ObjectProperty rdf:about="&fibo-der-der-opt;hasRelativePaymentDate">
		<rdfs:subPropertyOf rdf:resource="&fibo-fnd-dt-fd;hasDate"/>
		<rdfs:label xml:lang="en">has relative payment date</rdfs:label>
		<rdfs:range rdf:resource="&fibo-fnd-dt-fd;RelativeDate"/>
		<skos:definition xml:lang="en">The payment date for the Option Premium.</skos:definition>
		<fibo-fnd-utl-av:explanatoryNote xml:lang="en">This can be expressed as either an adjustable or relative date. FpML: &apos;The payment date, which can be expressed as either an adjustable or relative date.&apos;</fibo-fnd-utl-av:explanatoryNote>
	</owl:ObjectProperty>
	
	<owl:ObjectProperty rdf:about="&fibo-der-der-opt;hasStrikeRate">
		<rdfs:subPropertyOf rdf:resource="&fibo-fnd-qt-qtu;hasQuantityValue"/>
		<rdfs:label xml:lang="en">has strike rate</rdfs:label>
		<rdfs:range rdf:resource="&fibo-fnd-acc-cur;ExchangeRate"/>
		<skos:definition xml:lang="en">rate of exchange between two currencies as compared with the value of the underlying rate at which the contract may be exercised</skos:definition>
	</owl:ObjectProperty>
	
	<owl:Class rdf:about="&fibo-fbc-fi-fi;Option">
		<rdfs:subClassOf>
			<owl:Restriction>
				<owl:onProperty rdf:resource="&fibo-der-der-opt;hasPremium"/>
				<owl:minQualifiedCardinality rdf:datatype="&xsd;nonNegativeInteger">0</owl:minQualifiedCardinality>
				<owl:someValuesFrom rdf:resource="&fibo-der-der-opt;OptionPremium"/>
			</owl:Restriction>
		</rdfs:subClassOf>
		<rdfs:subClassOf>
			<owl:Restriction>
				<owl:onProperty rdf:resource="&fibo-der-drc-bsc;hasContractSize"/>
				<owl:someValuesFrom rdf:resource="&xsd;integer"/>
			</owl:Restriction>
		</rdfs:subClassOf>
		<rdfs:subClassOf>
			<owl:Restriction>
				<owl:onProperty rdf:resource="&fibo-der-der-opt;hasExercisePrice"/>
				<owl:someValuesFrom rdf:resource="&fibo-fnd-acc-cur;MonetaryPrice"/>
			</owl:Restriction>
		</rdfs:subClassOf>
		<rdfs:subClassOf>
			<owl:Restriction>
				<owl:onProperty rdf:resource="&fibo-der-der-opt;hasExerciseSchedule"/>
				<owl:someValuesFrom rdf:resource="&fibo-fnd-dt-fd;Schedule"/>
			</owl:Restriction>
		</rdfs:subClassOf>
		<rdfs:subClassOf>
			<owl:Restriction>
				<owl:onProperty rdf:resource="&fibo-fnd-pas-pas;hasBuyer"/>
				<owl:someValuesFrom rdf:resource="&fibo-fnd-pas-pas;Buyer"/>
			</owl:Restriction>
		</rdfs:subClassOf>
		<rdfs:subClassOf>
			<owl:Restriction>
				<owl:onProperty rdf:resource="&fibo-fnd-pas-pas;hasSeller"/>
				<owl:someValuesFrom rdf:resource="&fibo-fnd-pas-pas;Seller"/>
			</owl:Restriction>
		</rdfs:subClassOf>
	</owl:Class>

</rdf:RDF>