<?xml version="1.0" encoding="UTF-8"?>
<!DOCTYPE rdf:RDF [
	<!ENTITY dct "http://purl.org/dc/terms/">
	<!ENTITY fibo-be-fctx-spv "https://spec.edmcouncil.org/fibo/ontology/BE/FunctionalEntitiesExt/SPVs/">
	<!ENTITY fibo-bp-iss-doc "https://spec.edmcouncil.org/fibo/ontology/BP/SecuritiesIssuance/IssuanceDocuments/">
	<!ENTITY fibo-bp-iss-trm "https://spec.edmcouncil.org/fibo/ontology/BP/SecuritiesIssuance/IssuanceProcessTerms/">
	<!ENTITY fibo-der-drc-raw "https://spec.edmcouncil.org/fibo/ontology/DER/DerivativesContracts/RightsAndWarrants/">
	<!ENTITY fibo-fbc-dae-gty "https://spec.edmcouncil.org/fibo/ontology/FBC/DebtAndEquities/Guaranty/">
	<!ENTITY fibo-fnd-acc-cur "https://spec.edmcouncil.org/fibo/ontology/FND/Accounting/CurrencyAmount/">
	<!ENTITY fibo-fnd-agr-ctr "https://spec.edmcouncil.org/fibo/ontology/FND/Agreements/Contracts/">
	<!ENTITY fibo-fnd-arrxx-ins "https://spec.edmcouncil.org/fibo/ontology/FND/ArrangementsExt/ToolsAndInstruments/">
	<!ENTITY fibo-fnd-utl-av "https://spec.edmcouncil.org/fibo/ontology/FND/Utilities/AnnotationVocabulary/">
	<!ENTITY fibo-fnd-utl-val "https://spec.edmcouncil.org/fibo/ontology/FND/Utilities/Values/">
	<!ENTITY fibo-sec-dbt-bo-bo "https://spec.edmcouncil.org/fibo/ontology/SEC/Debt/Bonds/BondsCommon/">
	<!ENTITY fibo-sec-dbt-dbt-iss "https://spec.edmcouncil.org/fibo/ontology/SEC/Debt/DebtFoundations/DebtIssuanceTerms/">
	<!ENTITY fibo-sec-dbt-dbti "https://spec.edmcouncil.org/fibo/ontology/SEC/Debt/DebtInstruments/">
	<!ENTITY fibo-sec-sec-iss "https://spec.edmcouncil.org/fibo/ontology/SEC/Securities/SecuritiesIssuance/">
	<!ENTITY owl "http://www.w3.org/2002/07/owl#">
	<!ENTITY rdf "http://www.w3.org/1999/02/22-rdf-syntax-ns#">
	<!ENTITY rdfs "http://www.w3.org/2000/01/rdf-schema#">
	<!ENTITY skos "http://www.w3.org/2004/02/skos/core#">
	<!ENTITY xsd "http://www.w3.org/2001/XMLSchema#">
]>
<rdf:RDF xml:base="https://spec.edmcouncil.org/fibo/ontology/SEC/Debt/DebtFoundations/DebtIssuanceTerms/"
	xmlns:dct="http://purl.org/dc/terms/"
	xmlns:fibo-be-fctx-spv="https://spec.edmcouncil.org/fibo/ontology/BE/FunctionalEntitiesExt/SPVs/"
	xmlns:fibo-bp-iss-doc="https://spec.edmcouncil.org/fibo/ontology/BP/SecuritiesIssuance/IssuanceDocuments/"
	xmlns:fibo-bp-iss-trm="https://spec.edmcouncil.org/fibo/ontology/BP/SecuritiesIssuance/IssuanceProcessTerms/"
	xmlns:fibo-der-drc-raw="https://spec.edmcouncil.org/fibo/ontology/DER/DerivativesContracts/RightsAndWarrants/"
	xmlns:fibo-fbc-dae-gty="https://spec.edmcouncil.org/fibo/ontology/FBC/DebtAndEquities/Guaranty/"
	xmlns:fibo-fnd-acc-cur="https://spec.edmcouncil.org/fibo/ontology/FND/Accounting/CurrencyAmount/"
	xmlns:fibo-fnd-agr-ctr="https://spec.edmcouncil.org/fibo/ontology/FND/Agreements/Contracts/"
	xmlns:fibo-fnd-arrxx-ins="https://spec.edmcouncil.org/fibo/ontology/FND/ArrangementsExt/ToolsAndInstruments/"
	xmlns:fibo-fnd-utl-av="https://spec.edmcouncil.org/fibo/ontology/FND/Utilities/AnnotationVocabulary/"
	xmlns:fibo-fnd-utl-val="https://spec.edmcouncil.org/fibo/ontology/FND/Utilities/Values/"
	xmlns:fibo-sec-dbt-bo-bo="https://spec.edmcouncil.org/fibo/ontology/SEC/Debt/Bonds/BondsCommon/"
	xmlns:fibo-sec-dbt-dbt-iss="https://spec.edmcouncil.org/fibo/ontology/SEC/Debt/DebtFoundations/DebtIssuanceTerms/"
	xmlns:fibo-sec-dbt-dbti="https://spec.edmcouncil.org/fibo/ontology/SEC/Debt/DebtInstruments/"
	xmlns:fibo-sec-sec-iss="https://spec.edmcouncil.org/fibo/ontology/SEC/Securities/SecuritiesIssuance/"
	xmlns:owl="http://www.w3.org/2002/07/owl#"
	xmlns:rdf="http://www.w3.org/1999/02/22-rdf-syntax-ns#"
	xmlns:rdfs="http://www.w3.org/2000/01/rdf-schema#"
	xmlns:skos="http://www.w3.org/2004/02/skos/core#"
	xmlns:xsd="http://www.w3.org/2001/XMLSchema#">
	
	<owl:Ontology rdf:about="https://spec.edmcouncil.org/fibo/ontology/SEC/Debt/DebtFoundations/DebtIssuanceTerms/">
		<rdfs:label xml:lang="en">DebtIssuanceTerms</rdfs:label>
		<dct:abstract>This ontology defines a number of kinds of information which arise out of the various issuance processes by which debt instruments may be issued, such as auction and syndication. 
		These concepts have been derived with reference to the process models in the Business Process domain for various kinds of debt instrument issuance process. Different processes generate and consume different kinds of information, documents etc., and a sub set of these variants will appear in security master file data for these different kinds of instrument. That is the sub set modeled here, ased on earlier ISO TC68 Working Group 11 work.</dct:abstract>
		<owl:imports rdf:resource="https://spec.edmcouncil.org/fibo/ontology/BE/FunctionalEntitiesExt/SPVs/"/>
		<owl:imports rdf:resource="https://spec.edmcouncil.org/fibo/ontology/BP/SecuritiesIssuance/IssuanceDocuments/"/>
		<owl:imports rdf:resource="https://spec.edmcouncil.org/fibo/ontology/BP/SecuritiesIssuance/IssuanceProcessTerms/"/>
		<owl:imports rdf:resource="https://spec.edmcouncil.org/fibo/ontology/DER/DerivativesContracts/RightsAndWarrants/"/>
		<owl:imports rdf:resource="https://spec.edmcouncil.org/fibo/ontology/FBC/DebtAndEquities/Guaranty/"/>
		<owl:imports rdf:resource="https://spec.edmcouncil.org/fibo/ontology/FBC/FinancialInstruments/FinancialInstruments/"/>
		<owl:imports rdf:resource="https://spec.edmcouncil.org/fibo/ontology/FND/Accounting/CurrencyAmount/"/>
		<owl:imports rdf:resource="https://spec.edmcouncil.org/fibo/ontology/FND/Agreements/Contracts/"/>
		<owl:imports rdf:resource="https://spec.edmcouncil.org/fibo/ontology/FND/ArrangementsExt/ToolsAndInstruments/"/>
		<owl:imports rdf:resource="https://spec.edmcouncil.org/fibo/ontology/FND/Utilities/AnnotationVocabulary/"/>
		<owl:imports rdf:resource="https://spec.edmcouncil.org/fibo/ontology/FND/Utilities/Values/"/>
		<owl:imports rdf:resource="https://spec.edmcouncil.org/fibo/ontology/SEC/Debt/Bonds/BondsCommon/"/>
		<owl:imports rdf:resource="https://spec.edmcouncil.org/fibo/ontology/SEC/Debt/DebtInstruments/"/>
		<owl:imports rdf:resource="https://spec.edmcouncil.org/fibo/ontology/SEC/Securities/Pools/"/>
		<owl:imports rdf:resource="https://spec.edmcouncil.org/fibo/ontology/SEC/Securities/SecuritiesIssuance/"/>
		<owl:versionIRI rdf:resource="https://spec.edmcouncil.org/fibo/ontology/SEC/Debt/DebtFoundations/DebtIssuanceTerms/"/>
		<fibo-fnd-utl-av:hasMaturityLevel rdf:resource="&fibo-fnd-utl-av;Provisional"/>
	</owl:Ontology>
	
	<owl:Class rdf:about="&fibo-sec-dbt-dbt-iss;AdvancedRefunding">
		<rdfs:subClassOf rdf:resource="&fibo-sec-dbt-dbt-iss;RefundingPurpose"/>
		<rdfs:label xml:lang="en">advance refunding</rdfs:label>
		<skos:definition xml:lang="en">A bond issuance in which new bonds are sold at a lower rate than outstanding ones. The proceeds are then invested, and when the older bonds become callable they are paid off with the invested proceeds.</skos:definition>
		<fibo-fnd-utl-av:definitionOrigin xml:lang="en">http://www.investopedia.com/terms/a/advancedrefunding.asp#ixzz4K90cVzeN</fibo-fnd-utl-av:definitionOrigin>
	</owl:Class>
	
	<owl:Class rdf:about="&fibo-sec-dbt-dbt-iss;BondIssuanceProgram">
		<rdfs:subClassOf rdf:resource="&fibo-sec-dbt-dbt-iss;DebtIssuanceProgram"/>
		<rdfs:subClassOf>
			<owl:Restriction>
				<owl:onProperty rdf:resource="&fibo-sec-dbt-dbt-iss;isANumberOf"/>
				<owl:someValuesFrom rdf:resource="&fibo-sec-dbt-dbt-iss;BondOffering"/>
			</owl:Restriction>
		</rdfs:subClassOf>
		<rdfs:label xml:lang="en">bond issuance program</rdfs:label>
		<skos:definition xml:lang="en">A series of bond issuances over time.</skos:definition>
	</owl:Class>
	
	<owl:Class rdf:about="&fibo-sec-dbt-dbt-iss;BondIssueInformation">
		<rdfs:subClassOf rdf:resource="&fibo-sec-dbt-dbt-iss;DebtInstrumentIssueInformation"/>
		<rdfs:label xml:lang="en">bond issue information</rdfs:label>
		<skos:definition xml:lang="en">Information about the Issuance of a Bond, which is maintained throughout the life of the Security.</skos:definition>
	</owl:Class>
	
	<owl:Class rdf:about="&fibo-sec-dbt-dbt-iss;BondOffering">
		<rdfs:subClassOf rdf:resource="&fibo-sec-dbt-dbti;DebtOffering"/>
		<rdfs:label xml:lang="en">bond offering</rdfs:label>
		<skos:definition xml:lang="en">a debt offering of one or more bonds, as all or part of an offering of those bonds to the market</skos:definition>
	</owl:Class>
	
	<owl:Class rdf:about="&fibo-sec-dbt-dbt-iss;BondOfferingWithWarrant">
		<rdfs:subClassOf rdf:resource="&fibo-sec-dbt-dbt-iss;BondOffering"/>
		<rdfs:subClassOf>
			<owl:Restriction>
				<owl:onProperty rdf:resource="&fibo-bp-iss-trm;isIssueOf"/>
				<owl:someValuesFrom>
					<owl:Class>
						<owl:unionOf rdf:parseType="Collection">
							<rdf:Description rdf:about="&fibo-der-drc-raw;TraditionalWarrant">
							</rdf:Description>
							<rdf:Description rdf:about="&fibo-sec-dbt-bo-bo;Bond">
							</rdf:Description>
						</owl:unionOf>
					</owl:Class>
				</owl:someValuesFrom>
			</owl:Restriction>
		</rdfs:subClassOf>
		<rdfs:label xml:lang="en">bond offering with warrant</rdfs:label>
		<owl:disjointWith rdf:resource="&fibo-sec-dbt-dbt-iss;MediumTermNoteIssue"/>
		<skos:definition xml:lang="en">a bond offering where the issue includes a warrant; Further notes: ISO 10962 CFI definition is A bond that is issued together with one or more warrant(s) attached as part of the offer, the warrant(s) granting the holder the right to purchase a designated security, often the common stock of the issuer of the debt, at a specified price. Review notes: This need not be any specific type of bond. The warrant is used as a sweetener to encourage people to subscribe to a new bond issue. The Bond and the Warrant trade together as a unit (called &quot;Bond Unit&quot;).</skos:definition>
	</owl:Class>
	
	<owl:Class rdf:about="&fibo-sec-dbt-dbt-iss;DebtInstrumentIssueInformation">
		<rdfs:subClassOf rdf:resource="&fibo-bp-iss-trm;IssuedSecurityIssueInformation"/>
		<rdfs:label xml:lang="en">debt instrument issue information</rdfs:label>
		<skos:definition xml:lang="en">Information about the Issuance of a Debt Security, which is maintained throughout the life of the Security.</skos:definition>
	</owl:Class>
	
	<owl:Class rdf:about="&fibo-sec-dbt-dbt-iss;DebtIssuanceProcessInformation">
		<rdfs:subClassOf rdf:resource="&fibo-bp-iss-trm;TradedInstrumentIssuanceProcessInformation"/>
		<rdfs:subClassOf>
			<owl:Restriction>
				<owl:onProperty rdf:resource="&fibo-sec-dbt-dbt-iss;hasDebtIssuancePurpose"/>
				<owl:onClass rdf:resource="&fibo-sec-dbt-dbt-iss;DebtIssuancePurpose"/>
				<owl:maxQualifiedCardinality rdf:datatype="&xsd;nonNegativeInteger">1</owl:maxQualifiedCardinality>
			</owl:Restriction>
		</rdfs:subClassOf>
		<rdfs:subClassOf>
			<owl:Restriction>
				<owl:onProperty rdf:resource="&fibo-sec-dbt-dbt-iss;becomesPartOfTerms"/>
				<owl:someValuesFrom rdf:resource="&fibo-sec-dbt-dbt-iss;DebtInstrumentIssueInformation"/>
			</owl:Restriction>
		</rdfs:subClassOf>
		<rdfs:label xml:lang="en">debt issuance process information</rdfs:label>
		<skos:definition xml:lang="en">Information specific to the Issuance of a Debt security.</skos:definition>
	</owl:Class>
	
	<owl:Class rdf:about="&fibo-sec-dbt-dbt-iss;DebtIssuanceProgram">
		<rdfs:subClassOf rdf:resource="&fibo-bp-iss-trm;IssuanceProgram"/>
		<rdfs:subClassOf>
			<owl:Restriction>
				<owl:onProperty rdf:resource="&fibo-sec-dbt-dbt-iss;isANumberOf"/>
				<owl:someValuesFrom rdf:resource="&fibo-sec-dbt-dbti;DebtOffering"/>
			</owl:Restriction>
		</rdfs:subClassOf>
		<rdfs:label xml:lang="en">debt issuance program</rdfs:label>
		<skos:definition xml:lang="en">A series of debt security issuances over time.</skos:definition>
	</owl:Class>
	
	<owl:Class rdf:about="&fibo-sec-dbt-dbt-iss;DebtIssuancePurpose">
		<rdfs:subClassOf rdf:resource="&fibo-fnd-arrxx-ins;Purpose"/>
		<rdfs:label xml:lang="en">debt issuance purpose</rdfs:label>
		<skos:definition xml:lang="en">Purpose for the Issuance of a Debt Security. Also defines processes to be followed in some instances.</skos:definition>
	</owl:Class>
	
	<owl:Class rdf:about="&fibo-sec-dbt-dbt-iss;DebtIssueProspectus">
		<rdfs:subClassOf rdf:resource="&fibo-bp-iss-doc;SecurityFinalProspectus"/>
		<rdfs:label xml:lang="en">debt issue prospectus</rdfs:label>
		<skos:definition xml:lang="en">The prospectus for the debt issue, describing the terms of the issue and each of the instruments included in the debt issue. Term origin:SMER</skos:definition>
	</owl:Class>
	
	<owl:Class rdf:about="&fibo-sec-dbt-dbt-iss;MTNOfferProgram">
		<rdfs:subClassOf rdf:resource="&fibo-sec-dbt-dbt-iss;BondIssuanceProgram"/>
		<rdfs:subClassOf>
			<owl:Restriction>
				<owl:onProperty rdf:resource="&fibo-sec-dbt-dbt-iss;issues"/>
				<owl:someValuesFrom rdf:resource="&fibo-sec-dbt-dbt-iss;MediumTermNoteIssue"/>
			</owl:Restriction>
		</rdfs:subClassOf>
		<rdfs:label xml:lang="en">m t n offer program</rdfs:label>
		<skos:definition xml:lang="en">A program of offerings of Medium Term Note debt securities. This is a set of issues where the maturity is defined after the rest of the terms have been registered with some authority. These are registered up front so that then the company wants to borrow more money they don&apos;t have to go through the registration period but have the facility up front to issue another security.</skos:definition>
	</owl:Class>
	
	<owl:Class rdf:about="&fibo-sec-dbt-dbt-iss;MediumTermNoteIssue">
		<rdfs:subClassOf rdf:resource="&fibo-sec-dbt-dbt-iss;BondOffering"/>
		<rdfs:label xml:lang="en">medium term note issue</rdfs:label>
	</owl:Class>
	
	<owl:Class rdf:about="&fibo-sec-dbt-dbt-iss;MunicipalBondIssuanceProcessInformation">
		<rdfs:subClassOf rdf:resource="&fibo-sec-dbt-dbt-iss;DebtIssuanceProcessInformation"/>
		<rdfs:subClassOf>
			<owl:Restriction>
				<owl:onProperty rdf:resource="&fibo-sec-dbt-dbt-iss;hasDebtIssuancePurpose"/>
				<owl:onClass rdf:resource="&fibo-sec-dbt-dbt-iss;DebtIssuancePurpose"/>
				<owl:maxQualifiedCardinality rdf:datatype="&xsd;nonNegativeInteger">1</owl:maxQualifiedCardinality>
			</owl:Restriction>
		</rdfs:subClassOf>
		<rdfs:subClassOf>
			<owl:Restriction>
				<owl:onProperty rdf:resource="&fibo-sec-dbt-dbt-iss;becomesPartOfTerms"/>
				<owl:someValuesFrom rdf:resource="&fibo-sec-dbt-dbt-iss;MunicipalBondIssueInformation"/>
			</owl:Restriction>
		</rdfs:subClassOf>
		<rdfs:subClassOf>
			<owl:Restriction>
				<owl:onProperty rdf:resource="&fibo-sec-dbt-dbt-iss;hasDebtIssuancePurpose"/>
				<owl:someValuesFrom rdf:resource="&fibo-sec-dbt-dbt-iss;DebtIssuancePurpose"/>
			</owl:Restriction>
		</rdfs:subClassOf>
		<rdfs:label xml:lang="en">municipal bond issuance process information</rdfs:label>
		<skos:definition xml:lang="en">Information specific to the Issuance of a Municipal Bond.</skos:definition>
	</owl:Class>
	
	<owl:Class rdf:about="&fibo-sec-dbt-dbt-iss;MunicipalBondIssueInformation">
		<rdfs:subClassOf rdf:resource="&fibo-sec-dbt-dbt-iss;BondIssueInformation"/>
		<rdfs:subClassOf>
			<owl:Restriction>
				<owl:onProperty rdf:resource="&fibo-sec-dbt-dbt-iss;debtIssuancePurpose"/>
				<owl:maxQualifiedCardinality rdf:datatype="&xsd;nonNegativeInteger">1</owl:maxQualifiedCardinality>
				<owl:onDataRange rdf:resource="&xsd;string"/>
			</owl:Restriction>
		</rdfs:subClassOf>
		<rdfs:subClassOf>
			<owl:Restriction>
				<owl:onProperty rdf:resource="&fibo-sec-dbt-dbt-iss;debtIssuancePurpose"/>
				<owl:someValuesFrom rdf:resource="&xsd;string"/>
			</owl:Restriction>
		</rdfs:subClassOf>
		<rdfs:label xml:lang="en">municipal bond issue information</rdfs:label>
		<skos:definition xml:lang="en">Information about the Issuance of a Municipal Bond, which is maintained throughout the life of the Security.</skos:definition>
	</owl:Class>
	
	<owl:Class rdf:about="&fibo-sec-dbt-dbt-iss;NewMoneyPurpose">
		<rdfs:subClassOf rdf:resource="&fibo-sec-dbt-dbt-iss;DebtIssuancePurpose"/>
		<rdfs:label xml:lang="en">new money purpose</rdfs:label>
		<skos:definition xml:lang="en">Securities Issued for new Project or Purpose.</skos:definition>
	</owl:Class>
	
	<owl:Class rdf:about="&fibo-sec-dbt-dbt-iss;RefundingPurpose">
		<rdfs:subClassOf rdf:resource="&fibo-sec-dbt-dbt-iss;DebtIssuancePurpose"/>
		<rdfs:label xml:lang="en">refunding purpose</rdfs:label>
		<skos:definition xml:lang="en">A procedure whereby an issuer refinances outstanding bonds by issuing new bonds.</skos:definition>
	</owl:Class>
	
	<owl:Class rdf:about="&fibo-sec-dbt-dbt-iss;RemarketingPurpose">
		<rdfs:subClassOf rdf:resource="&fibo-sec-dbt-dbt-iss;DebtIssuancePurpose"/>
		<rdfs:label xml:lang="en">remarketing purpose</rdfs:label>
		<skos:definition xml:lang="en">The process of reselling securities to the public that have been tendered for purchase by the previous owners thereof.</skos:definition>
	</owl:Class>
	
	<owl:Class rdf:about="&fibo-sec-dbt-dbt-iss;UnderwriterTakedownForDebt">
		<rdfs:subClassOf rdf:resource="&fibo-bp-iss-trm;UnderwriterTakedown"/>
		<rdfs:label xml:lang="en">underwriter takedown for debt</rdfs:label>
		<skos:definition xml:lang="en">Infomation on Takedown quantity of the Debt security handled by the underwriter (that will be brought into DTC).</skos:definition>
	</owl:Class>
	
	<owl:DatatypeProperty rdf:about="&fibo-sec-dbt-dbt-iss;bankQualified.1">
		<rdfs:label xml:lang="en">bank qualified</rdfs:label>
		<rdfs:domain rdf:resource="&fibo-sec-dbt-dbt-iss;MunicipalBondIssueInformation"/>
		<rdfs:range rdf:resource="&xsd;boolean"/>
		<skos:definition xml:lang="en">Designation given to a public purpose bond offering by the issuer if it reasonably expects to issue in the calendar year of such offering no more than $10 million par amount of bonds of the type required to be included in making such calculation under the Internal Revenue Code.  When purchased by a commercial bank for its portfolio, the bank may receive an 80% tax deduction for the interest cost of carry for the issue.  A bond that is bank qualified is also known as a qualified tax-exempt obligation.</skos:definition>
	</owl:DatatypeProperty>
	
	<owl:ObjectProperty rdf:about="&fibo-sec-dbt-dbt-iss;becomesPartOfTerms">
		<rdfs:subPropertyOf rdf:resource="&fibo-bp-iss-trm;becomesPartOf"/>
		<rdfs:label xml:lang="en">becomes part of terms</rdfs:label>
		<rdfs:domain rdf:resource="&fibo-sec-dbt-dbt-iss;DebtIssuanceProcessInformation"/>
		<rdfs:range rdf:resource="&fibo-sec-dbt-dbt-iss;DebtInstrumentIssueInformation"/>
		<skos:definition xml:lang="en">The information required throughout the life of the Security becomes the Issuance information maintained for that security.</skos:definition>
	</owl:ObjectProperty>
	
	<owl:DatatypeProperty rdf:about="&fibo-sec-dbt-dbt-iss;debtIssuancePurpose">
		<rdfs:label xml:lang="en">debt issuance purpose</rdfs:label>
		<rdfs:domain rdf:resource="&fibo-sec-dbt-dbt-iss;DebtInstrumentIssueInformation"/>
		<rdfs:range rdf:resource="&xsd;string"/>
		<skos:definition xml:lang="en">Purpose of the Issue of a Debt Security.</skos:definition>
	</owl:DatatypeProperty>
	
	<owl:ObjectProperty rdf:about="&fibo-sec-dbt-dbt-iss;hasDebtIssuancePurpose">
		<rdfs:label xml:lang="en">has debt issuance purpose</rdfs:label>
		<rdfs:domain rdf:resource="&fibo-sec-dbt-dbt-iss;DebtIssuanceProcessInformation"/>
		<rdfs:range rdf:resource="&fibo-sec-dbt-dbt-iss;DebtIssuancePurpose"/>
	</owl:ObjectProperty>
	
	<owl:ObjectProperty rdf:about="&fibo-sec-dbt-dbt-iss;isANumberOf">
		<rdfs:subPropertyOf rdf:resource="&fibo-bp-iss-trm;isCollectionOf"/>
		<rdfs:label xml:lang="en">is a number of</rdfs:label>
		<rdfs:domain rdf:resource="&fibo-sec-dbt-dbt-iss;DebtIssuanceProgram"/>
		<rdfs:range rdf:resource="&fibo-sec-dbt-dbti;DebtOffering"/>
	</owl:ObjectProperty>
	
	<owl:ObjectProperty rdf:about="&fibo-sec-dbt-dbt-iss;issueNominalAmount">
		<rdfs:label xml:lang="en">issue nominal amount</rdfs:label>
		<rdfs:domain rdf:resource="&fibo-sec-dbt-dbt-iss;DebtInstrumentIssueInformation"/>
		<rdfs:range rdf:resource="&fibo-fnd-acc-cur;MonetaryAmount"/>
		<skos:definition xml:lang="en">Total original amount issued, expressed as a monetary amount.</skos:definition>
	</owl:ObjectProperty>
	
	<owl:ObjectProperty rdf:about="&fibo-sec-dbt-dbt-iss;issues">
		<rdfs:label xml:lang="en">issues</rdfs:label>
		<rdfs:domain rdf:resource="&fibo-sec-dbt-dbt-iss;MTNOfferProgram"/>
		<rdfs:range rdf:resource="&fibo-sec-dbt-dbt-iss;MediumTermNoteIssue"/>
	</owl:ObjectProperty>
	
	<owl:ObjectProperty rdf:about="&fibo-sec-dbt-dbt-iss;oID">
		<rdfs:label xml:lang="en">o i d</rdfs:label>
		<rdfs:domain rdf:resource="&fibo-sec-dbt-dbt-iss;BondIssueInformation"/>
		<rdfs:range rdf:resource="&fibo-fnd-utl-val;PercentageValue"/>
		<skos:definition xml:lang="en">Discount from par value at the time a bond or other debt instrument is issued.</skos:definition>
	</owl:ObjectProperty>
	
	<owl:DatatypeProperty rdf:about="&fibo-sec-dbt-dbt-iss;toBeBankQualified">
		<rdfs:label xml:lang="en">to be bank qualified</rdfs:label>
		<rdfs:domain rdf:resource="&fibo-sec-dbt-dbt-iss;MunicipalBondIssuanceProcessInformation"/>
		<rdfs:range rdf:resource="&xsd;boolean"/>
		<skos:definition xml:lang="en">Designation given to a public purpose bond offering by the issuer if it reasonably expects to issue in the calendar year of such offering no more than $10 million par amount of bonds of the type required to be included in making such calculation under the Internal Revenue Code.  When purchased by a commercial bank for its portfolio, the bank may receive an 80% tax deduction for the interest cost of carry for the issue.  A bond that is bank qualified is also known as a qualified tax-exempt obligation.</skos:definition>
	</owl:DatatypeProperty>
	
	<owl:ObjectProperty rdf:about="&fibo-sec-dbt-dbt-iss;underwriterTakedownAmount">
		<rdfs:label xml:lang="en">underwriter takedown amount</rdfs:label>
		<rdfs:domain rdf:resource="&fibo-sec-dbt-dbt-iss;UnderwriterTakedownForDebt"/>
		<rdfs:range rdf:resource="&fibo-fnd-acc-cur;MonetaryAmount"/>
		<skos:definition xml:lang="en">Takedown amount of the security handled by the underwriter(that will be brought into DTC).</skos:definition>
	</owl:ObjectProperty>
	
	<owl:Class rdf:about="&fibo-sec-dbt-dbti;DebtOffering">
		<rdfs:subClassOf>
			<owl:Restriction>
				<owl:onProperty rdf:resource="&fibo-bp-iss-trm;isIssueOf"/>
				<owl:someValuesFrom rdf:resource="&fibo-sec-dbt-dbti;TradableDebtInstrument"/>
			</owl:Restriction>
		</rdfs:subClassOf>
		<rdfs:subClassOf>
			<owl:Restriction>
				<owl:onProperty rdf:resource="&fibo-fnd-agr-ctr;isEvidencedBy"/>
				<owl:someValuesFrom rdf:resource="&fibo-sec-dbt-dbt-iss;DebtIssueProspectus"/>
			</owl:Restriction>
		</rdfs:subClassOf>
		<rdfs:subClassOf>
			<owl:Restriction>
				<owl:onProperty rdf:resource="&fibo-sec-sec-iss;isUnderwrittenBy"/>
				<owl:someValuesFrom rdf:resource="&fibo-sec-sec-iss;SecurityUnderwriter"/>
			</owl:Restriction>
		</rdfs:subClassOf>
	</owl:Class>

</rdf:RDF>