<?xml version="1.0" encoding="UTF-8"?>
<!DOCTYPE rdf:RDF [
	<!ENTITY dct "http://purl.org/dc/terms/">
	<!ENTITY fibo-be-le-cb "https://spec.edmcouncil.org/fibo/ontology/BE/LegalEntities/CorporateBodies/">
	<!ENTITY fibo-fbc-dae-cre "https://spec.edmcouncil.org/fibo/ontology/FBC/DebtAndEquities/CreditEvents/">
	<!ENTITY fibo-fbc-dae-dbt "https://spec.edmcouncil.org/fibo/ontology/FBC/DebtAndEquities/Debt/">
	<!ENTITY fibo-fnd-acc-cur "https://spec.edmcouncil.org/fibo/ontology/FND/Accounting/CurrencyAmount/">
	<!ENTITY fibo-fnd-arr-cd "https://spec.edmcouncil.org/fibo/ontology/FND/Arrangements/Codes/">
	<!ENTITY fibo-fnd-dt-fd "https://spec.edmcouncil.org/fibo/ontology/FND/DatesAndTimes/FinancialDates/">
	<!ENTITY fibo-fnd-dt-oc "https://spec.edmcouncil.org/fibo/ontology/FND/DatesAndTimes/Occurrences/">
	<!ENTITY fibo-fnd-org-fm "https://spec.edmcouncil.org/fibo/ontology/FND/Organizations/FormalOrganizations/">
	<!ENTITY fibo-fnd-rel-rel "https://spec.edmcouncil.org/fibo/ontology/FND/Relations/Relations/">
	<!ENTITY fibo-fnd-utl-av "https://spec.edmcouncil.org/fibo/ontology/FND/Utilities/AnnotationVocabulary/">
	<!ENTITY owl "http://www.w3.org/2002/07/owl#">
	<!ENTITY rdf "http://www.w3.org/1999/02/22-rdf-syntax-ns#">
	<!ENTITY rdfs "http://www.w3.org/2000/01/rdf-schema#">
	<!ENTITY skos "http://www.w3.org/2004/02/skos/core#">
	<!ENTITY sm "http://www.omg.org/techprocess/ab/SpecificationMetadata/">
	<!ENTITY xsd "http://www.w3.org/2001/XMLSchema#">
]>
<rdf:RDF xml:base="https://spec.edmcouncil.org/fibo/ontology/FBC/DebtAndEquities/CreditEvents/"
	xmlns:dct="http://purl.org/dc/terms/"
	xmlns:fibo-be-le-cb="https://spec.edmcouncil.org/fibo/ontology/BE/LegalEntities/CorporateBodies/"
	xmlns:fibo-fbc-dae-cre="https://spec.edmcouncil.org/fibo/ontology/FBC/DebtAndEquities/CreditEvents/"
	xmlns:fibo-fbc-dae-dbt="https://spec.edmcouncil.org/fibo/ontology/FBC/DebtAndEquities/Debt/"
	xmlns:fibo-fnd-acc-cur="https://spec.edmcouncil.org/fibo/ontology/FND/Accounting/CurrencyAmount/"
	xmlns:fibo-fnd-arr-cd="https://spec.edmcouncil.org/fibo/ontology/FND/Arrangements/Codes/"
	xmlns:fibo-fnd-dt-fd="https://spec.edmcouncil.org/fibo/ontology/FND/DatesAndTimes/FinancialDates/"
	xmlns:fibo-fnd-dt-oc="https://spec.edmcouncil.org/fibo/ontology/FND/DatesAndTimes/Occurrences/"
	xmlns:fibo-fnd-org-fm="https://spec.edmcouncil.org/fibo/ontology/FND/Organizations/FormalOrganizations/"
	xmlns:fibo-fnd-rel-rel="https://spec.edmcouncil.org/fibo/ontology/FND/Relations/Relations/"
	xmlns:fibo-fnd-utl-av="https://spec.edmcouncil.org/fibo/ontology/FND/Utilities/AnnotationVocabulary/"
	xmlns:owl="http://www.w3.org/2002/07/owl#"
	xmlns:rdf="http://www.w3.org/1999/02/22-rdf-syntax-ns#"
	xmlns:rdfs="http://www.w3.org/2000/01/rdf-schema#"
	xmlns:skos="http://www.w3.org/2004/02/skos/core#"
	xmlns:sm="http://www.omg.org/techprocess/ab/SpecificationMetadata/"
	xmlns:xsd="http://www.w3.org/2001/XMLSchema#">
	
	<owl:Ontology rdf:about="https://spec.edmcouncil.org/fibo/ontology/FBC/DebtAndEquities/CreditEvents/">
		<rdfs:label xml:lang="en">Credit Events Ontology</rdfs:label>
		<dct:abstract>This ontology defines a range of credit events, that is events in which some payment or payments are not made. These include credit events relating to a specific debt obligation and events relating to the business entity as a whole. 
		Note: these were derived from the credit default swaps model, with extensive reference to the FpML standard for those instruments. Additional kinds of credit event may be needed for loan and other contexts.</dct:abstract>
		<dct:license rdf:datatype="&xsd;anyURI">http://opensource.org/licenses/MIT</dct:license>
		<sm:contentLanguage rdf:datatype="&xsd;anyURI">http://www.w3.org/standards/techs/owl#w3c_all</sm:contentLanguage>
		<sm:copyright>Copyright (c) 2019 EDM Council, Inc.</sm:copyright>
		<sm:dependsOn rdf:resource="https://spec.edmcouncil.org/fibo/ontology/BE/"/>
		<sm:dependsOn rdf:resource="https://spec.edmcouncil.org/fibo/ontology/FBC/DebtAndEquities/Debt/"/>
		<sm:dependsOn rdf:resource="https://spec.edmcouncil.org/fibo/ontology/FND/"/>
		<sm:fileAbbreviation>fibo-fbc-dae-cre</sm:fileAbbreviation>
		<sm:filename>CreditEvents.rdf</sm:filename>
		<owl:imports rdf:resource="https://spec.edmcouncil.org/fibo/ontology/BE/LegalEntities/CorporateBodies/"/>
		<owl:imports rdf:resource="https://spec.edmcouncil.org/fibo/ontology/FBC/DebtAndEquities/Debt/"/>
		<owl:imports rdf:resource="https://spec.edmcouncil.org/fibo/ontology/FND/Accounting/CurrencyAmount/"/>
		<owl:imports rdf:resource="https://spec.edmcouncil.org/fibo/ontology/FND/Arrangements/Codes/"/>
		<owl:imports rdf:resource="https://spec.edmcouncil.org/fibo/ontology/FND/DatesAndTimes/FinancialDates/"/>
		<owl:imports rdf:resource="https://spec.edmcouncil.org/fibo/ontology/FND/DatesAndTimes/Occurrences/"/>
		<owl:imports rdf:resource="https://spec.edmcouncil.org/fibo/ontology/FND/Organizations/FormalOrganizations/"/>
		<owl:imports rdf:resource="https://spec.edmcouncil.org/fibo/ontology/FND/Utilities/AnnotationVocabulary/"/>
		<owl:versionIRI rdf:resource="https://spec.edmcouncil.org/fibo/ontology/FBC/DebtAndEquities/CreditEvents/"/>
		<fibo-fnd-utl-av:hasMaturityLevel rdf:resource="&fibo-fnd-utl-av;Provisional"/>
	</owl:Ontology>
	
	<owl:Class rdf:about="&fibo-fbc-dae-cre;Bankruptcy">
		<rdfs:subClassOf rdf:resource="&fibo-fbc-dae-cre;CreditEvent"/>
		<rdfs:label xml:lang="en">bankruptcy</rdfs:label>
		<skos:definition xml:lang="en">credit event involving a change in state or condition in which a party becomes insolvent or unable to meet debt obligations</skos:definition>
		<fibo-fnd-utl-av:adaptedFrom>Barron&apos;s Dictionary of Banking Terms, Sixth Edition, 2012</fibo-fnd-utl-av:adaptedFrom>
		<fibo-fnd-utl-av:adaptedFrom rdf:datatype="&xsd;anyURI">https://thelawdictionary.org/bankruptcy/</fibo-fnd-utl-av:adaptedFrom>
	</owl:Class>
	
	<owl:Class rdf:about="&fibo-fbc-dae-cre;BreachOfCovenant">
		<rdfs:subClassOf rdf:resource="&fibo-fbc-dae-cre;CreditEvent"/>
		<rdfs:label xml:lang="en">breach of covenant</rdfs:label>
		<skos:definition xml:lang="en">credit event representing a violation of an express, or implied, condition of a contract to do or not to do something that has a negative financial impact</skos:definition>
	</owl:Class>
	
	<owl:Class rdf:about="&fibo-fbc-dae-cre;CreditEvent">
		<rdfs:subClassOf rdf:resource="&fibo-fnd-dt-oc;Occurrence"/>
		<rdfs:label xml:lang="en">credit event</rdfs:label>
		<skos:definition xml:lang="en">event signifying a sudden change in a borrower&apos;s credit standing, such as bankruptcy or a violation of a bond indenture or loan agreement, that raises doubts about the borrower&apos;s ability to meet current or future obligations</skos:definition>
	</owl:Class>
	
	<owl:Class rdf:about="&fibo-fbc-dae-cre;DefaultEvent">
		<rdfs:subClassOf rdf:resource="&fibo-fbc-dae-cre;CreditEvent"/>
		<rdfs:label xml:lang="en">default event</rdfs:label>
		<skos:definition xml:lang="en">credit event representing a failure to meet a contractual obligation, such as, but not limited to, failure to repay a debt including interest or principal on a loan or security</skos:definition>
		<fibo-fnd-utl-av:explanatoryNote xml:lang="en">A default can occur when a borrower is unable to make timely payments, misses payments, or avoids or stops making payments. A default has adverse effects on the borrower&apos;s credit and ability to borrow in the future.</fibo-fnd-utl-av:explanatoryNote>
	</owl:Class>
	
	<owl:Class rdf:about="&fibo-fbc-dae-cre;DistressedRatingsDowngrade">
		<rdfs:subClassOf rdf:resource="&fibo-fbc-dae-cre;ObligationSpecificCreditEvent"/>
		<rdfs:label xml:lang="en">distressed ratings downgrade</rdfs:label>
		<skos:definition xml:lang="en">credit event triggered when the credit rating of the reference obligation is downgraded to a distressed rating level or the rating is withdrawn by one or more ratings agency</skos:definition>
	</owl:Class>
	
	<owl:Class rdf:about="&fibo-fbc-dae-cre;EntitySpecificCreditEvent">
		<rdfs:subClassOf rdf:resource="&fibo-fbc-dae-cre;CreditEvent"/>
		<rdfs:subClassOf>
			<owl:Restriction>
				<owl:onProperty rdf:resource="&fibo-fnd-rel-rel;involves"/>
				<owl:someValuesFrom rdf:resource="&fibo-fnd-org-fm;FormalOrganization"/>
			</owl:Restriction>
		</rdfs:subClassOf>
		<rdfs:label xml:lang="en">entity-specific credit event</rdfs:label>
		<owl:disjointWith rdf:resource="&fibo-fbc-dae-cre;ObligationSpecificCreditEvent"/>
		<skos:definition xml:lang="en">credit event specified for a given formal organization rather than on a specific reference obligation</skos:definition>
	</owl:Class>
	
	<owl:Class rdf:about="&fibo-fbc-dae-cre;FailureToPay">
		<rdfs:subClassOf rdf:resource="&fibo-fbc-dae-cre;DefaultEvent"/>
		<rdfs:subClassOf>
			<owl:Restriction>
				<owl:onProperty rdf:resource="&fibo-fbc-dae-cre;hasGracePeriod"/>
				<owl:onClass rdf:resource="&fibo-fnd-dt-fd;DatePeriod"/>
				<owl:maxQualifiedCardinality rdf:datatype="&xsd;nonNegativeInteger">1</owl:maxQualifiedCardinality>
			</owl:Restriction>
		</rdfs:subClassOf>
		<rdfs:label xml:lang="en">failure to pay</rdfs:label>
		<skos:definition xml:lang="en">default event that is triggered following any applicable grace period in which a payment obligation is missed</skos:definition>
	</owl:Class>
	
	<owl:Class rdf:about="&fibo-fbc-dae-cre;FailureToPayInterest">
		<rdfs:subClassOf rdf:resource="&fibo-fbc-dae-cre;FailureToPay"/>
		<rdfs:label xml:lang="en">failure to pay interest</rdfs:label>
		<skos:definition xml:lang="en">The failure by the Reference Entity to pay an expected interest amount or the payment of an actual interest amount that is less than the expected interest amount. Further notes: A credit event. ISDA 2003 Term: Failure to Pay Interest. FpML full definition: &apos;A credit event. Corresponds to the failure by the Reference Entity to pay an expected interest amount or the payment of an actual interest amount that is less than the expected interest amount. ISDA 2003 Term: Failure to Pay Interest.&apos;</skos:definition>
	</owl:Class>
	
	<owl:Class rdf:about="&fibo-fbc-dae-cre;FailureToPayPrincipal">
		<rdfs:subClassOf rdf:resource="&fibo-fbc-dae-cre;FailureToPay"/>
		<rdfs:label xml:lang="en">failure to pay principal</rdfs:label>
		<skos:definition xml:lang="en">The failure by the Reference Entity to pay an expected principal amount or the payment of an actual principal amount that is less than the expected principal amount. Further notes: A credit event. ISDA 2003 Term: Failure to Pay Principal.&apos; FpML full definition: &apos;A credit event. Corresponds to the failure by the Reference Entity to pay an expected principal amount or the payment of an actual principal amount that is less than the expected principal amount. ISDA 2003 Term: Failure to Pay Principal.&apos;</skos:definition>
	</owl:Class>
	
	<owl:Class rdf:about="&fibo-fbc-dae-cre;FilingForBankruptcy">
		<rdfs:subClassOf rdf:resource="&fibo-fbc-dae-cre;EntitySpecificCreditEvent"/>
		<rdfs:label xml:lang="en">filing for bankruptcy</rdfs:label>
		<skos:definition xml:lang="en">An event in which an organization files for bankruptcy.</skos:definition>
		<fibo-fnd-utl-av:explanatoryNote xml:lang="en">This may be defined as the Credit Event in a CDS.</fibo-fnd-utl-av:explanatoryNote>
	</owl:Class>
	
	<owl:Class rdf:about="&fibo-fbc-dae-cre;HardCreditEvent">
		<rdfs:subClassOf rdf:resource="&fibo-fbc-dae-cre;DefaultEvent"/>
		<rdfs:label xml:lang="en">hard credit event</rdfs:label>
		<skos:definition xml:lang="en">Hard default. This is defined by the event not being repairable.</skos:definition>
		<fibo-fnd-utl-av:explanatoryNote xml:lang="en">Soft and Hard defaults are defined by whether or not the event is repairable. Typically defined by the crossing of some threshold in some measurement. If you don&apos;t repair, this becomes a &quot;failure to repair&quot; credit event. The &quot;failure to repair&quot; triggers either a hard default or there is a whole lot of possible terms about the extension of the grace period.</fibo-fnd-utl-av:explanatoryNote>
	</owl:Class>
	
	<owl:Class rdf:about="&fibo-fbc-dae-cre;InstallmentDefault">
		<rdfs:subClassOf rdf:resource="&fibo-fbc-dae-cre;DefaultEvent"/>
		<rdfs:label xml:lang="en">installment default</rdfs:label>
		<skos:definition xml:lang="en">Non payment of a call by the beneficial owner, resulting in either a court action by the issuer or the sale of the securities to recover costs and/or a forfeit of partially paid securities. SWIFT = INDE</skos:definition>
	</owl:Class>
	
	<owl:Class rdf:about="&fibo-fbc-dae-cre;MaturityExtension">
		<rdfs:subClassOf rdf:resource="&fibo-fbc-dae-cre;ObligationSpecificCreditEvent"/>
		<rdfs:label xml:lang="en">maturity extension</rdfs:label>
		<skos:definition xml:lang="en">credit event involving extension of payments beyond the original maturity date of the obligation</skos:definition>
		<fibo-fnd-utl-av:explanatoryNote xml:lang="en">As stipulated in the terms and conditions for a bond, for example, the issuer or the bondholder may prolong the maturity date. After extension, the security may differ from original issue (new rate or maturity date). May be subject to bondholder&apos;s approval.</fibo-fnd-utl-av:explanatoryNote>
	</owl:Class>
	
	<owl:Class rdf:about="&fibo-fbc-dae-cre;ObligationAcceleration">
		<rdfs:subClassOf rdf:resource="&fibo-fbc-dae-cre;ObligationSpecificCreditEvent"/>
		<rdfs:label xml:lang="en">obligation acceleration</rdfs:label>
		<skos:definition xml:lang="en">credit event triggered when one or more reference obligations become immediately due and payable as a result of a default or covenant breach on the reference entity&apos;s other debt instruments, subject to a materiality threshold</skos:definition>
	</owl:Class>
	
	<owl:Class rdf:about="&fibo-fbc-dae-cre;ObligationDefault">
		<rdfs:subClassOf rdf:resource="&fibo-fbc-dae-cre;DefaultEvent"/>
		<rdfs:subClassOf rdf:resource="&fibo-fbc-dae-cre;ObligationSpecificCreditEvent"/>
		<rdfs:label xml:lang="en">obligation default</rdfs:label>
		<skos:definition xml:lang="en">credit event triggered as a result of an obligation-specific default</skos:definition>
	</owl:Class>
	
	<owl:Class rdf:about="&fibo-fbc-dae-cre;ObligationSpecificCreditEvent">
		<rdfs:subClassOf rdf:resource="&fibo-fbc-dae-cre;CreditEvent"/>
		<rdfs:subClassOf>
			<owl:Restriction>
				<owl:onProperty rdf:resource="&fibo-fnd-rel-rel;involves"/>
				<owl:someValuesFrom rdf:resource="&fibo-fbc-dae-dbt;CreditAgreement"/>
			</owl:Restriction>
		</rdfs:subClassOf>
		<rdfs:label xml:lang="en">obligation-specific credit event</rdfs:label>
		<skos:definition xml:lang="en">credit event that relates to an individual credit agreement or debt instrument (reference obligation)</skos:definition>
	</owl:Class>
	
	<owl:Class rdf:about="&fibo-fbc-dae-cre;RepudiationOrMoratorium">
		<rdfs:subClassOf rdf:resource="&fibo-fbc-dae-cre;EntitySpecificCreditEvent"/>
		<rdfs:label xml:lang="en">repudiation or moratorium</rdfs:label>
		<skos:definition xml:lang="en">The reference entity, or a governmental authority, either refuses to recognise or challenges the validity of one or more obligations of the reference entity, or imposes a moratorium thereby postponing payments on one or more of the obligations of the reference entity.</skos:definition>
		<fibo-fnd-utl-av:explanatoryNote xml:lang="en">Subject to the default requirement amount. This is a Credit Event. ISDA 2003 Term: Repudiation/Moratorium FpML full definition: &apos;A credit event. The reference entity, or a governmental authority, either refuses to recognise or challenges the validity of one or more obligations of the reference entity, or imposes a moratorium thereby postponing payments on one or more of the obligations of the reference entity. Subject to the default requirement amount. ISDA 2003 Term: Repudiation/Moratorium.&apos;</fibo-fnd-utl-av:explanatoryNote>
	</owl:Class>
	
	<owl:Class rdf:about="&fibo-fbc-dae-cre;Restructuring">
		<rdfs:subClassOf rdf:resource="&fibo-fbc-dae-cre;EntitySpecificCreditEvent"/>
		<rdfs:subClassOf>
			<owl:Restriction>
				<owl:onProperty rdf:resource="&fibo-fbc-dae-cre;hasRestructuringTypeCode"/>
				<owl:allValuesFrom rdf:resource="&fibo-fbc-dae-cre;RestructuringTypeCode"/>
			</owl:Restriction>
		</rdfs:subClassOf>
		<rdfs:label xml:lang="en">restructuring</rdfs:label>
		<skos:definition xml:lang="en">event that materially impacts the reference entity&apos;s obligations, such as an interest rate reduction, principal reduction, deferral of interest or principal, change in priority ranking, or change in currency or composition of payment</skos:definition>
	</owl:Class>
	
	<owl:Class rdf:about="&fibo-fbc-dae-cre;RestructuringTypeCode">
		<rdfs:subClassOf rdf:resource="&fibo-fnd-arr-cd;CodeElement"/>
		<rdfs:subClassOf>
			<owl:Restriction>
				<owl:onProperty rdf:resource="&fibo-fnd-rel-rel;isDefinedIn"/>
				<owl:someValuesFrom rdf:resource="&fibo-fbc-dae-cre;RestructuringTypeScheme"/>
			</owl:Restriction>
		</rdfs:subClassOf>
		<rdfs:label xml:lang="en">restructuring type code</rdfs:label>
		<skos:definition xml:lang="en">A textual code identifying the type of restructuring event in relation to some restructuring type scheme. This is information about the event rather than an aspect of the event itself, and is commonly identified in messages.</skos:definition>
		<skos:editorialNote xml:lang="en">This is derived from the FpML term, the contents of which are a URI for the applicable Restructuring scheme. 

Modeling notes:
This is therefore modeled as a reference to a suitable scheme rather than to a given type of restructuring, on the assumption that the CDS Contract will be set up in this way. A more complete semantics would identify the type as a type of restructuring event and treat the scheme as ancillary, but for now we will assume that this is sufficient for the formal definition of these terms in a CDS Contract. To be confirmed at review. 

FpML Full Definition:
&apos;Specifies the type of restructuring that is applicable.&apos;

Term Origin:FpML = restructuringType
Definition Origin:SR Draft

Consensus:Review</skos:editorialNote>
		<skos:editorialNote xml:lang="en">is of type defined in: The scheme which defines the type of restructuring that is applicable. (former property)</skos:editorialNote>
	</owl:Class>
	
	<owl:Class rdf:about="&fibo-fbc-dae-cre;RestructuringTypeScheme">
		<rdfs:subClassOf rdf:resource="&fibo-fnd-arr-cd;CodeSet"/>
		<rdfs:label xml:lang="en">restructuring type scheme</rdfs:label>
		<skos:definition xml:lang="en">The scheme which defines the restructuring type in a Restructuring credit event.</skos:definition>
		<skos:editorialNote xml:lang="en">No definition given in the FpML schema. This is given as a URI with which to identify the scheme.</skos:editorialNote>
	</owl:Class>
	
	<owl:Class rdf:about="&fibo-fbc-dae-cre;SoftCreditEvent">
		<rdfs:subClassOf rdf:resource="&fibo-fbc-dae-cre;DefaultEvent"/>
		<rdfs:label xml:lang="en">soft credit event</rdfs:label>
		<skos:definition xml:lang="en">Soft default. This is defined by the event being repairable.</skos:definition>
		<fibo-fnd-utl-av:explanatoryNote xml:lang="en">Soft and Hard defaults are defined by whether or not the event is repairable. Typically defined by the crossing of some threshold in some measurement. If you don&apos;t repair, this becomes a &quot;failure to repair&quot; credit event. The &quot;failure to repair&quot; (Failure To Pay) triggers either a hard default or there is a whole lot of possible terms about the extension of the grace period. Grace period extension applicability would in principle apply to the soft credit event. The hard credit event (e.g. Failure to Repair) is after such a period, if it exists, has passed.</fibo-fnd-utl-av:explanatoryNote>
	</owl:Class>
	
	<owl:Class rdf:about="&fibo-fbc-dae-cre;Writedown">
		<rdfs:subClassOf rdf:resource="&fibo-fbc-dae-cre;ObligationSpecificCreditEvent"/>
		<rdfs:label xml:lang="en">writedown</rdfs:label>
		<skos:definition xml:lang="en">The fact that the underlier writes down its outstanding principal amount. Further notes: A credit event. FpML full definition: &apos;A credit event. Results from the fact that the underlier writes down its outstanding principal amount.&apos;</skos:definition>
	</owl:Class>
	
	<owl:ObjectProperty rdf:about="&fibo-fbc-dae-cre;hasDefaultThresholdAmount">
		<rdfs:label xml:lang="en">has default threshold amount</rdfs:label>
		<rdfs:domain rdf:resource="&fibo-fbc-dae-cre;EntitySpecificCreditEvent"/>
		<rdfs:range rdf:resource="&fibo-fnd-acc-cur;MonetaryAmount"/>
		<skos:definition xml:lang="en">specifies an amount of money that triggers a repudiation/moratorium or restructuring event</skos:definition>
	</owl:ObjectProperty>
	
	<owl:DatatypeProperty rdf:about="&fibo-fbc-dae-cre;hasExtendableGracePeriod">
		<rdfs:label xml:lang="en">has extendable grace period</rdfs:label>
		<rdfs:domain rdf:resource="&fibo-fbc-dae-cre;FailureToPay"/>
		<rdfs:range rdf:resource="&xsd;boolean"/>
		<skos:definition xml:lang="en">indicates whether or not the grace period may be extended, which may be jurisdiction specific</skos:definition>
	</owl:DatatypeProperty>
	
	<owl:ObjectProperty rdf:about="&fibo-fbc-dae-cre;hasGracePeriod">
		<rdfs:label xml:lang="en">has grace period</rdfs:label>
		<rdfs:domain rdf:resource="&fibo-fbc-dae-cre;FailureToPay"/>
		<rdfs:range rdf:resource="&fibo-fnd-dt-fd;DatePeriod"/>
		<skos:definition xml:lang="en">Note that this may be a period denominated in business days or calendar days.</skos:definition>
		<skos:definition xml:lang="en">window following any payment due date during which a party must fulfil its obligations before a failure to pay credit event occurs. Further notes: ISDA 2003 Term: Grace Period. Note this may be a period denominated in business days or calendar days - this is a qualifying fact about the referenced term &quot;Date Period&quot;. FpML full definition: &apos;The number of calendar or business days after any due date that the reference entity has to fulfil its obligations before a failure to pay credit event is deemed to have occurred. ISDA 2003 Term: Grace Period.&apos;</skos:definition>
	</owl:ObjectProperty>
	
	<owl:ObjectProperty rdf:about="&fibo-fbc-dae-cre;hasRestructuringTypeCode">
		<rdfs:label xml:lang="en">has restructuring type code</rdfs:label>
		<rdfs:domain rdf:resource="&fibo-fbc-dae-cre;Restructuring"/>
		<rdfs:range rdf:resource="&fibo-fbc-dae-cre;RestructuringTypeCode"/>
		<skos:definition xml:lang="en">has a code representing the kind of restructuring event in relation to some defined scheme of such</skos:definition>
	</owl:ObjectProperty>
	
	<owl:DatatypeProperty rdf:about="&fibo-fbc-dae-cre;hasSchemeReference">
		<rdfs:label xml:lang="en">has scheme reference</rdfs:label>
		<rdfs:domain rdf:resource="&fibo-fbc-dae-cre;RestructuringTypeScheme"/>
		<rdfs:range rdf:resource="&xsd;anyURI"/>
		<skos:definition xml:lang="en">The reference by which the scheme is identified, as a URI.</skos:definition>
	</owl:DatatypeProperty>
	
	<owl:DatatypeProperty rdf:about="&fibo-fbc-dae-cre;multipleCreditEvent">
		<rdfs:label xml:lang="en">multiple credit event</rdfs:label>
		<rdfs:domain rdf:resource="&fibo-fbc-dae-cre;Restructuring"/>
		<rdfs:range rdf:resource="&xsd;boolean"/>
		<skos:definition xml:lang="en">Section 3.9 of the ISDA 2003 Credit Derivatives Definitions shall apply.</skos:definition>
	</owl:DatatypeProperty>
	
	<owl:DatatypeProperty rdf:about="&fibo-fbc-dae-cre;multipleHolderObligation">
		<rdfs:label xml:lang="en">multiple holder obligation</rdfs:label>
		<rdfs:domain rdf:resource="&fibo-fbc-dae-cre;Restructuring"/>
		<rdfs:range rdf:resource="&xsd;boolean"/>
		<skos:definition xml:lang="en">A multiple holder obligation means an obligation that is held by more than three holders that are not affiliates of each other and where at least two thirds of the holders must agree to the event that constitutes the restructuring credit event.</skos:definition>
	</owl:DatatypeProperty>
	
	<owl:ObjectProperty rdf:about="&fibo-fbc-dae-cre;paymentRequirement">
		<rdfs:label xml:lang="en">payment requirement</rdfs:label>
		<rdfs:domain rdf:resource="&fibo-fbc-dae-cre;FailureToPay"/>
		<rdfs:range rdf:resource="&fibo-fnd-acc-cur;MonetaryAmount"/>
		<skos:definition xml:lang="en">A threshold for the failure to pay credit event. Further notes: Market standard is USD 1,000,000 (JPY 100,000,000 for Japanese Yen trades) or its equivalent in the relevant obligation currency. This is applied on an aggregate basis across all Obligations of the Reference Entity. Intended to prevent technical/operational errors from triggering credit events. ISDA 2003 Term: Payment Requirement. FpML full definition: &apos;Specifies a threshold for the failure to pay credit event. Market standard is USD 1,000,000 (JPY 100,000,000 for Japanese Yen trades) or its equivalent in the relevant obligation currency. This is applied on an aggregate basis across all Obligations of the Reference Entity. Intended to prevent technical/operational errors from triggering credit events. ISDA 2003 Term: Payment Requirement.&apos;</skos:definition>
	</owl:ObjectProperty>

</rdf:RDF>