<?xml version="1.0" encoding="UTF-8"?>
<rdf:RDF xmlns:xsd="http://www.w3.org/2001/XMLSchema#"
         xmlns:fibo-prov="http://www.omg.org/spec/FIBO/Foundation/Annotation/ProvenanceAnnotation/"
         xmlns:fibo-ann="http://www.omg.org/spec/FIBO/Foundation/Annotation/FIBOAnnotation/"
         xmlns:fibo-arch="http://www.omg.org/spec/FIBO/Foundation/Annotation/FIBOArchetype/"
         xmlns:rdf="http://www.w3.org/1999/02/22-rdf-syntax-ns#"
         xmlns:fibo-fac="http://www.omg.org/spec/FIBO/Foundation/Annotation/FIBOFacet/"
         xmlns:rdfs="http://www.w3.org/2000/01/rdf-schema#"
         xmlns:owl="http://www.w3.org/2002/07/owl#"
         xmlns:skos="http://www.w3.org/2004/02/skos/core#"
         xmlns:dc="http://purl.org/dc/terms/"
         xml:base="http://www.omg.org/spec/FIBO/BE/Trust/TrustCommon">

   <owl:Ontology rdf:about="http://www.omg.org/spec/FIBO/BE/Trust/TrustCommon">
      <owl:imports rdf:resource="http://www.omg.org/spec/FIBO/BE/BusinessOrganization/FormalOrganization"/>
   </owl:Ontology>

   <!--Datatypes-->

<!--Object Properties-->

<owl:ObjectProperty rdf:about="http://www.omg.org/spec/FIBO/BE/Trust/TrustCommon/fundManagerIdentity">
      <skos:definition>The entity which fulfills the role of the Trust Fund Manager</skos:definition>
      <skos:definition>The entity which fulfills the role of the Trust Fund Manager</skos:definition>
      <rdfs:subPropertyOf rdf:resource="http://www.omg.org/spec/FIBO/BE/BusinessOrganization/OrganizationMember/organizationMemberIdentity"/>
      <rdfs:domain rdf:resource="http://www.omg.org/spec/FIBO/BE/Trust/TrustCommon/TrustFundManager"/>
      <rdfs:range rdf:resource="http://www.omg.org/spec/FIBO/BE/LegalPerson/LegalPersonCommon/LegalPerson"/>
   </owl:ObjectProperty>

   <owl:ObjectProperty rdf:about="http://www.omg.org/spec/FIBO/BE/Trust/TrustCommon/definesBeneficiary">
      <skos:definition>The party formally identified in the Trust Agreement as the Beneficiary.</skos:definition>
      <skos:definition>The party formally identified in the Trust Agreement as the Beneficiary.</skos:definition>
      <rdfs:subPropertyOf rdf:resource="http://www.omg.org/spec/FIBO/Foundation/Legal/Contract/hasParty"/>
      <rdfs:domain rdf:resource="http://www.omg.org/spec/FIBO/BE/Trust/TrustCommon/TrustAgreement"/>
      <rdfs:range rdf:resource="http://www.omg.org/spec/FIBO/BE/Trust/TrustCommon/Beneficiary"/>
   </owl:ObjectProperty>

   <owl:ObjectProperty rdf:about="http://www.omg.org/spec/FIBO/BE/Trust/TrustCommon/definesTrustorParty">
      <skos:definition>The party formally identified in the Trust Agreement as the Sponsor.</skos:definition>
      <skos:definition>The party formally identified in the Trust Agreement as the Sponsor.</skos:definition>
      <rdfs:subPropertyOf rdf:resource="http://www.omg.org/spec/FIBO/Foundation/Legal/Contract/hasParty"/>
      <rdfs:domain rdf:resource="http://www.omg.org/spec/FIBO/BE/Trust/TrustCommon/TrustAgreement"/>
      <rdfs:range rdf:resource="http://www.omg.org/spec/FIBO/BE/Trust/TrustCommon/Trustor"/>
   </owl:ObjectProperty>

   <owl:ObjectProperty rdf:about="http://www.omg.org/spec/FIBO/BE/Trust/TrustCommon/definesTrusteeParty">
      <skos:definition>The party formally identified in the Trust Agreement as the Trustee.</skos:definition>
      <skos:definition>The party formally identified in the Trust Agreement as the Trustee.</skos:definition>
      <rdfs:subPropertyOf rdf:resource="http://www.omg.org/spec/FIBO/Foundation/Legal/Contract/hasParty"/>
      <rdfs:domain rdf:resource="http://www.omg.org/spec/FIBO/BE/Trust/TrustCommon/TrustAgreement"/>
      <rdfs:range rdf:resource="http://www.omg.org/spec/FIBO/BE/Trust/TrustCommon/Trustee"/>
   </owl:ObjectProperty>

   <owl:ObjectProperty rdf:about="http://www.omg.org/spec/FIBO/BE/Trust/TrustCommon/hasBeneficiary">
      <skos:definition>Some unit holder in the Trust Fund</skos:definition>
      <skos:definition>Some unit holder in the Trust Fund</skos:definition>
      <rdfs:subPropertyOf rdf:resource="http://www.omg.org/spec/FIBO/BE/Trust/TrustCommon/hasPartyBeneficiary"/>
      <rdfs:domain rdf:resource="http://www.omg.org/spec/FIBO/BE/Trust/TrustCommon/TrustFundTrust"/>
      <rdfs:range rdf:resource="http://www.omg.org/spec/FIBO/BE/Trust/TrustCommon/FundUnitHolder"/>
   </owl:ObjectProperty>

   <owl:ObjectProperty rdf:about="http://www.omg.org/spec/FIBO/BE/Trust/TrustCommon/trusteeIdentity">
      <skos:definition>The entity which fulfills the role of the Trustee.</skos:definition>
      <skos:definition>The entity which fulfills the role of the Trustee.</skos:definition>
      <rdfs:subPropertyOf rdf:resource="http://www.omg.org/spec/FIBO/BE/BusinessOrganization/OrganizationMember/organizationMemberIdentity"/>
      <rdfs:domain rdf:resource="http://www.omg.org/spec/FIBO/BE/Trust/TrustCommon/Trustee"/>
      <rdfs:range rdf:resource="http://www.omg.org/spec/FIBO/BE/LegalPerson/LegalPersonCommon/LegalPerson"/>
   </owl:ObjectProperty>

   <owl:ObjectProperty rdf:about="http://www.omg.org/spec/FIBO/BE/Trust/TrustCommon/governedByTrustAgreement">
      <skos:definition>The agreement which governs the relationships among the principals in the Trust.</skos:definition>
      <skos:definition>The agreement which governs the relationships among the principals in the Trust.</skos:definition>
      <rdfs:subPropertyOf rdf:resource="http://www.omg.org/spec/FIBO/BE/BusinessOrganization/FormalOrganization/governedBy"/>
      <rdfs:domain rdf:resource="http://www.omg.org/spec/FIBO/BE/Trust/TrustCommon/Trust"/>
      <rdfs:range rdf:resource="http://www.omg.org/spec/FIBO/BE/Trust/TrustCommon/TrustAgreement"/>
   </owl:ObjectProperty>

   <owl:ObjectProperty rdf:about="http://www.omg.org/spec/FIBO/BE/Trust/TrustCommon/hasFundManager">
      <skos:definition>The party which is the manager of the Trust Fund.</skos:definition>
      <skos:definition>The party which is the manager of the Trust Fund.</skos:definition>
      <rdfs:domain rdf:resource="http://www.omg.org/spec/FIBO/BE/Trust/TrustCommon/TrustFundTrust"/>
      <rdfs:range rdf:resource="http://www.omg.org/spec/FIBO/BE/Trust/TrustCommon/TrustFundManager"/>
   </owl:ObjectProperty>

   <owl:ObjectProperty rdf:about="http://www.omg.org/spec/FIBO/BE/Trust/TrustCommon/hasPartyBeneficiary">
      <skos:definition>Has a Beneficiary of the Trust</skos:definition>
      <skos:definition>Has a Beneficiary of the Trust</skos:definition>
      <rdfs:subPropertyOf rdf:resource="http://www.omg.org/spec/FIBO/BE/BusinessOrganization/OrganizationMember/hasOrganizationMember"/>
      <rdfs:domain rdf:resource="http://www.omg.org/spec/FIBO/BE/Trust/TrustCommon/Trust"/>
      <rdfs:range rdf:resource="http://www.omg.org/spec/FIBO/BE/Trust/TrustCommon/Beneficiary"/>
   </owl:ObjectProperty>

   <owl:ObjectProperty rdf:about="http://www.omg.org/spec/FIBO/BE/Trust/TrustCommon/hasPartySponsor">
      <skos:definition>Has a sponsor of the Trust.</skos:definition>
      <skos:definition>Has a sponsor of the Trust.</skos:definition>
      <rdfs:subPropertyOf rdf:resource="http://www.omg.org/spec/FIBO/BE/BusinessOrganization/OrganizationMember/hasOrganizationMember"/>
      <rdfs:domain rdf:resource="http://www.omg.org/spec/FIBO/BE/Trust/TrustCommon/Trust"/>
      <rdfs:range rdf:resource="http://www.omg.org/spec/FIBO/BE/Trust/TrustCommon/Trustor"/>
   </owl:ObjectProperty>

   <owl:ObjectProperty rdf:about="http://www.omg.org/spec/FIBO/BE/Trust/TrustCommon/hasPartyTrustee">
      <skos:definition>Has a Trustee of the Trust</skos:definition>
      <skos:definition>Has a Trustee of the Trust</skos:definition>
      <rdfs:subPropertyOf rdf:resource="http://www.omg.org/spec/FIBO/BE/BusinessOrganization/OrganizationMember/hasOrganizationMember"/>
      <rdfs:domain rdf:resource="http://www.omg.org/spec/FIBO/BE/Trust/TrustCommon/Trust"/>
      <rdfs:range rdf:resource="http://www.omg.org/spec/FIBO/BE/Trust/TrustCommon/Trustee"/>
   </owl:ObjectProperty>

   <owl:ObjectProperty rdf:about="http://www.omg.org/spec/FIBO/BE/Trust/TrustCommon/unitHolder">
      <skos:definition>The holder of units in a trust.</skos:definition>
      <skos:editorialNote>This is a legal entity. REVIEW: This term was added during some early discussions of Funds (pre 2012). Need to determine whether this is something that exists for all Trusts (probably not), or if it is a fact about specific kinds of trusts that are used in funds / CIV, in which case there would be a sub-class of Trust with this property.</skos:editorialNote>
      <skos:editorialNote>This is a legal entity. REVIEW: This term was added during some early discussions of Funds (pre 2012). Need to determine whether this is something that exists for all Trusts (probably not), or if it is a fact about specific kinds of trusts that are used in funds / CIV, in which case there would be a sub-class of Trust with this property.</skos:editorialNote>
      <skos:definition>The holder of units in a trust.</skos:definition>
      <rdfs:subPropertyOf rdf:resource="http://www.omg.org/spec/FIBO/BE/BusinessOrganization/OrganizationPart/hasMember"/>
      <rdfs:domain rdf:resource="http://www.omg.org/spec/FIBO/BE/Trust/TrustCommon/TrustFundTrust"/>
      <rdfs:range rdf:resource="http://www.omg.org/spec/FIBO/BE/LegalPerson/LegalPersonCommon/LegalPerson"/>
   </owl:ObjectProperty>

   <!--Data Properties-->

<!--Annotation Properties-->

<!--Classes-->

<owl:Class rdf:about="http://www.omg.org/spec/FIBO/BE/Trust/TrustCommon/Beneficiary">
      <rdfs:label>Beneficiary</rdfs:label>
      <skos:definition>The Beneficiary of the Trust</skos:definition>
      <skos:definition>The Beneficiary of the Trust</skos:definition>
      <rdfs:subClassOf rdf:resource="http://www.omg.org/spec/FIBO/BE/BusinessOrganization/OrganizationMember/OrganizationMember"/>
   </owl:Class>

   <owl:Class rdf:about="http://www.omg.org/spec/FIBO/BE/Trust/TrustCommon/FundUnitHolder">
      <rdfs:label>Fund Unit holder</rdfs:label>
      <skos:definition>A party which holds some unit in the Trust Fund.</skos:definition>
      <skos:definition>A party which holds some unit in the Trust Fund.</skos:definition>
      <rdfs:subClassOf rdf:resource="http://www.omg.org/spec/FIBO/BE/Trust/TrustCommon/Beneficiary"/>
   </owl:Class>

   <owl:Class rdf:about="http://www.omg.org/spec/FIBO/BE/Trust/TrustCommon/TrustAgreement">
      <rdfs:label>Trust Agreement</rdfs:label>
      <skos:definition>The formal contract by which the Trust exists.</skos:definition>
      <skos:definition>The formal contract by which the Trust exists.</skos:definition>
      <skos:editorialNote>See also Deed. These are distinct from Contracts in that they impose obligations but without necessarily reciprocating rights.</skos:editorialNote>
      <skos:editorialNote>See also Deed. These are distinct from Contracts in that they impose obligations but without necessarily reciprocating rights.</skos:editorialNote>
      <rdfs:subClassOf rdf:resource="http://www.omg.org/spec/FIBO/BE/BusinessOrganization/FormalOrganization/OrganizationCoveringAgreement"/>
   </owl:Class>

   <owl:Class rdf:about="http://www.omg.org/spec/FIBO/BE/Trust/TrustCommon/TrustFundManager">
      <rdfs:label>Trust Fund Manager</rdfs:label>
      <skos:definition>Trust Fund Manager acts on behalf of the Trustee to manage the assets of the Trust.</skos:definition>
      <skos:definition>Trust Fund Manager acts on behalf of the Trustee to manage the assets of the Trust.</skos:definition>
   </owl:Class>

   <owl:Class rdf:about="http://www.omg.org/spec/FIBO/BE/Trust/TrustCommon/TrustFundTrust">
      <rdfs:label>Trust Fund Trust</rdfs:label>
      <skos:definition>A trust which forms the basis for a fund.</skos:definition>
      <skos:editorialNote>The fund is identified as being a kind of Trust Fund.</skos:editorialNote>
      <skos:definition>A trust which forms the basis for a fund.</skos:definition>
      <skos:editorialNote>The fund is identified as being a kind of Trust Fund.</skos:editorialNote>
      <rdfs:subClassOf rdf:resource="http://www.omg.org/spec/FIBO/BE/Trust/TrustCommon/Trust"/>
   </owl:Class>

   <owl:Class rdf:about="http://www.omg.org/spec/FIBO/BE/Trust/TrustCommon/Trustee">
      <rdfs:label>Trustee</rdfs:label>
      <skos:definition>The Trustee of the Trust</skos:definition>
      <skos:definition>The Trustee of the Trust</skos:definition>
      <rdfs:subClassOf rdf:resource="http://www.omg.org/spec/FIBO/Foundation/Legal/Contract/ContractParty"/>
   </owl:Class>

   <owl:Class rdf:about="http://www.omg.org/spec/FIBO/BE/Trust/TrustCommon/Trustor">
      <rdfs:label>Trustor</rdfs:label>
      <skos:definition>The sponsor of the Trust.</skos:definition>
      <skos:definition>The sponsor of the Trust.</skos:definition>
   </owl:Class>

   <owl:Class rdf:about="http://www.omg.org/spec/FIBO/BE/Trust/TrustCommon/Trust">
      <rdfs:label>Trust</rdfs:label>
      <skos:definition>A fiduciary relationship in which one party, known as a trustor, gives another party, the trustee, the right to hold title to property or assets for the benefit of a third party, the beneficiary.</skos:definition>
      <skos:editorialNote>This is a legal agreement between parties that someone owns, and is thereby an asset that they own. They can be taxed on this as any other asset. There are generally accepted things such as the source of funds that will determine who the revenue agency will go after. Definition reference URL: &lt;a href="http://www.investopedia.com/terms/t/trust.asp \l ixzz2MtESDTlP"&gt;&lt;font color="#0000ff"&gt;&lt;u&gt;http://www.investopedia.com/terms/t/trust.asp#ixzz2MtESDTlP&lt;/u&gt;&lt;/font&gt;&lt;/a&gt;</skos:editorialNote>
      <skos:definition>A fiduciary relationship in which one party, known as a trustor, gives another party, the trustee, the right to hold title to property or assets for the benefit of a third party, the beneficiary.</skos:definition>
      <skos:editorialNote>This is a legal agreement between parties that someone owns, and is thereby an asset that they own. They can be taxed on this as any other asset. There are generally accepted things such as the source of funds that will determine who the revenue agency will go after. Definition reference URL: &lt;a href="http://www.investopedia.com/terms/t/trust.asp \l ixzz2MtESDTlP"&gt;&lt;font color="#0000ff"&gt;&lt;u&gt;http://www.investopedia.com/terms/t/trust.asp#ixzz2MtESDTlP&lt;/u&gt;&lt;/font&gt;&lt;/a&gt;</skos:editorialNote>
      <rdfs:subClassOf rdf:resource="http://www.omg.org/spec/FIBO/BE/BusinessOrganization/OrganizationType/FormalOrganization"/>
   </owl:Class>

   <!--Individuals-->

</rdf:RDF>